<?xml version="1.0"?>
<rdf:RDF xmlns="http://www.w3.org/2003/12/exif/ns#"
     xml:base="http://www.w3.org/2003/12/exif/ns"
     xmlns:dc="http://purl.org/dc/elements/1.1/"
     xmlns:ex="http://example.org/"
     xmlns:owl="http://www.w3.org/2002/07/owl#"
     xmlns:rdf="http://www.w3.org/1999/02/22-rdf-syntax-ns#"
     xmlns:xml="http://www.w3.org/XML/1998/namespace"
     xmlns:xsd="http://www.w3.org/2001/XMLSchema#"
     xmlns:exif="http://www.w3.org/2003/12/exif/ns#"
     xmlns:foaf="http://xmlns.com/foaf/0.1/"
     xmlns:rdfs="http://www.w3.org/2000/01/rdf-schema#"
     xmlns:dcterms="http://purl.org/dc/terms/">
    <owl:Ontology rdf:about="http://www.w3.org/2003/12/exif/ns">
        <dc:description xml:lang="ja">Exifフォーマットの写真からデータを取りだしてRDFで表現するため、Exif 2.2の全てのタグをRDFプロパティとして定義し、さらにそれを記述するのに必要な語彙を追加したボキャブラリ</dc:description>
        <dc:description xml:lang="fr">Vocabulaire pour décrire les données Exif d&apos;une photographie. Toutes les balises Exif 2.2 sont définies comme des propriétés RDF, ainsi que plusieurs termes pour donner de l&apos;aide.</dc:description>
        <dc:description xml:lang="en">Vocabulary to describe an Exif format picture data. All Exif 2.2 tags are defined as RDF properties, as well as several terms to help this schema.</dc:description>
        <dc:source rdf:resource="http://tsc.jeita.or.jp/avs/data/cp3451.pdf"/>
        <dc:title xml:lang="en">Exif data description vocabulary</dc:title>
        <dcterms:created xml:lang="en">2003-07-18</dcterms:created>
        <dcterms:modified xml:lang="en">2003-08-19</dcterms:modified>
        <owl:versionInfo xml:lang="en">Experimental version.</owl:versionInfo>
        <foaf:maker rdf:resource="urn:pin:MK705"/>
    </owl:Ontology>
    


    <!-- 
    ///////////////////////////////////////////////////////////////////////////////////////
    //
    // Annotation properties
    //
    ///////////////////////////////////////////////////////////////////////////////////////
     -->

    


    <!-- http://example.org/code -->

    <owl:AnnotationProperty rdf:about="http://example.org/code"/>
    


    <!-- http://example.org/trial -->

    <owl:AnnotationProperty rdf:about="http://example.org/trial"/>
    


    <!-- http://purl.org/dc/elements/1.1/creator -->

    <owl:AnnotationProperty rdf:about="http://purl.org/dc/elements/1.1/creator"/>
    


    <!-- http://purl.org/dc/elements/1.1/date -->

    <owl:AnnotationProperty rdf:about="http://purl.org/dc/elements/1.1/date"/>
    


    <!-- http://purl.org/dc/elements/1.1/description -->

    <owl:AnnotationProperty rdf:about="http://purl.org/dc/elements/1.1/description"/>
    


    <!-- http://purl.org/dc/elements/1.1/format -->

    <owl:AnnotationProperty rdf:about="http://purl.org/dc/elements/1.1/format"/>
    


    <!-- http://purl.org/dc/elements/1.1/identifier -->

    <owl:AnnotationProperty rdf:about="http://purl.org/dc/elements/1.1/identifier"/>
    


    <!-- http://purl.org/dc/elements/1.1/rights -->

    <owl:AnnotationProperty rdf:about="http://purl.org/dc/elements/1.1/rights"/>
    


    <!-- http://purl.org/dc/elements/1.1/source -->

    <owl:AnnotationProperty rdf:about="http://purl.org/dc/elements/1.1/source"/>
    


    <!-- http://purl.org/dc/elements/1.1/title -->

    <owl:AnnotationProperty rdf:about="http://purl.org/dc/elements/1.1/title"/>
    


    <!-- http://purl.org/dc/elements/1.1/type -->

    <owl:AnnotationProperty rdf:about="http://purl.org/dc/elements/1.1/type"/>
    


    <!-- http://purl.org/dc/terms/created -->

    <owl:AnnotationProperty rdf:about="http://purl.org/dc/terms/created"/>
    


    <!-- http://purl.org/dc/terms/modified -->

    <owl:AnnotationProperty rdf:about="http://purl.org/dc/terms/modified"/>
    


    <!-- http://www.w3.org/2003/12/exif/ns#apertureValue -->

    <owl:AnnotationProperty rdf:about="http://www.w3.org/2003/12/exif/ns#apertureValue">
        <rdfs:subPropertyOf rdf:resource="http://www.w3.org/2003/12/exif/ns#pictTaking"/>
    </owl:AnnotationProperty>
    


    <!-- http://www.w3.org/2003/12/exif/ns#artist -->

    <owl:AnnotationProperty rdf:about="http://www.w3.org/2003/12/exif/ns#artist">
        <rdfs:comment xml:lang="en">Person who created the image</rdfs:comment>
        <rdfs:label xml:lang="en">Artist</rdfs:label>
        <tagNumber xml:lang="en">315</tagNumber>
        <rdfs:subPropertyOf rdf:resource="http://purl.org/dc/elements/1.1/creator"/>
        <rdfs:subPropertyOf rdf:resource="http://www.w3.org/2003/12/exif/ns#exifAttribute"/>
    </owl:AnnotationProperty>
    


    <!-- http://www.w3.org/2003/12/exif/ns#bitsPerSample -->

    <owl:AnnotationProperty rdf:about="http://www.w3.org/2003/12/exif/ns#bitsPerSample">
        <rdfs:comment xml:lang="en">The number of bits per image component. In this standard each component of the image is 8 bits, so the value for this tag is 8. See also SamplesPerPixel. In JPEG compressed data a JPEG marker is used instead of this tag.</rdfs:comment>
        <rdfs:label xml:lang="en">BitsPerSample</rdfs:label>
        <tagNumber xml:lang="en">258</tagNumber>
        <rdfs:subPropertyOf rdf:resource="http://www.w3.org/2003/12/exif/ns#imageDataStruct"/>
        <rdfs:subPropertyOf rdf:resource="http://www.w3.org/2003/12/exif/ns#resolution"/>
    </owl:AnnotationProperty>
    


    <!-- http://www.w3.org/2003/12/exif/ns#brightnessValue -->

    <owl:AnnotationProperty rdf:about="http://www.w3.org/2003/12/exif/ns#brightnessValue">
        <rdfs:comment xml:lang="en">The value of brightness. The unit is the APEX value. Ordinarily it is given in the range of -99.99 to 99.99. Note that if the numerator of the recorded value is FFFFFFFF.H, Unknown shall be indicated.</rdfs:comment>
        <rdfs:comment xml:lang="ja">画像撮影時の撮影対象物の明るさ（APEX値）。EVにするにはISO感度の値を足す必要があり、Ev:Exposure, Bv:BrightnessValue, Sv:SensitivityValueとしてEv=Bv+Sv Sv=log^2(ISOSpeedRating/3.125)という計算式を使う。ISO感度100の場合Sv=5、ISO200の場合Sv=6、ISO125ではSv=5.32</rdfs:comment>
        <rdfs:label xml:lang="en">BrightnessValue</rdfs:label>
        <tagNumber xml:lang="en">37379</tagNumber>
        <rdfs:subPropertyOf rdf:resource="http://www.w3.org/2003/12/exif/ns#pictTaking"/>
    </owl:AnnotationProperty>
    


    <!-- http://www.w3.org/2003/12/exif/ns#cfaPattern -->

    <owl:AnnotationProperty rdf:about="http://www.w3.org/2003/12/exif/ns#cfaPattern">
        <rdfs:comment xml:lang="ja">CCDに付いているColor filter array(CFA)のパターン。例えば普通のRGBフィルターだと、CFAPatternのデータは 02 02 00 01 01 02</rdfs:comment>
        <rdfs:comment xml:lang="en">The color filter array (CFA) geometric pattern of the image sensor when a one-chip color area sensor is used. It does not apply to all sensing methods.</rdfs:comment>
        <rdfs:label xml:lang="en">CFAPattern</rdfs:label>
        <tagNumber xml:lang="en">41730</tagNumber>
        <rdfs:subPropertyOf rdf:resource="http://www.w3.org/2003/12/exif/ns#pictTaking"/>
    </owl:AnnotationProperty>
    


    <!-- http://www.w3.org/2003/12/exif/ns#colorSpace -->

    <owl:AnnotationProperty rdf:about="http://www.w3.org/2003/12/exif/ns#colorSpace">
        <rdfs:comment xml:lang="en">The color space information tag (ColorSpace) is always recorded as the color space specifier. Normally sRGB (=1) is used to define the color space based on the PC monitor conditions and environment.</rdfs:comment>
        <rdfs:comment xml:lang="ja">使われる色空間。通常sRGB</rdfs:comment>
        <rdfs:label xml:lang="en">ColorSpace</rdfs:label>
        <tagNumber xml:lang="en">40961</tagNumber>
        <rdfs:subPropertyOf rdf:resource="http://www.w3.org/2003/12/exif/ns#imageDataCharacter"/>
    </owl:AnnotationProperty>
    


    <!-- http://www.w3.org/2003/12/exif/ns#componentsConfiguration -->

    <owl:AnnotationProperty rdf:about="http://www.w3.org/2003/12/exif/ns#componentsConfiguration">
        <rdfs:comment xml:lang="en">Information specific to compressed data. The channels of each component are arranged in order from the 1st component to the 4th. For uncompressed data the data arrangement is given in the PhotometricInterpretation tag. However, since PhotometricInterpretation can only express the order of Y,Cb and Cr, this tag is provided for cases when compressed data uses components other than Y, Cb, and Cr and to enable support of other sequences.</rdfs:comment>
        <rdfs:comment xml:lang="ja">圧縮データがYCC以外の並びの場合、4バイトでその並びを示す。それぞれの値は0:not exist,1:Y,2:Cb,3:Cr,4:R,5:G,6:B</rdfs:comment>
        <rdfs:label xml:lang="en">ComponentsConfiguration</rdfs:label>
        <tagNumber xml:lang="en">37121</tagNumber>
        <rdfs:subPropertyOf rdf:resource="http://www.w3.org/2003/12/exif/ns#imageConfig"/>
    </owl:AnnotationProperty>
    


    <!-- http://www.w3.org/2003/12/exif/ns#compressedBitsPerPixel -->

    <owl:AnnotationProperty rdf:about="http://www.w3.org/2003/12/exif/ns#compressedBitsPerPixel">
        <rdfs:comment xml:lang="en">Information specific to compressed data. The compression mode used for a compressed image is indicated in unit bits per pixel.</rdfs:comment>
        <rdfs:comment xml:lang="ja">画像の圧縮率</rdfs:comment>
        <rdfs:label xml:lang="en">CompressedBitsPerPixel</rdfs:label>
        <tagNumber xml:lang="en">37122</tagNumber>
        <rdfs:subPropertyOf rdf:resource="http://www.w3.org/2003/12/exif/ns#imageConfig"/>
    </owl:AnnotationProperty>
    


    <!-- http://www.w3.org/2003/12/exif/ns#compression -->

    <owl:AnnotationProperty rdf:about="http://www.w3.org/2003/12/exif/ns#compression">
        <rdfs:comment xml:lang="en">The compression scheme used for the image data. When a primary image is JPEG compressed, this designation is not necessary and is omitted. When thumbnails use JPEG compression, this tag value is set to 6.</rdfs:comment>
        <rdfs:label xml:lang="en">Compression</rdfs:label>
        <tagNumber xml:lang="en">259</tagNumber>
        <rdfs:subPropertyOf rdf:resource="http://www.w3.org/2003/12/exif/ns#imageDataStruct"/>
    </owl:AnnotationProperty>
    


    <!-- http://www.w3.org/2003/12/exif/ns#contrast -->

    <owl:AnnotationProperty rdf:about="http://www.w3.org/2003/12/exif/ns#contrast">
        <rdfs:comment xml:lang="en">The direction of contrast processing applied by the camera when the image was shot.</rdfs:comment>
        <rdfs:label xml:lang="en">Contrast</rdfs:label>
        <tagNumber xml:lang="en">41992</tagNumber>
        <rdfs:subPropertyOf rdf:resource="http://www.w3.org/2003/12/exif/ns#pictTaking"/>
    </owl:AnnotationProperty>
    


    <!-- http://www.w3.org/2003/12/exif/ns#copyright -->

    <owl:AnnotationProperty rdf:about="http://www.w3.org/2003/12/exif/ns#copyright">
        <rdfs:comment xml:lang="en">Copyright information. In this standard the tag is used to indicate both the photographer and editor copyrights. It is the copyright notice of the person or organization claiming rights to the image.</rdfs:comment>
        <rdfs:comment xml:lang="ja">この画像の撮影者および編集者の著作権情報</rdfs:comment>
        <rdfs:label xml:lang="en">Copyright</rdfs:label>
        <tagNumber xml:lang="en">33432</tagNumber>
        <rdfs:subPropertyOf rdf:resource="http://purl.org/dc/elements/1.1/rights"/>
        <rdfs:subPropertyOf rdf:resource="http://www.w3.org/2003/12/exif/ns#exifAttribute"/>
    </owl:AnnotationProperty>
    


    <!-- http://www.w3.org/2003/12/exif/ns#customRendered -->

    <owl:AnnotationProperty rdf:about="http://www.w3.org/2003/12/exif/ns#customRendered">
        <rdfs:comment xml:lang="en">The use of special processing on image data, such as rendering geared to output. When special processing is performed, the reader is expected to disable or minimize any further processing.</rdfs:comment>
        <rdfs:comment xml:lang="ja">特別なレンダリング処理を行っているかどうか</rdfs:comment>
        <rdfs:label xml:lang="en">CustomRendered</rdfs:label>
        <tagNumber xml:lang="en">41985</tagNumber>
        <rdfs:subPropertyOf rdf:resource="http://www.w3.org/2003/12/exif/ns#pictTaking"/>
    </owl:AnnotationProperty>
    


    <!-- http://www.w3.org/2003/12/exif/ns#datatype -->

    <owl:AnnotationProperty rdf:about="http://www.w3.org/2003/12/exif/ns#datatype">
        <rdfs:comment xml:lang="en">The Exif field data type, such as ascii, byte, short etc.</rdfs:comment>
        <rdfs:label xml:lang="en">Data Type</rdfs:label>
        <rdfs:subPropertyOf rdf:resource="http://purl.org/dc/elements/1.1/type"/>
    </owl:AnnotationProperty>
    


    <!-- http://www.w3.org/2003/12/exif/ns#date -->

    <owl:AnnotationProperty rdf:about="http://www.w3.org/2003/12/exif/ns#date">
        <rdfs:comment xml:lang="en">a date information. Usually saved as YYYY:MM:DD (HH:MM:SS) format in Exif data, but represented here as W3C-DTF format</rdfs:comment>
        <rdfs:label xml:lang="en">Date</rdfs:label>
        <rdfs:subPropertyOf rdf:resource="http://purl.org/dc/elements/1.1/date"/>
    </owl:AnnotationProperty>
    


    <!-- http://www.w3.org/2003/12/exif/ns#dateAndOrTime -->

    <owl:AnnotationProperty rdf:about="http://www.w3.org/2003/12/exif/ns#dateAndOrTime">
        <rdfs:comment xml:lang="en">An attribute relating to Date and/or Time</rdfs:comment>
        <rdfs:label xml:lang="en">Date and/or Time</rdfs:label>
        <rdfs:subPropertyOf rdf:resource="http://www.w3.org/2003/12/exif/ns#exifAttribute"/>
    </owl:AnnotationProperty>
    


    <!-- http://www.w3.org/2003/12/exif/ns#dateTime -->

    <owl:AnnotationProperty rdf:about="http://www.w3.org/2003/12/exif/ns#dateTime">
        <rdfs:comment xml:lang="en">The date and time of image creation. In this standard it is the date and time the file was changed.</rdfs:comment>
        <rdfs:comment xml:lang="ja">この画像が作成（あるいは最後に変更された）日時。通常はDateTimeOriginaと同じ値</rdfs:comment>
        <rdfs:label xml:lang="en">DateTime</rdfs:label>
        <tagNumber xml:lang="en">306</tagNumber>
        <rdfs:subPropertyOf rdf:resource="http://www.w3.org/2003/12/exif/ns#date"/>
        <rdfs:subPropertyOf rdf:resource="http://www.w3.org/2003/12/exif/ns#exifAttribute"/>
    </owl:AnnotationProperty>
    


    <!-- http://www.w3.org/2003/12/exif/ns#dateTimeDigitized -->

    <owl:AnnotationProperty rdf:about="http://www.w3.org/2003/12/exif/ns#dateTimeDigitized">
        <rdfs:comment xml:lang="en">The date and time when the image was stored as digital data. If, for example, an image was captured by DSC and at the same time the file was recorded, then the DateTimeOriginal and DateTimeDigitized will have the same contents.</rdfs:comment>
        <rdfs:comment xml:lang="ja">画像がデジタル化された日時。デジカメ画像なら通常DateTimeOriginalと同じ値</rdfs:comment>
        <rdfs:label xml:lang="en">DateTimeDigitized</rdfs:label>
        <tagNumber xml:lang="en">36868</tagNumber>
        <rdfs:subPropertyOf rdf:resource="http://www.w3.org/2003/12/exif/ns#date"/>
        <rdfs:subPropertyOf rdf:resource="http://www.w3.org/2003/12/exif/ns#dateAndOrTime"/>
    </owl:AnnotationProperty>
    


    <!-- http://www.w3.org/2003/12/exif/ns#dateTimeOriginal -->

    <owl:AnnotationProperty rdf:about="http://www.w3.org/2003/12/exif/ns#dateTimeOriginal">
        <rdfs:comment xml:lang="en">The date and time when the original image data was generated. For a DSC the date and time the picture was taken are recorded.</rdfs:comment>
        <rdfs:comment xml:lang="ja">オリジナル画像が作成（撮影）された日時</rdfs:comment>
        <rdfs:label xml:lang="en">DateTimeOriginal</rdfs:label>
        <tagNumber xml:lang="en">36867</tagNumber>
        <rdfs:subPropertyOf rdf:resource="http://www.w3.org/2003/12/exif/ns#date"/>
        <rdfs:subPropertyOf rdf:resource="http://www.w3.org/2003/12/exif/ns#dateAndOrTime"/>
    </owl:AnnotationProperty>
    


    <!-- http://www.w3.org/2003/12/exif/ns#deviceSettingDescription -->

    <owl:AnnotationProperty rdf:about="http://www.w3.org/2003/12/exif/ns#deviceSettingDescription">
        <rdfs:comment xml:lang="en">Information on the picture-taking conditions of a particular camera model. The tag is used only to indicate the picture-taking conditions in the reader.</rdfs:comment>
        <rdfs:label xml:lang="en">DeviceSettingDescription</rdfs:label>
        <tagNumber xml:lang="en">41995</tagNumber>
        <rdfs:subPropertyOf rdf:resource="http://www.w3.org/2003/12/exif/ns#pictTaking"/>
    </owl:AnnotationProperty>
    


    <!-- http://www.w3.org/2003/12/exif/ns#digitalZoomRatio -->

    <owl:AnnotationProperty rdf:about="http://www.w3.org/2003/12/exif/ns#digitalZoomRatio">
        <rdfs:comment xml:lang="en">The digital zoom ratio when the image was shot. If the numerator of the recorded value is 0, this indicates that digital zoom was not used.</rdfs:comment>
        <rdfs:comment xml:lang="ja">デジタルズームが使われた場合、その比率</rdfs:comment>
        <rdfs:label xml:lang="en">DigitalZoomRatio</rdfs:label>
        <tagNumber xml:lang="en">41988</tagNumber>
        <rdfs:subPropertyOf rdf:resource="http://www.w3.org/2003/12/exif/ns#pictTaking"/>
    </owl:AnnotationProperty>
    


    <!-- http://www.w3.org/2003/12/exif/ns#exifAttribute -->

    <owl:AnnotationProperty rdf:about="http://www.w3.org/2003/12/exif/ns#exifAttribute">
        <rdfs:comment xml:lang="en">A property that connects an IFD to one of its entries. Super property which integrates all Exif tags.</rdfs:comment>
        <rdfs:label xml:lang="en">Exif Attribute</rdfs:label>
        <rdfs:domain rdf:resource="http://www.w3.org/2003/12/exif/ns#IFD"/>
    </owl:AnnotationProperty>
    


    <!-- http://www.w3.org/2003/12/exif/ns#exifVersion -->

    <owl:AnnotationProperty rdf:about="http://www.w3.org/2003/12/exif/ns#exifVersion">
        <rdfs:comment xml:lang="en">Exif Version</rdfs:comment>
        <rdfs:comment xml:lang="ja">Exif形式のバージョン</rdfs:comment>
        <rdfs:label xml:lang="en">ExifVersion</rdfs:label>
        <tagNumber xml:lang="en">36864</tagNumber>
        <rdfs:subPropertyOf rdf:resource="http://www.w3.org/2003/12/exif/ns#versionInfo"/>
    </owl:AnnotationProperty>
    


    <!-- http://www.w3.org/2003/12/exif/ns#exif_IFD_Pointer -->

    <owl:AnnotationProperty rdf:about="http://www.w3.org/2003/12/exif/ns#exif_IFD_Pointer">
        <rdfs:comment xml:lang="en">A pointer to the Exif IFD, which is a set of tags for recording Exif-specific attribute information.</rdfs:comment>
        <rdfs:comment xml:lang="ja">Exif IFDへのポインタ</rdfs:comment>
        <rdfs:label xml:lang="en">Exif IFD Pointer</rdfs:label>
        <tagNumber xml:lang="en">34665</tagNumber>
        <rdfs:subPropertyOf rdf:resource="http://www.w3.org/2003/12/exif/ns#ifdPointer"/>
    </owl:AnnotationProperty>
    


    <!-- http://www.w3.org/2003/12/exif/ns#exposureBiasValue -->

    <owl:AnnotationProperty rdf:about="http://www.w3.org/2003/12/exif/ns#exposureBiasValue">
        <rdfs:comment xml:lang="en">The exposure bias. The unit is the APEX value. Ordinarily it is given in the range of -99.99 to 99.99.</rdfs:comment>
        <rdfs:comment xml:lang="ja">撮影時の露光補正量。単位はAPEX値(EV)</rdfs:comment>
        <rdfs:label xml:lang="en">ExposureBiasValue</rdfs:label>
        <tagNumber xml:lang="en">37380</tagNumber>
        <rdfs:subPropertyOf rdf:resource="http://www.w3.org/2003/12/exif/ns#pictTaking"/>
    </owl:AnnotationProperty>
    


    <!-- http://www.w3.org/2003/12/exif/ns#exposureIndex -->

    <owl:AnnotationProperty rdf:about="http://www.w3.org/2003/12/exif/ns#exposureIndex">
        <rdfs:comment xml:lang="ja">CCD感度。データ形式が符号なし分数である事を除き、ISOSpeedRatingsと同じ</rdfs:comment>
        <rdfs:comment xml:lang="en">The exposure index selected on the camera or input device at the time the image is captured.</rdfs:comment>
        <rdfs:label xml:lang="en">ExposureIndex</rdfs:label>
        <tagNumber xml:lang="en">41493</tagNumber>
        <rdfs:subPropertyOf rdf:resource="http://www.w3.org/2003/12/exif/ns#pictTaking"/>
    </owl:AnnotationProperty>
    


    <!-- http://www.w3.org/2003/12/exif/ns#exposureMode -->

    <owl:AnnotationProperty rdf:about="http://www.w3.org/2003/12/exif/ns#exposureMode">
        <rdfs:comment xml:lang="en">the exposure mode set when the image was shot. In auto-bracketing mode, the camera shoots a series of frames of the same scene at different exposure settings.</rdfs:comment>
        <rdfs:comment xml:lang="ja">露光モード</rdfs:comment>
        <rdfs:label xml:lang="en">ExposureMode</rdfs:label>
        <tagNumber xml:lang="en">41986</tagNumber>
        <rdfs:subPropertyOf rdf:resource="http://www.w3.org/2003/12/exif/ns#pictTaking"/>
    </owl:AnnotationProperty>
    


    <!-- http://www.w3.org/2003/12/exif/ns#exposureProgram -->

    <owl:AnnotationProperty rdf:about="http://www.w3.org/2003/12/exif/ns#exposureProgram">
        <rdfs:comment xml:lang="en">The class of the program used by the camera to set exposure when the picture is taken.</rdfs:comment>
        <rdfs:comment xml:lang="ja">露光制御のモード</rdfs:comment>
        <rdfs:label xml:lang="en">ExposureProgram</rdfs:label>
        <tagNumber xml:lang="en">34850</tagNumber>
        <rdfs:subPropertyOf rdf:resource="http://www.w3.org/2003/12/exif/ns#pictTaking"/>
    </owl:AnnotationProperty>
    


    <!-- http://www.w3.org/2003/12/exif/ns#exposureTime -->

    <owl:AnnotationProperty rdf:about="http://www.w3.org/2003/12/exif/ns#exposureTime">
        <rdfs:comment xml:lang="en">Exposure time, given in seconds (sec).</rdfs:comment>
        <rdfs:comment xml:lang="ja">露光時間（シャッター速度の逆数）。単位は秒</rdfs:comment>
        <rdfs:label xml:lang="en">ExposureTime</rdfs:label>
        <tagNumber xml:lang="en">33434</tagNumber>
        <rdfs:subPropertyOf rdf:resource="http://www.w3.org/2003/12/exif/ns#pictTaking"/>
        <rdfs:subPropertyOf rdf:resource="http://www.w3.org/2003/12/exif/ns#seconds"/>
    </owl:AnnotationProperty>
    


    <!-- http://www.w3.org/2003/12/exif/ns#fNumber -->

    <owl:AnnotationProperty rdf:about="http://www.w3.org/2003/12/exif/ns#fNumber">
        <rdfs:comment xml:lang="en">F number</rdfs:comment>
        <rdfs:comment xml:lang="ja">レンズのF値</rdfs:comment>
        <rdfs:label xml:lang="en">FNumber</rdfs:label>
        <tagNumber xml:lang="en">33437</tagNumber>
        <rdfs:subPropertyOf rdf:resource="http://www.w3.org/2003/12/exif/ns#pictTaking"/>
    </owl:AnnotationProperty>
    


    <!-- http://www.w3.org/2003/12/exif/ns#fileSource -->

    <owl:AnnotationProperty rdf:about="http://www.w3.org/2003/12/exif/ns#fileSource">
        <rdfs:comment xml:lang="en">The image source. If a DSC recorded the image, this tag value of this tag always be set to 3, indicating that the image was recorded on a DSC.</rdfs:comment>
        <rdfs:comment xml:lang="ja">画像がどういうデバイスから得られたか。通常3=DSC</rdfs:comment>
        <rdfs:label xml:lang="en">FileSource</rdfs:label>
        <tagNumber xml:lang="en">41728</tagNumber>
        <rdfs:subPropertyOf rdf:resource="http://www.w3.org/2003/12/exif/ns#pictTaking"/>
    </owl:AnnotationProperty>
    


    <!-- http://www.w3.org/2003/12/exif/ns#flash -->

    <owl:AnnotationProperty rdf:about="http://www.w3.org/2003/12/exif/ns#flash">
        <rdfs:comment xml:lang="en">The status of flash when the image was shot.</rdfs:comment>
        <rdfs:comment xml:lang="ja">フラッシュ発光の状態</rdfs:comment>
        <rdfs:label xml:lang="en">Flash</rdfs:label>
        <tagNumber xml:lang="en">37385</tagNumber>
        <rdfs:subPropertyOf rdf:resource="http://www.w3.org/2003/12/exif/ns#pictTaking"/>
    </owl:AnnotationProperty>
    


    <!-- http://www.w3.org/2003/12/exif/ns#flashEnergy -->

    <owl:AnnotationProperty rdf:about="http://www.w3.org/2003/12/exif/ns#flashEnergy">
        <rdfs:comment xml:lang="ja">BCPSによるストロボの強度</rdfs:comment>
        <rdfs:comment xml:lang="en">The strobe energy at the time the image is captured, as measured in Beam Candle Power Seconds (BCPS).</rdfs:comment>
        <rdfs:label xml:lang="en">FlashEnergy</rdfs:label>
        <tagNumber xml:lang="en">41483</tagNumber>
        <rdfs:subPropertyOf rdf:resource="http://www.w3.org/2003/12/exif/ns#pictTaking"/>
    </owl:AnnotationProperty>
    


    <!-- http://www.w3.org/2003/12/exif/ns#flashpixVersion -->

    <owl:AnnotationProperty rdf:about="http://www.w3.org/2003/12/exif/ns#flashpixVersion">
        <rdfs:comment xml:lang="en">The Flashpix format version supported by a FPXR file. If the FPXR function supports Flashpix format Ver. 1.0, this is indicated similarly to ExifVersion by recording &quot;0100&quot; as 4-byte ASCII.</rdfs:comment>
        <rdfs:label xml:lang="en">FlashpixVersion</rdfs:label>
        <tagNumber xml:lang="en">40960</tagNumber>
        <rdfs:subPropertyOf rdf:resource="http://www.w3.org/2003/12/exif/ns#versionInfo"/>
    </owl:AnnotationProperty>
    


    <!-- http://www.w3.org/2003/12/exif/ns#focalLength -->

    <owl:AnnotationProperty rdf:about="http://www.w3.org/2003/12/exif/ns#focalLength">
        <rdfs:comment xml:lang="en">The actual focal length of the lens, in mm. Conversion is not made to the focal length of a 35 mm film camera.</rdfs:comment>
        <rdfs:comment xml:lang="ja">レンズの焦点距離。単位はmm</rdfs:comment>
        <rdfs:label xml:lang="en">FocalLength</rdfs:label>
        <tagNumber xml:lang="en">37386</tagNumber>
        <rdfs:subPropertyOf rdf:resource="http://www.w3.org/2003/12/exif/ns#mm"/>
        <rdfs:subPropertyOf rdf:resource="http://www.w3.org/2003/12/exif/ns#pictTaking"/>
    </owl:AnnotationProperty>
    


    <!-- http://www.w3.org/2003/12/exif/ns#focalLengthIn35mmFilm -->

    <owl:AnnotationProperty rdf:about="http://www.w3.org/2003/12/exif/ns#focalLengthIn35mmFilm">
        <rdfs:comment xml:lang="ja">35mm換算した焦点距離</rdfs:comment>
        <rdfs:comment xml:lang="en">The equivalent focal length assuming a 35mm film camera, in mm. A value of 0 means the focal length is unknown. Note that this tag differs from the FocalLength tag.</rdfs:comment>
        <rdfs:label xml:lang="en">FocalLengthIn35mmFilm</rdfs:label>
        <tagNumber xml:lang="en">41989</tagNumber>
        <rdfs:subPropertyOf rdf:resource="http://www.w3.org/2003/12/exif/ns#length"/>
        <rdfs:subPropertyOf rdf:resource="http://www.w3.org/2003/12/exif/ns#pictTaking"/>
    </owl:AnnotationProperty>
    


    <!-- http://www.w3.org/2003/12/exif/ns#focalPlaneResolutionUnit -->

    <owl:AnnotationProperty rdf:about="http://www.w3.org/2003/12/exif/ns#focalPlaneResolutionUnit">
        <rdfs:comment xml:lang="ja">CCD画素密度の単位</rdfs:comment>
        <rdfs:comment xml:lang="en">The unit for measuring FocalPlaneXResolution and FocalPlaneYResolution. This value is the same as the ResolutionUnit.</rdfs:comment>
        <rdfs:label xml:lang="en">FocalPlaneResolutionUnit</rdfs:label>
        <tagNumber xml:lang="en">41488</tagNumber>
        <rdfs:subPropertyOf rdf:resource="http://www.w3.org/2003/12/exif/ns#pictTaking"/>
    </owl:AnnotationProperty>
    


    <!-- http://www.w3.org/2003/12/exif/ns#focalPlaneXResolution -->

    <owl:AnnotationProperty rdf:about="http://www.w3.org/2003/12/exif/ns#focalPlaneXResolution">
        <rdfs:comment xml:lang="en">The number of pixels in the image width (X) direction per FocalPlaneResolutionUnit on the camera focal plane.</rdfs:comment>
        <rdfs:comment xml:lang="ja">撮影画像のCCD位置での水平解像度。この値とFocalPlaneYResolution、FocalLengthを使うと、レンズ焦点距離の35mmカメラ換算値が計算できる。例えば200万画素機を使いVGAモードの画像を撮ったような場合はこの値はVGAの解像度でリサンプルされた値になっており、CCDの画素ピッチそのままの値ではないので注意が必要</rdfs:comment>
        <rdfs:label xml:lang="en">FocalPlaneXResolution</rdfs:label>
        <tagNumber xml:lang="en">41486</tagNumber>
        <rdfs:subPropertyOf rdf:resource="http://www.w3.org/2003/12/exif/ns#pictTaking"/>
        <rdfs:subPropertyOf rdf:resource="http://www.w3.org/2003/12/exif/ns#resolution"/>
    </owl:AnnotationProperty>
    


    <!-- http://www.w3.org/2003/12/exif/ns#focalPlaneYResolution -->

    <owl:AnnotationProperty rdf:about="http://www.w3.org/2003/12/exif/ns#focalPlaneYResolution">
        <rdfs:comment xml:lang="en">The number of pixels in the image height (Y) direction per FocalPlaneResolutionUnit on the camera focal plane.</rdfs:comment>
        <rdfs:comment xml:lang="ja">撮影画像のCCD位置での垂直解像度</rdfs:comment>
        <rdfs:label xml:lang="en">FocalPlaneYResolution</rdfs:label>
        <tagNumber xml:lang="en">41487</tagNumber>
        <rdfs:subPropertyOf rdf:resource="http://www.w3.org/2003/12/exif/ns#pictTaking"/>
        <rdfs:subPropertyOf rdf:resource="http://www.w3.org/2003/12/exif/ns#resolution"/>
    </owl:AnnotationProperty>
    


    <!-- http://www.w3.org/2003/12/exif/ns#gainControl -->

    <owl:AnnotationProperty rdf:about="http://www.w3.org/2003/12/exif/ns#gainControl">
        <rdfs:comment xml:lang="en">The degree of overall image gain adjustment.</rdfs:comment>
        <rdfs:label xml:lang="en">GainControl</rdfs:label>
        <tagNumber xml:lang="en">41991</tagNumber>
        <rdfs:subPropertyOf rdf:resource="http://www.w3.org/2003/12/exif/ns#pictTaking"/>
    </owl:AnnotationProperty>
    


    <!-- http://www.w3.org/2003/12/exif/ns#geo -->

    <owl:AnnotationProperty rdf:about="http://www.w3.org/2003/12/exif/ns#geo">
        <rdfs:comment xml:lang="en">Geometric data such as latitude, longitude and altitude. Usually saved as rational number.</rdfs:comment>
        <rdfs:label xml:lang="en">Geometric data</rdfs:label>
    </owl:AnnotationProperty>
    


    <!-- http://www.w3.org/2003/12/exif/ns#gpsAltitude -->

    <owl:AnnotationProperty rdf:about="http://www.w3.org/2003/12/exif/ns#gpsAltitude">
        <rdfs:comment xml:lang="en">The altitude based on the reference in GPSAltitudeRef. Altitude is expressed as one RATIONAL value. The reference unit is meters.</rdfs:comment>
        <rdfs:label xml:lang="en">GPSAltitude</rdfs:label>
        <tagNumber xml:lang="en">6</tagNumber>
        <rdfs:subPropertyOf rdf:resource="http://www.w3.org/2003/12/exif/ns#geo"/>
        <rdfs:subPropertyOf rdf:resource="http://www.w3.org/2003/12/exif/ns#gpsInfo"/>
    </owl:AnnotationProperty>
    


    <!-- http://www.w3.org/2003/12/exif/ns#gpsAltitudeRef -->

    <owl:AnnotationProperty rdf:about="http://www.w3.org/2003/12/exif/ns#gpsAltitudeRef">
        <rdfs:comment xml:lang="en">Indicates the altitude used as the reference altitude. If the reference is sea level and the altitude is above sea level, 0 is given. If the altitude is below sea level, a value of 1 is given and the altitude is indicated as an absolute value in the GPSAltitude tag. The reference unit is meters.</rdfs:comment>
        <rdfs:label xml:lang="en">GPSAltitudeRef</rdfs:label>
        <tagNumber xml:lang="en">5</tagNumber>
        <rdfs:subPropertyOf rdf:resource="http://www.w3.org/2003/12/exif/ns#gpsInfo"/>
    </owl:AnnotationProperty>
    


    <!-- http://www.w3.org/2003/12/exif/ns#gpsAreaInformation -->

    <owl:AnnotationProperty rdf:about="http://www.w3.org/2003/12/exif/ns#gpsAreaInformation">
        <rdfs:comment xml:lang="en">A character string recording the name of the GPS area. The first byte indicates the character code used, and this is followed by the name of the GPS area.</rdfs:comment>
        <rdfs:label xml:lang="en">GPSAreaInformation</rdfs:label>
        <tagNumber xml:lang="en">28</tagNumber>
        <rdfs:subPropertyOf rdf:resource="http://www.w3.org/2003/12/exif/ns#gpsInfo"/>
    </owl:AnnotationProperty>
    


    <!-- http://www.w3.org/2003/12/exif/ns#gpsDOP -->

    <owl:AnnotationProperty rdf:about="http://www.w3.org/2003/12/exif/ns#gpsDOP">
        <rdfs:comment xml:lang="en">The GPS DOP (data degree of precision). An HDOP value is written during two-dimensional measurement, and PDOP during three-dimensional measurement.</rdfs:comment>
        <rdfs:label xml:lang="en">GPSDOP</rdfs:label>
        <tagNumber xml:lang="en">11</tagNumber>
        <rdfs:subPropertyOf rdf:resource="http://www.w3.org/2003/12/exif/ns#gpsInfo"/>
    </owl:AnnotationProperty>
    


    <!-- http://www.w3.org/2003/12/exif/ns#gpsDateStamp -->

    <owl:AnnotationProperty rdf:about="http://www.w3.org/2003/12/exif/ns#gpsDateStamp">
        <rdfs:comment xml:lang="en">date and time information relative to UTC (Coordinated Universal Time). The record format is &quot;YYYY:MM:DD&quot; while converted to W3C-DTF to use in RDF</rdfs:comment>
        <rdfs:label xml:lang="en">GPSDateStamp</rdfs:label>
        <tagNumber xml:lang="en">29</tagNumber>
        <rdfs:subPropertyOf rdf:resource="http://www.w3.org/2003/12/exif/ns#date"/>
        <rdfs:subPropertyOf rdf:resource="http://www.w3.org/2003/12/exif/ns#gpsInfo"/>
    </owl:AnnotationProperty>
    


    <!-- http://www.w3.org/2003/12/exif/ns#gpsDestBearing -->

    <owl:AnnotationProperty rdf:about="http://www.w3.org/2003/12/exif/ns#gpsDestBearing">
        <rdfs:comment xml:lang="en">The bearing to the destination point. The range of values is from 0.00 to 359.99.</rdfs:comment>
        <rdfs:label xml:lang="en">GPSDestBearing</rdfs:label>
        <tagNumber xml:lang="en">24</tagNumber>
        <rdfs:subPropertyOf rdf:resource="http://www.w3.org/2003/12/exif/ns#gpsInfo"/>
    </owl:AnnotationProperty>
    


    <!-- http://www.w3.org/2003/12/exif/ns#gpsDestBearingRef -->

    <owl:AnnotationProperty rdf:about="http://www.w3.org/2003/12/exif/ns#gpsDestBearingRef">
        <rdfs:comment xml:lang="en">Indicates the reference used for giving the bearing to the destination point. &apos;T&apos; denotes true direction and &apos;M&apos; is magnetic direction.</rdfs:comment>
        <rdfs:label xml:lang="en">GPSDestBearingRef</rdfs:label>
        <tagNumber xml:lang="en">23</tagNumber>
        <rdfs:subPropertyOf rdf:resource="http://www.w3.org/2003/12/exif/ns#gpsInfo"/>
    </owl:AnnotationProperty>
    


    <!-- http://www.w3.org/2003/12/exif/ns#gpsDestDistance -->

    <owl:AnnotationProperty rdf:about="http://www.w3.org/2003/12/exif/ns#gpsDestDistance">
        <rdfs:comment xml:lang="en">The distance to the destination point.</rdfs:comment>
        <rdfs:label xml:lang="en">GPSDestDistance</rdfs:label>
        <tagNumber xml:lang="en">26</tagNumber>
        <rdfs:subPropertyOf rdf:resource="http://www.w3.org/2003/12/exif/ns#gpsInfo"/>
    </owl:AnnotationProperty>
    


    <!-- http://www.w3.org/2003/12/exif/ns#gpsDestDistanceRef -->

    <owl:AnnotationProperty rdf:about="http://www.w3.org/2003/12/exif/ns#gpsDestDistanceRef">
        <rdfs:comment xml:lang="en">Indicates the unit used to express the distance to the destination point. &apos;K&apos;, &apos;M&apos; and &apos;N&apos; represent kilometers, miles and knots.</rdfs:comment>
        <rdfs:label xml:lang="en">GPSDestDistanceRef</rdfs:label>
        <tagNumber xml:lang="en">25</tagNumber>
        <rdfs:subPropertyOf rdf:resource="http://www.w3.org/2003/12/exif/ns#gpsInfo"/>
    </owl:AnnotationProperty>
    


    <!-- http://www.w3.org/2003/12/exif/ns#gpsDestLatitude -->

    <owl:AnnotationProperty rdf:about="http://www.w3.org/2003/12/exif/ns#gpsDestLatitude">
        <rdfs:comment xml:lang="en">Latitude of destination, expressed as three values giving the degrees, minutes, and seconds, respectively.</rdfs:comment>
        <rdfs:label xml:lang="en">GPSDestLatitude</rdfs:label>
        <tagNumber xml:lang="en">20</tagNumber>
        <rdfs:subPropertyOf rdf:resource="http://www.w3.org/2003/12/exif/ns#geo"/>
        <rdfs:subPropertyOf rdf:resource="http://www.w3.org/2003/12/exif/ns#gpsInfo"/>
    </owl:AnnotationProperty>
    


    <!-- http://www.w3.org/2003/12/exif/ns#gpsDestLatitudeRef -->

    <owl:AnnotationProperty rdf:about="http://www.w3.org/2003/12/exif/ns#gpsDestLatitudeRef">
        <rdfs:comment xml:lang="en">Reference for latitude of destination</rdfs:comment>
        <rdfs:label xml:lang="en">GPSDestLatitudeRef</rdfs:label>
        <tagNumber xml:lang="en">19</tagNumber>
        <rdfs:subPropertyOf rdf:resource="http://www.w3.org/2003/12/exif/ns#gpsInfo"/>
    </owl:AnnotationProperty>
    


    <!-- http://www.w3.org/2003/12/exif/ns#gpsDestLongitude -->

    <owl:AnnotationProperty rdf:about="http://www.w3.org/2003/12/exif/ns#gpsDestLongitude">
        <rdfs:comment xml:lang="en">Longitude of destination, expressed as three values giving the degrees, minutes, and seconds, respectively.</rdfs:comment>
        <rdfs:label xml:lang="en">GPSDestLongitude</rdfs:label>
        <tagNumber xml:lang="en">22</tagNumber>
        <rdfs:subPropertyOf rdf:resource="http://www.w3.org/2003/12/exif/ns#geo"/>
        <rdfs:subPropertyOf rdf:resource="http://www.w3.org/2003/12/exif/ns#gpsInfo"/>
    </owl:AnnotationProperty>
    


    <!-- http://www.w3.org/2003/12/exif/ns#gpsDestLongitudeRef -->

    <owl:AnnotationProperty rdf:about="http://www.w3.org/2003/12/exif/ns#gpsDestLongitudeRef">
        <rdfs:comment xml:lang="en">Reference for longitude of destination</rdfs:comment>
        <rdfs:label xml:lang="en">GPSDestLongitudeRef</rdfs:label>
        <tagNumber xml:lang="en">21</tagNumber>
        <rdfs:subPropertyOf rdf:resource="http://www.w3.org/2003/12/exif/ns#gpsInfo"/>
    </owl:AnnotationProperty>
    


    <!-- http://www.w3.org/2003/12/exif/ns#gpsDifferential -->

    <owl:AnnotationProperty rdf:about="http://www.w3.org/2003/12/exif/ns#gpsDifferential">
        <rdfs:comment xml:lang="en">Indicates whether differential correction is applied to the GPS receiver.</rdfs:comment>
        <rdfs:label xml:lang="en">GPSDifferential</rdfs:label>
        <tagNumber xml:lang="en">30</tagNumber>
        <rdfs:subPropertyOf rdf:resource="http://www.w3.org/2003/12/exif/ns#gpsInfo"/>
    </owl:AnnotationProperty>
    


    <!-- http://www.w3.org/2003/12/exif/ns#gpsImgDirection -->

    <owl:AnnotationProperty rdf:about="http://www.w3.org/2003/12/exif/ns#gpsImgDirection">
        <rdfs:comment xml:lang="en">The direction of the image when it was captured. The range of values is from 0.00 to 359.99.</rdfs:comment>
        <rdfs:label xml:lang="en">GPSImgDirection</rdfs:label>
        <tagNumber xml:lang="en">17</tagNumber>
        <rdfs:subPropertyOf rdf:resource="http://www.w3.org/2003/12/exif/ns#gpsInfo"/>
    </owl:AnnotationProperty>
    


    <!-- http://www.w3.org/2003/12/exif/ns#gpsImgDirectionRef -->

    <owl:AnnotationProperty rdf:about="http://www.w3.org/2003/12/exif/ns#gpsImgDirectionRef">
        <rdfs:comment xml:lang="en">The reference for giving the direction of the image when it is captured. &apos;T&apos; denotes true direction and &apos;M&apos; is magnetic direction.</rdfs:comment>
        <rdfs:label xml:lang="en">GPSImgDirectionRef</rdfs:label>
        <tagNumber xml:lang="en">16</tagNumber>
        <rdfs:subPropertyOf rdf:resource="http://www.w3.org/2003/12/exif/ns#gpsInfo"/>
    </owl:AnnotationProperty>
    


    <!-- http://www.w3.org/2003/12/exif/ns#gpsInfo -->

    <owl:AnnotationProperty rdf:about="http://www.w3.org/2003/12/exif/ns#gpsInfo">
        <rdfs:comment xml:lang="en">An attribute relating to GPS information</rdfs:comment>
        <rdfs:label xml:lang="en">GPS Info</rdfs:label>
        <rdfs:subPropertyOf rdf:resource="http://www.w3.org/2003/12/exif/ns#exifAttribute"/>
    </owl:AnnotationProperty>
    


    <!-- http://www.w3.org/2003/12/exif/ns#gpsInfo_IFD_Pointer -->

    <owl:AnnotationProperty rdf:about="http://www.w3.org/2003/12/exif/ns#gpsInfo_IFD_Pointer">
        <rdfs:comment xml:lang="en">A pointer to the GPS IFD, which is a set of tags for recording GPS information.</rdfs:comment>
        <rdfs:comment xml:lang="ja">GPS IFDへのポインタ</rdfs:comment>
        <rdfs:label xml:lang="en">GPSInfo IFD Pointer</rdfs:label>
        <tagNumber xml:lang="en">34853</tagNumber>
        <rdfs:subPropertyOf rdf:resource="http://www.w3.org/2003/12/exif/ns#ifdPointer"/>
    </owl:AnnotationProperty>
    


    <!-- http://www.w3.org/2003/12/exif/ns#gpsLatitude -->

    <owl:AnnotationProperty rdf:about="http://www.w3.org/2003/12/exif/ns#gpsLatitude">
        <rdfs:subPropertyOf rdf:resource="http://www.w3.org/2003/12/exif/ns#geo"/>
        <rdfs:subPropertyOf rdf:resource="http://www.w3.org/2003/12/exif/ns#gpsInfo"/>
    </owl:AnnotationProperty>
    


    <!-- http://www.w3.org/2003/12/exif/ns#gpsLatitudeRef -->

    <owl:AnnotationProperty rdf:about="http://www.w3.org/2003/12/exif/ns#gpsLatitudeRef">
        <rdfs:comment xml:lang="en">Indicates whether the latitude is north or south latitude. The ASCII value &apos;N&apos; indicates north latitude, and &apos;S&apos; is south latitude.</rdfs:comment>
        <rdfs:comment xml:lang="ja">緯度の北緯もしくは南緯</rdfs:comment>
        <rdfs:label xml:lang="en">GPSLatitudeRef</rdfs:label>
        <tagNumber xml:lang="en">1</tagNumber>
        <rdfs:subPropertyOf rdf:resource="http://www.w3.org/2003/12/exif/ns#gpsInfo"/>
    </owl:AnnotationProperty>
    


    <!-- http://www.w3.org/2003/12/exif/ns#gpsLongitude -->

    <owl:AnnotationProperty rdf:about="http://www.w3.org/2003/12/exif/ns#gpsLongitude">
        <rdfs:subPropertyOf rdf:resource="http://www.w3.org/2003/12/exif/ns#geo"/>
        <rdfs:subPropertyOf rdf:resource="http://www.w3.org/2003/12/exif/ns#gpsInfo"/>
    </owl:AnnotationProperty>
    


    <!-- http://www.w3.org/2003/12/exif/ns#gpsLongitudeRef -->

    <owl:AnnotationProperty rdf:about="http://www.w3.org/2003/12/exif/ns#gpsLongitudeRef">
        <rdfs:comment xml:lang="en">Indicates whether the longitude is east or west longitude. ASCII &apos;E&apos; indicates east longitude, and &apos;W&apos; is west longitude.</rdfs:comment>
        <rdfs:comment xml:lang="ja">経度の東経もしくは西経</rdfs:comment>
        <rdfs:label xml:lang="en">GPSLongitudeRef</rdfs:label>
        <tagNumber xml:lang="en">3</tagNumber>
        <rdfs:subPropertyOf rdf:resource="http://www.w3.org/2003/12/exif/ns#gpsInfo"/>
    </owl:AnnotationProperty>
    


    <!-- http://www.w3.org/2003/12/exif/ns#gpsMapDatum -->

    <owl:AnnotationProperty rdf:about="http://www.w3.org/2003/12/exif/ns#gpsMapDatum">
        <rdfs:comment xml:lang="en">The geodetic survey data used by the GPS receiver. If the survey data is restricted to Japan, the value of this tag is &apos;TOKYO&apos; or &apos;WGS-84&apos;. If a GPS Info tag is recorded, it is strongly recommended that this tag be recorded.</rdfs:comment>
        <rdfs:comment xml:lang="ja">測地系。日本なら&apos;TOKYO&apos;もしくは&apos;WGS-84&apos;</rdfs:comment>
        <rdfs:label xml:lang="en">GPSMapDatum</rdfs:label>
        <tagNumber xml:lang="en">18</tagNumber>
        <rdfs:subPropertyOf rdf:resource="http://www.w3.org/2003/12/exif/ns#gpsInfo"/>
    </owl:AnnotationProperty>
    


    <!-- http://www.w3.org/2003/12/exif/ns#gpsMeasureMode -->

    <owl:AnnotationProperty rdf:about="http://www.w3.org/2003/12/exif/ns#gpsMeasureMode">
        <rdfs:comment xml:lang="en">The GPS measurement mode. &apos;2&apos; means two-dimensional measurement and &apos;3&apos; means three-dimensional measurement is in progress.</rdfs:comment>
        <rdfs:label xml:lang="en">GPSMeasureMode</rdfs:label>
        <tagNumber xml:lang="en">10</tagNumber>
        <rdfs:subPropertyOf rdf:resource="http://www.w3.org/2003/12/exif/ns#gpsInfo"/>
    </owl:AnnotationProperty>
    


    <!-- http://www.w3.org/2003/12/exif/ns#gpsProcessingMethod -->

    <owl:AnnotationProperty rdf:about="http://www.w3.org/2003/12/exif/ns#gpsProcessingMethod">
        <rdfs:comment xml:lang="en">A character string recording the name of the method used for location finding. The first byte indicates the character code used, and this is followed by the name of the method.</rdfs:comment>
        <rdfs:label xml:lang="en">GPSProcessingMethod</rdfs:label>
        <tagNumber xml:lang="en">27</tagNumber>
        <rdfs:subPropertyOf rdf:resource="http://www.w3.org/2003/12/exif/ns#gpsInfo"/>
    </owl:AnnotationProperty>
    


    <!-- http://www.w3.org/2003/12/exif/ns#gpsSatellites -->

    <owl:AnnotationProperty rdf:about="http://www.w3.org/2003/12/exif/ns#gpsSatellites">
        <rdfs:comment xml:lang="en">The GPS satellites used for measurements. This tag can be used to describe the number of satellites, their ID number, angle of elevation, azimuth, SNR and other information in ASCII notation. The format is not specified. If the GPS receiver is incapable of taking measurements, value of the tag shall be set to NULL.</rdfs:comment>
        <rdfs:label xml:lang="en">GPSSatellites</rdfs:label>
        <tagNumber xml:lang="en">8</tagNumber>
        <rdfs:subPropertyOf rdf:resource="http://www.w3.org/2003/12/exif/ns#gpsInfo"/>
    </owl:AnnotationProperty>
    


    <!-- http://www.w3.org/2003/12/exif/ns#gpsSpeed -->

    <owl:AnnotationProperty rdf:about="http://www.w3.org/2003/12/exif/ns#gpsSpeed">
        <rdfs:comment xml:lang="en">The speed of GPS receiver movement.</rdfs:comment>
        <rdfs:label xml:lang="en">GPSSpeed</rdfs:label>
        <tagNumber xml:lang="en">13</tagNumber>
        <rdfs:subPropertyOf rdf:resource="http://www.w3.org/2003/12/exif/ns#gpsInfo"/>
    </owl:AnnotationProperty>
    


    <!-- http://www.w3.org/2003/12/exif/ns#gpsSpeedRef -->

    <owl:AnnotationProperty rdf:about="http://www.w3.org/2003/12/exif/ns#gpsSpeedRef">
        <rdfs:comment xml:lang="en">The unit used to express the GPS receiver speed of movement. &apos;K&apos; &apos;M&apos; and &apos;N&apos; represents kilometers per hour, miles per hour, and knots.</rdfs:comment>
        <rdfs:label xml:lang="en">GPSSpeedRef</rdfs:label>
        <tagNumber xml:lang="en">12</tagNumber>
        <rdfs:subPropertyOf rdf:resource="http://www.w3.org/2003/12/exif/ns#gpsInfo"/>
    </owl:AnnotationProperty>
    


    <!-- http://www.w3.org/2003/12/exif/ns#gpsStatus -->

    <owl:AnnotationProperty rdf:about="http://www.w3.org/2003/12/exif/ns#gpsStatus">
        <rdfs:comment xml:lang="en">The status of the GPS receiver when the image is recorded. &apos;A&apos; means measurement is in progress, and &apos;V&apos; means the measurement is Interoperability.</rdfs:comment>
        <rdfs:label xml:lang="en">GPSStatus</rdfs:label>
        <tagNumber xml:lang="en">9</tagNumber>
        <rdfs:subPropertyOf rdf:resource="http://www.w3.org/2003/12/exif/ns#gpsInfo"/>
    </owl:AnnotationProperty>
    


    <!-- http://www.w3.org/2003/12/exif/ns#gpsTimeStamp -->

    <owl:AnnotationProperty rdf:about="http://www.w3.org/2003/12/exif/ns#gpsTimeStamp">
        <rdfs:comment xml:lang="en">The time as UTC (Coordinated Universal Time). TimeStamp is expressed as three RATIONAL values giving the hour, minute, and second.</rdfs:comment>
        <rdfs:label xml:lang="en">GPSTimeStamp</rdfs:label>
        <tagNumber xml:lang="en">7</tagNumber>
        <rdfs:subPropertyOf rdf:resource="http://www.w3.org/2003/12/exif/ns#gpsInfo"/>
    </owl:AnnotationProperty>
    


    <!-- http://www.w3.org/2003/12/exif/ns#gpsTrack -->

    <owl:AnnotationProperty rdf:about="http://www.w3.org/2003/12/exif/ns#gpsTrack">
        <rdfs:comment xml:lang="en">The direction of GPS receiver movement. The range of values is from 0.00 to 359.99.</rdfs:comment>
        <rdfs:label xml:lang="en">GPSTrack</rdfs:label>
        <tagNumber xml:lang="en">15</tagNumber>
        <rdfs:subPropertyOf rdf:resource="http://www.w3.org/2003/12/exif/ns#gpsInfo"/>
    </owl:AnnotationProperty>
    


    <!-- http://www.w3.org/2003/12/exif/ns#gpsTrackRef -->

    <owl:AnnotationProperty rdf:about="http://www.w3.org/2003/12/exif/ns#gpsTrackRef">
        <rdfs:comment xml:lang="en">The reference for giving the direction of GPS receiver movement. &apos;T&apos; denotes true direction and &apos;M&apos; is magnetic direction.</rdfs:comment>
        <rdfs:label xml:lang="en">GPSTrackRef</rdfs:label>
        <tagNumber xml:lang="en">14</tagNumber>
        <rdfs:subPropertyOf rdf:resource="http://www.w3.org/2003/12/exif/ns#gpsInfo"/>
    </owl:AnnotationProperty>
    


    <!-- http://www.w3.org/2003/12/exif/ns#gpsVersionID -->

    <owl:AnnotationProperty rdf:about="http://www.w3.org/2003/12/exif/ns#gpsVersionID">
        <rdfs:comment xml:lang="en">The version of GPSInfoIFD. The version is given as 2.2.0.0. This tag is mandatory when GPSInfo tag is present.</rdfs:comment>
        <rdfs:label xml:lang="en">GPSVersionID</rdfs:label>
        <tagNumber xml:lang="en">0</tagNumber>
        <rdfs:subPropertyOf rdf:resource="http://www.w3.org/2003/12/exif/ns#gpsInfo"/>
        <rdfs:subPropertyOf rdf:resource="http://www.w3.org/2003/12/exif/ns#versionInfo"/>
    </owl:AnnotationProperty>
    


    <!-- http://www.w3.org/2003/12/exif/ns#height -->

    <owl:AnnotationProperty rdf:about="http://www.w3.org/2003/12/exif/ns#height">
        <rdfs:comment xml:lang="en">Height of an object</rdfs:comment>
        <rdfs:label xml:lang="en">Height</rdfs:label>
        <rdfs:subPropertyOf rdf:resource="http://www.w3.org/2003/12/exif/ns#length"/>
    </owl:AnnotationProperty>
    


    <!-- http://www.w3.org/2003/12/exif/ns#ifdPointer -->

    <owl:AnnotationProperty rdf:about="http://www.w3.org/2003/12/exif/ns#ifdPointer">
        <rdfs:comment xml:lang="en">A tag that refers a child IFD</rdfs:comment>
        <rdfs:label xml:lang="en">IFD Pointer</rdfs:label>
        <rdfs:subPropertyOf rdf:resource="http://www.w3.org/2003/12/exif/ns#exifAttribute"/>
    </owl:AnnotationProperty>
    


    <!-- http://www.w3.org/2003/12/exif/ns#imageConfig -->

    <owl:AnnotationProperty rdf:about="http://www.w3.org/2003/12/exif/ns#imageConfig">
        <rdfs:comment xml:lang="en">An attribute relating to Image Configuration</rdfs:comment>
        <rdfs:label xml:lang="en">Image Config</rdfs:label>
        <rdfs:subPropertyOf rdf:resource="http://www.w3.org/2003/12/exif/ns#exifAttribute"/>
    </owl:AnnotationProperty>
    


    <!-- http://www.w3.org/2003/12/exif/ns#imageDataCharacter -->

    <owl:AnnotationProperty rdf:about="http://www.w3.org/2003/12/exif/ns#imageDataCharacter">
        <rdfs:comment xml:lang="en">An attribute relating to image data characteristics</rdfs:comment>
        <rdfs:label xml:lang="en">Image Data Character</rdfs:label>
        <rdfs:subPropertyOf rdf:resource="http://www.w3.org/2003/12/exif/ns#exifAttribute"/>
    </owl:AnnotationProperty>
    


    <!-- http://www.w3.org/2003/12/exif/ns#imageDataStruct -->

    <owl:AnnotationProperty rdf:about="http://www.w3.org/2003/12/exif/ns#imageDataStruct">
        <rdfs:comment xml:lang="en">An attribute relating to image data structure</rdfs:comment>
        <rdfs:label xml:lang="en">Image Data Structure</rdfs:label>
        <rdfs:subPropertyOf rdf:resource="http://www.w3.org/2003/12/exif/ns#exifAttribute"/>
    </owl:AnnotationProperty>
    


    <!-- http://www.w3.org/2003/12/exif/ns#imageDescription -->

    <owl:AnnotationProperty rdf:about="http://www.w3.org/2003/12/exif/ns#imageDescription">
        <rdfs:comment xml:lang="en">A character string giving the title of the image. It may be a comment such as &quot;1988 company picnic&quot; or the like. Two-byte character codes cannot be used. When a 2-byte code is necessary, the Exif Private tag UserComment is to be used.</rdfs:comment>
        <rdfs:comment xml:lang="ja">この画像についての説明。漢字等の2バイト文字の使用は禁止</rdfs:comment>
        <rdfs:label xml:lang="en">ImageDescription</rdfs:label>
        <tagNumber xml:lang="en">270</tagNumber>
        <rdfs:subPropertyOf rdf:resource="http://purl.org/dc/elements/1.1/title"/>
        <rdfs:subPropertyOf rdf:resource="http://www.w3.org/2003/12/exif/ns#exifAttribute"/>
    </owl:AnnotationProperty>
    


    <!-- http://www.w3.org/2003/12/exif/ns#imageLength -->

    <owl:AnnotationProperty rdf:about="http://www.w3.org/2003/12/exif/ns#imageLength">
        <rdfs:comment xml:lang="en">Image height. The number of rows of image data. In JPEG compressed data a JPEG marker is used.</rdfs:comment>
        <rdfs:label xml:lang="en">ImageLength</rdfs:label>
        <tagNumber xml:lang="en">257</tagNumber>
        <rdfs:subPropertyOf rdf:resource="http://www.w3.org/2003/12/exif/ns#height"/>
        <rdfs:subPropertyOf rdf:resource="http://www.w3.org/2003/12/exif/ns#imageDataStruct"/>
    </owl:AnnotationProperty>
    


    <!-- http://www.w3.org/2003/12/exif/ns#imageUniqueID -->

    <owl:AnnotationProperty rdf:about="http://www.w3.org/2003/12/exif/ns#imageUniqueID">
        <rdfs:comment xml:lang="en">An identifier assigned uniquely to each image. It is recorded as an ASCII string equivalent to hexadecimal notation and 128-bit fixed length.</rdfs:comment>
        <rdfs:label xml:lang="en">ImageUniqueID</rdfs:label>
        <tagNumber xml:lang="en">42016</tagNumber>
        <rdfs:subPropertyOf rdf:resource="http://purl.org/dc/elements/1.1/identifier"/>
        <rdfs:subPropertyOf rdf:resource="http://www.w3.org/2003/12/exif/ns#exifAttribute"/>
    </owl:AnnotationProperty>
    


    <!-- http://www.w3.org/2003/12/exif/ns#imageWidth -->

    <owl:AnnotationProperty rdf:about="http://www.w3.org/2003/12/exif/ns#imageWidth">
        <rdfs:comment xml:lang="en">Image width. The number of columns of image data, equal to the number of pixels per row. In JPEG compressed data a JPEG marker is used instead of this tag.</rdfs:comment>
        <rdfs:label xml:lang="en">ImageWidth</rdfs:label>
        <tagNumber xml:lang="en">256</tagNumber>
        <rdfs:subPropertyOf rdf:resource="http://www.w3.org/2003/12/exif/ns#imageDataStruct"/>
        <rdfs:subPropertyOf rdf:resource="http://www.w3.org/2003/12/exif/ns#width"/>
    </owl:AnnotationProperty>
    


    <!-- http://www.w3.org/2003/12/exif/ns#interopInfo -->

    <owl:AnnotationProperty rdf:about="http://www.w3.org/2003/12/exif/ns#interopInfo">
        <rdfs:comment xml:lang="en">An attribute relating to Interoperability. Tags stored in
Interoperability IFD may be defined dependently to each Interoperability rule.</rdfs:comment>
        <rdfs:label xml:lang="en">Interoperability Info</rdfs:label>
        <rdfs:subPropertyOf rdf:resource="http://www.w3.org/2003/12/exif/ns#exifAttribute"/>
    </owl:AnnotationProperty>
    


    <!-- http://www.w3.org/2003/12/exif/ns#interoperabilityIndex -->

    <owl:AnnotationProperty rdf:about="http://www.w3.org/2003/12/exif/ns#interoperabilityIndex">
        <rdfs:comment xml:lang="en">Indicates the identification of the Interoperability rule. &apos;R98&apos; = conforming to R98 file specification of Recommended Exif Interoperability Rules (ExifR98) or to DCF basic file stipulated by Design Rule for Camera File System. &apos;THM&apos; = conforming to DCF thumbnail file stipulated by Design rule for Camera File System.</rdfs:comment>
        <rdfs:comment xml:lang="ja">メイン画像のInteroperability IFDで、データの内容がExifR98 v1.0準拠の場合は、&apos;R98&apos;の文字列。サムネィル画像のInteroperability IFDの場合は、&apos;THM&apos;の文字列</rdfs:comment>
        <rdfs:label xml:lang="en">InteroperabilityIndex</rdfs:label>
        <tagNumber xml:lang="en">1</tagNumber>
        <rdfs:subPropertyOf rdf:resource="http://www.w3.org/2003/12/exif/ns#interopInfo"/>
    </owl:AnnotationProperty>
    


    <!-- http://www.w3.org/2003/12/exif/ns#interoperabilityVersion -->

    <owl:AnnotationProperty rdf:about="http://www.w3.org/2003/12/exif/ns#interoperabilityVersion">
        <rdfs:comment xml:lang="en">Interoperability Version</rdfs:comment>
        <rdfs:comment xml:lang="ja">データの内容がExifR98 v1.0準拠の場合は、&apos;0100&apos;の文字列。</rdfs:comment>
        <rdfs:label xml:lang="en">InteroperabilityVersion</rdfs:label>
        <tagNumber xml:lang="en">2</tagNumber>
        <rdfs:subPropertyOf rdf:resource="http://www.w3.org/2003/12/exif/ns#interopInfo"/>
    </owl:AnnotationProperty>
    


    <!-- http://www.w3.org/2003/12/exif/ns#interoperability_IFD_Pointer -->

    <owl:AnnotationProperty rdf:about="http://www.w3.org/2003/12/exif/ns#interoperability_IFD_Pointer">
        <rdfs:comment xml:lang="en">A pointer to the Interoperability IFD, which is composed of tags storing the information to ensure the Interoperability</rdfs:comment>
        <rdfs:comment xml:lang="ja">Interoperability IFDへのポインタ</rdfs:comment>
        <rdfs:label xml:lang="en">Interoperability IFD Pointer</rdfs:label>
        <tagNumber xml:lang="en">40965</tagNumber>
        <rdfs:subPropertyOf rdf:resource="http://www.w3.org/2003/12/exif/ns#ifdPointer"/>
    </owl:AnnotationProperty>
    


    <!-- http://www.w3.org/2003/12/exif/ns#isoSpeedRatings -->

    <owl:AnnotationProperty rdf:about="http://www.w3.org/2003/12/exif/ns#isoSpeedRatings">
        <rdfs:subPropertyOf rdf:resource="http://www.w3.org/2003/12/exif/ns#pictTaking"/>
    </owl:AnnotationProperty>
    


    <!-- http://www.w3.org/2003/12/exif/ns#jpegInterchangeFormat -->

    <owl:AnnotationProperty rdf:about="http://www.w3.org/2003/12/exif/ns#jpegInterchangeFormat">
        <rdfs:comment xml:lang="en">The offset to the start byte (SOI) of JPEG compressed thumbnail data. This is not used for primary image JPEG data.</rdfs:comment>
        <rdfs:comment xml:lang="ja">圧縮されたサムネイルへのオフセット</rdfs:comment>
        <rdfs:label xml:lang="en">JPEGInterchangeFormat</rdfs:label>
        <tagNumber xml:lang="en">513</tagNumber>
        <rdfs:subPropertyOf rdf:resource="http://www.w3.org/2003/12/exif/ns#recOffset"/>
    </owl:AnnotationProperty>
    


    <!-- http://www.w3.org/2003/12/exif/ns#jpegInterchangeFormatLength -->

    <owl:AnnotationProperty rdf:about="http://www.w3.org/2003/12/exif/ns#jpegInterchangeFormatLength">
        <rdfs:comment xml:lang="en">The number of bytes of JPEG compressed thumbnail data. This is not used for primary image JPEG data.</rdfs:comment>
        <rdfs:comment xml:lang="ja">圧縮されたサムネイルのサイズ</rdfs:comment>
        <rdfs:label xml:lang="en">JPEGInterchangeFormatLength</rdfs:label>
        <tagNumber xml:lang="en">514</tagNumber>
        <rdfs:subPropertyOf rdf:resource="http://www.w3.org/2003/12/exif/ns#recOffset"/>
    </owl:AnnotationProperty>
    


    <!-- http://www.w3.org/2003/12/exif/ns#length -->

    <owl:AnnotationProperty rdf:about="http://www.w3.org/2003/12/exif/ns#length">
        <rdfs:comment xml:lang="en">Length of an object. Could be a subProperty of other general schema.</rdfs:comment>
        <rdfs:label xml:lang="en">Length</rdfs:label>
    </owl:AnnotationProperty>
    


    <!-- http://www.w3.org/2003/12/exif/ns#lightSource -->

    <owl:AnnotationProperty rdf:about="http://www.w3.org/2003/12/exif/ns#lightSource">
        <rdfs:subPropertyOf rdf:resource="http://www.w3.org/2003/12/exif/ns#pictTaking"/>
    </owl:AnnotationProperty>
    


    <!-- http://www.w3.org/2003/12/exif/ns#make -->

    <owl:AnnotationProperty rdf:about="http://www.w3.org/2003/12/exif/ns#make">
        <rdfs:comment xml:lang="en">Manufacturer of image input equipment</rdfs:comment>
        <rdfs:comment xml:lang="ja">カメラのメーカー名。DCFでは必須</rdfs:comment>
        <rdfs:label xml:lang="en">Make</rdfs:label>
        <tagNumber xml:lang="en">271</tagNumber>
        <rdfs:subPropertyOf rdf:resource="http://www.w3.org/2000/01/rdf-schema#label"/>
        <rdfs:subPropertyOf rdf:resource="http://www.w3.org/2003/12/exif/ns#exifAttribute"/>
    </owl:AnnotationProperty>
    


    <!-- http://www.w3.org/2003/12/exif/ns#makerNote -->

    <owl:AnnotationProperty rdf:about="http://www.w3.org/2003/12/exif/ns#makerNote">
        <rdfs:comment xml:lang="en">Manufacturer notes</rdfs:comment>
        <rdfs:comment xml:lang="ja">カメラの内部情報等、メーカー依存データ</rdfs:comment>
        <rdfs:label xml:lang="en">MakerNote</rdfs:label>
        <tagNumber xml:lang="en">37500</tagNumber>
        <rdfs:subPropertyOf rdf:resource="http://www.w3.org/2003/12/exif/ns#userInfo"/>
    </owl:AnnotationProperty>
    


    <!-- http://www.w3.org/2003/12/exif/ns#maxApertureValue -->

    <owl:AnnotationProperty rdf:about="http://www.w3.org/2003/12/exif/ns#maxApertureValue">
        <rdfs:comment xml:lang="en">The smallest F number of the lens. The unit is the APEX value. Ordinarily it is given in the range of 00.00 to 99.99, but it is not limited to this range.</rdfs:comment>
        <rdfs:comment xml:lang="ja">レンズの開放F値。ApertureValue同様、ルート2のベキ乗を取ると通常の絞り値に換算できる</rdfs:comment>
        <rdfs:label xml:lang="en">MaxApertureValue</rdfs:label>
        <tagNumber xml:lang="en">37381</tagNumber>
        <rdfs:subPropertyOf rdf:resource="http://www.w3.org/2003/12/exif/ns#pictTaking"/>
    </owl:AnnotationProperty>
    


    <!-- http://www.w3.org/2003/12/exif/ns#meter -->

    <owl:AnnotationProperty rdf:about="http://www.w3.org/2003/12/exif/ns#meter">
        <rdfs:comment xml:lang="en">A length with unit of meter</rdfs:comment>
        <rdfs:label xml:lang="en">Meter</rdfs:label>
        <rdfs:subPropertyOf rdf:resource="http://www.w3.org/2003/12/exif/ns#length"/>
    </owl:AnnotationProperty>
    


    <!-- http://www.w3.org/2003/12/exif/ns#meteringMode -->

    <owl:AnnotationProperty rdf:about="http://www.w3.org/2003/12/exif/ns#meteringMode">
        <rdfs:comment xml:lang="en">Metering mode, such as CenterWeightedAverage, Spot, MultiSpot,Pattern, Partial etc.</rdfs:comment>
        <rdfs:comment xml:lang="ja">自動露出の測光モード</rdfs:comment>
        <rdfs:label xml:lang="en">MeteringMode</rdfs:label>
        <tagNumber xml:lang="en">37383</tagNumber>
        <rdfs:subPropertyOf rdf:resource="http://www.w3.org/2003/12/exif/ns#pictTaking"/>
    </owl:AnnotationProperty>
    


    <!-- http://www.w3.org/2003/12/exif/ns#mm -->

    <owl:AnnotationProperty rdf:about="http://www.w3.org/2003/12/exif/ns#mm">
        <rdfs:comment xml:lang="en">A length with unit of mm</rdfs:comment>
        <rdfs:label xml:lang="en">Milimeter</rdfs:label>
        <rdfs:subPropertyOf rdf:resource="http://www.w3.org/2003/12/exif/ns#length"/>
    </owl:AnnotationProperty>
    


    <!-- http://www.w3.org/2003/12/exif/ns#model -->

    <owl:AnnotationProperty rdf:about="http://www.w3.org/2003/12/exif/ns#model">
        <rdfs:comment xml:lang="en">Model of image input equipment</rdfs:comment>
        <rdfs:comment xml:lang="ja">カメラの機種名。DCFでは必須</rdfs:comment>
        <rdfs:label xml:lang="en">Model</rdfs:label>
        <tagNumber xml:lang="en">272</tagNumber>
        <rdfs:subPropertyOf rdf:resource="http://www.w3.org/2000/01/rdf-schema#label"/>
        <rdfs:subPropertyOf rdf:resource="http://www.w3.org/2003/12/exif/ns#exifAttribute"/>
    </owl:AnnotationProperty>
    


    <!-- http://www.w3.org/2003/12/exif/ns#oecf -->

    <owl:AnnotationProperty rdf:about="http://www.w3.org/2003/12/exif/ns#oecf">
        <rdfs:comment xml:lang="en">Indicates the Opto-Electric Conversion Function (OECF) specified in ISO 14524. OECF is the relationship between the camera optical input and the image values.</rdfs:comment>
        <rdfs:label xml:lang="en">OECF</rdfs:label>
        <tagNumber xml:lang="en">34856</tagNumber>
        <rdfs:subPropertyOf rdf:resource="http://www.w3.org/2003/12/exif/ns#pictTaking"/>
    </owl:AnnotationProperty>
    


    <!-- http://www.w3.org/2003/12/exif/ns#orientation -->

    <owl:AnnotationProperty rdf:about="http://www.w3.org/2003/12/exif/ns#orientation">
        <rdfs:comment xml:lang="en">The image orientation viewed in terms of rows and columns.</rdfs:comment>
        <rdfs:comment xml:lang="ja">画像データがどこ(top-leftなど）を起点として、どの向きで格納されているか</rdfs:comment>
        <rdfs:label xml:lang="en">Orientation</rdfs:label>
        <tagNumber xml:lang="en">274</tagNumber>
        <rdfs:subPropertyOf rdf:resource="http://www.w3.org/2003/12/exif/ns#imageDataStruct"/>
    </owl:AnnotationProperty>
    


    <!-- http://www.w3.org/2003/12/exif/ns#photometricInterpretation -->

    <owl:AnnotationProperty rdf:about="http://www.w3.org/2003/12/exif/ns#photometricInterpretation">
        <rdfs:comment xml:lang="en">Pixel composition. In JPEG compressed data a JPEG marker is used instead of this tag.</rdfs:comment>
        <rdfs:label xml:lang="en">PhotometricInterpretation</rdfs:label>
        <tagNumber xml:lang="en">262</tagNumber>
        <rdfs:subPropertyOf rdf:resource="http://www.w3.org/2003/12/exif/ns#imageDataStruct"/>
    </owl:AnnotationProperty>
    


    <!-- http://www.w3.org/2003/12/exif/ns#pictTaking -->

    <owl:AnnotationProperty rdf:about="http://www.w3.org/2003/12/exif/ns#pictTaking">
        <rdfs:comment xml:lang="en">An attribute relating to Picture-Taking Conditions</rdfs:comment>
        <rdfs:label xml:lang="en">PictTaking</rdfs:label>
        <rdfs:subPropertyOf rdf:resource="http://www.w3.org/2003/12/exif/ns#exifAttribute"/>
    </owl:AnnotationProperty>
    


    <!-- http://www.w3.org/2003/12/exif/ns#pimBrightness -->

    <owl:AnnotationProperty rdf:about="http://www.w3.org/2003/12/exif/ns#pimBrightness">
        <rdfs:comment xml:lang="en">Brightness info for print image matching</rdfs:comment>
        <rdfs:label xml:lang="en">PrintIM Brightness</rdfs:label>
        <tagNumber xml:lang="en">10</tagNumber>
        <rdfs:subPropertyOf rdf:resource="http://www.w3.org/2003/12/exif/ns#pimInfo"/>
    </owl:AnnotationProperty>
    


    <!-- http://www.w3.org/2003/12/exif/ns#pimColorBalance -->

    <owl:AnnotationProperty rdf:about="http://www.w3.org/2003/12/exif/ns#pimColorBalance">
        <rdfs:comment xml:lang="en">ColorBalance info for print image matching</rdfs:comment>
        <rdfs:label xml:lang="en">PrintIM ColorBalance</rdfs:label>
        <tagNumber xml:lang="en">11</tagNumber>
        <rdfs:subPropertyOf rdf:resource="http://www.w3.org/2003/12/exif/ns#pimInfo"/>
    </owl:AnnotationProperty>
    


    <!-- http://www.w3.org/2003/12/exif/ns#pimContrast -->

    <owl:AnnotationProperty rdf:about="http://www.w3.org/2003/12/exif/ns#pimContrast">
        <rdfs:comment xml:lang="en">Contrast info for print image matching</rdfs:comment>
        <rdfs:label xml:lang="en">PrintIM Contrast</rdfs:label>
        <tagNumber xml:lang="en">9</tagNumber>
        <rdfs:subPropertyOf rdf:resource="http://www.w3.org/2003/12/exif/ns#pimInfo"/>
    </owl:AnnotationProperty>
    


    <!-- http://www.w3.org/2003/12/exif/ns#pimInfo -->

    <owl:AnnotationProperty rdf:about="http://www.w3.org/2003/12/exif/ns#pimInfo">
        <rdfs:comment xml:lang="en">An attribute relating to print image matching</rdfs:comment>
        <rdfs:label xml:lang="en">PIM Info</rdfs:label>
        <rdfs:subPropertyOf rdf:resource="http://www.w3.org/2003/12/exif/ns#exifAttribute"/>
    </owl:AnnotationProperty>
    


    <!-- http://www.w3.org/2003/12/exif/ns#pimSaturation -->

    <owl:AnnotationProperty rdf:about="http://www.w3.org/2003/12/exif/ns#pimSaturation">
        <rdfs:comment xml:lang="en">Saturation info for print image matching</rdfs:comment>
        <rdfs:label xml:lang="en">PrintIM Saturation</rdfs:label>
        <tagNumber xml:lang="en">12</tagNumber>
        <rdfs:subPropertyOf rdf:resource="http://www.w3.org/2003/12/exif/ns#pimInfo"/>
    </owl:AnnotationProperty>
    


    <!-- http://www.w3.org/2003/12/exif/ns#pimSharpness -->

    <owl:AnnotationProperty rdf:about="http://www.w3.org/2003/12/exif/ns#pimSharpness">
        <rdfs:comment xml:lang="en">Sharpness info for print image matching</rdfs:comment>
        <rdfs:label xml:lang="en">PrintIM Sharpness</rdfs:label>
        <tagNumber xml:lang="en">13</tagNumber>
        <rdfs:subPropertyOf rdf:resource="http://www.w3.org/2003/12/exif/ns#pimInfo"/>
    </owl:AnnotationProperty>
    


    <!-- http://www.w3.org/2003/12/exif/ns#pixelXDimension -->

    <owl:AnnotationProperty rdf:about="http://www.w3.org/2003/12/exif/ns#pixelXDimension">
        <rdfs:comment xml:lang="en">Information specific to compressed data. When a compressed file is recorded, the valid width of the meaningful image shall be recorded in this tag, whether or not there is padding data or a restart marker. This tag should not exist in an uncompressed file.</rdfs:comment>
        <rdfs:label xml:lang="en">PixelXDimension</rdfs:label>
        <tagNumber xml:lang="en">40962</tagNumber>
        <rdfs:subPropertyOf rdf:resource="http://www.w3.org/2003/12/exif/ns#imageConfig"/>
        <rdfs:subPropertyOf rdf:resource="http://www.w3.org/2003/12/exif/ns#width"/>
    </owl:AnnotationProperty>
    


    <!-- http://www.w3.org/2003/12/exif/ns#pixelYDimension -->

    <owl:AnnotationProperty rdf:about="http://www.w3.org/2003/12/exif/ns#pixelYDimension">
        <rdfs:comment xml:lang="en">Information specific to compressed data. When a compressed file is recorded, the valid height of the meaningful image shall be recorded in this tag, whether or not there is padding data or a restart marker. This tag should not exist in an uncompressed file. Since data padding is unnecessary in the vertical direction, the number of lines recorded in this valid image height tag will in fact be the same as that recorded in the SOF.</rdfs:comment>
        <rdfs:label xml:lang="en">PixelYDimension</rdfs:label>
        <tagNumber xml:lang="en">40963</tagNumber>
        <rdfs:subPropertyOf rdf:resource="http://www.w3.org/2003/12/exif/ns#height"/>
        <rdfs:subPropertyOf rdf:resource="http://www.w3.org/2003/12/exif/ns#imageConfig"/>
    </owl:AnnotationProperty>
    


    <!-- http://www.w3.org/2003/12/exif/ns#planarConfiguration -->

    <owl:AnnotationProperty rdf:about="http://www.w3.org/2003/12/exif/ns#planarConfiguration">
        <rdfs:comment xml:lang="en">Indicates whether pixel components are recorded in chunky or planar format. In JPEG compressed files a JPEG marker is used instead of this tag. If this field does not exist, the TIFF default of 1 (chunky) is assumed.</rdfs:comment>
        <rdfs:label xml:lang="en">PlanarConfiguration</rdfs:label>
        <tagNumber xml:lang="en">284</tagNumber>
        <rdfs:subPropertyOf rdf:resource="http://www.w3.org/2003/12/exif/ns#imageDataStruct"/>
    </owl:AnnotationProperty>
    


    <!-- http://www.w3.org/2003/12/exif/ns#primaryChromaticities -->

    <owl:AnnotationProperty rdf:about="http://www.w3.org/2003/12/exif/ns#primaryChromaticities">
        <rdfs:comment xml:lang="en">The chromaticity of the three primary colors of the image. Normally this tag is not necessary, since color space is specified in the color space information tag (ColorSpace).</rdfs:comment>
        <rdfs:comment xml:lang="ja">原色の色度。CCIR REcommendation 709 primariesを使っている場合は、&apos;640/1000,330/1000,300/1000,600/1000,150/1000,60/1000&apos;という値。通常はColorSpaceタグがあるので不要</rdfs:comment>
        <rdfs:label xml:lang="en">PrimaryChromaticities</rdfs:label>
        <tagNumber xml:lang="en">319</tagNumber>
        <rdfs:subPropertyOf rdf:resource="http://www.w3.org/2003/12/exif/ns#imageDataCharacter"/>
    </owl:AnnotationProperty>
    


    <!-- http://www.w3.org/2003/12/exif/ns#printImageMatching_IFD_Pointer -->

    <owl:AnnotationProperty rdf:about="http://www.w3.org/2003/12/exif/ns#printImageMatching_IFD_Pointer">
        <rdfs:comment xml:lang="en">A pointer to the print image matching IFD</rdfs:comment>
        <rdfs:label xml:lang="en">PrintImageMatching IFD Pointer</rdfs:label>
        <tagNumber xml:lang="en">50341</tagNumber>
        <rdfs:subPropertyOf rdf:resource="http://www.w3.org/2003/12/exif/ns#ifdPointer"/>
    </owl:AnnotationProperty>
    


    <!-- http://www.w3.org/2003/12/exif/ns#recOffset -->

    <owl:AnnotationProperty rdf:about="http://www.w3.org/2003/12/exif/ns#recOffset">
        <rdfs:comment xml:lang="en">An attribute relating to recording offset</rdfs:comment>
        <rdfs:label xml:lang="en">Recording Offset</rdfs:label>
        <rdfs:subPropertyOf rdf:resource="http://www.w3.org/2003/12/exif/ns#exifAttribute"/>
    </owl:AnnotationProperty>
    


    <!-- http://www.w3.org/2003/12/exif/ns#referenceBlackWhite -->

    <owl:AnnotationProperty rdf:about="http://www.w3.org/2003/12/exif/ns#referenceBlackWhite">
        <rdfs:comment xml:lang="en">The reference black point value and reference white point value. The color space is declared in a color space information tag, with the default being the value that gives the optimal image characteristics Interoperability these conditions.</rdfs:comment>
        <rdfs:comment xml:lang="ja">画像情報の黒点・白点値。YCbCr形式の場合、最初の２つの値がY(輝度)の黒点・白点、次がCb、最後がCrとなり、デフォルト値は&apos;0,255,0,128,0,128&apos;。RGB形式の場合はR、G、Bの順で黒点・白点値が並んでおり、デフォルト値は&apos;0,255,0,255,0,255&apos;。</rdfs:comment>
        <rdfs:label xml:lang="en">ReferenceBlackWhite</rdfs:label>
        <tagNumber xml:lang="en">532</tagNumber>
        <rdfs:subPropertyOf rdf:resource="http://www.w3.org/2003/12/exif/ns#imageDataCharacter"/>
    </owl:AnnotationProperty>
    


    <!-- http://www.w3.org/2003/12/exif/ns#relatedFile -->

    <owl:AnnotationProperty rdf:about="http://www.w3.org/2003/12/exif/ns#relatedFile">
        <rdfs:comment xml:lang="en">Tag Relating to Related File Information</rdfs:comment>
        <rdfs:label xml:lang="en">Related File</rdfs:label>
        <rdfs:subPropertyOf rdf:resource="http://www.w3.org/2003/12/exif/ns#exifAttribute"/>
    </owl:AnnotationProperty>
    


    <!-- http://www.w3.org/2003/12/exif/ns#relatedImageFileFormat -->

    <owl:AnnotationProperty rdf:about="http://www.w3.org/2003/12/exif/ns#relatedImageFileFormat">
        <rdfs:comment xml:lang="en">Related image file format</rdfs:comment>
        <rdfs:comment xml:lang="ja">画像フォーマットを&apos;Exif JPEG Ver. 2.1&apos;などの文字列で示す。通常はサムネィル画像に使う</rdfs:comment>
        <rdfs:label xml:lang="en">RelatedImageFileFormat</rdfs:label>
        <tagNumber xml:lang="en">4096</tagNumber>
        <rdfs:subPropertyOf rdf:resource="http://www.w3.org/2003/12/exif/ns#interopInfo"/>
    </owl:AnnotationProperty>
    


    <!-- http://www.w3.org/2003/12/exif/ns#relatedImageLength -->

    <owl:AnnotationProperty rdf:about="http://www.w3.org/2003/12/exif/ns#relatedImageLength">
        <rdfs:comment xml:lang="en">Related image length</rdfs:comment>
        <rdfs:comment xml:lang="ja">画像高。通常はサムネイル画像のInteroperability IFDに使う</rdfs:comment>
        <rdfs:label xml:lang="en">RelatedImageLength</rdfs:label>
        <tagNumber xml:lang="en">4098</tagNumber>
        <rdfs:subPropertyOf rdf:resource="http://www.w3.org/2003/12/exif/ns#height"/>
        <rdfs:subPropertyOf rdf:resource="http://www.w3.org/2003/12/exif/ns#interopInfo"/>
    </owl:AnnotationProperty>
    


    <!-- http://www.w3.org/2003/12/exif/ns#relatedImageWidth -->

    <owl:AnnotationProperty rdf:about="http://www.w3.org/2003/12/exif/ns#relatedImageWidth">
        <rdfs:comment xml:lang="en">Related image width</rdfs:comment>
        <rdfs:comment xml:lang="ja">画像幅。通常はサムネイル画像のInteroperability IFDに使う</rdfs:comment>
        <rdfs:label xml:lang="en">RelatedImageWidth</rdfs:label>
        <tagNumber xml:lang="en">4097</tagNumber>
        <rdfs:subPropertyOf rdf:resource="http://www.w3.org/2003/12/exif/ns#interopInfo"/>
        <rdfs:subPropertyOf rdf:resource="http://www.w3.org/2003/12/exif/ns#width"/>
    </owl:AnnotationProperty>
    


    <!-- http://www.w3.org/2003/12/exif/ns#relatedSoundFile -->

    <owl:AnnotationProperty rdf:about="http://www.w3.org/2003/12/exif/ns#relatedSoundFile">
        <rdfs:comment xml:lang="en">Related audio file</rdfs:comment>
        <rdfs:comment xml:lang="ja">画像と一緒に音声録音できる機種の場合に、音声ファイルの名前</rdfs:comment>
        <rdfs:label xml:lang="en">RelatedSoundFile</rdfs:label>
        <tagNumber xml:lang="en">40964</tagNumber>
        <rdfs:subPropertyOf rdf:resource="http://www.w3.org/2003/12/exif/ns#relatedFile"/>
    </owl:AnnotationProperty>
    


    <!-- http://www.w3.org/2003/12/exif/ns#resolution -->

    <owl:AnnotationProperty rdf:about="http://www.w3.org/2003/12/exif/ns#resolution">
        <rdfs:comment xml:lang="en">a rational number representing a resolution. Could be a subProperty of other general schema.</rdfs:comment>
        <rdfs:label xml:lang="en">Resolution</rdfs:label>
    </owl:AnnotationProperty>
    


    <!-- http://www.w3.org/2003/12/exif/ns#resolutionUnit -->

    <owl:AnnotationProperty rdf:about="http://www.w3.org/2003/12/exif/ns#resolutionUnit">
        <rdfs:comment xml:lang="en">The unit for measuring XResolution and YResolution. The same unit is used for both XResolution and YResolution. If the image resolution in unknown, 2 (inches) is designated.</rdfs:comment>
        <rdfs:comment xml:lang="ja">XResolution/YResolutionの解像度の単位</rdfs:comment>
        <rdfs:label xml:lang="en">ResolutionUnit</rdfs:label>
        <tagNumber xml:lang="en">296</tagNumber>
        <rdfs:subPropertyOf rdf:resource="http://www.w3.org/2003/12/exif/ns#imageDataStruct"/>
    </owl:AnnotationProperty>
    


    <!-- http://www.w3.org/2003/12/exif/ns#rowsPerStrip -->

    <owl:AnnotationProperty rdf:about="http://www.w3.org/2003/12/exif/ns#rowsPerStrip">
        <rdfs:comment xml:lang="en">The number of rows per strip. This is the number of rows in the image of one strip when an image is divided into strips. With JPEG compressed data this designation is not needed and is omitted.</rdfs:comment>
        <rdfs:label xml:lang="en">RowsPerStrip</rdfs:label>
        <tagNumber xml:lang="en">278</tagNumber>
        <rdfs:subPropertyOf rdf:resource="http://www.w3.org/2003/12/exif/ns#recOffset"/>
    </owl:AnnotationProperty>
    


    <!-- http://www.w3.org/2003/12/exif/ns#samplesPerPixel -->

    <owl:AnnotationProperty rdf:about="http://www.w3.org/2003/12/exif/ns#samplesPerPixel">
        <rdfs:comment xml:lang="en">The number of components per pixel. Since this standard applies to RGB and YCbCr images, the value set for this tag is 3. In JPEG compressed data a JPEG marker is used instead of this tag.</rdfs:comment>
        <rdfs:label xml:lang="en">SamplesPerPixel</rdfs:label>
        <tagNumber xml:lang="en">277</tagNumber>
        <rdfs:subPropertyOf rdf:resource="http://www.w3.org/2003/12/exif/ns#imageDataStruct"/>
    </owl:AnnotationProperty>
    


    <!-- http://www.w3.org/2003/12/exif/ns#saturation -->

    <owl:AnnotationProperty rdf:about="http://www.w3.org/2003/12/exif/ns#saturation">
        <rdfs:comment xml:lang="en">The direction of saturation processing applied by the camera when the image was shot.</rdfs:comment>
        <rdfs:label xml:lang="en">Saturation</rdfs:label>
        <tagNumber xml:lang="en">41993</tagNumber>
        <rdfs:subPropertyOf rdf:resource="http://www.w3.org/2003/12/exif/ns#pictTaking"/>
    </owl:AnnotationProperty>
    


    <!-- http://www.w3.org/2003/12/exif/ns#sceneCaptureType -->

    <owl:AnnotationProperty rdf:about="http://www.w3.org/2003/12/exif/ns#sceneCaptureType">
        <rdfs:comment xml:lang="en">The type of scene that was shot. It can also be used to record the mode in which the image was shot, such as Landscape, Portrait etc. Note that this differs from the scene type (SceneType) tag.</rdfs:comment>
        <rdfs:label xml:lang="en">SceneCaptureType</rdfs:label>
        <tagNumber xml:lang="en">41990</tagNumber>
        <rdfs:subPropertyOf rdf:resource="http://www.w3.org/2003/12/exif/ns#pictTaking"/>
    </owl:AnnotationProperty>
    


    <!-- http://www.w3.org/2003/12/exif/ns#sceneType -->

    <owl:AnnotationProperty rdf:about="http://www.w3.org/2003/12/exif/ns#sceneType">
        <rdfs:comment xml:lang="en">The type of scene. If a DSC recorded the image, this tag value shall always be set to 1, indicating that the image was directly photographed.</rdfs:comment>
        <rdfs:comment xml:lang="ja">画像がどうやって撮られたか。デジカメの場合は通常1=A directly photographed image</rdfs:comment>
        <rdfs:label xml:lang="en">SceneType</rdfs:label>
        <tagNumber xml:lang="en">41729</tagNumber>
        <rdfs:subPropertyOf rdf:resource="http://www.w3.org/2003/12/exif/ns#pictTaking"/>
    </owl:AnnotationProperty>
    


    <!-- http://www.w3.org/2003/12/exif/ns#seconds -->

    <owl:AnnotationProperty rdf:about="http://www.w3.org/2003/12/exif/ns#seconds">
        <rdfs:comment xml:lang="en">a mesurement of time length with unit of second</rdfs:comment>
        <rdfs:label xml:lang="en">Seconds</rdfs:label>
    </owl:AnnotationProperty>
    


    <!-- http://www.w3.org/2003/12/exif/ns#sensingMethod -->

    <owl:AnnotationProperty rdf:about="http://www.w3.org/2003/12/exif/ns#sensingMethod">
        <rdfs:comment xml:lang="en">The image sensor type on the camera or input device, such as One-chip color area sensor etc.</rdfs:comment>
        <rdfs:comment xml:lang="ja">イメージセンサーの形式。One-chip color area sensor、Color sequential area sensor、Trilinear sensorなど</rdfs:comment>
        <rdfs:label xml:lang="en">SensingMethod</rdfs:label>
        <tagNumber xml:lang="en">41495</tagNumber>
        <rdfs:subPropertyOf rdf:resource="http://www.w3.org/2003/12/exif/ns#pictTaking"/>
    </owl:AnnotationProperty>
    


    <!-- http://www.w3.org/2003/12/exif/ns#sharpness -->

    <owl:AnnotationProperty rdf:about="http://www.w3.org/2003/12/exif/ns#sharpness">
        <rdfs:comment xml:lang="en">The direction of sharpness processing applied by the camera when the image was shot.</rdfs:comment>
        <rdfs:label xml:lang="en">Sharpness</rdfs:label>
        <tagNumber xml:lang="en">41994</tagNumber>
        <rdfs:subPropertyOf rdf:resource="http://www.w3.org/2003/12/exif/ns#pictTaking"/>
    </owl:AnnotationProperty>
    


    <!-- http://www.w3.org/2003/12/exif/ns#shutterSpeedValue -->

    <owl:AnnotationProperty rdf:about="http://www.w3.org/2003/12/exif/ns#shutterSpeedValue">
        <rdfs:subPropertyOf rdf:resource="http://www.w3.org/2003/12/exif/ns#pictTaking"/>
    </owl:AnnotationProperty>
    


    <!-- http://www.w3.org/2003/12/exif/ns#software -->

    <owl:AnnotationProperty rdf:about="http://www.w3.org/2003/12/exif/ns#software">
        <rdfs:comment xml:lang="en">The name and version of the software or firmware of the camera or image input device used to generate the image.</rdfs:comment>
        <rdfs:comment xml:lang="ja">デジカメ（もしくは入力機器）の内蔵ソフトウェア/ファームウェアの名称とバージョン</rdfs:comment>
        <rdfs:label xml:lang="en">Software</rdfs:label>
        <tagNumber xml:lang="en">305</tagNumber>
        <rdfs:subPropertyOf rdf:resource="http://www.w3.org/2000/01/rdf-schema#label"/>
        <rdfs:subPropertyOf rdf:resource="http://www.w3.org/2003/12/exif/ns#exifAttribute"/>
    </owl:AnnotationProperty>
    


    <!-- http://www.w3.org/2003/12/exif/ns#spatialFrequencyResponse -->

    <owl:AnnotationProperty rdf:about="http://www.w3.org/2003/12/exif/ns#spatialFrequencyResponse">
        <rdfs:comment xml:lang="en">This tag records the camera or input device spatial frequency table and SFR values in the direction of image width, image height, and diagonal direction, as specified in ISO 12233.</rdfs:comment>
        <rdfs:label xml:lang="en">SpatialFrequencyResponse</rdfs:label>
        <tagNumber xml:lang="en">41484</tagNumber>
        <rdfs:subPropertyOf rdf:resource="http://www.w3.org/2003/12/exif/ns#pictTaking"/>
    </owl:AnnotationProperty>
    


    <!-- http://www.w3.org/2003/12/exif/ns#spectralSensitivity -->

    <owl:AnnotationProperty rdf:about="http://www.w3.org/2003/12/exif/ns#spectralSensitivity">
        <rdfs:comment xml:lang="en">Indicates the spectral sensitivity of each channel of the camera used. The tag value is an ASCII string compatible with the standard developed by the ASTM Technical committee.</rdfs:comment>
        <rdfs:label xml:lang="en">SpectralSensitivity</rdfs:label>
        <tagNumber xml:lang="en">34852</tagNumber>
        <rdfs:subPropertyOf rdf:resource="http://www.w3.org/2003/12/exif/ns#pictTaking"/>
    </owl:AnnotationProperty>
    


    <!-- http://www.w3.org/2003/12/exif/ns#stripByteCounts -->

    <owl:AnnotationProperty rdf:about="http://www.w3.org/2003/12/exif/ns#stripByteCounts">
        <rdfs:comment xml:lang="en">The total number of bytes in each strip. With JPEG compressed data this designation is not needed and is omitted.</rdfs:comment>
        <rdfs:label xml:lang="en">StripByteCounts</rdfs:label>
        <tagNumber xml:lang="en">279</tagNumber>
        <rdfs:subPropertyOf rdf:resource="http://www.w3.org/2003/12/exif/ns#recOffset"/>
    </owl:AnnotationProperty>
    


    <!-- http://www.w3.org/2003/12/exif/ns#stripOffsets -->

    <owl:AnnotationProperty rdf:about="http://www.w3.org/2003/12/exif/ns#stripOffsets">
        <rdfs:comment xml:lang="en">For each strip, the byte offset of that strip. With JPEG compressed data this designation is not needed and is omitted.</rdfs:comment>
        <rdfs:label xml:lang="en">StripOffsets</rdfs:label>
        <tagNumber xml:lang="en">273</tagNumber>
        <rdfs:subPropertyOf rdf:resource="http://www.w3.org/2003/12/exif/ns#recOffset"/>
    </owl:AnnotationProperty>
    


    <!-- http://www.w3.org/2003/12/exif/ns#subSecTime -->

    <owl:AnnotationProperty rdf:about="http://www.w3.org/2003/12/exif/ns#subSecTime">
        <rdfs:comment xml:lang="en">DateTime subseconds</rdfs:comment>
        <rdfs:label xml:lang="en">SubSecTime</rdfs:label>
        <tagNumber xml:lang="en">37520</tagNumber>
        <rdfs:subPropertyOf rdf:resource="http://www.w3.org/2003/12/exif/ns#dateAndOrTime"/>
        <rdfs:subPropertyOf rdf:resource="http://www.w3.org/2003/12/exif/ns#subsecond"/>
    </owl:AnnotationProperty>
    


    <!-- http://www.w3.org/2003/12/exif/ns#subSecTimeDigitized -->

    <owl:AnnotationProperty rdf:about="http://www.w3.org/2003/12/exif/ns#subSecTimeDigitized">
        <rdfs:comment xml:lang="en">DateTimeDigitized subseconds</rdfs:comment>
        <rdfs:label xml:lang="en">SubSecTimeDigitized</rdfs:label>
        <tagNumber xml:lang="en">37522</tagNumber>
        <rdfs:subPropertyOf rdf:resource="http://www.w3.org/2003/12/exif/ns#dateAndOrTime"/>
        <rdfs:subPropertyOf rdf:resource="http://www.w3.org/2003/12/exif/ns#subsecond"/>
    </owl:AnnotationProperty>
    


    <!-- http://www.w3.org/2003/12/exif/ns#subSecTimeOriginal -->

    <owl:AnnotationProperty rdf:about="http://www.w3.org/2003/12/exif/ns#subSecTimeOriginal">
        <rdfs:comment xml:lang="en">DateTimeOriginal subseconds</rdfs:comment>
        <rdfs:label xml:lang="en">SubSecTimeOriginal</rdfs:label>
        <tagNumber xml:lang="en">37521</tagNumber>
        <rdfs:subPropertyOf rdf:resource="http://www.w3.org/2003/12/exif/ns#dateAndOrTime"/>
        <rdfs:subPropertyOf rdf:resource="http://www.w3.org/2003/12/exif/ns#subsecond"/>
    </owl:AnnotationProperty>
    


    <!-- http://www.w3.org/2003/12/exif/ns#subjectArea -->

    <owl:AnnotationProperty rdf:about="http://www.w3.org/2003/12/exif/ns#subjectArea">
        <rdfs:comment xml:lang="en">The location and area of the main subject in the overall scene.</rdfs:comment>
        <rdfs:comment xml:lang="ja">画面中の主たる被写体の位置。2値によるXY座標、3値による円、4値による長方形座標の3通りの示し方がある</rdfs:comment>
        <rdfs:label xml:lang="en">SubjectArea</rdfs:label>
        <tagNumber xml:lang="en">37396</tagNumber>
        <rdfs:subPropertyOf rdf:resource="http://www.w3.org/2003/12/exif/ns#pictTaking"/>
    </owl:AnnotationProperty>
    


    <!-- http://www.w3.org/2003/12/exif/ns#subjectDistance -->

    <owl:AnnotationProperty rdf:about="http://www.w3.org/2003/12/exif/ns#subjectDistance">
        <rdfs:comment xml:lang="en">The distance to the subject, given in meters. Note that if the numerator of the recorded value is FFFFFFFF.H, Infinity shall be indicated; and if the numerator is 0, Distance unknown shall be indicated.</rdfs:comment>
        <rdfs:comment xml:lang="ja">被写体までの距離。単位はm</rdfs:comment>
        <rdfs:label xml:lang="en">SubjectDistance</rdfs:label>
        <tagNumber xml:lang="en">37382</tagNumber>
        <rdfs:subPropertyOf rdf:resource="http://www.w3.org/2003/12/exif/ns#meter"/>
        <rdfs:subPropertyOf rdf:resource="http://www.w3.org/2003/12/exif/ns#pictTaking"/>
    </owl:AnnotationProperty>
    


    <!-- http://www.w3.org/2003/12/exif/ns#subjectDistanceRange -->

    <owl:AnnotationProperty rdf:about="http://www.w3.org/2003/12/exif/ns#subjectDistanceRange">
        <rdfs:comment xml:lang="en">The distance to the subject, such as Macro, Close View or Distant View.</rdfs:comment>
        <rdfs:label xml:lang="en">SubjectDistanceRange</rdfs:label>
        <tagNumber xml:lang="en">41996</tagNumber>
        <rdfs:subPropertyOf rdf:resource="http://www.w3.org/2003/12/exif/ns#pictTaking"/>
    </owl:AnnotationProperty>
    


    <!-- http://www.w3.org/2003/12/exif/ns#subjectLocation -->

    <owl:AnnotationProperty rdf:about="http://www.w3.org/2003/12/exif/ns#subjectLocation">
        <rdfs:comment xml:lang="en">The location of the main subject in the scene. The value of this tag represents the pixel at the center of the main subject relative to the left edge, prior to rotation processing as per the Rotation tag. The first value indicates the X column number and second indicates the Y row number.</rdfs:comment>
        <rdfs:comment xml:lang="ja">画面中の主要被写体のXY座標</rdfs:comment>
        <rdfs:label xml:lang="en">SubjectLocation</rdfs:label>
        <tagNumber xml:lang="en">41492</tagNumber>
        <rdfs:subPropertyOf rdf:resource="http://www.w3.org/2003/12/exif/ns#pictTaking"/>
    </owl:AnnotationProperty>
    


    <!-- http://www.w3.org/2003/12/exif/ns#subsecond -->

    <owl:AnnotationProperty rdf:about="http://www.w3.org/2003/12/exif/ns#subsecond"/>
    


    <!-- http://www.w3.org/2003/12/exif/ns#tagNumber -->

    <owl:AnnotationProperty rdf:about="http://www.w3.org/2003/12/exif/ns#tagNumber"/>
    


    <!-- http://www.w3.org/2003/12/exif/ns#tag_number -->

    <owl:AnnotationProperty rdf:about="http://www.w3.org/2003/12/exif/ns#tag_number">
        <rdfs:comment xml:lang="en">The Exif tag number</rdfs:comment>
        <rdfs:label xml:lang="en">Tag number</rdfs:label>
        <rdfs:subPropertyOf rdf:resource="http://purl.org/dc/elements/1.1/identifier"/>
    </owl:AnnotationProperty>
    


    <!-- http://www.w3.org/2003/12/exif/ns#tagid -->

    <owl:AnnotationProperty rdf:about="http://www.w3.org/2003/12/exif/ns#tagid">
        <rdfs:comment xml:lang="en">The Exif tag number with context prefix, such as IFD type or maker name</rdfs:comment>
        <rdfs:label xml:lang="en">Tag ID</rdfs:label>
        <rdfs:subPropertyOf rdf:resource="http://www.w3.org/2003/12/exif/ns#tag_number"/>
    </owl:AnnotationProperty>
    


    <!-- http://www.w3.org/2003/12/exif/ns#transferFunction -->

    <owl:AnnotationProperty rdf:about="http://www.w3.org/2003/12/exif/ns#transferFunction">
        <rdfs:comment xml:lang="en">A transfer function for the image, described in tabular style. Normally this tag is not necessary, since color space is specified in the color space information tag (ColorSpace).</rdfs:comment>
        <rdfs:label xml:lang="en">TransferFunction</rdfs:label>
        <tagNumber xml:lang="en">301</tagNumber>
        <rdfs:subPropertyOf rdf:resource="http://www.w3.org/2003/12/exif/ns#imageDataCharacter"/>
    </owl:AnnotationProperty>
    


    <!-- http://www.w3.org/2003/12/exif/ns#userComment -->

    <owl:AnnotationProperty rdf:about="http://www.w3.org/2003/12/exif/ns#userComment">
        <rdfs:comment xml:lang="en">A tag for Exif users to write keywords or comments on the image besides those in ImageDescription, and without the character code limitations of the ImageDescription tag. The character code used in the UserComment tag is identified based on an ID code in a fixed 8-byte area at the start of the tag data area.</rdfs:comment>
        <rdfs:comment xml:lang="ja">ユーザーコメント。ImageDescriptionタグと違って、こちらはJIS2バイトコード、Unicode等での記述が許されており、最初の8バイトが文字コード</rdfs:comment>
        <rdfs:label xml:lang="en">UserComment</rdfs:label>
        <tagNumber xml:lang="en">37510</tagNumber>
        <rdfs:subPropertyOf rdf:resource="http://www.w3.org/2003/12/exif/ns#userInfo"/>
    </owl:AnnotationProperty>
    


    <!-- http://www.w3.org/2003/12/exif/ns#userInfo -->

    <owl:AnnotationProperty rdf:about="http://www.w3.org/2003/12/exif/ns#userInfo">
        <rdfs:comment xml:lang="en">An attribute relating to User Information</rdfs:comment>
        <rdfs:label xml:lang="en">User Info</rdfs:label>
        <rdfs:subPropertyOf rdf:resource="http://www.w3.org/2003/12/exif/ns#exifAttribute"/>
    </owl:AnnotationProperty>
    


    <!-- http://www.w3.org/2003/12/exif/ns#versionInfo -->

    <owl:AnnotationProperty rdf:about="http://www.w3.org/2003/12/exif/ns#versionInfo">
        <rdfs:comment xml:lang="en">An attribute relating to Version</rdfs:comment>
        <rdfs:label xml:lang="en">Version Info</rdfs:label>
        <rdfs:subPropertyOf rdf:resource="http://www.w3.org/2003/12/exif/ns#exifAttribute"/>
    </owl:AnnotationProperty>
    


    <!-- http://www.w3.org/2003/12/exif/ns#whiteBalance -->

    <owl:AnnotationProperty rdf:about="http://www.w3.org/2003/12/exif/ns#whiteBalance">
        <rdfs:comment xml:lang="en">The white balance mode set when the image was shot.</rdfs:comment>
        <rdfs:comment xml:lang="ja">ホワイトバランスのモード</rdfs:comment>
        <rdfs:label xml:lang="en">WhiteBalance</rdfs:label>
        <tagNumber xml:lang="en">41987</tagNumber>
        <rdfs:subPropertyOf rdf:resource="http://www.w3.org/2003/12/exif/ns#pictTaking"/>
    </owl:AnnotationProperty>
    


    <!-- http://www.w3.org/2003/12/exif/ns#whitePoint -->

    <owl:AnnotationProperty rdf:about="http://www.w3.org/2003/12/exif/ns#whitePoint">
        <rdfs:comment xml:lang="en">The chromaticity of the white point of the image. Normally this tag is not necessary, since color space is specified in the color space information tag (ColorSpace).</rdfs:comment>
        <rdfs:comment xml:lang="ja">白点の色度。CIE Standard Illuminant D65(いわゆる昼光色の世界標準値)を使っていれば、&apos;3127/10000,3290/10000&apos;という値。通常はColorSpaceタグがあるので不要</rdfs:comment>
        <rdfs:label xml:lang="en">WhitePoint</rdfs:label>
        <tagNumber xml:lang="en">318</tagNumber>
        <rdfs:subPropertyOf rdf:resource="http://www.w3.org/2003/12/exif/ns#imageDataCharacter"/>
    </owl:AnnotationProperty>
    


    <!-- http://www.w3.org/2003/12/exif/ns#width -->

    <owl:AnnotationProperty rdf:about="http://www.w3.org/2003/12/exif/ns#width">
        <rdfs:comment xml:lang="en">Width of an object</rdfs:comment>
        <rdfs:label xml:lang="en">Width</rdfs:label>
        <rdfs:subPropertyOf rdf:resource="http://www.w3.org/2003/12/exif/ns#length"/>
    </owl:AnnotationProperty>
    


    <!-- http://www.w3.org/2003/12/exif/ns#xResolution -->

    <owl:AnnotationProperty rdf:about="http://www.w3.org/2003/12/exif/ns#xResolution">
        <rdfs:comment xml:lang="en">The number of pixels per ResolutionUnit in the ImageWidth direction. When the image resolution is unknown, 72 [dpi] is designated.</rdfs:comment>
        <rdfs:comment xml:lang="ja">画像の表示・印刷時の水平解像度</rdfs:comment>
        <rdfs:label xml:lang="en">XResolution</rdfs:label>
        <tagNumber xml:lang="en">282</tagNumber>
        <rdfs:subPropertyOf rdf:resource="http://www.w3.org/2003/12/exif/ns#imageDataStruct"/>
        <rdfs:subPropertyOf rdf:resource="http://www.w3.org/2003/12/exif/ns#resolution"/>
    </owl:AnnotationProperty>
    


    <!-- http://www.w3.org/2003/12/exif/ns#yCbCrCoefficients -->

    <owl:AnnotationProperty rdf:about="http://www.w3.org/2003/12/exif/ns#yCbCrCoefficients">
        <rdfs:comment xml:lang="ja">RGB形式からYCbCr形式に変換するための3つの係数。通常は0.299、0.587、0.114という値</rdfs:comment>
        <rdfs:comment xml:lang="en">The matrix coefficients for transformation from RGB to YCbCr image data.</rdfs:comment>
        <rdfs:label xml:lang="en">YCbCrCoefficients</rdfs:label>
        <tagNumber xml:lang="en">529</tagNumber>
        <rdfs:subPropertyOf rdf:resource="http://www.w3.org/2003/12/exif/ns#imageDataCharacter"/>
    </owl:AnnotationProperty>
    


    <!-- http://www.w3.org/2003/12/exif/ns#yCbCrPositioning -->

    <owl:AnnotationProperty rdf:about="http://www.w3.org/2003/12/exif/ns#yCbCrPositioning">
        <rdfs:comment xml:lang="en">The position of chrominance components in relation to the luminance component. This field is designated only for JPEG compressed data or uncompressed YCbCr data.</rdfs:comment>
        <rdfs:comment xml:lang="ja">色情報のサンプリングを間引きしている場合に、色情報のサンプルポイントがどこになるか。1=&apos;centered&apos;なら点集合の中央、2＝&apos;co-sited&apos;なら点集合の原点</rdfs:comment>
        <rdfs:label xml:lang="en">YCbCrPositioning</rdfs:label>
        <tagNumber xml:lang="en">531</tagNumber>
        <rdfs:subPropertyOf rdf:resource="http://www.w3.org/2003/12/exif/ns#imageDataStruct"/>
    </owl:AnnotationProperty>
    


    <!-- http://www.w3.org/2003/12/exif/ns#yCbCrSubSampling -->

    <owl:AnnotationProperty rdf:about="http://www.w3.org/2003/12/exif/ns#yCbCrSubSampling">
        <rdfs:comment xml:lang="en">The sampling ratio of chrominance components in relation to the luminance component. In JPEG compressed data a JPEG marker is used instead of this tag.</rdfs:comment>
        <rdfs:label xml:lang="en">YCbCrSubSampling</rdfs:label>
        <tagNumber xml:lang="en">530</tagNumber>
        <rdfs:subPropertyOf rdf:resource="http://www.w3.org/2003/12/exif/ns#imageDataStruct"/>
    </owl:AnnotationProperty>
    


    <!-- http://www.w3.org/2003/12/exif/ns#yResolution -->

    <owl:AnnotationProperty rdf:about="http://www.w3.org/2003/12/exif/ns#yResolution">
        <rdfs:comment xml:lang="en">The number of pixels per ResolutionUnit in the ImageLength direction. The same value as XResolution is designated.</rdfs:comment>
        <rdfs:comment xml:lang="ja">画像の表示・印刷時の垂直解像度</rdfs:comment>
        <rdfs:label xml:lang="en">YResolution</rdfs:label>
        <tagNumber xml:lang="en">283</tagNumber>
        <rdfs:subPropertyOf rdf:resource="http://www.w3.org/2003/12/exif/ns#imageDataStruct"/>
        <rdfs:subPropertyOf rdf:resource="http://www.w3.org/2003/12/exif/ns#resolution"/>
    </owl:AnnotationProperty>
    


    <!-- http://xmlns.com/foaf/0.1/maker -->

    <owl:AnnotationProperty rdf:about="http://xmlns.com/foaf/0.1/maker"/>
    


    <!-- http://xmlns.com/foaf/0.1/name -->

    <owl:AnnotationProperty rdf:about="http://xmlns.com/foaf/0.1/name"/>
    


    <!-- 
    ///////////////////////////////////////////////////////////////////////////////////////
    //
    // Object Properties
    //
    ///////////////////////////////////////////////////////////////////////////////////////
     -->

    


    <!-- http://www.w3.org/2003/12/exif/ns#apertureValue -->

    <owl:ObjectProperty rdf:about="http://www.w3.org/2003/12/exif/ns#apertureValue"/>
    


    <!-- http://www.w3.org/2003/12/exif/ns#gpsLatitude -->

    <owl:ObjectProperty rdf:about="http://www.w3.org/2003/12/exif/ns#gpsLatitude"/>
    


    <!-- http://www.w3.org/2003/12/exif/ns#gpsLongitude -->

    <owl:ObjectProperty rdf:about="http://www.w3.org/2003/12/exif/ns#gpsLongitude"/>
    


    <!-- http://www.w3.org/2003/12/exif/ns#isoSpeedRatings -->

    <owl:ObjectProperty rdf:about="http://www.w3.org/2003/12/exif/ns#isoSpeedRatings"/>
    


    <!-- http://www.w3.org/2003/12/exif/ns#lightSource -->

    <owl:ObjectProperty rdf:about="http://www.w3.org/2003/12/exif/ns#lightSource"/>
    


    <!-- http://www.w3.org/2003/12/exif/ns#shutterSpeedValue -->

    <owl:ObjectProperty rdf:about="http://www.w3.org/2003/12/exif/ns#shutterSpeedValue"/>
    


    <!-- 
    ///////////////////////////////////////////////////////////////////////////////////////
    //
    // Classes
    //
    ///////////////////////////////////////////////////////////////////////////////////////
     -->

    


    <!-- http://example.org/Example -->

    <owl:Class rdf:about="http://example.org/Example"/>
    


    <!-- http://www.w3.org/2003/12/exif/ns#IFD -->

    <owl:Class rdf:about="http://www.w3.org/2003/12/exif/ns#IFD">
        <rdfs:comment xml:lang="en">An Image File Directory</rdfs:comment>
        <rdfs:label xml:lang="en">IFD</rdfs:label>
    </owl:Class>
    


    <!-- http://xmlns.com/foaf/0.1/Person -->

    <owl:Class rdf:about="http://xmlns.com/foaf/0.1/Person"/>
    


    <!-- 
    ///////////////////////////////////////////////////////////////////////////////////////
    //
    // Individuals
    //
    ///////////////////////////////////////////////////////////////////////////////////////
     -->

    


    <!-- urn:pin:MK705 -->

    <owl:NamedIndividual rdf:about="urn:pin:MK705">
        <rdf:type rdf:resource="http://xmlns.com/foaf/0.1/Person"/>
        <rdfs:seeAlso rdf:resource="http://www.kanzaki.com/info/webwho.rdf"/>
        <foaf:name xml:lang="ja">神崎正英</foaf:name>
    </owl:NamedIndividual>
    <rdf:Description>
        <rdf:type rdf:resource="http://example.org/Example"/>
        <ex:code xml:lang="en">
 &lt;exif:IFD rdf:ID=&quot;Primary_Image&quot;&gt;
   &lt;exif:make&gt;Canon&lt;/exif:make&gt;
   &lt;exif:model&gt;Canon IXY DIGITAL 30&lt;/exif:model&gt;
   &lt;exif:orientation&gt;top-left&lt;/exif:orientation&gt;
   &lt;exif:xResolution&gt;180/1&lt;/exif:xResolution&gt;
   &lt;exif:yResolution&gt;180/1&lt;/exif:yResolution&gt;
   &lt;exif:resolutionUnit&gt;inch&lt;/exif:resolutionUnit&gt;
   &lt;exif:dateTime&gt;2003-01-18T16:07:30&lt;/exif:dateTime&gt;
   &lt;exif:yCbCrPositioning&gt;centered&lt;/exif:yCbCrPositioning&gt;
   &lt;exif:exif_IFD_Pointer&gt;
    &lt;exif:IFD&gt;
      &lt;exif:exposureTime&gt;1/400&lt;/exif:exposureTime&gt;
      &lt;exif:fNumber&gt;35/10&lt;/exif:fNumber&gt;
      &lt;exif:exifVersion&gt;2.20&lt;/exif:exifVersion&gt;
      &lt;exif:dateTimeOriginal&gt;2003-01-18T16:07:30&lt;/exif:dateTimeOriginal&gt;
      &lt;exif:dateTimeDigitized&gt;2003-01-18T16:07:30&lt;/exif:dateTimeDigitized&gt;
      &lt;exif:componentsConfiguration&gt;01 02 03 00&lt;/exif:componentsConfiguration&gt;
      &lt;exif:compressedBitsPerPixel&gt;5/1&lt;/exif:compressedBitsPerPixel&gt;
      &lt;exif:shutterSpeedValue&gt;76&lt;/exif:shutterSpeedValue&gt;
      &lt;exif:apertureValue&gt;116/32&lt;/exif:apertureValue&gt;
      &lt;exif:exposureBiasValue&gt;96&lt;/exif:exposureBiasValue&gt;
      &lt;exif:maxApertureValue&gt;116/32&lt;/exif:maxApertureValue&gt;
      &lt;exif:meteringMode&gt;Pattern&lt;/exif:meteringMode&gt;
      &lt;exif:flash&gt;Flash fired, compulsory flash mode, red-eye reduction mode&lt;/exif:flash&gt;
      &lt;exif:focalLength&gt;294/32&lt;/exif:focalLength&gt;
      &lt;exif:flashpixVersion&gt;1.00&lt;/exif:flashpixVersion&gt;
      &lt;exif:colorSpace&gt;sRGB&lt;/exif:colorSpace&gt;
    &lt;/exif:IFD&gt;
   &lt;/exif:exif_IFD_Pointer&gt;
 &lt;/exif:IFD&gt;
 </ex:code>
        <ex:trial rdf:resource="http://www.kanzaki.com/test/exif2rdf"/>
        <dc:description xml:lang="en">IFD nodes correspond Exif&apos;s IFD directories. Each tag in the directory is described as a property. Some tags are defined as integer in EXIF, but may be better to use (controlled) string value, e.g, use &apos;top-left&apos; instead of integer value &apos;1&apos; for &apos;orientation&apos; tag.</dc:description>
        <dc:description xml:lang="ja">IFDノードはExifのIFDディレクトリに、それぞれのタグはプロパティに対応。Exifタグの多くは数値で記録されているが、&apos;orientation&apos;の値を&apos;1&apos;とするよりは&apos;top-left&apos;とするほうが利用しやすいと思われる（これには統制語彙リストが必要か）。</dc:description>
    </rdf:Description>
    


    <!-- 
    ///////////////////////////////////////////////////////////////////////////////////////
    //
    // Annotations
    //
    ///////////////////////////////////////////////////////////////////////////////////////
     -->

    <rdf:Description rdf:about="http://tsc.jeita.or.jp/avs/data/cp3451.pdf">
        <dc:format xml:lang="en">PDF</dc:format>
        <dc:title xml:lang="en">JEITA CP-3451/EXIF 2.2 Specification</dc:title>
    </rdf:Description>
    <rdf:Description rdf:about="http://www.w3.org/2003/12/exif/ns#_unknown">
        <rdfs:comment xml:lang="en">An Exif tag whose meaning is not known</rdfs:comment>
        <rdfs:label xml:lang="en">Unknown tag</rdfs:label>
    </rdf:Description>
    <rdf:Description rdf:about="http://www.w3.org/2003/12/exif/ns#apertureValue">
        <rdfs:comment xml:lang="ja">レンズ絞り値（APEX値）。この値のルート2のベキ乗を取ると、通常の絞り値となる。例えば&apos;5&apos;の場合だと√2^5=F5.6</rdfs:comment>
        <rdfs:label xml:lang="en">ApertureValue</rdfs:label>
        <rdfs:comment xml:lang="en">The lens aperture. The unit is the APEX value.</rdfs:comment>
        <tagNumber xml:lang="en">37378</tagNumber>
    </rdf:Description>
    <rdf:Description rdf:about="http://www.w3.org/2003/12/exif/ns#exifdata">
        <rdfs:comment xml:lang="en">An Exif IFD data entry</rdfs:comment>
        <rdfs:label xml:lang="en">Exif data</rdfs:label>
    </rdf:Description>
    <rdf:Description rdf:about="http://www.w3.org/2003/12/exif/ns#gpsLatitude">
        <rdfs:label xml:lang="en">GPSLatitude</rdfs:label>
        <tagNumber xml:lang="en">2</tagNumber>
        <rdfs:comment xml:lang="en">The latitude, expressed as three values giving the degrees, minutes, and seconds, respectively.</rdfs:comment>
        <rdfs:comment xml:lang="ja">緯度</rdfs:comment>
    </rdf:Description>
    <rdf:Description rdf:about="http://www.w3.org/2003/12/exif/ns#gpsLongitude">
        <tagNumber xml:lang="en">4</tagNumber>
        <rdfs:comment xml:lang="en">The longitude, expressed as three values giving the degrees, minutes, and seconds, respectively.</rdfs:comment>
        <rdfs:comment xml:lang="ja">経度</rdfs:comment>
        <rdfs:label xml:lang="en">GPSLongitude</rdfs:label>
    </rdf:Description>
    <rdf:Description rdf:about="http://www.w3.org/2003/12/exif/ns#isoSpeedRatings">
        <rdfs:comment xml:lang="en">Indicates the ISO Speed and ISO Latitude of the camera or input device as specified in ISO 12232.</rdfs:comment>
        <tagNumber xml:lang="en">34855</tagNumber>
        <rdfs:label xml:lang="en">ISOSpeedRatings</rdfs:label>
        <rdfs:comment xml:lang="ja">CCD感度の銀塩フィルム換算値</rdfs:comment>
    </rdf:Description>
    <rdf:Description rdf:about="http://www.w3.org/2003/12/exif/ns#lightSource">
        <tagNumber xml:lang="en">37384</tagNumber>
        <rdfs:label xml:lang="en">LightSource</rdfs:label>
        <rdfs:comment xml:lang="en">Light source such as Daylight, Tungsten, Flash etc.</rdfs:comment>
        <rdfs:comment xml:lang="ja">光源。これはマニュアルでホワイトバランスを設定した場合のモード値となる</rdfs:comment>
    </rdf:Description>
    <rdf:Description rdf:about="http://www.w3.org/2003/12/exif/ns#shutterSpeedValue">
        <rdfs:comment xml:lang="ja">シャッター速度（APEX値）。この値の2のベキ乗をとって逆数にすると、通常のシャッター速度表示になる。例えば&apos;4&apos;の場合だと1/(2^4)=1/16秒</rdfs:comment>
        <tagNumber xml:lang="en">37377</tagNumber>
        <rdfs:comment xml:lang="en">Shutter speed. The unit is the APEX (Additive System of Photographic Exposure) setting</rdfs:comment>
        <rdfs:label xml:lang="en">ShutterSpeedValue</rdfs:label>
    </rdf:Description>
    <rdf:Description rdf:about="http://www.w3.org/2003/12/exif/ns#subseconds">
        <rdfs:comment xml:lang="en">A tag used to record fractions of seconds for a date property</rdfs:comment>
        <rdfs:label xml:lang="en">Subseconds</rdfs:label>
    </rdf:Description>
</rdf:RDF>



<!-- Generated by the OWL API (version 4.5.9.2019-02-01T07:24:44Z) https://github.com/owlcs/owlapi -->

