@prefix : <https://www.morphosource.org/terms/morphosource#> .
@prefix owl: <http://www.w3.org/2002/07/owl#> .
@prefix rdf: <http://www.w3.org/1999/02/22-rdf-syntax-ns#> .
@prefix xml: <http://www.w3.org/XML/1998/namespace> .
@prefix xsd: <http://www.w3.org/2001/XMLSchema#> .
@prefix rdfs: <http://www.w3.org/2000/01/rdf-schema#> .
@base <https://www.morphosource.org/terms/morphosource#> .

<https://www.morphosource.org/terms/morphosource> rdf:type owl:Ontology ;
                                                   rdfs:comment "Test description for MorphoSource Terms Vocabulary"@en ;
                                                   rdfs:label "MorphoSource Terms Vocabulary"@en ;
                                                   owl:versionInfo "0.3.0" .

#################################################################
#    Annotation properties
#################################################################

###  http://purl.org/dc/dcam/domainIncludes
<http://purl.org/dc/dcam/domainIncludes> rdf:type owl:AnnotationProperty .


###  http://purl.org/dc/dcam/memberOf
<http://purl.org/dc/dcam/memberOf> rdf:type owl:AnnotationProperty .


###  http://purl.org/dc/dcam/rangeIncludes
<http://purl.org/dc/dcam/rangeIncludes> rdf:type owl:AnnotationProperty .


###  http://purl.org/dc/elements/1.1/format
<http://purl.org/dc/elements/1.1/format> rdf:type owl:AnnotationProperty .


###  http://purl.org/dc/terms/description
<http://purl.org/dc/terms/description> rdf:type owl:AnnotationProperty .


###  http://purl.org/dc/terms/hasVersion
<http://purl.org/dc/terms/hasVersion> rdf:type owl:AnnotationProperty .


###  http://purl.org/dc/terms/isPartOf
<http://purl.org/dc/terms/isPartOf> rdf:type owl:AnnotationProperty .


###  http://purl.org/dc/terms/isVersionOf
<http://purl.org/dc/terms/isVersionOf> rdf:type owl:AnnotationProperty .


###  http://purl.org/dc/terms/issued
<http://purl.org/dc/terms/issued> rdf:type owl:AnnotationProperty .


###  http://purl.org/dc/terms/references
<http://purl.org/dc/terms/references> rdf:type owl:AnnotationProperty .


###  http://purl.org/dc/terms/replaces
<http://purl.org/dc/terms/replaces> rdf:type owl:AnnotationProperty .


###  http://rs.tdwg.org/dwc/terms/attributes/abcdEquivalence
<http://rs.tdwg.org/dwc/terms/attributes/abcdEquivalence> rdf:type owl:AnnotationProperty .


###  http://rs.tdwg.org/dwc/terms/attributes/decision
<http://rs.tdwg.org/dwc/terms/attributes/decision> rdf:type owl:AnnotationProperty .


###  http://rs.tdwg.org/dwc/terms/attributes/organizedInClass
<http://rs.tdwg.org/dwc/terms/attributes/organizedInClass> rdf:type owl:AnnotationProperty .


###  http://rs.tdwg.org/dwc/terms/attributes/repeatable
<http://rs.tdwg.org/dwc/terms/attributes/repeatable> rdf:type owl:AnnotationProperty .


###  http://rs.tdwg.org/dwc/terms/attributes/required
<http://rs.tdwg.org/dwc/terms/attributes/required> rdf:type owl:AnnotationProperty .


###  http://rs.tdwg.org/dwc/terms/attributes/usageScope
<http://rs.tdwg.org/dwc/terms/attributes/usageScope> rdf:type owl:AnnotationProperty .


###  http://www.loc.gov/mads/rdf/v1#authoritativeLabel
<http://www.loc.gov/mads/rdf/v1#authoritativeLabel> rdf:type owl:AnnotationProperty .


###  http://www.loc.gov/mads/rdf/v1#code
<http://www.loc.gov/mads/rdf/v1#code> rdf:type owl:AnnotationProperty .


###  http://www.loc.gov/mads/rdf/v1#definitionNote
<http://www.loc.gov/mads/rdf/v1#definitionNote> rdf:type owl:AnnotationProperty .


###  http://www.loc.gov/mads/rdf/v1#hasBroaderAuthority
<http://www.loc.gov/mads/rdf/v1#hasBroaderAuthority> rdf:type owl:AnnotationProperty .


###  http://www.loc.gov/mads/rdf/v1#historyNote
<http://www.loc.gov/mads/rdf/v1#historyNote> rdf:type owl:AnnotationProperty .


###  http://www.loc.gov/mads/rdf/v1#isMemberOfMADSCollection
<http://www.loc.gov/mads/rdf/v1#isMemberOfMADSCollection> rdf:type owl:AnnotationProperty .


###  http://www.loc.gov/mads/rdf/v1#isMemberOfMADSScheme
<http://www.loc.gov/mads/rdf/v1#isMemberOfMADSScheme> rdf:type owl:AnnotationProperty .


###  http://www.w3.org/1999/02/22-rdf-syntax-ns#type
rdf:type rdf:type owl:AnnotationProperty .


###  http://www.w3.org/2003/12/exif/ns#tagNumber
<http://www.w3.org/2003/12/exif/ns#tagNumber> rdf:type owl:AnnotationProperty .


###  http://www.w3.org/2004/02/skos/core#altLabel
<http://www.w3.org/2004/02/skos/core#altLabel> rdf:type owl:AnnotationProperty .


###  http://www.w3.org/2004/02/skos/core#broader
<http://www.w3.org/2004/02/skos/core#broader> rdf:type owl:AnnotationProperty .


###  http://www.w3.org/2004/02/skos/core#changeNote
<http://www.w3.org/2004/02/skos/core#changeNote> rdf:type owl:AnnotationProperty .


###  http://www.w3.org/2004/02/skos/core#definition
<http://www.w3.org/2004/02/skos/core#definition> rdf:type owl:AnnotationProperty .


###  http://www.w3.org/2004/02/skos/core#example
<http://www.w3.org/2004/02/skos/core#example> rdf:type owl:AnnotationProperty .


###  http://www.w3.org/2004/02/skos/core#historyNote
<http://www.w3.org/2004/02/skos/core#historyNote> rdf:type owl:AnnotationProperty .


###  http://www.w3.org/2004/02/skos/core#inScheme
<http://www.w3.org/2004/02/skos/core#inScheme> rdf:type owl:AnnotationProperty .


###  http://www.w3.org/2004/02/skos/core#notation
<http://www.w3.org/2004/02/skos/core#notation> rdf:type owl:AnnotationProperty .


###  http://www.w3.org/2004/02/skos/core#note
<http://www.w3.org/2004/02/skos/core#note> rdf:type owl:AnnotationProperty .


###  http://www.w3.org/2004/02/skos/core#prefLabel
<http://www.w3.org/2004/02/skos/core#prefLabel> rdf:type owl:AnnotationProperty .


###  http://www.w3.org/2004/02/skos/core#scopeNote
<http://www.w3.org/2004/02/skos/core#scopeNote> rdf:type owl:AnnotationProperty .


#################################################################
#    Datatypes
#################################################################

###  http://www.w3.org/2001/XMLSchema#date
xsd:date rdf:type rdfs:Datatype .


#################################################################
#    Object Properties
#################################################################

###  http://id.loc.gov/vocabulary/relators/dpt
<http://id.loc.gov/vocabulary/relators/dpt> rdf:type owl:ObjectProperty ;
                                            owl:equivalentProperty :depositor ;
                                            <http://www.loc.gov/mads/rdf/v1#authoritativeLabel> "Depositor" ;
                                            <http://www.loc.gov/mads/rdf/v1#code> "dpt" ;
                                            <http://www.loc.gov/mads/rdf/v1#definitionNote> "A current owner of an item who deposited the item into the custody of another person, family, or organization, while still retaining ownership"@en ;
                                            <http://www.loc.gov/mads/rdf/v1#hasBroaderAuthority> <http://id.loc.gov/vocabulary/relators/own> ;
                                            <http://www.loc.gov/mads/rdf/v1#historyNote> "MARC bib: 1XX/7XX/8XX $4"@en ;
                                            <http://www.loc.gov/mads/rdf/v1#isMemberOfMADSCollection> <http://id.loc.gov/vocabulary/relators/collection_BIBFRAME> ,
                                                                                                      <http://id.loc.gov/vocabulary/relators/collection_PastPresentRelatorsEntries> ,
                                                                                                      <http://id.loc.gov/vocabulary/relators/collection_RDA> ,
                                                                                                      <http://id.loc.gov/vocabulary/relators/collection_RDAItem> ,
                                                                                                      <http://id.loc.gov/vocabulary/relators/collection_RDAOwner> ;
                                            <http://www.loc.gov/mads/rdf/v1#isMemberOfMADSScheme> <http://id.loc.gov/vocabulary/relators> ;
                                            <http://www.w3.org/2004/02/skos/core#broader> <http://id.loc.gov/vocabulary/relators/own> ;
                                            <http://www.w3.org/2004/02/skos/core#changeNote> _:genid1 ;
                                            <http://www.w3.org/2004/02/skos/core#definition> "A current owner of an item who deposited the item into the custody of another person, family, or organization, while still retaining ownership"@en ;
                                            <http://www.w3.org/2004/02/skos/core#historyNote> "MARC bib: 1XX/7XX/8XX $4"@en ;
                                            <http://www.w3.org/2004/02/skos/core#inScheme> <http://id.loc.gov/vocabulary/relators> ;
                                            <http://www.w3.org/2004/02/skos/core#notation> "dpt" ;
                                            <http://www.w3.org/2004/02/skos/core#prefLabel> "Depositor" .


###  http://pcdm.org/models#fileOf
<http://pcdm.org/models#fileOf> rdf:type owl:ObjectProperty ;
                                owl:inverseOf <http://pcdm.org/models#hasFile> ;
                                rdfs:domain <http://pcdm.org/models#File> ;
                                rdfs:range :FileSet ;
                                rdfs:comment "Links from a File to its containing Object."@en ;
                                rdfs:isDefinedBy <http://pcdm.org/models#> ;
                                rdfs:label "is file of"@en .


###  http://pcdm.org/models#hasFile
<http://pcdm.org/models#hasFile> rdf:type owl:ObjectProperty ;
                                 rdfs:domain :FileSet ;
                                 rdfs:range <http://pcdm.org/models#File> ;
                                 rdfs:comment "Links to a File contained by this Object."@en ;
                                 rdfs:isDefinedBy <http://pcdm.org/models#> ;
                                 rdfs:label "has file"@en .


###  http://pcdm.org/models#hasMember
<http://pcdm.org/models#hasMember> rdf:type owl:ObjectProperty ;
                                   owl:inverseOf <http://pcdm.org/models#memberOf> ;
                                   rdfs:domain :ImagingEvent ,
                                               :Media ,
                                               :Organization ,
                                               :ProcessingEvent ;
                                   rdfs:range :Device ,
                                              :FileSet ,
                                              :Media ,
                                              :ProcessingEvent ;
                                   rdfs:comment """Links to a subsidiary Object or Collection. Typically used to link
          to component parts, such as a book linking to a page.  Note on transitivity: hasMember is
          not defined as transitive, but applications may treat it as transitive as local needs
          dictate."""@en ;
                                   rdfs:isDefinedBy <http://pcdm.org/models#> ;
                                   rdfs:label "has member"@en .


###  http://pcdm.org/models#memberOf
<http://pcdm.org/models#memberOf> rdf:type owl:ObjectProperty ;
                                  rdfs:domain :Device ,
                                              :FileSet ,
                                              :Media ,
                                              :ProcessingEvent ;
                                  rdfs:range :ImagingEvent ,
                                             :Media ,
                                             :Organization ,
                                             :ProcessingEvent ;
                                  rdfs:comment "Links from an Object or Collection to a containing Object or Collection."@en ;
                                  rdfs:isDefinedBy <http://pcdm.org/models#> ;
                                  rdfs:label "is member of"@en .


###  http://purl.org/dc/terms/TGN
<http://purl.org/dc/terms/TGN> rdf:type owl:ObjectProperty ;
                               rdfs:domain :PhysicalObject ;
                               rdfs:range <http://vocab.getty.edu/tgn/7029392> .


###  http://purl.org/dc/terms/license
<http://purl.org/dc/terms/license> rdf:type owl:ObjectProperty ;
                                   rdfs:domain :Media ,
                                               :Organization ;
                                   rdfs:range <http://creativecommons.org/ns#License> ;
                                   <http://purl.org/dc/dcam/rangeIncludes> <http://purl.org/dc/terms/LicenseDocument> ;
                                   <http://purl.org/dc/terms/description> "Recommended practice is to identify the license document with a URI. If this is not possible or feasible, a literal value that identifies the license may be provided."@en ;
                                   rdfs:comment "A legal document giving official permission to do something with the resource."@en ;
                                   rdfs:isDefinedBy <http://purl.org/dc/terms/> ;
                                   rdfs:label "License"@en .


###  http://purl.org/healthcarevocab/v1#AcquisitionType
<http://purl.org/healthcarevocab/v1#AcquisitionType> rdf:type owl:ObjectProperty ;
                                                     rdfs:domain :CTImageSeriesImagingEvent ;
                                                     rdfs:range :AcquisitionType ;
                                                     rdfs:comment """Description of the method used during acquisition of this frame. See Section C.8.15.3.2.1 for Defined Terms.

Required if Frame Type (0008,9007) Value 1 of this frame is ORIGINAL. May be present otherwise."""@en ;
                                                     rdfs:label "Acquisition Type"@en .


###  http://purl.org/healthcarevocab/v1#DetectorDescription
<http://purl.org/healthcarevocab/v1#DetectorDescription> rdf:type owl:ObjectProperty ;
                                                         rdfs:domain :FileSet ;
                                                         rdfs:comment "Free text description of detector."@en ;
                                                         rdfs:label "Detector Description"@en .


###  http://purl.org/healthcarevocab/v1#Modality
<http://purl.org/healthcarevocab/v1#Modality> rdf:type owl:ObjectProperty ;
                                              rdfs:domain :FileSet ;
                                              rdfs:comment "Type of equipment that originally acquired the data used to create the images in this Series. See Section C.7.3.1.1.1 for Defined Terms."@en ;
                                              rdfs:label "Modality"@en .


###  http://purl.org/healthcarevocab/v1#PhotometricInterpretation
<http://purl.org/healthcarevocab/v1#PhotometricInterpretation> rdf:type owl:ObjectProperty ;
                                                               rdfs:domain :FileSet ;
                                                               rdfs:comment "Specifies the intended interpretation of the pixel data. See Section C.7.6.3.1.2 for further explanation."@en ;
                                                               rdfs:label "Photometric Interpretation"@en .


###  http://purl.org/healthcarevocab/v1#PixelSpacingCalibrationType
<http://purl.org/healthcarevocab/v1#PixelSpacingCalibrationType> rdf:type owl:ObjectProperty ;
                                                                 rdfs:domain :FileSet ;
                                                                 rdfs:comment "The type of correction for the effect of geometric magnification or calibration against an object of known size, if any. See Section 10.7.1.2."@en ;
                                                                 rdfs:label "Pixel Spacing Calibration Type"@en .


###  http://rs.tdwg.org/ac/terms/captureDevice
<http://rs.tdwg.org/ac/terms/captureDevice> rdf:type owl:ObjectProperty ;
                                            <http://purl.org/dc/terms/description> "It is best practice to record the device; this may include a combination such as camera plus lens, or camera plus microscope. Examples: \"Canon Supershot 2000\", \"Makroscan Scanner 2000\", \"Zeiss Axioscope with Camera IIIu\", \"SEM (Scanning Electron Microscope)\"."@en ;
                                            <http://purl.org/dc/terms/hasVersion> <http://rs.tdwg.org/ac/terms/version/captureDevice-2013-10-28> ,
                                                                                  <http://rs.tdwg.org/ac/terms/version/captureDevice-2020-01-27> ;
                                            <http://purl.org/dc/terms/isPartOf> <http://rs.tdwg.org/ac/terms/> ;
                                            <http://rs.tdwg.org/dwc/terms/attributes/organizedInClass> <http://rs.tdwg.org/dwc/terms/attributes/ResourceCreation> ;
                                            <http://rs.tdwg.org/dwc/terms/attributes/repeatable> "No" ;
                                            <http://rs.tdwg.org/dwc/terms/attributes/required> "No" ;
                                            rdfs:comment "Free form text describing the device or devices used to create the resource."@en ;
                                            rdfs:isDefinedBy <http://rs.tdwg.org/ac/terms/> ;
                                            rdfs:label "Capture Device"@en .


###  http://rs.tdwg.org/ac/terms/comments
<http://rs.tdwg.org/ac/terms/comments> rdf:type owl:ObjectProperty ;
                                       <http://purl.org/dc/terms/description> "Comments may refer to the resource itself (e. g., asserting a taxon name or location of a biological subject in an image), or to the relation between resource and associated metadata (e. g., asserting that the taxon name given in the metadata is wrong, without asserting a positive identification). There is a separate item for Reviewer Comments, which is defined more as an expert-level review. Implementers or communities of practice might establish conventions about the meaning of the absence of a commenter, but this specification is silent on that matter."@en ;
                                       <http://purl.org/dc/terms/hasVersion> <http://rs.tdwg.org/ac/terms/version/comments-2013-10-28> ,
                                                                             <http://rs.tdwg.org/ac/terms/version/comments-2020-01-27> ;
                                       <http://purl.org/dc/terms/isPartOf> <http://rs.tdwg.org/ac/terms/> ;
                                       <http://rs.tdwg.org/dwc/terms/attributes/organizedInClass> <http://rs.tdwg.org/dwc/terms/attributes/Management> ;
                                       <http://rs.tdwg.org/dwc/terms/attributes/repeatable> "Yes" ;
                                       <http://rs.tdwg.org/dwc/terms/attributes/required> "No" ;
                                       rdfs:comment "Any comment provided on the media resource, as free-form text."@en ;
                                       rdfs:isDefinedBy <http://rs.tdwg.org/ac/terms/> ;
                                       rdfs:label "Comments"@en ;
                                       <http://www.w3.org/2004/02/skos/core#scopeNote> "Best practice would also identify the commenter."@en .


###  http://rs.tdwg.org/ac/terms/subtypeLiteral
<http://rs.tdwg.org/ac/terms/subtypeLiteral> rdf:type owl:ObjectProperty ;
                                             <http://purl.org/dc/terms/hasVersion> <http://rs.tdwg.org/ac/terms/version/subtypeLiteral-2013-10-28> ,
                                                                                   <http://rs.tdwg.org/ac/terms/version/subtypeLiteral-2020-01-27> ,
                                                                                   <http://rs.tdwg.org/ac/terms/version/subtypeLiteral-2020-10-13> ,
                                                                                   <http://rs.tdwg.org/ac/terms/version/subtypeLiteral-2021-02-01> ;
                                             <http://purl.org/dc/terms/isPartOf> <http://rs.tdwg.org/ac/terms/> ;
                                             <http://rs.tdwg.org/dwc/terms/attributes/organizedInClass> <http://rs.tdwg.org/dwc/terms/attributes/Management> ;
                                             <http://rs.tdwg.org/dwc/terms/attributes/repeatable> "Yes" ;
                                             <http://rs.tdwg.org/dwc/terms/attributes/required> "No" ;
                                             rdfs:comment "A class, represented by a controlled value string, that provides for more specialization of the media item type than dc:type."@en ;
                                             rdfs:isDefinedBy <http://rs.tdwg.org/ac/terms/> ;
                                             rdfs:label "Subtype (literal)"@en ;
                                             <http://www.w3.org/2004/02/skos/core#scopeNote> "The subtypeLiteral term MUST NOT be applied to Collection objects. However, the Description term in the Content Coverage Vocabulary might add further description to a Collection object. Controlled string values SHOULD be selected from the Controlled Vocabulary for Audubon Core subtype. Human-readable information about the Controlled Vocabulary for subtype is at http://rs.tdwg.org/ac/doc/subtype/ . It is best practice to use ac:subtype instead of ac:subytpeLiteral whenever practical."@en .


###  http://rs.tdwg.org/dwc/terms/country
<http://rs.tdwg.org/dwc/terms/country> rdf:type owl:ObjectProperty ;
                                       rdfs:domain :Organization ,
                                                   :PhysicalObject ;
                                       <http://purl.org/dc/terms/description> "Recommended best practice is to use a controlled vocabulary such as the Getty Thesaurus of Geographic Names. Recommended best practice is to leave this field blank if the Location spans multiple entities at this administrative level or if the Location might be in one or another of multiple possible entities at this level. Multiplicity and uncertainty of the geographic entity can be captured either in the term higherGeography or in the term locality, or both."@en ;
                                       <http://purl.org/dc/terms/hasVersion> <http://rs.tdwg.org/dwc/terms/version/country-2009-04-24> ,
                                                                             <http://rs.tdwg.org/dwc/terms/version/country-2017-10-06> ,
                                                                             <http://rs.tdwg.org/dwc/terms/version/country-2021-07-15> ;
                                       <http://purl.org/dc/terms/isPartOf> <http://rs.tdwg.org/dwc/terms/> ;
                                       <http://purl.org/dc/terms/replaces> <http://rs.tdwg.org/dwc/dwcore/Country> ;
                                       <http://rs.tdwg.org/dwc/terms/attributes/abcdEquivalence> "DataSets/DataSet/Units/Unit/Gathering/Country/Name" ;
                                       <http://rs.tdwg.org/dwc/terms/attributes/organizedInClass> <http://purl.org/dc/terms/Location> ;
                                       <http://rs.tdwg.org/dwc/terms/attributes/usageScope> "simple" ;
                                       rdfs:comment "The name of the country or major administrative unit in which the Location occurs."@en ;
                                       rdfs:isDefinedBy <http://rs.tdwg.org/dwc/terms/> ;
                                       rdfs:label "Country"@en ;
                                       <http://www.w3.org/2004/02/skos/core#example> "`Denmark`, `Colombia`, `España`"@en .


###  http://rs.tdwg.org/dwc/terms/sex
<http://rs.tdwg.org/dwc/terms/sex> rdf:type owl:ObjectProperty ;
                                   rdfs:domain :BiologicalSpecimenObject ;
                                   rdfs:range :Sex ;
                                   <http://purl.org/dc/terms/description> "Recommended best practice is to use a controlled vocabulary."@en ;
                                   <http://purl.org/dc/terms/hasVersion> <http://rs.tdwg.org/dwc/terms/version/sex-2009-04-24> ,
                                                                         <http://rs.tdwg.org/dwc/terms/version/sex-2017-10-06> ;
                                   <http://purl.org/dc/terms/isPartOf> <http://rs.tdwg.org/dwc/terms/> ;
                                   <http://purl.org/dc/terms/replaces> <http://rs.tdwg.org/dwc/dwcore/Sex> ;
                                   <http://rs.tdwg.org/dwc/terms/attributes/abcdEquivalence> "DataSets/DataSet/Units/Unit/Sex" ;
                                   <http://rs.tdwg.org/dwc/terms/attributes/organizedInClass> <http://rs.tdwg.org/dwc/terms/Occurrence> ;
                                   <http://rs.tdwg.org/dwc/terms/attributes/usageScope> "simple" ;
                                   rdfs:comment "The sex of the biological individual(s) represented in the Occurrence."@en ;
                                   rdfs:isDefinedBy <http://rs.tdwg.org/dwc/terms/> ;
                                   rdfs:label "Sex"@en ;
                                   <http://www.w3.org/2004/02/skos/core#example> "`female`, `male`, `hermaphrodite`"@en .


###  http://rs.tdwg.org/dwc/terms/stateProvince
<http://rs.tdwg.org/dwc/terms/stateProvince> rdf:type owl:ObjectProperty ;
                                             rdfs:domain :Organization ,
                                                         :PhysicalObject ;
                                             <http://purl.org/dc/terms/description> "Recommended best practice is to use a controlled vocabulary such as the Getty Thesaurus of Geographic Names."@en ;
                                             <http://purl.org/dc/terms/hasVersion> <http://rs.tdwg.org/dwc/terms/version/stateProvince-2009-04-24> ,
                                                                                   <http://rs.tdwg.org/dwc/terms/version/stateProvince-2017-10-06> ;
                                             <http://purl.org/dc/terms/isPartOf> <http://rs.tdwg.org/dwc/terms/> ;
                                             <http://purl.org/dc/terms/replaces> <http://rs.tdwg.org/dwc/dwcore/StateProvince> ;
                                             <http://rs.tdwg.org/dwc/terms/attributes/abcdEquivalence> "DataSets/DataSet/Units/Unit/Gathering/NamedAreas/NamedArea/AreaName with NamedAreas/NamedArea/AreaClass= State or = Province (etc.)" ;
                                             <http://rs.tdwg.org/dwc/terms/attributes/organizedInClass> <http://purl.org/dc/terms/Location> ;
                                             <http://rs.tdwg.org/dwc/terms/attributes/usageScope> "simple" ;
                                             rdfs:comment "The name of the next smaller administrative region than country (state, province, canton, department, region, etc.) in which the Location occurs."@en ;
                                             rdfs:isDefinedBy <http://rs.tdwg.org/dwc/terms/> ;
                                             rdfs:label "State Province"@en ;
                                             <http://www.w3.org/2004/02/skos/core#example> "`Montana`, `Minas Gerais`, `Córdoba`"@en .


###  http://www.europeana.eu/schemas/edm/rights
<http://www.europeana.eu/schemas/edm/rights> rdf:type owl:ObjectProperty ;
                                             rdfs:comment "Information about copyright of the digital object."@en ;
                                             rdfs:label "Europeana Rights"@en .


###  http://www.w3.org/2003/12/exif/ns#lightSource
<http://www.w3.org/2003/12/exif/ns#lightSource> rdf:type owl:ObjectProperty ;
                                                rdfs:domain :PhotogrammetryImagingEvent ,
                                                            :PhotographyImagingEvent ;
                                                rdfs:range :LightSourceType ;
                                                rdfs:comment "Light source such as Daylight, Tungsten, Flash etc."@en ,
                                                             "光源。これはマニュアルでホワイトバランスを設定した場合のモード値となる"@ja ;
                                                rdfs:label "LightSource"@en ;
                                                <http://www.w3.org/2003/12/exif/ns#tagNumber> "37384"@en .


###  https://www.morphosource.org/terms/morphosource#aatAttribute
:aatAttribute rdf:type owl:ObjectProperty ;
              rdfs:domain :CulturalHeritageObject ;
              rdfs:range <http://vocab.getty.edu/aat/300264087> ;
              rdfs:comment "Physical attributes of an object, including characteristics such as size and shape, chemical properties of materials, qualities of texture and hardness, and features such as surface ornament. Values must be from the controlled vocabulary Getty Arts and Architecture Thesaurus Physical Attributes Facet (http://vocab.getty.edu/page/aat/300264087). Use of this property is preferred over the custom morphosource:choAttribute property."@en ;
              rdfs:label "Getty Arts and Architecture Thesaurus Attribute"@en ;
              <http://www.w3.org/2004/02/skos/core#example> "`round`, `waterlogged`, `brittleness`"@en .


###  https://www.morphosource.org/terms/morphosource#aatMaterial
:aatMaterial rdf:type owl:ObjectProperty ;
             rdfs:domain :CulturalHeritageObject ;
             rdfs:range <http://vocab.getty.edu/aat/300264091> ;
             rdfs:comment "Material(s) from which an object is made. Values must be from the controlled vocabulary Getty Arts and Architecture Thesaurus Materials Facet (http://vocab.getty.edu/page/aat/300264091). Use of this property is preferred over the custom morphosource:Material property."@en ;
             rdfs:label "Getty Arts and Architecture Thesaurus Material"@en ;
             <http://www.w3.org/2004/02/skos/core#example> "`iron`, `clay`, `millwork`"@en .


###  https://www.morphosource.org/terms/morphosource#aatPeriod
:aatPeriod rdf:type owl:ObjectProperty ;
           rdfs:domain :CulturalHeritageObject ;
           rdfs:range <http://vocab.getty.edu/aat/300264088> ;
           rdfs:comment "Time period associated with the production or creation of an object. Values must be from the controlled vocabulary Getty Arts and Architecture Thesaurus Styles and Periods Facet (http://vocab.getty.edu/page/aat/300264088)."@en ;
           rdfs:label "Getty Arts and Architecture Thesaurus Time Period"@en ;
           <http://www.w3.org/2004/02/skos/core#example> "`Neolithic`,`Pliocene`"@en .


###  https://www.morphosource.org/terms/morphosource#aatType
:aatType rdf:type owl:ObjectProperty ;
         rdfs:domain :CulturalHeritageObject ;
         rdfs:range <http://vocab.getty.edu/aat/300264092> ;
         rdfs:comment "Type, genre, category, or classification of an object. Values must be from the controlled vocabulary Getty Arts and Architecture Thesaurus Objects Facet (http://vocab.getty.edu/page/aat/300264092). Use of this property is preferred over the custom morphosource:choType property."@en ;
         rdfs:label "Getty Arts and Architecture Thesaurus Type"@en ;
         <http://www.w3.org/2004/02/skos/core#example> "`vases`, `paintings (visual works)`, `hammers (tools)`"@en .


###  https://www.morphosource.org/terms/morphosource#colorFormat
:colorFormat rdf:type owl:ObjectProperty ;
             rdfs:domain :FileSet ;
             rdfs:comment "How 3D color information is formatted and codified for a 3D object, if color information is present with the object. Values may include \"vertex color\", \"face color\", \"UV texture\", or others."@en ;
             rdfs:label "Color Format"@en .


###  https://www.morphosource.org/terms/morphosource#colorSpace
:colorSpace rdf:type owl:ObjectProperty ;
            rdfs:domain :FileSet ;
            rdfs:comment "Color space of image data. Values should be from the controlled vocabulary of short string labels for color spaces defined in the TIFF Tag PhotometricInterpretation (https://www.awaresystems.be/imaging/tiff/tifftags/photometricinterpretation.html)."@en ;
            rdfs:label "Color Space"@en ;
            <http://www.w3.org/2004/02/skos/core#example> "`BlackIsZero`, `RGB`, `YCbCr`"@en .


###  https://www.morphosource.org/terms/morphosource#compression
:compression rdf:type owl:ObjectProperty ;
             rdfs:domain :FileSet ;
             rdfs:comment "Compression scheme used on image data. Values should be from the controlled vocabulary of short string labels for compression schemes defined in the TIFF Tag Compression (https://www.awaresystems.be/imaging/tiff/tifftags/compression.html)."@en ;
             rdfs:label "Compression"@en ;
             <http://www.w3.org/2004/02/skos/core#example> "`Uncompressed`, `JPEG`, `PackBits`"@en .


###  https://www.morphosource.org/terms/morphosource#dataManager
:dataManager rdf:type owl:ObjectProperty ;
             rdfs:domain :Organization ;
             rdfs:range :User ;
             rdfs:comment "User intended to have long-term data management over Media representing Organization Physical Objects."@en ;
             rdfs:label "Data Manager"@en .


###  https://www.morphosource.org/terms/morphosource#depositor
:depositor rdf:type owl:ObjectProperty ;
           rdfs:domain :Device ,
                       :FileSet ,
                       :ImagingEvent ,
                       :Media ,
                       :Organization ,
                       :PhysicalObject ,
                       :ProcessingEvent ;
           rdfs:range :User ;
           <http://www.loc.gov/mads/rdf/v1#authoritativeLabel> "Depositor" ;
           <http://www.loc.gov/mads/rdf/v1#code> "dpt" ;
           <http://www.loc.gov/mads/rdf/v1#definitionNote> "A current owner of an item who deposited the item into the custody of another person, family, or organization, while still retaining ownership"@en ;
           <http://www.loc.gov/mads/rdf/v1#hasBroaderAuthority> <http://id.loc.gov/vocabulary/relators/own> ;
           <http://www.loc.gov/mads/rdf/v1#historyNote> "MARC bib: 1XX/7XX/8XX $4"@en ;
           rdfs:comment "A current owner of an item who deposited the item into the custody of another person, family, or organization, while still retaining ownership"@en ;
           rdfs:label "Depositor"@en ;
           <http://www.w3.org/2004/02/skos/core#broader> <http://id.loc.gov/vocabulary/relators/own> ;
           <http://www.w3.org/2004/02/skos/core#changeNote> _:genid1 ;
           <http://www.w3.org/2004/02/skos/core#historyNote> "MARC bib: 1XX/7XX/8XX $4"@en ;
           <http://www.w3.org/2004/02/skos/core#notation> "dpt" .


###  https://www.morphosource.org/terms/morphosource#detectorConfiguration
:detectorConfiguration rdf:type owl:ObjectProperty ;
                       rdfs:domain :CTImageSeriesImagingEvent ;
                       rdfs:range :XRayDetectorConfiguration ;
                       rdfs:comment "The physical configuration of the X-Ray detector. Value must be from the X-Ray Detector Configuration controlled vocabulary (https://www.morphosource.org/terms/morphosource#XRayDetectorConfiguration). This property should be a sub-property of dicom:DetectorConfiguration."@en ;
                       rdfs:label "Detector Configuration"@en ;
                       <http://www.w3.org/2004/02/skos/core#example> "`Area (single or tiled detector)`, `Slot (scanned slot, slit, or spot)`"@en .


###  https://www.morphosource.org/terms/morphosource#detectorType
:detectorType rdf:type owl:ObjectProperty ;
              rdfs:subPropertyOf <http://purl.org/healthcarevocab/v1#DetectorDescription> ;
              rdfs:domain :CTImageSeriesImagingEvent ;
              rdfs:range :XRayDetectorType ;
              <http://purl.org/dc/terms/isVersionOf> <http://purl.org/healthcarevocab/v1#DetectorDescription> ;
              rdfs:comment "Type of detector used to acquire this image. This property is more accurately a sub-property of dicom:DetectorType and should be changed accordingly. Value must be from X-Ray Detector Type controlled vocabulary (https://www.morphosource.org/terms/morphosource#XRayDetectorType)."@en ;
              rdfs:label "Detector Type"@en ;
              <http://www.w3.org/2004/02/skos/core#example> "`Direct (X-Ray photoconductor)`, `Scintillator (Phosphor used)`, `Storage (Storage Phosphor)`, `Film (Scanned film/screen)`"@en .


###  https://www.morphosource.org/terms/morphosource#downloadPermission
:downloadPermission rdf:type owl:ObjectProperty ;
                    rdfs:domain :Organization ;
                    rdfs:range :PublicationStatus ;
                    rdfs:comment "Preferred Publication Status (morphosource:visibility) for Media representing Organization Physical Objects. Value must be from Publication Status controlled vocabulary (https://www.morphosource.org/terms/morphosource#PublicationStatus)."@en ;
                    rdfs:label "Download Permission"@en ;
                    <http://www.w3.org/2004/02/skos/core#example> "`Open`, `Restricted`, `Private`"@en .


###  https://www.morphosource.org/terms/morphosource#downloadReviewer
:downloadReviewer rdf:type owl:ObjectProperty ;
                  rdfs:domain :Media ,
                              :Organization ;
                  rdfs:range :User ;
                  rdfs:comment "User(s) that receive and may decide approval requests to download media that is Published with Restricted Download."@en ;
                  rdfs:label "Download Reviewer"@en .


###  https://www.morphosource.org/terms/morphosource#filesetAccessibility
:filesetAccessibility rdf:type owl:ObjectProperty ;
                      rdfs:label "FileSet Accessibility"@en .


###  https://www.morphosource.org/terms/morphosource#focalLengthType
:focalLengthType rdf:type owl:ObjectProperty ;
                 rdfs:domain :PhotogrammetryImagingEvent ;
                 rdfs:range :FocalLengthType ;
                 rdfs:comment "Whether focal length is variable or fixed. Values must be from FocalLengthType controlled vocabulary (https://www.morphosource.org/terms/morphosource#FocalLengthType)."@en ;
                 rdfs:label "Focal Length Type"@en ;
                 <http://www.w3.org/2004/02/skos/core#example> "`Variable`, `Fixed`"@en .


###  https://www.morphosource.org/terms/morphosource#ieModality
:ieModality rdf:type owl:ObjectProperty ;
            rdfs:subPropertyOf <http://rs.tdwg.org/ac/terms/captureDevice> ;
            rdfs:domain :ImagingEvent ;
            rdfs:range :ImageModalityType ;
            <http://purl.org/dc/terms/isVersionOf> <http://rs.tdwg.org/ac/terms/captureDevice> ;
            rdfs:comment "The imaging modality used in the imaging event. Value must be from Image Modality controlled vocabulary (https://www.morphosource.org/terms/morphosource#ImageModality)."@en ;
            rdfs:label "Imaging Event Modality"@en ;
            <http://www.w3.org/2004/02/skos/core#example> "`MicroNanoXRayComputedTomography`, `Photogrammetry`, `Video`"@en .


###  https://www.morphosource.org/terms/morphosource#mapType
:mapType rdf:type owl:ObjectProperty ;
         rdfs:domain :Media ;
         rdfs:range :MeshMapType ;
         rdfs:comment "Type of texture map or projection that accompanies a 3D mesh model Media, such as color or normal maps. Values must be from the Mesh Map Type controlled vocabulary (https://www.morphosource.org/terms/morphosource#MeshMapType). This only applies to Mesh Media."@en ;
         rdfs:label "Map Type"@en ;
         <http://www.w3.org/2004/02/skos/core#example> "`Color`, `Normal`"@en .


###  https://www.morphosource.org/terms/morphosource#mediaType
:mediaType rdf:type owl:ObjectProperty ;
           rdfs:subPropertyOf <http://rs.tdwg.org/ac/terms/subtypeLiteral> ;
           rdfs:domain :Media ;
           rdfs:range :MediaType ;
           <http://purl.org/dc/terms/isVersionOf> <http://rs.tdwg.org/ac/terms/subtypeLiteral> ;
           rdfs:comment "Type, nature, or classification of a Media file dataset, which may include one or more specific files. This is the general or high-level type of all file data, it is not the file type of any specific file. Most Media Types encompass a variety of different specific file types. Values must be from the Media Type controlled vocabulary (https://www.morphosource.org/terms/morphosource#MediaType)."@en ;
           rdfs:label "Media Type"@en ;
           <http://www.w3.org/2004/02/skos/core#example> "`Mesh`,`Image`,`CTImageSeries`"@en .


###  https://www.morphosource.org/terms/morphosource#modality3D
:modality3D rdf:type owl:ObjectProperty ;
            rdfs:domain :Device ;
            rdfs:range :ImageModalityType ;
            rdfs:comment "The list of imaging modalities that a device is capable of using when imaging objects. Despite the name, this can include non-3D imaging event modalities. Value must be from Image Modality controlled vocabulary (https://www.morphosource.org/terms/morphosource#ImageModality)."@en ;
            rdfs:label "Modality"@en ;
            <http://www.w3.org/2004/02/skos/core#example> "`MicroNanoXRayComputedTomography`, `Photogrammetry`, `Video`"@en .


###  https://www.morphosource.org/terms/morphosource#morphosourceUseAgreementType
:morphosourceUseAgreementType rdf:type owl:ObjectProperty ;
                              rdfs:domain :Media ,
                                          :Organization ;
                              rdfs:range :UseAgreementType ;
                              rdfs:comment "Type of MorphoSource use agreement that users must agree to in order to download Media and that is packaged with an associated Media download. Values must be from the Use Agreement Type controlled vocabulary (https://www.morphosource.org/terms/morphosource#UseAgreementType)."@en ;
                              rdfs:label "MorphoSource Use Agreement Type"@en ;
                              <http://www.w3.org/2004/02/skos/core#example> "`Standard`, `Permissive`"@en .


###  https://www.morphosource.org/terms/morphosource#organizationType
:organizationType rdf:type owl:ObjectProperty ;
                  rdfs:domain :Organization ;
                  rdfs:range :OrganizationType ;
                  rdfs:comment "Type of Organization to distinguish between collections managing Physical Objects, scanning facilities, and entities that both operate scanning equipment and manage Physical Objects. Values must be from Organization Type controlled vocabulary (https://www.morphosource.org/terms/morphosource#OrganizationType)."@en ;
                  rdfs:label "Organization Type"@en ;
                  <http://www.w3.org/2004/02/skos/core#example> "`Museum, Department, or Lab Collection`, `Scanning Facility`, `Collection and Scanning Facility`"@en .


###  https://www.morphosource.org/terms/morphosource#owner
:owner rdf:type owl:ObjectProperty ;
       rdfs:domain :FileSet ,
                   :Media ;
       rdfs:range :User ;
       rdfs:comment "The user that has the highest level of management control over a Media or another Work record. For Media, this user is also known as the Data Manager."@en ;
       rdfs:label "Owner"@en .


###  https://www.morphosource.org/terms/morphosource#permits3DUse
:permits3DUse rdf:type owl:ObjectProperty ;
              rdfs:domain :Media ,
                          :Organization ;
              rdfs:range <https://www.morphosource.org/terms/morphosource#3DPrintingPermission> ;
              rdfs:comment "Whether Media may be 3D printed freely, may be 3D printed in limited ways, or if 3D printing is prohibited. Values must be from the 3D Printing Permission controlled vocabulary (https://www.morphosource.org/terms/morphosource#3DPrintingPermission)."@en ;
              rdfs:label "Permits 3D Use"@en ;
              <http://www.w3.org/2004/02/skos/core#example> "`3DPrintingPermitted`, `3DPrintingLimited`, `3DPrintingProhibited`"@en .


###  https://www.morphosource.org/terms/morphosource#permitsCommercialUse
:permitsCommercialUse rdf:type owl:ObjectProperty ;
                      rdfs:domain :Media ,
                                  :Organization ;
                      rdfs:range :CommercialUsePermission ;
                      rdfs:comment "Whether commercial use of Media is permitted. Values must be from the Commercial Use Permission controlled vocabulary (https://www.morphosource.org/terms/morphosource#CommercialUsePermission)."@en ;
                      rdfs:label "Permits Commercial Use"@en ;
                      <http://www.w3.org/2004/02/skos/core#example> "`CommercialUseNotPermitted`, `CommercialUsePermitted`"@en .


###  https://www.morphosource.org/terms/morphosource#pixelSpacingCalibration
:pixelSpacingCalibration rdf:type owl:ObjectProperty ;
                         rdfs:subPropertyOf <http://purl.org/healthcarevocab/v1#PixelSpacingCalibrationType> ;
                         rdfs:domain :CTImageSeriesImagingEvent ;
                         rdfs:range :PixelSpacingCalibrationType ;
                         <http://purl.org/dc/terms/isVersionOf> <http://purl.org/healthcarevocab/v1#PixelSpacingCalibrationType> ;
                         rdfs:comment "The type of correction for the effect of geometric magnification or calibration against an object of known size, if any. Value must be from Pixel Spacing Calibration Type controlled vocabulary (https://www.morphosource.org/terms/morphosource#PixelSpacingCalibrationType)."@en ;
                         rdfs:label "Pixel Spacing Calibration"@en ;
                         <http://www.w3.org/2004/02/skos/core#example> "`Geometry`, `Fiducial`"@en .


###  https://www.morphosource.org/terms/morphosource#processingActivityType
:processingActivityType rdf:type owl:ObjectProperty ;
                        rdfs:domain :ProcessingEvent ;
                        rdfs:range :ProcessingActivityType ;
                        rdfs:comment "Type of a specific discrete processing activity. Value must be from Processing Activity Type controlled vocabulary (https://www.morphosource.org/terms/morphosource#ProcessingActivityType)."@en ;
                        rdfs:label "Processing Activity Type"@en ;
                        <http://www.w3.org/2004/02/skos/core#example> "`AlignParts`, `Patch`, `Reconstruction`"@en .


###  https://www.morphosource.org/terms/morphosource#requiredArchivalOfPublishedDerivatives
:requiredArchivalOfPublishedDerivatives rdf:type owl:ObjectProperty ;
                                        rdfs:domain :Media ,
                                                    :Organization ;
                                        rdfs:range :DerivativeRearchivalStatement ;
                                        rdfs:comment "Whether and how future derivatives created from Media must be rearchived on a public-facing digital repository such as MorphoSource. Values may include mandatory requirements or optional suggestions. Values must be from Derivative Rearchival Statement controlled vocabulary (https://www.morphosource.org/terms/morphosource#DerivativeRearchivalStatement)."@en ;
                                        rdfs:label "Required Archival Of Published Derivatives"@en ;
                                        <http://www.w3.org/2004/02/skos/core#example> "`OnMorphoSource`, `OnAnyRepository`, `EncouragedButNotRequired`"@en .


###  https://www.morphosource.org/terms/morphosource#rightsStatement
:rightsStatement rdf:type owl:ObjectProperty ;
                 rdfs:subPropertyOf <http://www.europeana.eu/schemas/edm/rights> ;
                 rdfs:domain :Media ,
                             :Organization ;
                 rdfs:range <http://purl.org/dc/terms/RightsStatement> ;
                 <http://purl.org/dc/terms/isVersionOf> <http://www.europeana.eu/schemas/edm/rights> ;
                 rdfs:comment "Standardized rights statement used to communicate the copyright and/or reuse status of digital objects. Values must be from the Rights Statement controlled vocabulary (https://rightsstatements.org)."@en ;
                 rdfs:label "Rights Statement"@en ;
                 <http://www.w3.org/2004/02/skos/core#example> "`http://rightsstatements.org/vocab/NoC-NC/1.0/`, `http://rightsstatements.org/vocab/UND/1.0/`, `http://rightsstatements.org/vocab/InC/1.0/`"@en .


###  https://www.morphosource.org/terms/morphosource#seriesType
:seriesType rdf:type owl:ObjectProperty ;
            rdfs:domain :Media ;
            rdfs:range :CTImageSeriesType ;
            rdfs:comment "Broad type or kind of CT image series, distiguishing between initial X-Ray projections and other derived series forms. Values must be from the CT Image Series Type controlled vocabulary (https://www.morphosource.org/terms/morphosource#CTImageSeriesType)."@en ;
            rdfs:label "Series Type"@en ;
            <http://www.w3.org/2004/02/skos/core#example> "`Projections`, `Sinograms`, `Reconstructed image stack`"@en .


###  https://www.morphosource.org/terms/morphosource#side
:side rdf:type owl:ObjectProperty ;
      rdfs:subPropertyOf <http://rs.tdwg.org/ac/terms/comments> ;
      rdfs:domain :Media ;
      rdfs:range :Side ;
      <http://purl.org/dc/terms/isVersionOf> <http://rs.tdwg.org/ac/terms/comments> ;
      rdfs:comment "The side of a larger object on which is located a represented component part, if media represents a component part of a larger whole object. Values must be from the Side controlled vocabulary (https://www.morphosource.org/terms/morphosource#Side). Values are somewhat oriented toward objects with bilateral symmetry, but may in some cases be applied for objects with other kinds of symmetry."@en ;
      rdfs:label "Side"@en ;
      <http://www.w3.org/2004/02/skos/core#example> "`Left`, `Midline`, `Not Applicable`"@en .


###  https://www.morphosource.org/terms/morphosource#slideType
:slideType rdf:type owl:ObjectProperty ;
           rdfs:domain :SequentialSectionImagingEvent ;
           rdfs:range :SlideType ;
           rdfs:comment "Type of sequential section slide imaged. Value must be \"Histological\" or \"Other\"."@en ;
           rdfs:label "Slide Type"@en ;
           <http://www.w3.org/2004/02/skos/core#example> "`Histological`, `Other`"@en .


###  https://www.morphosource.org/terms/morphosource#targetType
:targetType rdf:type owl:ObjectProperty ;
            rdfs:domain :CTImageSeriesImagingEvent ;
            rdfs:range :XRayTargetType ;
            rdfs:comment "Type of the anode of the X-Ray source. Value must be from the X-Ray Target Type controlled vocabulary (https://www.morphosource.org/terms/morphosource#XRayTargetType)."@en ;
            rdfs:label "Target Type"@en ;
            <http://www.w3.org/2004/02/skos/core#example> "`Reflection`,`Transmission`"@en .


###  https://www.morphosource.org/terms/morphosource#unit
:unit rdf:type owl:ObjectProperty ;
      rdfs:domain :Media ;
      rdfs:range :LengthMeasurementUnit ;
      rdfs:comment "Length measurement unit. For Mesh Media, this is the length unit associated with the 3D coordinate space of the mesh. For CTImageSeries Media, this is the length unit for X/Y/Z pixel spacing. Values must be from the Length Measurement Unit controlled vocabulary (https://www.morphosource.org/terms/morphosource#LengthMeasurementUnit)."@en ;
      rdfs:label "Unit"@en ;
      <http://www.w3.org/2004/02/skos/core#example> "`Mm`, `Um`, `M`"@en .


###  https://www.morphosource.org/terms/morphosource#visibility
:visibility rdf:type owl:ObjectProperty ;
            rdfs:subPropertyOf :filesetAccessibility ;
            rdfs:domain :Media ;
            rdfs:range :PublicationStatus ;
            rdfs:comment "Publication status, denoting whether or not Media may be found in public search and whether or not Media files may be downloaded. Values must be from Publication Status controlled vocabulary (https://www.morphosource.org/terms/morphosource#PublicationStatus)."@en ;
            rdfs:label "Visibility"@en ;
            <http://www.w3.org/2004/02/skos/core#example> "`Open`, `Restricted`, `Private`"@en .


#################################################################
#    Data properties
#################################################################

###  http://ns.adobe.com/photoshop/1.0/Credit
<http://ns.adobe.com/photoshop/1.0/Credit> rdf:type owl:DatatypeProperty ;
                                           rdfs:comment "The credit to person(s) and/or organisation(s) required by the supplier of the item to be used when published. This is a free-text field."@en ;
                                           rdfs:label "Credit Line"@en .


###  http://ns.adobe.com/xap/1.0/rights/Owner
<http://ns.adobe.com/xap/1.0/rights/Owner> rdf:type owl:DatatypeProperty ;
                                           rdfs:comment "A list of legal owners of the resource."@en ;
                                           rdfs:label "Owner"@en .


###  http://ns.adobe.com/xap/1.0/rights/UsageTerms
<http://ns.adobe.com/xap/1.0/rights/UsageTerms> rdf:type owl:DatatypeProperty ;
                                                rdfs:comment "A collection of text instructions on how a resource can be legally used, given in a variety of languages."@en ;
                                                rdfs:label "Usage Rights"@en .


###  http://purl.org/dc/dcmitype/Software
<http://purl.org/dc/dcmitype/Software> rdf:type owl:DatatypeProperty ;
                                       rdfs:domain :ProcessingEvent ;
                                       <http://purl.org/dc/dcam/memberOf> <http://purl.org/dc/terms/DCMIType> ;
                                       <http://purl.org/dc/terms/description> "Examples include a C source file, MS-Windows .exe executable, or Perl script."@en ;
                                       <http://purl.org/dc/terms/issued> "2000-07-11"^^xsd:date ;
                                       rdfs:comment "A computer program in source or compiled form."@en ;
                                       rdfs:isDefinedBy <http://purl.org/dc/dcmitype/> ;
                                       rdfs:label "Software"@en .


###  http://purl.org/dc/elements/1.1/creator
<http://purl.org/dc/elements/1.1/creator> rdf:type owl:DatatypeProperty ;
                                          rdfs:domain :Device ,
                                                      :ImagingEvent ,
                                                      :Media ,
                                                      :PhysicalObject ,
                                                      :ProcessingEvent ;
                                          rdfs:range xsd:string ;
                                          <http://purl.org/dc/terms/description> "Examples of a Creator include a person, an organization, or a service. Typically, the name of a Creator should be used to indicate the entity."@en ;
                                          <http://purl.org/dc/terms/issued> "1999-07-02"^^xsd:date ;
                                          rdfs:comment "An entity primarily responsible for making the resource."@en ;
                                          rdfs:isDefinedBy <http://purl.org/dc/elements/1.1/> ;
                                          rdfs:label "Creator"@en ;
                                          <http://www.w3.org/2004/02/skos/core#note> "A [second property](/specifications/dublin-core/dcmi-terms/#http://purl.org/dc/terms/creator) with the same name as this property has been declared in the [dcterms: namespace](http://purl.org/dc/terms/).  See the Introduction to the document [DCMI Metadata Terms](/specifications/dublin-core/dcmi-terms/) for an explanation."@en .


###  http://purl.org/dc/elements/1.1/description
<http://purl.org/dc/elements/1.1/description> rdf:type owl:DatatypeProperty ;
                                              rdfs:domain :Device ,
                                                          :ImagingEvent ,
                                                          :Media ,
                                                          :Organization ,
                                                          :PhysicalObject ,
                                                          :ProcessingEvent ;
                                              <http://purl.org/dc/terms/description> "Description may include but is not limited to: an abstract, a table of contents, a graphical representation, or a free-text account of the resource."@en ;
                                              <http://purl.org/dc/terms/issued> "1999-07-02"^^xsd:date ;
                                              rdfs:comment "An account of the resource."@en ;
                                              rdfs:isDefinedBy <http://purl.org/dc/elements/1.1/> ;
                                              rdfs:label "Description"@en ;
                                              <http://www.w3.org/2004/02/skos/core#note> "A [second property](/specifications/dublin-core/dcmi-terms/#http://purl.org/dc/terms/description) with the same name as this property has been declared in the [dcterms: namespace](http://purl.org/dc/terms/).  See the Introduction to the document [DCMI Metadata Terms](/specifications/dublin-core/dcmi-terms/) for an explanation."@en .


###  http://purl.org/dc/elements/1.1/publisher
<http://purl.org/dc/elements/1.1/publisher> rdf:type owl:DatatypeProperty ;
                                            rdfs:domain :Media ;
                                            rdfs:range xsd:string ;
                                            <http://purl.org/dc/terms/description> "Examples of a Publisher include a person, an organization, or a service. Typically, the name of a Publisher should be used to indicate the entity."@en ;
                                            <http://purl.org/dc/terms/issued> "1999-07-02"^^xsd:date ;
                                            rdfs:comment "An entity responsible for making the resource available."@en ;
                                            rdfs:isDefinedBy <http://purl.org/dc/elements/1.1/> ;
                                            rdfs:label "Publisher"@en ;
                                            <http://www.w3.org/2004/02/skos/core#note> "A [second property](/specifications/dublin-core/dcmi-terms/#http://purl.org/dc/terms/publisher) with the same name as this property has been declared in the [dcterms: namespace](http://purl.org/dc/terms/).  See the Introduction to the document [DCMI Metadata Terms](/specifications/dublin-core/dcmi-terms/) for an explanation."@en .


###  http://purl.org/dc/terms/available
<http://purl.org/dc/terms/available> rdf:type owl:DatatypeProperty ;
                                     rdfs:domain :Media ;
                                     rdfs:range xsd:dateTime ;
                                     <http://purl.org/dc/terms/description> "Recommended practice is to describe the date, date/time, or period of time as recommended for the property Date, of which this is a subproperty."@en ;
                                     <http://purl.org/dc/terms/issued> "2000-07-11"^^xsd:date ;
                                     rdfs:comment "Date that the resource became or will become available."@en ;
                                     rdfs:isDefinedBy <http://purl.org/dc/terms/> ;
                                     rdfs:label "Date Available"@en .


###  http://purl.org/dc/terms/created
<http://purl.org/dc/terms/created> rdf:type owl:DatatypeProperty ;
                                   rdfs:domain :ImagingEvent ,
                                               :Media ,
                                               :ProcessingEvent ;
                                   rdfs:range xsd:dateTime ;
                                   <http://purl.org/dc/terms/description> "Recommended practice is to describe the date, date/time, or period of time as recommended for the property Date, of which this is a subproperty."@en ;
                                   <http://purl.org/dc/terms/issued> "2000-07-11"^^xsd:date ;
                                   rdfs:comment "Date of creation of the resource."@en ;
                                   rdfs:isDefinedBy <http://purl.org/dc/terms/> ;
                                   rdfs:label "Date Created"@en .


###  http://purl.org/dc/terms/dateSubmitted
<http://purl.org/dc/terms/dateSubmitted> rdf:type owl:DatatypeProperty ;
                                         <http://purl.org/dc/terms/description> "Recommended practice is to describe the date, date/time, or period of time as recommended for the property Date, of which this is a subproperty.  Examples of resources to which a 'Date Submitted' may be relevant include a thesis (submitted to a university department) or an article (submitted to a journal)."@en ;
                                         rdfs:comment "Date of submission of the resource."@en ;
                                         rdfs:isDefinedBy <http://purl.org/dc/terms/> ;
                                         rdfs:label "Date Submitted"@en .


###  http://purl.org/dc/terms/format
<http://purl.org/dc/terms/format> rdf:type owl:DatatypeProperty ;
                                  <http://purl.org/dc/dcam/rangeIncludes> <http://purl.org/dc/terms/Extent> ,
                                                                          <http://purl.org/dc/terms/MediaType> ;
                                  <http://purl.org/dc/terms/description> "Recommended practice is to use a controlled vocabulary where available. For example, for file formats one could use the list of Internet Media Types [[MIME](https://www.iana.org/assignments/media-types/media-types.xhtml)].  Examples of dimensions include size and duration."@en ;
                                  <http://purl.org/dc/terms/issued> "2008-01-14"^^xsd:date ;
                                  rdfs:comment "The file format, physical medium, or dimensions of the resource."@en ;
                                  rdfs:isDefinedBy <http://purl.org/dc/terms/> ;
                                  rdfs:label "Format"@en .


###  http://purl.org/dc/terms/identifier
<http://purl.org/dc/terms/identifier> rdf:type owl:DatatypeProperty ;
                                      rdfs:domain :Media ,
                                                  :PhysicalObject ;
                                      rdfs:range xsd:string ;
                                      <http://purl.org/dc/terms/description> "Recommended practice is to identify the resource by means of a string conforming to an identification system. Examples include International Standard Book Number (ISBN), Digital Object Identifier (DOI), and Uniform Resource Name (URN).  Persistent identifiers should be provided as HTTP URIs."@en ;
                                      <http://purl.org/dc/terms/issued> "2008-01-14"^^xsd:date ;
                                      rdfs:comment "An unambiguous reference to the resource within a given context."@en ;
                                      rdfs:isDefinedBy <http://purl.org/dc/terms/> ;
                                      rdfs:label "Identifier"@en .


###  http://purl.org/dc/terms/medium
<http://purl.org/dc/terms/medium> rdf:type owl:DatatypeProperty ;
                                  <http://purl.org/dc/dcam/domainIncludes> <http://purl.org/dc/terms/PhysicalResource> ;
                                  <http://purl.org/dc/dcam/rangeIncludes> <http://purl.org/dc/terms/PhysicalMedium> ;
                                  <http://purl.org/dc/terms/issued> "2000-07-11"^^xsd:date ;
                                  rdfs:comment "The material or physical carrier of the resource."@en ;
                                  rdfs:isDefinedBy <http://purl.org/dc/terms/> ;
                                  rdfs:label "Medium"@en .


###  http://purl.org/dc/terms/modified
<http://purl.org/dc/terms/modified> rdf:type owl:DatatypeProperty ;
                                    owl:equivalentProperty :dateModified ;
                                    <http://purl.org/dc/terms/description> "Recommended practice is to describe the date, date/time, or period of time as recommended for the property Date, of which this is a subproperty."@en ;
                                    <http://purl.org/dc/terms/issued> "2000-07-11"^^xsd:date ;
                                    rdfs:comment "Date on which the resource was changed."@en ;
                                    rdfs:isDefinedBy <http://purl.org/dc/terms/> ;
                                    rdfs:label "Date Modified"@en .


###  http://purl.org/dc/terms/provenance
<http://purl.org/dc/terms/provenance> rdf:type owl:DatatypeProperty ;
                                      <http://purl.org/dc/dcam/rangeIncludes> <http://purl.org/dc/terms/ProvenanceStatement> ;
                                      <http://purl.org/dc/terms/description> "The statement may include a description of any changes successive custodians made to the resource."@en ;
                                      <http://purl.org/dc/terms/issued> "2004-09-20"^^xsd:date ;
                                      rdfs:comment "A statement of any changes in ownership and custody of the resource since its creation that are significant for its authenticity, integrity, and interpretation."@en ;
                                      rdfs:isDefinedBy <http://purl.org/dc/terms/> ;
                                      rdfs:label "Provenance"@en .


###  http://purl.org/dc/terms/title
<http://purl.org/dc/terms/title> rdf:type owl:DatatypeProperty ;
                                 rdfs:domain :Device ,
                                             :FileSet ,
                                             :ImagingEvent ,
                                             :Media ,
                                             :Organization ,
                                             :PhysicalObject ,
                                             :ProcessingEvent ;
                                 rdfs:range xsd:string ;
                                 rdfs:comment "A name given to the resource."@en ;
                                 rdfs:isDefinedBy <http://purl.org/dc/terms/> ;
                                 rdfs:label "Title"@en .


###  http://purl.org/healthcarevocab/v1#AccessionNumber
<http://purl.org/healthcarevocab/v1#AccessionNumber> rdf:type owl:DatatypeProperty ;
                                                     rdfs:domain :FileSet ;
                                                     rdfs:range xsd:string ;
                                                     rdfs:comment "A RIS generated number that identifies the order for the Study."@en ;
                                                     rdfs:label "Accession Number"@en .


###  http://purl.org/healthcarevocab/v1#AnodeTargetMaterial
<http://purl.org/healthcarevocab/v1#AnodeTargetMaterial> rdf:type owl:DatatypeProperty ;
                                                         rdfs:domain :FileSet ;
                                                         rdfs:comment "The primary material in the anode of the X-Ray source."@en ;
                                                         rdfs:label "Anode Target Material"@en ;
                                                         <http://www.w3.org/2004/02/skos/core#example> "`tungsten`, `molybdenum`, `copper`"@en .


###  http://purl.org/healthcarevocab/v1#BitsAllocated
<http://purl.org/healthcarevocab/v1#BitsAllocated> rdf:type owl:DatatypeProperty ;
                                                   rdfs:domain :FileSet ;
                                                   rdfs:range xsd:int ;
                                                   rdfs:comment "Number of bits allocated for each pixel sample. Each sample shall have the same number of bits allocated. Bits Allocated (0028,0100) shall be either 1, or a multiple of 8. See PS3.5 for further explanation."@en ;
                                                   rdfs:label "Bits Allocated"@en .


###  http://purl.org/healthcarevocab/v1#BitsStored
<http://purl.org/healthcarevocab/v1#BitsStored> rdf:type owl:DatatypeProperty ;
                                                rdfs:domain :FileSet ;
                                                rdfs:range xsd:int ;
                                                rdfs:comment "Number of bits stored for each pixel sample. Each sample shall have the same number of bits stored. See PS3.5 for further explanation."@en ;
                                                rdfs:label "Bits Stored"@en .


###  http://purl.org/healthcarevocab/v1#Columns
<http://purl.org/healthcarevocab/v1#Columns> rdf:type owl:DatatypeProperty ;
                                             rdfs:domain :FileSet ;
                                             rdfs:range xsd:int ;
                                             rdfs:comment """Number of columns in the image.

Shall be an exact multiple of the horizontal downsampling factor if any of the samples (planes) are encoded downsampled in the horizontal direction for pixel data encoded in a Native (uncompressed) format. E.g., required to be an even value for a Photometric Interpretation (0028,0004) of YBR_FULL_422."""@en ;
                                             rdfs:label "Columns"@en .


###  http://purl.org/healthcarevocab/v1#ContainerDescription
<http://purl.org/healthcarevocab/v1#ContainerDescription> rdf:type owl:DatatypeProperty ;
                                                          rdfs:domain :FileSet ;
                                                          rdfs:comment "Description of the container."@en ;
                                                          rdfs:label "Container Description"@en .


###  http://purl.org/healthcarevocab/v1#ContentDate
<http://purl.org/healthcarevocab/v1#ContentDate> rdf:type owl:DatatypeProperty ;
                                                 rdfs:domain :FileSet ;
                                                 rdfs:range xsd:date ;
                                                 rdfs:comment """The date the image pixel data creation started.

Required if image is part of a Series in which the images are temporally related. May be present otherwise."""@en ;
                                                 rdfs:label "Content Date"@en .


###  http://purl.org/healthcarevocab/v1#ContentTime
<http://purl.org/healthcarevocab/v1#ContentTime> rdf:type owl:DatatypeProperty ;
                                                 rdfs:domain :FileSet ;
                                                 rdfs:range xsd:dateTime ;
                                                 rdfs:comment """The time the image pixel data creation started.

Required if image is part of a Series in which the images are temporally related. May be present otherwise."""@en ;
                                                 rdfs:label "Content Time"@en .


###  http://purl.org/healthcarevocab/v1#ContrastFrameAveraging
<http://purl.org/healthcarevocab/v1#ContrastFrameAveraging> rdf:type owl:DatatypeProperty ;
                                                            rdfs:domain :FileSet ;
                                                            rdfs:range xsd:int ;
                                                            rdfs:comment "Specifies the number of contrast frames to average together before performing the mask operation. If the Attribute is missing, no averaging is performed."@en ;
                                                            rdfs:label "Contrast Frame Averaging"@en .


###  http://purl.org/healthcarevocab/v1#DistanceSourceToDetector
<http://purl.org/healthcarevocab/v1#DistanceSourceToDetector> rdf:type owl:DatatypeProperty ;
                                                              rdfs:domain :FileSet ;
                                                              rdfs:range xsd:float ;
                                                              rdfs:comment "Distance in mm from source to detector center."@en ;
                                                              rdfs:label "Distance From Source To Detector"@en .


###  http://purl.org/healthcarevocab/v1#DistanceSourceToPatient
<http://purl.org/healthcarevocab/v1#DistanceSourceToPatient> rdf:type owl:DatatypeProperty ;
                                                             rdfs:domain :FileSet ;
                                                             rdfs:range xsd:float ;
                                                             rdfs:comment "Distance in mm from source to isocenter (center of field of view)."@en ;
                                                             rdfs:label "Distance From Source To Patient"@en .


###  http://purl.org/healthcarevocab/v1#ExposureTime
<http://purl.org/healthcarevocab/v1#ExposureTime> rdf:type owl:DatatypeProperty ;
                                                  rdfs:domain :CTImageSeriesImagingEvent ,
                                                              :FileSet ;
                                                  rdfs:range xsd:float ;
                                                  rdfs:comment """Time of X-Ray exposure in msec.

If Acquisition Type (0018,9302) equals SPIRAL, the value of this Attribute shall be Revolution Time (0018,9305) divided by the Spiral Pitch Factor (0018,9311). See Section C.8.15.3.8.1 and Section C.8.15.3.2.1.

Shall not be present if this Attribute is present in Multi-energy CT Acquisition Sequence (0018,9362) and the value of this Attribute is not the same in all Items of the Multi-energy CT Acquisition Sequence (0018,9362)."""@en ;
                                                  rdfs:label "Exposure Time"@en .


###  http://purl.org/healthcarevocab/v1#GeneratorID
<http://purl.org/healthcarevocab/v1#GeneratorID> rdf:type owl:DatatypeProperty ;
                                                 rdfs:domain :FileSet ;
                                                 rdfs:range xsd:string ;
                                                 rdfs:comment "Identifier of the generator."@en ;
                                                 rdfs:label "Generator ID"@en .


###  http://purl.org/healthcarevocab/v1#GeneratorPower
<http://purl.org/healthcarevocab/v1#GeneratorPower> rdf:type owl:DatatypeProperty ;
                                                    rdfs:domain :FileSet ;
                                                    rdfs:range xsd:float ;
                                                    rdfs:comment """Power in kW to the X-Ray generator.

Shall not be present if this Attribute is present in Multi-energy CT Acquisition Sequence (0018,9362) and the value of this Attribute is not the same in all Items of the Multi-energy CT Acquisition Sequence (0018,9362)."""@en ;
                                                    rdfs:label "Generator Power"@en .


###  http://purl.org/healthcarevocab/v1#HighBit
<http://purl.org/healthcarevocab/v1#HighBit> rdf:type owl:DatatypeProperty ;
                                             rdfs:domain :FileSet ;
                                             rdfs:range xsd:int ;
                                             rdfs:comment "Most significant bit for pixel sample data. Each sample shall have the same high bit. High Bit (0028,0102) shall be one less than Bits Stored (0028,0101). See PS3.5 for further explanation."@en ;
                                             rdfs:label "High Bit"@en .


###  http://purl.org/healthcarevocab/v1#ImageOrientationPatient
<http://purl.org/healthcarevocab/v1#ImageOrientationPatient> rdf:type owl:DatatypeProperty ;
                                                             rdfs:domain :FileSet ;
                                                             rdfs:range xsd:string ;
                                                             rdfs:comment "The direction cosines of the first row and the first column with respect to the patient. See Section C.7.6.2.1.1 for further explanation."@en ;
                                                             rdfs:label "Image Orientation Patient"@en .


###  http://purl.org/healthcarevocab/v1#ImagePositionPatient
<http://purl.org/healthcarevocab/v1#ImagePositionPatient> rdf:type owl:DatatypeProperty ;
                                                          rdfs:domain :FileSet ;
                                                          rdfs:range xsd:string ;
                                                          rdfs:comment """Patient position descriptor relative to the equipment. See Section C.7.1.4.1.1.1.

See Section C.7.3.1.1.2 for Defined Terms and further explanation."""@en ;
                                                          rdfs:label "Image Position Patient"@en .


###  http://purl.org/healthcarevocab/v1#ImageType
<http://purl.org/healthcarevocab/v1#ImageType> rdf:type owl:DatatypeProperty ;
                                               rdfs:domain :FileSet ;
                                               rdfs:range xsd:string ;
                                               rdfs:comment "Image identification characteristics. See Section C.7.6.1.1.2 for Defined Terms and further explanation."@en ;
                                               rdfs:label "Image Type"@en .


###  http://purl.org/healthcarevocab/v1#ImagesInAcquisition
<http://purl.org/healthcarevocab/v1#ImagesInAcquisition> rdf:type owl:DatatypeProperty ;
                                                         rdfs:domain :FileSet ;
                                                         rdfs:range xsd:int ;
                                                         rdfs:comment "Number of images that resulted from this acquisition of data."@en ;
                                                         rdfs:label "Images in Acquisition"@en .


###  http://purl.org/healthcarevocab/v1#InstanceNumber
<http://purl.org/healthcarevocab/v1#InstanceNumber> rdf:type owl:DatatypeProperty ;
                                                    rdfs:domain :FileSet ;
                                                    rdfs:range xsd:string ;
                                                    rdfs:comment "A number that identifies this image."@en ;
                                                    rdfs:label "Instance Number"@en .


###  http://purl.org/healthcarevocab/v1#KVP
<http://purl.org/healthcarevocab/v1#KVP> rdf:type owl:DatatypeProperty ;
                                         rdfs:domain :FileSet ;
                                         rdfs:range xsd:float ;
                                         rdfs:comment """Peak kilo voltage output of the X-Ray generator used.

Shall be empty if this Attribute is present in Multi-energy CT Acquisition Sequence (0018,9362)."""@en ;
                                         rdfs:label "KVP"@en .


###  http://purl.org/healthcarevocab/v1#PixelRepresentation
<http://purl.org/healthcarevocab/v1#PixelRepresentation> rdf:type owl:DatatypeProperty ;
                                                         rdfs:domain :FileSet ;
                                                         rdfs:range xsd:string ;
                                                         rdfs:comment "Data representation of the pixel samples. Each sample shall have the same pixel representation."@en ;
                                                         rdfs:label "Pixel Representation"@en .


###  http://purl.org/healthcarevocab/v1#PixelSpacing
<http://purl.org/healthcarevocab/v1#PixelSpacing> rdf:type owl:DatatypeProperty ;
                                                  rdfs:domain :FileSet ;
                                                  rdfs:range xsd:string ;
                                                  rdfs:comment "Physical distance in the patient between the center of each pixel, specified by a numeric pair - adjacent row spacing (delimiter) adjacent column spacing in mm. See Section 10.7.1.3 for further explanation."@en ;
                                                  rdfs:label "Pixel Spacing"@en .


###  http://purl.org/healthcarevocab/v1#RescaleIntercept
<http://purl.org/healthcarevocab/v1#RescaleIntercept> rdf:type owl:DatatypeProperty ;
                                                      rdfs:domain :FileSet ;
                                                      rdfs:range xsd:string ;
                                                      rdfs:comment """The value b in relationship between stored values (SV) and the output units.

Output units = m*SV+b

If Image Type (0008,0008) Value 1 is ORIGINAL and Value 3 is not LOCALIZER, and Multi-energy CT Acquisition (0018,9361) is either absent or NO, output units shall be Hounsfield Units (HU)."""@en ;
                                                      rdfs:label "Rescale Intercept"@en .


###  http://purl.org/healthcarevocab/v1#RescaleSlope
<http://purl.org/healthcarevocab/v1#RescaleSlope> rdf:type owl:DatatypeProperty ;
                                                  rdfs:domain :FileSet ;
                                                  rdfs:range xsd:float ;
                                                  rdfs:comment "m in the equation specified in Rescale Intercept (0028,1052)."@en ;
                                                  rdfs:label "Rescale Slope"@en .


###  http://purl.org/healthcarevocab/v1#Rows
<http://purl.org/healthcarevocab/v1#Rows> rdf:type owl:DatatypeProperty ;
                                          rdfs:domain :FileSet ;
                                          rdfs:range xsd:int ;
                                          rdfs:comment """Number of rows in the image.

Shall be an exact multiple of the vertical downsampling factor if any of the samples (planes) are encoded downsampled in the vertical direction for pixel data encoded in a Native (uncompressed) format. E.g., required to be an even value for a Photometric Interpretation (0028,0004) of YBR_FULL_422."""@en ;
                                          rdfs:label "Rows"@en .


###  http://purl.org/healthcarevocab/v1#SamplesPerPixel
<http://purl.org/healthcarevocab/v1#SamplesPerPixel> rdf:type owl:DatatypeProperty ;
                                                     rdfs:domain :FileSet ;
                                                     rdfs:range xsd:int ;
                                                     rdfs:comment "Number of samples (planes) in this image. See Section C.7.6.3.1.1 for further explanation."@en ;
                                                     rdfs:label "Samples Per Pixel"@en .


###  http://purl.org/healthcarevocab/v1#SeriesDate
<http://purl.org/healthcarevocab/v1#SeriesDate> rdf:type owl:DatatypeProperty ;
                                                rdfs:domain :FileSet ;
                                                rdfs:range xsd:date ;
                                                rdfs:comment "Date the Series started."@en ;
                                                rdfs:label "Series Date"@en .


###  http://purl.org/healthcarevocab/v1#SeriesTime
<http://purl.org/healthcarevocab/v1#SeriesTime> rdf:type owl:DatatypeProperty ;
                                                rdfs:domain :FileSet ;
                                                rdfs:range xsd:dateTime ;
                                                rdfs:comment "Time the Series started."@en ;
                                                rdfs:label "Series Time"@en .


###  http://purl.org/healthcarevocab/v1#SliceThickness
<http://purl.org/healthcarevocab/v1#SliceThickness> rdf:type owl:DatatypeProperty ;
                                                    rdfs:domain :FileSet ,
                                                                :Media ;
                                                    rdfs:range xsd:float ;
                                                    rdfs:comment "Nominal slice thickness, in mm."@en ;
                                                    rdfs:label "Slice Thickness"@en .


###  http://purl.org/healthcarevocab/v1#SpacingBetweenSlices
<http://purl.org/healthcarevocab/v1#SpacingBetweenSlices> rdf:type owl:DatatypeProperty ;
                                                          rdfs:domain :FileSet ;
                                                          rdfs:range xsd:float ;
                                                          rdfs:comment "Spacing between slices, in mm. The spacing is measured from the center-to-center of each slice."@en ;
                                                          rdfs:label "Spacing Between Slices"@en .


###  http://purl.org/healthcarevocab/v1#SpiralPitchFactor
<http://purl.org/healthcarevocab/v1#SpiralPitchFactor> rdf:type owl:DatatypeProperty ;
                                                       rdfs:domain :FileSet ;
                                                       rdfs:range xsd:float ;
                                                       rdfs:comment "Ratio of the Table Feed per Rotation (0018,9310) to the Total Collimation Width (0018,9307)."@en ;
                                                       rdfs:label "Spiral Pitch Factor"@en .


###  http://purl.org/healthcarevocab/v1#StudyDate
<http://purl.org/healthcarevocab/v1#StudyDate> rdf:type owl:DatatypeProperty ;
                                               rdfs:domain :FileSet ;
                                               rdfs:range xsd:date ;
                                               rdfs:comment "Date the Study started."@en ;
                                               rdfs:label "Study Date"@en .


###  http://purl.org/healthcarevocab/v1#StudyTime
<http://purl.org/healthcarevocab/v1#StudyTime> rdf:type owl:DatatypeProperty ;
                                               rdfs:domain :FileSet ;
                                               rdfs:range xsd:dateTime ;
                                               rdfs:comment "Time the Study started."@en ;
                                               rdfs:label "Study Time"@en .


###  http://purl.org/healthcarevocab/v1#WindowCenter
<http://purl.org/healthcarevocab/v1#WindowCenter> rdf:type owl:DatatypeProperty ;
                                                  rdfs:domain :FileSet ;
                                                  rdfs:range xsd:string ;
                                                  rdfs:comment """Window Center for display.

See Section C.11.2.1.2 for further explanation.

Required if VOI LUT Sequence (0028,3010) is not present. May be present otherwise."""@en ;
                                                  rdfs:label "Window Center"@en .


###  http://purl.org/healthcarevocab/v1#WindowWidth
<http://purl.org/healthcarevocab/v1#WindowWidth> rdf:type owl:DatatypeProperty ;
                                                 rdfs:domain :FileSet ;
                                                 rdfs:range xsd:string ;
                                                 rdfs:comment """Window Width for display. See Section C.11.2.1.2 for further explanation.

Required if Window Center (0028,1050) is present."""@en ;
                                                 rdfs:label "Window Width"@en .


###  http://purl.org/healthcarevocab/v1#XRayTubeCurrent
<http://purl.org/healthcarevocab/v1#XRayTubeCurrent> rdf:type owl:DatatypeProperty ;
                                                     rdfs:domain :FileSet ;
                                                     rdfs:range xsd:float ;
                                                     rdfs:comment "X-Ray Tube Current in mA. Required if Exposure (0018,1152) is not present. May be present otherwise."@en ;
                                                     rdfs:label "X-Ray Tube Current"@en .


###  http://rs.tdwg.org/ac/terms/IDofContainingCollection
<http://rs.tdwg.org/ac/terms/IDofContainingCollection> rdf:type owl:DatatypeProperty ;
                                                       <http://purl.org/dc/terms/description> "Repeatable: A media resource may be member of multiple collections. The form of the identifier is left to implementers of specific implementations."@en ;
                                                       <http://purl.org/dc/terms/hasVersion> <http://rs.tdwg.org/ac/terms/version/IDofContainingCollection-2013-10-28> ,
                                                                                             <http://rs.tdwg.org/ac/terms/version/IDofContainingCollection-2020-01-27> ;
                                                       <http://purl.org/dc/terms/isPartOf> <http://rs.tdwg.org/ac/terms/> ;
                                                       <http://rs.tdwg.org/dwc/terms/attributes/organizedInClass> <http://rs.tdwg.org/dwc/terms/attributes/RelatedResources> ;
                                                       <http://rs.tdwg.org/dwc/terms/attributes/repeatable> "Yes" ;
                                                       <http://rs.tdwg.org/dwc/terms/attributes/required> "No" ;
                                                       rdfs:comment "If the resource is contained in a Collection, this field identifies that Collection uniquely."@en ;
                                                       rdfs:isDefinedBy <http://rs.tdwg.org/ac/terms/> ;
                                                       rdfs:label "ID of Containing Collection"@en .


###  http://rs.tdwg.org/ac/terms/fundingAttribution
<http://rs.tdwg.org/ac/terms/fundingAttribution> rdf:type owl:DatatypeProperty ;
                                                 <http://purl.org/dc/elements/1.1/format> "application/rdf+xml" ;
                                                 <http://purl.org/dc/terms/hasVersion> <http://rs.tdwg.org/ac/terms/version/fundingAttribution-2013-10-28> ,
                                                                                       <http://rs.tdwg.org/ac/terms/version/fundingAttribution-2020-01-27> ;
                                                 <http://purl.org/dc/terms/isPartOf> <http://rs.tdwg.org/ac/terms/> ;
                                                 <http://purl.org/dc/terms/references> <http://rs.tdwg.org/ac/terms/fundingAttribution> ;
                                                 <http://rs.tdwg.org/dwc/terms/attributes/organizedInClass> <http://rs.tdwg.org/dwc/terms/attributes/Attribution> ;
                                                 <http://rs.tdwg.org/dwc/terms/attributes/repeatable> "Yes" ;
                                                 <http://rs.tdwg.org/dwc/terms/attributes/required> "No" ;
                                                 rdfs:comment "Text description of organizations or individuals who funded the creation of the resource."@en ;
                                                 rdfs:isDefinedBy <http://rs.tdwg.org/ac/terms/> ;
                                                 rdfs:label "Funding"@en .


###  http://rs.tdwg.org/ac/terms/providerManagedID
<http://rs.tdwg.org/ac/terms/providerManagedID> rdf:type owl:DatatypeProperty ;
                                                <http://purl.org/dc/terms/description> "Ideally, this would be a globally unique identifier (GUID), but the provider is encouraged to supply any form of identifier that simplifies communications on resources within their project and helps to locate individual data items in the provider's data repositories. It is the provider's decision whether to expose this value or not."@en ;
                                                <http://purl.org/dc/terms/hasVersion> <http://rs.tdwg.org/ac/terms/version/providerManagedID-2013-10-28> ,
                                                                                      <http://rs.tdwg.org/ac/terms/version/providerManagedID-2020-01-27> ;
                                                <http://purl.org/dc/terms/isPartOf> <http://rs.tdwg.org/ac/terms/> ;
                                                <http://rs.tdwg.org/dwc/terms/attributes/organizedInClass> <http://rs.tdwg.org/dwc/terms/attributes/Management> ;
                                                <http://rs.tdwg.org/dwc/terms/attributes/repeatable> "No" ;
                                                <http://rs.tdwg.org/dwc/terms/attributes/required> "No" ;
                                                rdfs:comment "A free-form identifier (a simple number, an alphanumeric code, a URL, etc.) for the resource that is unique and meaningful primarily for the data provider."@en ;
                                                rdfs:isDefinedBy <http://rs.tdwg.org/ac/terms/> ;
                                                rdfs:label "Provider-managed ID"@en .


###  http://rs.tdwg.org/ac/terms/subjectOrientation
<http://rs.tdwg.org/ac/terms/subjectOrientation> rdf:type owl:DatatypeProperty ;
                                                 <http://purl.org/dc/terms/hasVersion> <http://rs.tdwg.org/ac/terms/version/subjectOrientation-2013-10-28> ,
                                                                                       <http://rs.tdwg.org/ac/terms/version/subjectOrientation-2020-01-27> ,
                                                                                       <http://rs.tdwg.org/ac/terms/version/subjectOrientation-2022-02-23> ;
                                                 <http://purl.org/dc/terms/isPartOf> <http://rs.tdwg.org/ac/terms/> ;
                                                 <http://rs.tdwg.org/dwc/terms/attributes/organizedInClass> <http://rs.tdwg.org/dwc/terms/attributes/TaxonomicCoverage> ;
                                                 <http://rs.tdwg.org/dwc/terms/attributes/repeatable> "No" ;
                                                 <http://rs.tdwg.org/dwc/terms/attributes/required> "No" ;
                                                 rdfs:comment "Specific orientation (= direction, view angle) of the subject represented in the media resource with respect to the acquisition device, denoted by an IRI."@en ;
                                                 rdfs:isDefinedBy <http://rs.tdwg.org/ac/terms/> ;
                                                 rdfs:label "Subject Orientation"@en ;
                                                 <http://www.w3.org/2004/02/skos/core#scopeNote> "Values SHOULD be selected from the Controlled Vocabulary for Audubon Core subjectOrientation. In text-based systems such as tables, IRI values MUST be in unabbreviated form."@en .


###  http://rs.tdwg.org/ac/terms/subjectPart
<http://rs.tdwg.org/ac/terms/subjectPart> rdf:type owl:DatatypeProperty ;
                                          <http://purl.org/dc/terms/hasVersion> <http://rs.tdwg.org/ac/terms/version/subjectPart-2013-10-28> ,
                                                                                <http://rs.tdwg.org/ac/terms/version/subjectPart-2020-01-27> ,
                                                                                <http://rs.tdwg.org/ac/terms/version/subjectPart-2022-02-23> ;
                                          <http://purl.org/dc/terms/isPartOf> <http://rs.tdwg.org/ac/terms/> ;
                                          <http://rs.tdwg.org/dwc/terms/attributes/organizedInClass> <http://rs.tdwg.org/dwc/terms/attributes/TaxonomicCoverage> ;
                                          <http://rs.tdwg.org/dwc/terms/attributes/repeatable> "No" ;
                                          <http://rs.tdwg.org/dwc/terms/attributes/required> "No" ;
                                          rdfs:comment "The portion or product of organism morphology, behaviour, environment, etc. that is either predominantly shown or particularly well exemplified by the media resource, denoted by an IRI."@en ;
                                          rdfs:isDefinedBy <http://rs.tdwg.org/ac/terms/> ;
                                          rdfs:label "Subject Part"@en ;
                                          <http://www.w3.org/2004/02/skos/core#scopeNote> "Values SHOULD be selected from the Controlled Vocabulary for Audubon Core subjectPart. In text-based systems such as tables, IRI values MUST be in unabbreviated form."@en .


###  http://rs.tdwg.org/dwc/terms/catalogNumber
<http://rs.tdwg.org/dwc/terms/catalogNumber> rdf:type owl:DatatypeProperty ;
                                             rdfs:domain :PhysicalObject ;
                                             rdfs:range xsd:string ;
                                             <http://purl.org/dc/terms/hasVersion> <http://rs.tdwg.org/dwc/terms/version/catalogNumber-2009-04-24> ,
                                                                                   <http://rs.tdwg.org/dwc/terms/version/catalogNumber-2017-10-06> ;
                                             <http://purl.org/dc/terms/isPartOf> <http://rs.tdwg.org/dwc/terms/> ;
                                             <http://purl.org/dc/terms/replaces> <http://rs.tdwg.org/dwc/dwcore/CatalogNumber> ;
                                             <http://rs.tdwg.org/dwc/terms/attributes/abcdEquivalence> "DataSets/DataSet/Units/Unit/UnitID" ;
                                             <http://rs.tdwg.org/dwc/terms/attributes/organizedInClass> <http://rs.tdwg.org/dwc/terms/Occurrence> ;
                                             <http://rs.tdwg.org/dwc/terms/attributes/usageScope> "simple" ;
                                             rdfs:comment "An identifier (preferably unique) for the record within the data set or collection."@en ;
                                             rdfs:isDefinedBy <http://rs.tdwg.org/dwc/terms/> ;
                                             rdfs:label "Catalog Number"@en ;
                                             <http://www.w3.org/2004/02/skos/core#example> "`145732`, `145732a`, `2008.1334`, `R-4313`"@en .


###  http://rs.tdwg.org/dwc/terms/collectionCode
<http://rs.tdwg.org/dwc/terms/collectionCode> rdf:type owl:DatatypeProperty ;
                                              rdfs:domain :Organization ,
                                                          :PhysicalObject ;
                                              rdfs:range xsd:string ;
                                              <http://purl.org/dc/terms/hasVersion> <http://rs.tdwg.org/dwc/terms/version/collectionCode-2009-04-24> ,
                                                                                    <http://rs.tdwg.org/dwc/terms/version/collectionCode-2009-08-24> ,
                                                                                    <http://rs.tdwg.org/dwc/terms/version/collectionCode-2009-09-11> ,
                                                                                    <http://rs.tdwg.org/dwc/terms/version/collectionCode-2017-10-06> ;
                                              <http://purl.org/dc/terms/isPartOf> <http://rs.tdwg.org/dwc/terms/> ;
                                              <http://purl.org/dc/terms/replaces> <http://rs.tdwg.org/dwc/dwcore/CollectionCode> ;
                                              <http://rs.tdwg.org/dwc/terms/attributes/abcdEquivalence> "DataSets/DataSet/Units/Unit/SourceID" ;
                                              <http://rs.tdwg.org/dwc/terms/attributes/organizedInClass> <http://rs.tdwg.org/dwc/terms/> ;
                                              <http://rs.tdwg.org/dwc/terms/attributes/usageScope> "simple" ;
                                              rdfs:comment "The name, acronym, coden, or initialism identifying the collection or data set from which the record was derived."@en ;
                                              rdfs:isDefinedBy <http://rs.tdwg.org/dwc/terms/> ;
                                              rdfs:label "Collection Code"@en ;
                                              <http://www.w3.org/2004/02/skos/core#example> "`Mammals`, `Hildebrandt`, `EBIRD`, `VP`"@en .


###  http://rs.tdwg.org/dwc/terms/datasetID
<http://rs.tdwg.org/dwc/terms/datasetID> rdf:type owl:DatatypeProperty ;
                                         <http://purl.org/dc/terms/hasVersion> <http://rs.tdwg.org/dwc/terms/version/datasetID-2009-04-24> ,
                                                                               <http://rs.tdwg.org/dwc/terms/version/datasetID-2009-09-11> ,
                                                                               <http://rs.tdwg.org/dwc/terms/version/datasetID-2017-10-06> ;
                                         <http://purl.org/dc/terms/isPartOf> <http://rs.tdwg.org/dwc/terms/> ;
                                         <http://rs.tdwg.org/dwc/terms/attributes/abcdEquivalence> "DataSets/DataSet/DataSetGUID" ;
                                         <http://rs.tdwg.org/dwc/terms/attributes/organizedInClass> <http://rs.tdwg.org/dwc/terms/> ;
                                         <http://rs.tdwg.org/dwc/terms/attributes/usageScope> "simple" ;
                                         rdfs:comment "An identifier for the set of data. May be a global unique identifier or an identifier specific to a collection or institution."@en ;
                                         rdfs:isDefinedBy <http://rs.tdwg.org/dwc/terms/> ;
                                         rdfs:label "Dataset ID"@en ;
                                         <http://www.w3.org/2004/02/skos/core#example> "`b15d4952-7d20-46f1-8a3e-556a512b04c5`"@en .


###  http://rs.tdwg.org/dwc/terms/disposition
<http://rs.tdwg.org/dwc/terms/disposition> rdf:type owl:DatatypeProperty ;
                                           <http://purl.org/dc/terms/description> "Recommended best practice is to use a controlled vocabulary."@en ;
                                           <http://purl.org/dc/terms/hasVersion> <http://rs.tdwg.org/dwc/terms/version/disposition-2009-04-24> ,
                                                                                 <http://rs.tdwg.org/dwc/terms/version/disposition-2017-10-06> ;
                                           <http://purl.org/dc/terms/isPartOf> <http://rs.tdwg.org/dwc/terms/> ;
                                           <http://purl.org/dc/terms/replaces> <http://rs.tdwg.org/dwc/curatorial/Disposition> ;
                                           <http://rs.tdwg.org/dwc/terms/attributes/abcdEquivalence> "DataSets/DataSet/Units/Unit/SpecimenUnit/Disposition" ;
                                           <http://rs.tdwg.org/dwc/terms/attributes/organizedInClass> <http://rs.tdwg.org/dwc/terms/Occurrence> ;
                                           <http://rs.tdwg.org/dwc/terms/attributes/usageScope> "simple" ;
                                           rdfs:comment "The current state of a specimen with respect to the collection identified in collectionCode or collectionID."@en ;
                                           rdfs:isDefinedBy <http://rs.tdwg.org/dwc/terms/> ;
                                           rdfs:label "Disposition"@en ;
                                           <http://www.w3.org/2004/02/skos/core#example> "`in collection`, `missing`, `voucher elsewhere`, `duplicates elsewhere`"@en .


###  http://rs.tdwg.org/dwc/terms/earliestEonOrLowestEonothem
<http://rs.tdwg.org/dwc/terms/earliestEonOrLowestEonothem> rdf:type owl:DatatypeProperty ;
                                                           <http://purl.org/dc/terms/hasVersion> <http://rs.tdwg.org/dwc/terms/version/earliestEonOrLowestEonothem-2009-04-24> ,
                                                                                                 <http://rs.tdwg.org/dwc/terms/version/earliestEonOrLowestEonothem-2017-10-06> ;
                                                           <http://purl.org/dc/terms/isPartOf> <http://rs.tdwg.org/dwc/terms/> ;
                                                           <http://purl.org/dc/terms/replaces> <http://digir.net/schema/conceptual/darwin/extension/paleontology/1.0/EarliestEonOrLowestEonothem> ;
                                                           <http://rs.tdwg.org/dwc/terms/attributes/abcdEquivalence> "not in ABCD" ;
                                                           <http://rs.tdwg.org/dwc/terms/attributes/organizedInClass> <http://rs.tdwg.org/dwc/terms/GeologicalContext> ;
                                                           <http://rs.tdwg.org/dwc/terms/attributes/usageScope> "simple" ;
                                                           rdfs:comment "The full name of the earliest possible geochronologic eon or lowest chrono-stratigraphic eonothem or the informal name (\"Precambrian\") attributable to the stratigraphic horizon from which the cataloged item was collected."@en ;
                                                           rdfs:isDefinedBy <http://rs.tdwg.org/dwc/terms/> ;
                                                           rdfs:label "Earliest Eon Or Lowest Eonothem"@en ;
                                                           <http://www.w3.org/2004/02/skos/core#example> "`Phanerozoic`, `Proterozoic`"@en .


###  http://rs.tdwg.org/dwc/terms/formation
<http://rs.tdwg.org/dwc/terms/formation> rdf:type owl:DatatypeProperty ;
                                         rdfs:domain :PhysicalObject ;
                                         rdfs:range xsd:string ;
                                         <http://purl.org/dc/terms/hasVersion> <http://rs.tdwg.org/dwc/terms/version/formation-2009-04-24> ,
                                                                               <http://rs.tdwg.org/dwc/terms/version/formation-2017-10-06> ;
                                         <http://purl.org/dc/terms/isPartOf> <http://rs.tdwg.org/dwc/terms/> ;
                                         <http://purl.org/dc/terms/replaces> <http://digir.net/schema/conceptual/darwin/extension/paleontology/1.0/Formation> ;
                                         <http://rs.tdwg.org/dwc/terms/attributes/abcdEquivalence> "not in ABCD" ;
                                         <http://rs.tdwg.org/dwc/terms/attributes/organizedInClass> <http://rs.tdwg.org/dwc/terms/GeologicalContext> ;
                                         <http://rs.tdwg.org/dwc/terms/attributes/usageScope> "simple" ;
                                         rdfs:comment "The full name of the lithostratigraphic formation from which the cataloged item was collected."@en ;
                                         rdfs:isDefinedBy <http://rs.tdwg.org/dwc/terms/> ;
                                         rdfs:label "Formation"@en ;
                                         <http://www.w3.org/2004/02/skos/core#example> "`Notch Peak Formation`, `House Limestone`, `Fillmore Formation`"@en .


###  http://rs.tdwg.org/dwc/terms/geologicalContextID
<http://rs.tdwg.org/dwc/terms/geologicalContextID> rdf:type owl:DatatypeProperty ;
                                                   <http://purl.org/dc/terms/hasVersion> <http://rs.tdwg.org/dwc/terms/version/geologicalContextID-2009-07-06> ,
                                                                                         <http://rs.tdwg.org/dwc/terms/version/geologicalContextID-2017-10-06> ;
                                                   <http://purl.org/dc/terms/isPartOf> <http://rs.tdwg.org/dwc/terms/> ;
                                                   <http://rs.tdwg.org/dwc/terms/attributes/abcdEquivalence> "not in ABCD" ;
                                                   <http://rs.tdwg.org/dwc/terms/attributes/organizedInClass> <http://rs.tdwg.org/dwc/terms/GeologicalContext> ;
                                                   <http://rs.tdwg.org/dwc/terms/attributes/usageScope> "simple" ;
                                                   rdfs:comment "An identifier for the set of information associated with a GeologicalContext (the location within a geological context, such as stratigraphy). May be a global unique identifier or an identifier specific to the data set."@en ;
                                                   rdfs:isDefinedBy <http://rs.tdwg.org/dwc/terms/> ;
                                                   rdfs:label "Geological Context ID"@en ;
                                                   <http://www.w3.org/2004/02/skos/core#example> "`https://opencontext.org/subjects/e54377f7-4452-4315-b676-40679b10c4d9`"@en .


###  http://rs.tdwg.org/dwc/terms/institutionCode
<http://rs.tdwg.org/dwc/terms/institutionCode> rdf:type owl:DatatypeProperty ;
                                               rdfs:domain :Organization ,
                                                           :PhysicalObject ;
                                               rdfs:range xsd:string ;
                                               <http://purl.org/dc/terms/hasVersion> <http://rs.tdwg.org/dwc/terms/version/institutionCode-2009-04-24> ,
                                                                                     <http://rs.tdwg.org/dwc/terms/version/institutionCode-2009-08-24> ,
                                                                                     <http://rs.tdwg.org/dwc/terms/version/institutionCode-2009-09-11> ,
                                                                                     <http://rs.tdwg.org/dwc/terms/version/institutionCode-2017-10-06> ;
                                               <http://purl.org/dc/terms/isPartOf> <http://rs.tdwg.org/dwc/terms/> ;
                                               <http://purl.org/dc/terms/replaces> <http://rs.tdwg.org/dwc/dwcore/InstitutionCode> ;
                                               <http://rs.tdwg.org/dwc/terms/attributes/abcdEquivalence> "DataSets/DataSet/Units/Unit/SourceInstitutionID" ;
                                               <http://rs.tdwg.org/dwc/terms/attributes/organizedInClass> <http://rs.tdwg.org/dwc/terms/> ;
                                               <http://rs.tdwg.org/dwc/terms/attributes/usageScope> "simple" ;
                                               rdfs:comment "The name (or acronym) in use by the institution having custody of the object(s) or information referred to in the record."@en ;
                                               rdfs:isDefinedBy <http://rs.tdwg.org/dwc/terms/> ;
                                               rdfs:label "Institution Code"@en ;
                                               <http://www.w3.org/2004/02/skos/core#example> "`MVZ`, `FMNH`, `CLO`, `UCMP`"@en .


###  http://rs.tdwg.org/dwc/terms/locality
<http://rs.tdwg.org/dwc/terms/locality> rdf:type owl:DatatypeProperty ;
                                        <http://purl.org/dc/terms/description> "Less specific geographic information can be provided in other geographic terms (higherGeography, continent, country, stateProvince, county, municipality, waterBody, island, islandGroup). This term may contain information modified from the original to correct perceived errors or standardize the description."@en ;
                                        <http://purl.org/dc/terms/hasVersion> <http://rs.tdwg.org/dwc/terms/version/locality-2009-04-24> ,
                                                                              <http://rs.tdwg.org/dwc/terms/version/locality-2017-10-06> ,
                                                                              <http://rs.tdwg.org/dwc/terms/version/locality-2021-07-15> ;
                                        <http://purl.org/dc/terms/isPartOf> <http://rs.tdwg.org/dwc/terms/> ;
                                        <http://purl.org/dc/terms/replaces> <http://rs.tdwg.org/dwc/dwcore/Locality> ;
                                        <http://rs.tdwg.org/dwc/terms/attributes/abcdEquivalence> "DataSets/DataSet/Units/Unit/Gathering/NamedAreas/NamedArea/AreaName" ;
                                        <http://rs.tdwg.org/dwc/terms/attributes/organizedInClass> <http://purl.org/dc/terms/Location> ;
                                        <http://rs.tdwg.org/dwc/terms/attributes/usageScope> "simple" ;
                                        rdfs:comment "The specific description of the place."@en ;
                                        rdfs:isDefinedBy <http://rs.tdwg.org/dwc/terms/> ;
                                        rdfs:label "Locality"@en ;
                                        <http://www.w3.org/2004/02/skos/core#example> "`Bariloche, 25 km NNE via Ruta Nacional 40 (=Ruta 237)`, `Queets Rainforest, Olympic National Park`"@en .


###  http://rs.tdwg.org/dwc/terms/municipality
<http://rs.tdwg.org/dwc/terms/municipality> rdf:type owl:DatatypeProperty ;
                                            <http://purl.org/dc/terms/description> "Recommended best practice is to use a controlled vocabulary such as the Getty Thesaurus of Geographic Names."@en ;
                                            <http://purl.org/dc/terms/hasVersion> <http://rs.tdwg.org/dwc/terms/version/municipality-2009-08-24> ,
                                                                                  <http://rs.tdwg.org/dwc/terms/version/municipality-2017-10-06> ;
                                            <http://purl.org/dc/terms/isPartOf> <http://rs.tdwg.org/dwc/terms/> ;
                                            <http://rs.tdwg.org/dwc/terms/attributes/abcdEquivalence> "DataSets/DataSet/Units/Unit/Gathering/NamedAreas/NamedArea/AreaName" ;
                                            <http://rs.tdwg.org/dwc/terms/attributes/organizedInClass> <http://purl.org/dc/terms/Location> ;
                                            <http://rs.tdwg.org/dwc/terms/attributes/usageScope> "simple" ;
                                            rdfs:comment "The full, unabbreviated name of the next smaller administrative region than county (city, municipality, etc.) in which the Location occurs. Do not use this term for a nearby named place that does not contain the actual location."@en ;
                                            rdfs:isDefinedBy <http://rs.tdwg.org/dwc/terms/> ;
                                            rdfs:label "Municipality"@en ;
                                            <http://www.w3.org/2004/02/skos/core#example> "`Holzminden`, `Araçatuba`, `Ga-Segonyana`"@en .


###  http://rs.tdwg.org/dwc/terms/occurrenceID
<http://rs.tdwg.org/dwc/terms/occurrenceID> rdf:type owl:DatatypeProperty ;
                                            rdfs:domain :BiologicalSpecimenObject ;
                                            rdfs:range xsd:string ;
                                            <http://purl.org/dc/terms/description> "Recommended best practice is to use a persistent, globally unique identifier."@en ;
                                            <http://purl.org/dc/terms/hasVersion> <http://rs.tdwg.org/dwc/terms/version/occurrenceID-2009-04-24> ,
                                                                                  <http://rs.tdwg.org/dwc/terms/version/occurrenceID-2017-10-06> ;
                                            <http://purl.org/dc/terms/isPartOf> <http://rs.tdwg.org/dwc/terms/> ;
                                            <http://purl.org/dc/terms/replaces> <http://rs.tdwg.org/dwc/dwcore/GlobalUniqueIdentifier> ;
                                            <http://rs.tdwg.org/dwc/terms/attributes/abcdEquivalence> "DataSets/DataSet/Units/Unit/UnitGUID" ;
                                            <http://rs.tdwg.org/dwc/terms/attributes/organizedInClass> <http://rs.tdwg.org/dwc/terms/Occurrence> ;
                                            <http://rs.tdwg.org/dwc/terms/attributes/usageScope> "simple" ;
                                            rdfs:comment "An identifier for the Occurrence (as opposed to a particular digital record of the occurrence). In the absence of a persistent global unique identifier, construct one from a combination of identifiers in the record that will most closely make the occurrenceID globally unique."@en ;
                                            rdfs:isDefinedBy <http://rs.tdwg.org/dwc/terms/> ;
                                            rdfs:label "Occurrence ID"@en ;
                                            <http://www.w3.org/2004/02/skos/core#example> "`http://arctos.database.museum/guid/MSB:Mamm:233627`, `000866d2-c177-4648-a200-ead4007051b9`, `urn:catalog:UWBM:Bird:89776`"@en .


###  http://rs.tdwg.org/dwc/terms/typeStatus
<http://rs.tdwg.org/dwc/terms/typeStatus> rdf:type owl:DatatypeProperty ;
                                          <http://purl.org/dc/terms/description> "Recommended best practice is to separate the values in a list with space vertical bar space (` | `)."@en ;
                                          <http://purl.org/dc/terms/hasVersion> <http://rs.tdwg.org/dwc/terms/version/typeStatus-2009-04-24> ,
                                                                                <http://rs.tdwg.org/dwc/terms/version/typeStatus-2014-10-23> ,
                                                                                <http://rs.tdwg.org/dwc/terms/version/typeStatus-2017-10-06> ;
                                          <http://purl.org/dc/terms/isPartOf> <http://rs.tdwg.org/dwc/terms/> ;
                                          <http://purl.org/dc/terms/replaces> <http://rs.tdwg.org/dwc/curatorial/TypeStatus> ;
                                          <http://rs.tdwg.org/dwc/terms/attributes/abcdEquivalence> "DataSets/DataSet/Units/Unit/SpecimenUnit/NomenclaturalTypeDesignations/NomenclaturalTypeText" ;
                                          <http://rs.tdwg.org/dwc/terms/attributes/decision> <http://rs.tdwg.org/dwc/terms/history/decisions/#Decision-2014-10-30_16> ;
                                          <http://rs.tdwg.org/dwc/terms/attributes/organizedInClass> <http://rs.tdwg.org/dwc/terms/Identification> ;
                                          <http://rs.tdwg.org/dwc/terms/attributes/usageScope> "simple" ;
                                          rdfs:comment "A list (concatenated and separated) of nomenclatural types (type status, typified scientific name, publication) applied to the subject."@en ;
                                          rdfs:isDefinedBy <http://rs.tdwg.org/dwc/terms/> ;
                                          rdfs:label "Type Status"@en ;
                                          <http://www.w3.org/2004/02/skos/core#definition> "A list (concatenated and separated) of nomenclatural types (type status, typified scientific name, publication) applied to the subject."@en ;
                                          <http://www.w3.org/2004/02/skos/core#example> "`holotype of Ctenomys sociabilis. Pearson O. P., and M. I. Christie. 1985. Historia Natural, 5(37):388`, `holotype of Pinus abies | holotype of Picea abies`"@en ;
                                          <http://www.w3.org/2004/02/skos/core#prefLabel> "Type Status"@en .


###  http://www.europeana.eu/schemas/edm/currentLocation
<http://www.europeana.eu/schemas/edm/currentLocation> rdf:type owl:DatatypeProperty ;
                                                      rdfs:domain :PhysicalObject ;
                                                      rdfs:range xsd:string ;
                                                      rdfs:comment "The geographic location and/or name of the repository, building, site, or other entity whose boundaries presently include the resource."@en ;
                                                      rdfs:label "Current Location"@en .


###  http://www.w3.org/2000/01/rdf-schema#seeAlso
rdfs:seeAlso rdf:type owl:DatatypeProperty .


###  http://www.w3.org/2003/12/exif/ns#apertureValue
<http://www.w3.org/2003/12/exif/ns#apertureValue> rdf:type owl:DatatypeProperty ;
                                                  rdfs:domain :FileSet ,
                                                              :PhotogrammetryImagingEvent ,
                                                              :PhotographyImagingEvent ;
                                                  rdfs:range xsd:float ;
                                                  rdfs:comment "The lens aperture. The unit is the APEX value."@en ,
                                                               "レンズ絞り値（APEX値）。この値のルート2のベキ乗を取ると、通常の絞り値となる。例えば'5'の場合だと√2^5=F5.6"@ja ;
                                                  rdfs:label "ApertureValue"@en ;
                                                  <http://www.w3.org/2003/12/exif/ns#tagNumber> "37378"@en .


###  http://www.w3.org/2003/12/exif/ns#bitsPerSample
<http://www.w3.org/2003/12/exif/ns#bitsPerSample> rdf:type owl:DatatypeProperty ;
                                                  rdfs:domain :FileSet ;
                                                  rdfs:range xsd:int ;
                                                  rdfs:comment "The number of bits per image component. In this standard each component of the image is 8 bits, so the value for this tag is 8. See also SamplesPerPixel. In JPEG compressed data a JPEG marker is used instead of this tag."@en ;
                                                  rdfs:label "BitsPerSample"@en ;
                                                  <http://www.w3.org/2003/12/exif/ns#tagNumber> "258"@en .


###  http://www.w3.org/2003/12/exif/ns#focalLength
<http://www.w3.org/2003/12/exif/ns#focalLength> rdf:type owl:DatatypeProperty ;
                                                rdfs:domain :FileSet ;
                                                rdfs:range xsd:float ;
                                                rdfs:comment "The actual focal length of the lens, in mm. Conversion is not made to the focal length of a 35 mm film camera."@en ,
                                                             "レンズの焦点距離。単位はmm"@ja ;
                                                rdfs:label "FocalLength"@en ;
                                                <http://www.w3.org/2003/12/exif/ns#tagNumber> "37386"@en .


###  http://www.w3.org/2003/12/exif/ns#gpsLatitude
<http://www.w3.org/2003/12/exif/ns#gpsLatitude> rdf:type owl:DatatypeProperty ;
                                                rdfs:comment "The latitude, expressed as three values giving the degrees, minutes, and seconds, respectively."@en ,
                                                             "緯度"@ja ;
                                                rdfs:label "GPSLatitude"@en ;
                                                <http://www.w3.org/2003/12/exif/ns#tagNumber> "2"@en .


###  http://www.w3.org/2003/12/exif/ns#gpsLongitude
<http://www.w3.org/2003/12/exif/ns#gpsLongitude> rdf:type owl:DatatypeProperty ;
                                                 rdfs:comment "The longitude, expressed as three values giving the degrees, minutes, and seconds, respectively."@en ,
                                                              "経度"@ja ;
                                                 rdfs:label "GPSLongitude"@en ;
                                                 <http://www.w3.org/2003/12/exif/ns#tagNumber> "4"@en .


###  http://www.w3.org/2003/12/exif/ns#isoSpeedRatings
<http://www.w3.org/2003/12/exif/ns#isoSpeedRatings> rdf:type owl:DatatypeProperty ;
                                                    rdfs:domain :FileSet ,
                                                                :PhotogrammetryImagingEvent ,
                                                                :PhotographyImagingEvent ;
                                                    rdfs:range xsd:string ;
                                                    rdfs:comment "CCD感度の銀塩フィルム換算値"@ja ,
                                                                 "Indicates the ISO Speed and ISO Latitude of the camera or input device as specified in ISO 12232."@en ;
                                                    rdfs:label "ISOSpeedRatings"@en ;
                                                    <http://www.w3.org/2003/12/exif/ns#tagNumber> "34855"@en .


###  http://www.w3.org/2003/12/exif/ns#shutterSpeedValue
<http://www.w3.org/2003/12/exif/ns#shutterSpeedValue> rdf:type owl:DatatypeProperty ;
                                                      rdfs:comment "Shutter speed. The unit is the APEX (Additive System of Photographic Exposure) setting"@en ,
                                                                   "シャッター速度（APEX値）。この値の2のベキ乗をとって逆数にすると、通常のシャッター速度表示になる。例えば'4'の場合だと1/(2^4)=1/16秒"@ja ;
                                                      rdfs:label "ShutterSpeedValue"@en ;
                                                      <http://www.w3.org/2003/12/exif/ns#tagNumber> "37377"@en .


###  https://www.morphosource.org/terms/morphosource#ID
:ID rdf:type owl:DatatypeProperty ;
    rdfs:domain :Device ,
                :FileSet ,
                :ImagingEvent ,
                :Media ,
                :Organization ,
                :PhysicalObject ,
                :ProcessingEvent ;
    rdfs:range xsd:string ;
    rdfs:comment "Morphosource-specific unique ID identifier for a Work (Media, Organization, Device, etc.)."@en ;
    rdfs:label "ID"@en .


###  https://www.morphosource.org/terms/morphosource#address
:address rdf:type owl:DatatypeProperty ;
         rdfs:subPropertyOf <http://rs.tdwg.org/dwc/terms/locality> ;
         rdfs:domain :Organization ,
                     :PhysicalObject ;
         rdfs:range xsd:string ;
         <http://purl.org/dc/terms/isVersionOf> "http://rs.tdwg.org/dwc/terms/locality" ;
         <http://rs.tdwg.org/dwc/terms/attributes/abcdEquivalence> "DataSets/DataSet/Units/Unit/Gathering/NamedAreas/NamedArea/AreaName" ;
         <http://rs.tdwg.org/dwc/terms/attributes/organizedInClass> <http://purl.org/dc/terms/Location> ;
         <http://rs.tdwg.org/dwc/terms/attributes/usageScope> "simple" ;
         rdfs:comment "The street address or other specific description of the place or location."@en ;
         rdfs:label "Address"@en ;
         <http://www.w3.org/2004/02/skos/core#example> "`130 Science Dr`"@en .


###  https://www.morphosource.org/terms/morphosource#agreementURI
:agreementURI rdf:type owl:DatatypeProperty ;
              rdfs:subPropertyOf <http://ns.adobe.com/xap/1.0/rights/UsageTerms> ;
              rdfs:domain :Media ,
                          :Organization ;
              rdfs:range xsd:anyURI ;
              <http://purl.org/dc/terms/isVersionOf> <http://ns.adobe.com/xap/1.0/rights/UsageTerms> ;
              rdfs:comment "A Web URI for a statement of the ownership and usage rights for Media. This more accurately maps to xmpRights:WebStatement than xmpRights:UsageTerms, and should be changed accordingly."@en ;
              rdfs:label "Agreement URI"@en .


###  https://www.morphosource.org/terms/morphosource#amperage
:amperage rdf:type owl:DatatypeProperty ;
          rdfs:subPropertyOf <http://purl.org/healthcarevocab/v1#XRayTubeCurrent> ;
          rdfs:domain :CTImageSeriesImagingEvent ;
          rdfs:range xsd:float ;
          <http://purl.org/dc/terms/isVersionOf> <http://purl.org/healthcarevocab/v1#XRayTubeCurrent> ;
          rdfs:comment "X-Ray Tube Current in mA."@en ;
          rdfs:label "Amperage"@en .


###  https://www.morphosource.org/terms/morphosource#ark
:ark rdf:type owl:DatatypeProperty ;
     rdfs:subPropertyOf :mediaARK ;
     rdfs:domain :Media ;
     rdfs:range xsd:string ;
     rdfs:comment "Persistent identifier for MorphoSource Media automatically created on Media submission. ARKs can apply to both unpublished and published media."@en ;
     rdfs:label "ARK (Archival Resource Key)"@en .


###  https://www.morphosource.org/terms/morphosource#attachmentFile
:attachmentFile rdf:type owl:DatatypeProperty ;
                rdfs:domain :ImagingEvent ,
                            :Media ,
                            :Organization ,
                            :ProcessingEvent ;
                rdfs:comment "A binary attachment file associated with a Work record. Often used to provide additional description beyond that allowed by object properties."@en ;
                rdfs:label "Attachment File"@en .


###  https://www.morphosource.org/terms/morphosource#boundingBoxX
:boundingBoxX rdf:type owl:DatatypeProperty ;
              rdfs:domain :FileSet ;
              rdfs:range xsd:float ;
              rdfs:comment "Length across the X axis of the rectangular bounding box surrounding a 3D digital object."@en ;
              rdfs:label "Bounding Box X"@en .


###  https://www.morphosource.org/terms/morphosource#boundingBoxY
:boundingBoxY rdf:type owl:DatatypeProperty ;
              rdfs:domain :FileSet ;
              rdfs:range xsd:float ;
              rdfs:comment "Length across the Y axis of the rectangular bounding box surrounding a 3D digital object."@en ;
              rdfs:label "Bounding Box Y"@en .


###  https://www.morphosource.org/terms/morphosource#boundingBoxZ
:boundingBoxZ rdf:type owl:DatatypeProperty ;
              rdfs:domain :FileSet ;
              rdfs:range xsd:float ;
              rdfs:comment "Length across the Z axis of the rectangular bounding box surrounding a 3D digital object."@en ;
              rdfs:label "Bounding Box Z"@en .


###  https://www.morphosource.org/terms/morphosource#canonicalTaxonomy
:canonicalTaxonomy rdf:type owl:DatatypeProperty ;
                   rdfs:subPropertyOf :ID ;
                   rdfs:domain :BiologicalSpecimenObject ;
                   rdfs:range xsd:string ;
                   rdfs:comment "MorphoSource-specific ID of Taxonomy record for taxonomic name attributed to the specimen physical object by the provider organization (museum, institution, or laboratory) responsible for managing the specimen. May not be present if no provider-supplied taxonomy is present. This may differ from taxonomic names attributed to the specimen by researchers or other individuals. Values for this property should be a subset of values for property morphosource:taxonomyID values, but morphosource:taxonomyID may include additional values as well."@en ;
                   rdfs:label "Canonical Taxonomy"@en .


###  https://www.morphosource.org/terms/morphosource#centroidX
:centroidX rdf:type owl:DatatypeProperty ;
           rdfs:domain :FileSet ;
           rdfs:range xsd:float ;
           rdfs:comment "X axis coordinate of the centroid of a 3D object, where the centroid is the geometric center point of the object."@en ;
           rdfs:label "Centroid X"@en .


###  https://www.morphosource.org/terms/morphosource#centroidY
:centroidY rdf:type owl:DatatypeProperty ;
           rdfs:domain :FileSet ;
           rdfs:range xsd:float ;
           rdfs:comment "Y axis coordinate of the centroid of a 3D object, where the centroid is the geometric center point of the object."@en ;
           rdfs:label "Centroid Y"@en .


###  https://www.morphosource.org/terms/morphosource#centroidZ
:centroidZ rdf:type owl:DatatypeProperty ;
           rdfs:domain :FileSet ;
           rdfs:range xsd:float ;
           rdfs:comment "Z axis coordinate of the centroid of a 3D object, where the centroid is the geometric center point of the object."@en ;
           rdfs:label "Centroid Z"@en .


###  https://www.morphosource.org/terms/morphosource#choAttribute
:choAttribute rdf:type owl:DatatypeProperty ;
              rdfs:domain :CulturalHeritageObject ;
              rdfs:range xsd:string ;
              rdfs:comment "Physical attributes of an object, including characteristics such as size and shape, chemical properties of materials, qualities of texture and hardness, and features such as surface ornament. It is preferred to use morphosource:aatAttribute when it is possible to express attributes using the Getty Arts and Architecture Thesaurus controlled vocabulary. This property is for custom attribute values not listed in the Getty AAT controlled vocabulary."@en ;
              rdfs:label "Cultural Heritage Object Attribute"@en .


###  https://www.morphosource.org/terms/morphosource#choType
:choType rdf:type owl:DatatypeProperty ;
         rdfs:domain :CulturalHeritageObject ;
         rdfs:range xsd:string ;
         rdfs:comment "Type, genre, category, or classification of an object. It is preferred to use morphosource:aatType when it is possible to express type using the Getty Arts and Architecture Thesaurus controlled vocabulary. This property is for custom type values not listed in the Getty AAT controlled vocabulary."@en ;
         rdfs:label "Cultural Heritage Object Type"@en .


###  https://www.morphosource.org/terms/morphosource#citeAs
:citeAs rdf:type owl:DatatypeProperty ;
        rdfs:subPropertyOf <http://ns.adobe.com/photoshop/1.0/Credit> ;
        rdfs:domain :Media ;
        rdfs:range xsd:string ;
        <http://purl.org/dc/terms/isVersionOf> <http://ns.adobe.com/photoshop/1.0/Credit> ;
        rdfs:comment "Instructions and guidelines for the citation of a Media. This should include additional instructions beyond those included in other metadata fields or in any download usage agreement."@en ;
        rdfs:label "Cite As"@en .


###  https://www.morphosource.org/terms/morphosource#city
:city rdf:type owl:DatatypeProperty ;
      rdfs:subPropertyOf <http://rs.tdwg.org/dwc/terms/municipality> ;
      rdfs:domain :Organization ,
                  :PhysicalObject ;
      rdfs:range xsd:string ;
      <http://purl.org/dc/terms/description> "Recommended best practice is to use a controlled vocabulary such as the Getty Thesaurus of Geographic Names."@en ;
      <http://purl.org/dc/terms/isVersionOf> <http://rs.tdwg.org/dwc/terms/municipality> ;
      <http://rs.tdwg.org/dwc/terms/attributes/abcdEquivalence> "DataSets/DataSet/Units/Unit/Gathering/NamedAreas/NamedArea/AreaName" ;
      <http://rs.tdwg.org/dwc/terms/attributes/organizedInClass> <http://purl.org/dc/terms/Location> ;
      <http://rs.tdwg.org/dwc/terms/attributes/usageScope> "simple" ;
      rdfs:comment "The full, unabbreviated name of the next smaller administrative region than county (city, municipality, etc.) in which the Location occurs. Do not use this term for a nearby named place that does not contain the actual location."@en ;
      rdfs:label "City"@en ;
      <http://www.w3.org/2004/02/skos/core#example> "`Holzminden`, `Araçatuba`, `Ga-Segonyana`"@en .


###  https://www.morphosource.org/terms/morphosource#contactUser
:contactUser rdf:type owl:DatatypeProperty ;
             rdfs:domain :Organization ;
             rdfs:range xsd:string ;
             rdfs:comment "Contact individual associated with the Organization. Does not need to be a MorphoSource User."@en ;
             rdfs:label "Contact User"@en .


###  https://www.morphosource.org/terms/morphosource#contentsAcceptedFileCount
:contentsAcceptedFileCount rdf:type owl:DatatypeProperty ;
                           rdfs:domain :FileSet ;
                           rdfs:range xsd:int ;
                           rdfs:comment "For a ZIP archive file, the largest number of system-recognized files with the same system-permissible file type located in a single directory. In MorphoSource, this is used to document the number of files in the primary image collection in a CT image stack or photogrammetry image collection."@en ;
                           rdfs:label "Contents Accepted File Count"@en .


###  https://www.morphosource.org/terms/morphosource#contentsFileName
:contentsFileName rdf:type owl:DatatypeProperty ;
                  rdfs:domain :FileSet ;
                  rdfs:range xsd:string ;
                  rdfs:comment "For a ZIP archive file, the file name of a single representative example of the largest number of system-recognized files with the same system-permissible file type located in a single directory. In MorphoSource, this is used to document a single file that is representative of the primary image collection in a CT image stack or photogrammetry image collection or the central mesh in a multi-file mesh archive."@en ;
                  rdfs:label "Contents File Name"@en .


###  https://www.morphosource.org/terms/morphosource#contentsFileSize
:contentsFileSize rdf:type owl:DatatypeProperty ;
                  rdfs:domain :FileSet ;
                  rdfs:range xsd:int ;
                  rdfs:comment "For a ZIP archive file, the file size of a single representative example of the largest number of system-recognized files with the same system-permissible file type located in a single directory. In MorphoSource, this is used to document file size for a single file that is representative of the primary image collection in a CT image stack or photogrammetry image collection or the central mesh in a multi-file mesh archive."@en ;
                  rdfs:label "Contents File Size"@en .


###  https://www.morphosource.org/terms/morphosource#contentsMimeType
:contentsMimeType rdf:type owl:DatatypeProperty ;
                  rdfs:domain :FileSet ;
                  rdfs:range xsd:string ;
                  rdfs:comment "For a ZIP archive file, the mime type of a single representative example of the largest number of system-recognized files with the same system-permissible file type located in a single directory. In MorphoSource, this is used to document a single file that is representative of the primary image collection in a CT image stack or photogrammetry image collection or the central mesh in a multi-file mesh archive."@en ;
                  rdfs:label "Contents Mime Type"@en ;
                  <http://www.w3.org/2004/02/skos/core#example> "`image/jpeg`, `image/tiff`, `application/stl`"@en .


###  https://www.morphosource.org/terms/morphosource#context
:context rdf:type owl:DatatypeProperty ;
         rdfs:subPropertyOf <http://rs.tdwg.org/dwc/terms/geologicalContextID> ;
         rdfs:domain :PhysicalObject ;
         rdfs:range xsd:string ;
         <http://purl.org/dc/terms/isVersionOf> <http://rs.tdwg.org/dwc/terms/geologicalContextID> ;
         <http://rs.tdwg.org/dwc/terms/attributes/abcdEquivalence> "not in ABCD" ;
         <http://rs.tdwg.org/dwc/terms/attributes/organizedInClass> <http://rs.tdwg.org/dwc/terms/GeologicalContext> ;
         <http://rs.tdwg.org/dwc/terms/attributes/usageScope> "simple" ;
         rdfs:comment "An identifier for the set of information associated with a GeologicalContext (the location within a geological context, such as stratigraphy). May be a global unique identifier or an identifier specific to the data set."@en ;
         rdfs:label "Geological Context"@en ;
         <http://www.w3.org/2004/02/skos/core#example> "`https://opencontext.org/subjects/e54377f7-4452-4315-b676-40679b10c4d9`"@en .


###  https://www.morphosource.org/terms/morphosource#crc32
:crc32 rdf:type owl:DatatypeProperty ;
       rdfs:domain :FileSet ;
       rdfs:range xsd:string ;
       rdfs:comment "Checksum hash used to verify the identity of a file and to detect accidental corruption."@en ;
       rdfs:label "CRC32"@en .


###  https://www.morphosource.org/terms/morphosource#dateModified
:dateModified rdf:type owl:DatatypeProperty ;
              rdfs:domain :Device ,
                          :FileSet ,
                          :ImagingEvent ,
                          :Media ,
                          :Organization ,
                          :PhysicalObject ,
                          :ProcessingEvent ;
              rdfs:range xsd:dateTime ;
              <http://purl.org/dc/terms/description> "Recommended practice is to describe the date, date/time, or period of time as recommended for the property Date, of which this is a subproperty."@en ;
              rdfs:comment "Date on which the resource was changed."@en ;
              rdfs:label "Date Modified"@en .


###  https://www.morphosource.org/terms/morphosource#dateUploaded
:dateUploaded rdf:type owl:DatatypeProperty ;
              rdfs:subPropertyOf <http://purl.org/dc/terms/dateSubmitted> ;
              rdfs:domain :Device ,
                          :FileSet ,
                          :ImagingEvent ,
                          :Media ,
                          :Organization ,
                          :PhysicalObject ,
                          :ProcessingEvent ;
              rdfs:range xsd:dateTime ;
              <http://purl.org/dc/terms/description> "Recommended practice is to describe the date, date/time, or period of time as recommended for the property Date, of which this is a subproperty."@en ;
              rdfs:comment "Date of upload of the resource."@en ;
              rdfs:label "Date Uploaded"@en .


###  https://www.morphosource.org/terms/morphosource#datingMethod
:datingMethod rdf:type owl:DatatypeProperty ;
              rdfs:domain :PhysicalObject ;
              rdfs:range xsd:string ;
              rdfs:comment "Method used to determine the date an object was created, produced, fossilized, or otherwise came into being."@en ;
              rdfs:label "Dating Method"@en .


###  https://www.morphosource.org/terms/morphosource#detectorPixelSizeX
:detectorPixelSizeX rdf:type owl:DatatypeProperty ;
                    rdfs:domain :CTImageSeriesImagingEvent ;
                    rdfs:range xsd:float ;
                    rdfs:comment "Length in mm of each pixel in the X direction."@en ;
                    rdfs:label "Detector Pixel Size X"@en .


###  https://www.morphosource.org/terms/morphosource#detectorPixelSizeY
:detectorPixelSizeY rdf:type owl:DatatypeProperty ;
                    rdfs:domain :CTImageSeriesImagingEvent ;
                    rdfs:range xsd:float ;
                    rdfs:comment "Length in mm of each pixel in the Y direction."@en ;
                    rdfs:label "Detector Pixel Size Y"@en .


###  https://www.morphosource.org/terms/morphosource#detectorPixelsX
:detectorPixelsX rdf:type owl:DatatypeProperty ;
                 rdfs:domain :CTImageSeriesImagingEvent ;
                 rdfs:range xsd:int ;
                 rdfs:comment "The number of pixels in the X direction of the detector (number of columns)."@en ;
                 rdfs:label "Detector Pixels X"@en .


###  https://www.morphosource.org/terms/morphosource#detectorPixelsY
:detectorPixelsY rdf:type owl:DatatypeProperty ;
                 rdfs:domain :CTImageSeriesImagingEvent ;
                 rdfs:range xsd:int ;
                 rdfs:comment "The number of pixels in the X direction of the detector (number of rows)."@en ;
                 rdfs:label "Detector Pixels Y"@en .


###  https://www.morphosource.org/terms/morphosource#deviceID
:deviceID rdf:type owl:DatatypeProperty ;
          rdfs:subPropertyOf :ID ;
          rdfs:domain :ImagingEvent ;
          rdfs:range xsd:string ;
          rdfs:comment "MorphoSource-specific unique ID identifier for a Device used in an Imaging Event to image a Physical Object."@en ;
          rdfs:label "Imaging Device ID"@en .


###  https://www.morphosource.org/terms/morphosource#dicomFileTypeExtension
:dicomFileTypeExtension rdf:type owl:DatatypeProperty ;
                        rdfs:domain :FileSet ;
                        rdfs:range xsd:string ;
                        rdfs:comment "Extension code indicating the file format of a file."@en ;
                        rdfs:label "File Type Extension"@en ;
                        <http://www.w3.org/2004/02/skos/core#example> "`dcm`, `ply`, `mp4`"@en .


###  https://www.morphosource.org/terms/morphosource#dicomNumberOfSeriesRelatedInstances
:dicomNumberOfSeriesRelatedInstances rdf:type owl:DatatypeProperty ;
                                     rdfs:label "Number of Series Related Instances"@en .


###  https://www.morphosource.org/terms/morphosource#dicomPixelSpacingHeight
:dicomPixelSpacingHeight rdf:type owl:DatatypeProperty ;
                         rdfs:label "Pixel Spacing Height"@en .


###  https://www.morphosource.org/terms/morphosource#dicomPixelSpacingWidth
:dicomPixelSpacingWidth rdf:type owl:DatatypeProperty ;
                        rdfs:label "Pixel Spacing Width"@en .


###  https://www.morphosource.org/terms/morphosource#dicomSecondaryCaptureDeviceManufacturer
:dicomSecondaryCaptureDeviceManufacturer rdf:type owl:DatatypeProperty ;
                                         rdfs:domain :FileSet ;
                                         rdfs:range xsd:string ;
                                         rdfs:comment "Manufacturer of the Secondary Capture Device. This field should map to some DICOM field."@en ;
                                         rdfs:label "Secondary Capture Device Manufacturer"@en .


###  https://www.morphosource.org/terms/morphosource#dicomSecondaryCaptureDeviceSoftwareVers
:dicomSecondaryCaptureDeviceSoftwareVers rdf:type owl:DatatypeProperty ;
                                         rdfs:domain :FileSet ;
                                         rdfs:range xsd:string ;
                                         rdfs:comment "Manufacturer's designation of software version of the Secondary Capture Device. This field should map to some DICOM field."@en ;
                                         rdfs:label "Secondary Capture Device Software Vers"@en .


###  https://www.morphosource.org/terms/morphosource#dicomSpacingBetweenSlices
:dicomSpacingBetweenSlices rdf:type owl:DatatypeProperty ;
                           rdfs:label "Spacing Between Slices"@en .


###  https://www.morphosource.org/terms/morphosource#dicomWindowCenterAndWidthExplanation
:dicomWindowCenterAndWidthExplanation rdf:type owl:DatatypeProperty ;
                                      rdfs:domain :FileSet ;
                                      rdfs:range xsd:string ;
                                      rdfs:comment "Free form explanation of the meaning of the Window Center and Width. Multiple values correspond to multiple Window Center and Width values. This field should map to dicom:WindowCenterAndWidthExplanation and should be changed accordingly."@en ;
                                      rdfs:label "Window Center and Width Explanation"@en .


###  https://www.morphosource.org/terms/morphosource#dimensions
:dimensions rdf:type owl:DatatypeProperty ;
            rdfs:subPropertyOf <http://purl.org/dc/terms/format> ;
            rdfs:domain :PhysicalObject ;
            rdfs:range xsd:string ;
            <http://purl.org/dc/terms/isVersionOf> <http://purl.org/dc/terms/format> ;
            <http://purl.org/dc/terms/issued> "2008-01-14"^^xsd:date ;
            rdfs:comment "The physical dimensions or measurements of the object."@en ;
            rdfs:label "Dimensions"@en .


###  https://www.morphosource.org/terms/morphosource#doi
:doi rdf:type owl:DatatypeProperty ;
     rdfs:subPropertyOf :mediaDOI ;
     rdfs:domain :Media ;
     rdfs:range xsd:string ;
     rdfs:comment "Persistent identifier for MorphoSource Media created only on user request. DOIs can apply only to published media."@en ;
     rdfs:label "DOI (Digital Object Identifier)"@en .


###  https://www.morphosource.org/terms/morphosource#edgesPerFace
:edgesPerFace rdf:type owl:DatatypeProperty ;
              rdfs:domain :FileSet ;
              rdfs:range xsd:int ;
              rdfs:comment "Number of polygonal edges that connect vertices or points and comprise each face of a polygonal 3D mesh. Values are commonly \"3\" for a triangular mesh or \"4\" for a quadrangular mesh."@en ;
              rdfs:label "Edges Per Face"@en .


###  https://www.morphosource.org/terms/morphosource#exifLensMake
:exifLensMake rdf:type owl:DatatypeProperty ;
              rdfs:label "Lens Make"@en .


###  https://www.morphosource.org/terms/morphosource#exifLensModel
:exifLensModel rdf:type owl:DatatypeProperty ;
               rdfs:label "Lens Model"@en .


###  https://www.morphosource.org/terms/morphosource#faceCount
:faceCount rdf:type owl:DatatypeProperty ;
           rdfs:domain :FileSet ;
           rdfs:range xsd:int ;
           rdfs:comment "Number of polygonal faces comprising a 3D mesh."@en ;
           rdfs:label "Face Count"@en .


###  https://www.morphosource.org/terms/morphosource#fileName
:fileName rdf:type owl:DatatypeProperty ;
          rdfs:domain :FileSet ;
          rdfs:range xsd:string ;
          rdfs:comment "Identifying name label given to a file."@en ;
          rdfs:label "File Name"@en .


###  https://www.morphosource.org/terms/morphosource#fileSize
:fileSize rdf:type owl:DatatypeProperty ;
          rdfs:domain :FileSet ;
          rdfs:range xsd:int ;
          rdfs:comment "Size of a file in bytes."@en ;
          rdfs:label "File Size"@en .


###  https://www.morphosource.org/terms/morphosource#filter
:filter rdf:type owl:DatatypeProperty ;
        rdfs:label "Filter"@en .


###  https://www.morphosource.org/terms/morphosource#fluxNormalization
:fluxNormalization rdf:type owl:DatatypeProperty ;
                   rdfs:domain :CTImageSeriesImagingEvent ;
                   rdfs:range xsd:string ;
                   rdfs:comment "Whether flux normalization calibration is used or not. If present, value must be \"Yes\" or \"No\"."@en ;
                   rdfs:label "Flux Normalization"@en ;
                   <http://www.w3.org/2004/02/skos/core#example> "`Yes`, `No`"@en .


###  https://www.morphosource.org/terms/morphosource#focalLength
:focalLength rdf:type owl:DatatypeProperty ;
             rdfs:domain :PhotogrammetryImagingEvent ,
                         :PhotographyImagingEvent ;
             rdfs:range xsd:float ;
             rdfs:comment "The actual focal length of the lens, in mm. This should probably map to exif:focalLength and should be updated accordingly."@en ;
             rdfs:label "Focal Length"@en .


###  https://www.morphosource.org/terms/morphosource#frameAveraging
:frameAveraging rdf:type owl:DatatypeProperty ;
                rdfs:subPropertyOf <http://purl.org/healthcarevocab/v1#ContrastFrameAveraging> ;
                rdfs:domain :CTImageSeriesImagingEvent ;
                rdfs:range xsd:int ;
                <http://purl.org/dc/terms/isVersionOf> <http://purl.org/healthcarevocab/v1#ContrastFrameAveraging> ;
                rdfs:comment "Number of images acquired at each projection angle and their average."@en ;
                rdfs:label "Frame Averaging"@en .


###  https://www.morphosource.org/terms/morphosource#funding
:funding rdf:type owl:DatatypeProperty ;
         rdfs:subPropertyOf <http://rs.tdwg.org/ac/terms/fundingAttribution> ;
         rdfs:domain :Media ;
         rdfs:range xsd:string ;
         <http://purl.org/dc/terms/isVersionOf> <http://rs.tdwg.org/ac/terms/fundingAttribution> ;
         <http://rs.tdwg.org/dwc/terms/attributes/repeatable> "Yes" ;
         <http://rs.tdwg.org/dwc/terms/attributes/required> "No" ;
         rdfs:comment "Text description of organizations or individuals who funded the creation of the resource."@en ;
         rdfs:label "Funding"@en .


###  https://www.morphosource.org/terms/morphosource#hasUVSpace
:hasUVSpace rdf:type owl:DatatypeProperty ;
            rdfs:domain :FileSet ;
            rdfs:range xsd:string ;
            rdfs:comment "Whether or not a mapping exists to project a 3D object's surface to a 2D image for texture mapping and is present with the 3D object. Values should be \"Yes\" or \"No\"."@en ;
            rdfs:label "Has UV Space"@en ;
            <http://www.w3.org/2004/02/skos/core#example> "`Yes`, `No`"@en .


###  https://www.morphosource.org/terms/morphosource#height
:height rdf:type owl:DatatypeProperty ;
        rdfs:domain :FileSet ;
        rdfs:range xsd:int ;
        rdfs:comment "Height of a 2D image in pixels."@en ;
        rdfs:label "Height in Pixels"@en .


###  https://www.morphosource.org/terms/morphosource#idigbioRecordsetID
:idigbioRecordsetID rdf:type owl:DatatypeProperty ;
                    rdfs:subPropertyOf <http://rs.tdwg.org/dwc/terms/datasetID> ;
                    rdfs:domain :BiologicalSpecimenObject ;
                    rdfs:range xsd:string ;
                    <http://purl.org/dc/terms/isVersionOf> <http://rs.tdwg.org/dwc/terms/datasetID> ;
                    <http://rs.tdwg.org/dwc/terms/attributes/abcdEquivalence> "DataSets/DataSet/DataSetGUID" ;
                    <http://rs.tdwg.org/dwc/terms/attributes/usageScope> "simple" ;
                    rdfs:comment "An identifier for an entire museum, institution, or laboratory specimen collection which includes the Biological Specimen. May be a global unique identifier or an identifier specific to a collection or institution."@en ;
                    rdfs:label "iDigBio Recordset ID"@en ;
                    <http://www.w3.org/2004/02/skos/core#example> "`b15d4952-7d20-46f1-8a3e-556a512b04c5`"@en .


###  https://www.morphosource.org/terms/morphosource#idigbioUUID
:idigbioUUID rdf:type owl:DatatypeProperty ;
             rdfs:domain :BiologicalSpecimenObject ;
             rdfs:range xsd:string ;
             rdfs:comment "Global unique identifier for the Biological Specimen provided by iDigBio and used as the primary identifier of the Biological Specimen's record in the iDigBio aggregator if present. This is sometimes used in addition to more general identifiers or Darwin Core triplets (institution code : collection code : catalog number) to uniquely identify Biological Specimen."@en ;
             rdfs:label "iDigBio UUID"@en .


###  https://www.morphosource.org/terms/morphosource#ieFilter
:ieFilter rdf:type owl:DatatypeProperty ;
          rdfs:subPropertyOf :filter ;
          rdfs:domain :CTImageSeriesImagingEvent ;
          rdfs:range xsd:string ;
          rdfs:comment "Type of filter(s) inserted into the X-Ray beam."@en ;
          rdfs:label "Imaging Event Filter"@en .


###  https://www.morphosource.org/terms/morphosource#imagingEventID
:imagingEventID rdf:type owl:DatatypeProperty ;
                rdfs:subPropertyOf :ID ;
                rdfs:domain :Media ;
                rdfs:range xsd:string ;
                rdfs:label "Imaging Event ID"@en .


###  https://www.morphosource.org/terms/morphosource#institutionName
:institutionName rdf:type owl:DatatypeProperty ;
                 rdfs:domain :Organization ;
                 rdfs:range xsd:string ;
                 rdfs:comment "Name of institution affiliated with Organization. This may be a university in the case of departments or a museum in the case of specific museum collections."@en ;
                 rdfs:label "Institution Name"@en .


###  https://www.morphosource.org/terms/morphosource#isTypeSpecimen
:isTypeSpecimen rdf:type owl:DatatypeProperty ;
                rdfs:subPropertyOf <http://rs.tdwg.org/dwc/terms/typeStatus> ;
                rdfs:domain :BiologicalSpecimenObject ;
                rdfs:range xsd:string ;
                <http://purl.org/dc/terms/isVersionOf> <http://rs.tdwg.org/dwc/terms/typeStatus> ;
                <http://rs.tdwg.org/dwc/terms/attributes/abcdEquivalence> "DataSets/DataSet/Units/Unit/SpecimenUnit/NomenclaturalTypeDesignations/NomenclaturalTypeText" ;
                <http://rs.tdwg.org/dwc/terms/attributes/organizedInClass> <http://rs.tdwg.org/dwc/terms/Identification> ;
                <http://rs.tdwg.org/dwc/terms/attributes/usageScope> "simple" ;
                rdfs:comment "Whether the Biological Specimen is a holotype or not. If present, value must be \"Yes\" or \"No\"."@en ;
                rdfs:label "Is Type Specimen"@en ;
                <http://www.w3.org/2004/02/skos/core#example> "`Yes`, `No`"@en .


###  https://www.morphosource.org/terms/morphosource#latitude
:latitude rdf:type owl:DatatypeProperty ;
          rdfs:subPropertyOf <http://www.w3.org/2003/12/exif/ns#gpsLatitude> ;
          rdfs:domain :PhysicalObject ;
          rdfs:range xsd:string ;
          <http://purl.org/dc/terms/isVersionOf> <http://www.w3.org/2003/12/exif/ns#gpsLatitude> ;
          rdfs:comment "The latitude, expressed as three values giving the degrees, minutes, and seconds, respectively."@en ,
                       "緯度"@ja ;
          rdfs:label "Latitude"@en ;
          <http://www.w3.org/2003/12/exif/ns#tagNumber> "2"@en ;
          <http://www.w3.org/2004/02/skos/core#example> "`41d 05' 54.03\" S`"@en .


###  https://www.morphosource.org/terms/morphosource#legacyMediaFileID
:legacyMediaFileID rdf:type owl:DatatypeProperty ;
                   rdfs:subPropertyOf <http://rs.tdwg.org/ac/terms/providerManagedID> ;
                   rdf:type owl:FunctionalProperty ;
                   rdfs:domain :Media ;
                   rdfs:range xsd:string ;
                   <http://purl.org/dc/terms/isVersionOf> <http://rs.tdwg.org/ac/terms/providerManagedID> ;
                   <http://rs.tdwg.org/dwc/terms/attributes/repeatable> "No" ;
                   <http://rs.tdwg.org/dwc/terms/attributes/required> "No" ;
                   rdfs:comment "MorphoSource-specific unique ID identifier that was used to represent a Media in the now-defunct 1.0 version of the MorphoSource repository. Only present if Media was originally contributed to MorphoSource 1.0. Different from morphosource:ID identifier."@en ;
                   rdfs:label "Legacy Media File ID"@en .


###  https://www.morphosource.org/terms/morphosource#legacyMediaGroupID
:legacyMediaGroupID rdf:type owl:DatatypeProperty ;
                    rdfs:subPropertyOf <http://rs.tdwg.org/ac/terms/IDofContainingCollection> ;
                    rdf:type owl:FunctionalProperty ;
                    rdfs:domain :Media ;
                    rdfs:range xsd:string ;
                    <http://purl.org/dc/terms/isVersionOf> <http://rs.tdwg.org/ac/terms/IDofContainingCollection> ;
                    <http://rs.tdwg.org/dwc/terms/attributes/repeatable> "No"@en ;
                    <http://rs.tdwg.org/dwc/terms/attributes/required> "No" ;
                    rdfs:comment "MorphoSource-specific unique ID identifier that was used to group Media together in the now-defunct 1.0 version of the MorphoSource repository. In MorphoSource 1.0, Media groups were used to collect all media derived from the same Imaging Event. Media groups are no longer used, with media-to-media imaging and processing event relationships now being used instead to track hierarchical relationships between Media. Only present if Media was originally contributed to MorphoSource 1.0. Different from morphosource:ID identifier."@en ;
                    rdfs:label "Legacy Media Group ID"@en .


###  https://www.morphosource.org/terms/morphosource#lensMake
:lensMake rdf:type owl:DatatypeProperty ;
          rdfs:subPropertyOf :exifLensMake ;
          rdfs:domain :PhotogrammetryImagingEvent ,
                      :PhotographyImagingEvent ;
          rdfs:range xsd:string ;
          rdfs:comment "The manufacturer of the camera lens. This should probably map directly to an EXIF term and should be updated accordingly."@en ;
          rdfs:label "Lens Make"@en .


###  https://www.morphosource.org/terms/morphosource#lensModel
:lensModel rdf:type owl:DatatypeProperty ;
           rdfs:subPropertyOf :exifLensModel ;
           rdfs:domain :PhotogrammetryImagingEvent ,
                       :PhotographyImagingEvent ;
           rdfs:range xsd:string ;
           rdfs:comment "The model of the camera lens. This should probably map directly to an EXIF term and should be updated accordingly."@en ;
           rdfs:label "Lens Model"@en .


###  https://www.morphosource.org/terms/morphosource#licenseBlank
:licenseBlank rdf:type owl:DatatypeProperty ;
              rdfs:domain :Organization ;
              rdfs:range xsd:string ;
              rdfs:comment "Whether the Organization's preferred policy is for Media representing Organization Physical Objects to specify no license in dc:license. This is distinct from an Organization expressing no preference on license choice. Values must be \"Yes\" or \"No\". If value is \"Yes\", then Organization explicitly prefers no license to be chosen."@en ;
              rdfs:label "License Intentionally Left Blank"@en ;
              <http://www.w3.org/2004/02/skos/core#example> "`Yes`, `No`"@en .


###  https://www.morphosource.org/terms/morphosource#longitude
:longitude rdf:type owl:DatatypeProperty ;
           rdfs:subPropertyOf <http://www.w3.org/2003/12/exif/ns#gpsLongitude> ;
           rdfs:domain :PhysicalObject ;
           rdfs:range xsd:string ;
           <http://purl.org/dc/terms/isVersionOf> <http://www.w3.org/2003/12/exif/ns#gpsLongitude> ;
           rdfs:comment "The longitude, expressed as three values giving the degrees, minutes, and seconds, respectively."@en ,
                        "経度"@ja ;
           rdfs:label "Longitude"@en ;
           <http://www.w3.org/2003/12/exif/ns#tagNumber> "4"@en ;
           <http://www.w3.org/2004/02/skos/core#example> "`121d 10' 34\" W`"@en .


###  https://www.morphosource.org/terms/morphosource#material
:material rdf:type owl:DatatypeProperty ;
          rdfs:subPropertyOf <http://purl.org/dc/terms/medium> ;
          rdfs:domain :CulturalHeritageObject ;
          rdfs:range xsd:string ;
          <http://purl.org/dc/terms/isVersionOf> <http://purl.org/dc/terms/medium> ;
          rdfs:comment "Material(s) from which an object is made. It is preferred to use morphosource:aatMaterial when it is possible to express materials using the Getty Arts and Architecture Thesaurus controlled vocabulary. This property is for custom material values not listed in the Getty AAT controlled vocabulary."@en ;
          rdfs:label "Material"@en .


###  https://www.morphosource.org/terms/morphosource#mediaARK
:mediaARK rdf:type owl:DatatypeProperty ;
          rdfs:label "Media ARK"@en .


###  https://www.morphosource.org/terms/morphosource#mediaDOI
:mediaDOI rdf:type owl:DatatypeProperty ;
          rdfs:label "Media DOI"@en .


###  https://www.morphosource.org/terms/morphosource#mediaParentID
:mediaParentID rdf:type owl:DatatypeProperty ;
               rdfs:subPropertyOf :ID ;
               rdfs:domain :Media ;
               rdfs:range xsd:string ;
               rdfs:comment "MorphoSource-specific unique ID identifier for the parent Media of a Media. This is the ID of the Media from which the current Media is immediately derived."@en ;
               rdfs:label "Media Parent ID"@en .


###  https://www.morphosource.org/terms/morphosource#mimeType
:mimeType rdf:type owl:DatatypeProperty ;
          rdfs:subPropertyOf <http://purl.org/dc/terms/format> ;
          rdfs:domain :FileSet ;
          rdfs:range xsd:string ;
          <http://purl.org/dc/terms/isVersionOf> <http://purl.org/dc/terms/format> ;
          rdfs:comment "Media type describing the nature and format of a file."@en ;
          rdfs:label "Mime Type"@en ;
          <http://www.w3.org/2004/02/skos/core#example> "`image/jpeg`, `image/tiff`, `application/stl`"@en .


###  https://www.morphosource.org/terms/morphosource#normalsFormat
:normalsFormat rdf:type owl:DatatypeProperty ;
               rdfs:domain :FileSet ;
               rdfs:range xsd:string ;
               rdfs:comment "How vertex or face normal information is formatted and codified for a 3D object, if normal information is present with the object."@en ;
               rdfs:label "Normals Format"@en .


###  https://www.morphosource.org/terms/morphosource#numberOfImagesInSet
:numberOfImagesInSet rdf:type owl:DatatypeProperty ;
                     rdfs:subPropertyOf :dicomNumberOfSeriesRelatedInstances ;
                     rdfs:domain :Media ;
                     rdfs:range xsd:int ;
                     rdfs:comment "For Media with a ZIP archive with many component files, this is the number of files in the primary image collection in a CT image stack or photogrammetry image collection. This only applies to CTImageSeries or PhotogrammetryImageSeries Media."@en ;
                     rdfs:label "Number of Images In Set"@en .


###  https://www.morphosource.org/terms/morphosource#numericTime
:numericTime rdf:type owl:DatatypeProperty ;
             rdfs:subPropertyOf <http://rs.tdwg.org/dwc/terms/earliestEonOrLowestEonothem> ;
             rdfs:domain :PhysicalObject ;
             rdfs:range xsd:string ;
             <http://purl.org/dc/terms/isVersionOf> <http://rs.tdwg.org/dwc/terms/earliestEonOrLowestEonothem> ;
             <http://rs.tdwg.org/dwc/terms/attributes/abcdEquivalence> "not in ABCD" ;
             <http://rs.tdwg.org/dwc/terms/attributes/usageScope> "simple" ;
             rdfs:comment "Free text numeric description of the absolute or specific chronological age of the physical object."@en ;
             rdfs:label "Numeric Time"@en ;
             <http://www.w3.org/2004/02/skos/core#example> "`20 MYA`,`4th Century`,`1142 C.E.`"@en .


###  https://www.morphosource.org/terms/morphosource#objectID
:objectID rdf:type owl:DatatypeProperty ;
          rdfs:subPropertyOf :ID ;
          rdfs:range xsd:string ;
          rdfs:comment "MorphoSource-specific unique ID identifier for a Physical Object."@en ;
          rdfs:label "Physical Object ID"@en .


###  https://www.morphosource.org/terms/morphosource#opticalMagnification
:opticalMagnification rdf:type owl:DatatypeProperty ;
                      rdfs:domain :CTImageSeriesImagingEvent ;
                      rdfs:range xsd:string ;
                      rdfs:comment "Whether optical magnification is used or not. This property is only for indicating optical magnification specifically, and is different from geometric magnification. If present, value must be \"Yes\" or \"No\"."@en ;
                      rdfs:label "Optical Magnification"@en ;
                      <http://www.w3.org/2004/02/skos/core#example> "`Yes`, `No`"@en .


###  https://www.morphosource.org/terms/morphosource#organizationID
:organizationID rdf:type owl:DatatypeProperty ;
                rdfs:subPropertyOf :ID ;
                rdfs:domain :PhysicalObject ;
                rdfs:range xsd:string ;
                rdfs:comment "MorphoSource-specific unique ID identifier for the provider Organization (museum, institution, or laboratory) responsible for managing the physical object."@en ;
                rdfs:label "Organization ID"@en .


###  https://www.morphosource.org/terms/morphosource#orientation
:orientation rdf:type owl:DatatypeProperty ;
             rdfs:subPropertyOf <http://rs.tdwg.org/ac/terms/subjectOrientation> ;
             rdfs:domain :Media ;
             rdfs:range xsd:string ;
             <http://purl.org/dc/terms/isVersionOf> <http://rs.tdwg.org/ac/terms/subjectOrientation> ;
             <http://rs.tdwg.org/dwc/terms/attributes/repeatable> "No" ;
             <http://rs.tdwg.org/dwc/terms/attributes/required> "No" ;
             rdfs:comment "Specific orientation (= direction, view angle) of the subject represented in the media resource with respect to the acquisition device, denoted by an IRI."@en ;
             rdfs:label "Orientation"@en .


###  https://www.morphosource.org/terms/morphosource#originalLocation
:originalLocation rdf:type owl:DatatypeProperty ;
                  rdfs:domain :PhysicalObject ;
                  rdfs:range xsd:string ;
                  rdfs:comment "Free text description of the original location where the physical object was created, produced, fossilized, or otherwise came into being."@en ;
                  rdfs:label "Original Location"@en .


###  https://www.morphosource.org/terms/morphosource#part
:part rdf:type owl:DatatypeProperty ;
      rdfs:subPropertyOf <http://rs.tdwg.org/ac/terms/subjectPart> ;
      rdfs:domain :Media ;
      rdfs:range xsd:string ;
      <http://purl.org/dc/terms/isVersionOf> <http://rs.tdwg.org/ac/terms/subjectPart> ;
      <http://rs.tdwg.org/dwc/terms/attributes/repeatable> "Yes"@en ;
      <http://rs.tdwg.org/dwc/terms/attributes/required> "No" ;
      rdfs:comment "The portion or product of organism morphology, behaviour, environment, etc. that is either predominantly shown or particularly well exemplified by the media resource, denoted by an IRI."@en ;
      rdfs:label "Part"@en .


###  https://www.morphosource.org/terms/morphosource#periodicTime
:periodicTime rdf:type owl:DatatypeProperty ;
              rdfs:domain :PhysicalObject ;
              rdfs:range xsd:string ;
              rdfs:comment "Free text description of the time period associated with the production or creation of the physical object."@en ;
              rdfs:label "Periodic Time"@en .


###  https://www.morphosource.org/terms/morphosource#phaseContrast
:phaseContrast rdf:type owl:DatatypeProperty ;
               rdfs:domain :CTImageSeriesImagingEvent ;
               rdfs:range xsd:string ;
               rdfs:comment "Whether phase contrast of X-Ray beam - in other words, modulating the beam between higher and lower energies to increase contrast between materials - is used or not. If present, value must be \"Yes\" or \"No\"."@en ;
               rdfs:label "Phase Contrast"@en ;
               <http://www.w3.org/2004/02/skos/core#example> "`Yes`, `No`"@en .


###  https://www.morphosource.org/terms/morphosource#photogrammetryBackgroundRemoval
:photogrammetryBackgroundRemoval rdf:type owl:DatatypeProperty ;
                                 rdfs:domain :PhotogrammetryImagingEvent ;
                                 rdfs:range xsd:string ;
                                 rdfs:comment "Free text description of background removal method."@en ;
                                 rdfs:label "Photogrammetry Background Removal"@en .


###  https://www.morphosource.org/terms/morphosource#photographicReference
:photographicReference rdf:type owl:DatatypeProperty ;
                       rdfs:subPropertyOf :attachmentFile ;
                       rdfs:domain :ImagingEvent ;
                       rdfs:range xsd:anyURI ;
                       rdfs:comment "A reference photograph image, often used to represent and record the object at the initial time of scanning."@en ;
                       rdfs:label "Photographic Reference"@en .


###  https://www.morphosource.org/terms/morphosource#physicalObjectID
:physicalObjectID rdf:type owl:DatatypeProperty ;
                  rdfs:subPropertyOf :objectID ;
                  rdfs:domain :ImagingEvent ,
                              :Media ;
                  <http://purl.org/dc/terms/isVersionOf> :objectID ;
                  rdfs:comment "MorphoSource-specific unique ID identifier for a Physical Object represented by a Media."@en ;
                  rdfs:label "Physical Object ID"@en .


###  https://www.morphosource.org/terms/morphosource#pointCount
:pointCount rdf:type owl:DatatypeProperty ;
            rdfs:domain :FileSet ;
            rdfs:range xsd:int ;
            rdfs:comment "Number of 3D coordinate points comprising a 3D mesh or point cloud."@en ;
            rdfs:label "Point Count"@en .


###  https://www.morphosource.org/terms/morphosource#postalCode
:postalCode rdf:type owl:DatatypeProperty ;
            rdfs:domain :Organization ;
            rdfs:range xsd:string ;
            rdfs:comment "Group of numbers or letters added to a postal address to assist in sorting of mail, such as a ZIP code in the United States."@en ;
            rdfs:label "Postal Code"@en ;
            <http://www.w3.org/2004/02/skos/core#example> "`27708`"@en .


###  https://www.morphosource.org/terms/morphosource#power
:power rdf:type owl:DatatypeProperty ;
       rdfs:subPropertyOf <http://purl.org/healthcarevocab/v1#GeneratorPower> ;
       rdfs:domain :CTImageSeriesImagingEvent ;
       rdfs:range xsd:float ;
       <http://purl.org/dc/terms/isVersionOf> <http://purl.org/healthcarevocab/v1#GeneratorPower> ;
       rdfs:comment "Power in kW to the X-Ray generator."@en ;
       rdfs:label "Power"@en .


###  https://www.morphosource.org/terms/morphosource#processingActivityDescription
:processingActivityDescription rdf:type owl:DatatypeProperty ;
                               rdfs:subPropertyOf <http://purl.org/dc/elements/1.1/description> ;
                               rdfs:domain :ProcessingEvent ;
                               rdfs:range xsd:string ;
                               rdfs:comment "Description of a specific discrete processing activity step."@en ;
                               rdfs:label "Processing Activity Description"@en .


###  https://www.morphosource.org/terms/morphosource#processingActivitySoftware
:processingActivitySoftware rdf:type owl:DatatypeProperty ;
                            rdfs:subPropertyOf <http://purl.org/dc/dcmitype/Software> ;
                            rdfs:domain :ProcessingEvent ;
                            rdfs:range xsd:string ;
                            rdfs:comment "Description of software used in a specific discrete processing activity step."@en ;
                            rdfs:label "Processing Activity Software"@en .


###  https://www.morphosource.org/terms/morphosource#projections
:projections rdf:type owl:DatatypeProperty ;
             rdfs:subPropertyOf <http://purl.org/healthcarevocab/v1#ImagesInAcquisition> ;
             rdfs:domain :CTImageSeriesImagingEvent ;
             rdfs:range xsd:int ;
             <http://purl.org/dc/terms/isVersionOf> <http://purl.org/healthcarevocab/v1#ImagesInAcquisition> ;
             rdfs:comment "Number of images at distinct angles used to create a 3D image."@en ;
             rdfs:label "Number of Projections"@en .


###  https://www.morphosource.org/terms/morphosource#provenanceDate
:provenanceDate rdf:type owl:DatatypeProperty ;
                rdfs:domain :PhysicalObject ;
                rdfs:range xsd:date ;
                rdfs:comment "Date the physical object was collected, excavated, or discovered. Values must be in MM/DD/YYYY date format."@en ;
                rdfs:label "Provenance Date"@en ;
                <http://www.w3.org/2004/02/skos/core#example> "`01/01/1985`, `12/30/2021`"@en .


###  https://www.morphosource.org/terms/morphosource#provenanceDetails
:provenanceDetails rdf:type owl:DatatypeProperty ;
                   rdfs:subPropertyOf <http://purl.org/dc/terms/provenance> ;
                   rdfs:domain :PhysicalObject ;
                   rdfs:range xsd:string ;
                   <http://purl.org/dc/terms/description> "The statement may include a description of any changes successive custodians made to the resource."@en ;
                   <http://purl.org/dc/terms/isVersionOf> <http://purl.org/dc/terms/provenance> ;
                   rdfs:comment "A statement detailing production, discovery, and/or ownership, describing the initial production/discovery context and listing any changes in ownership and custody of the resource since its creation that are significant for its authenticity, integrity, and interpretation."@en ;
                   rdfs:label "Provenance Details"@en .


###  https://www.morphosource.org/terms/morphosource#provenanceLocation
:provenanceLocation rdf:type owl:DatatypeProperty ;
                    rdfs:domain :PhysicalObject ;
                    rdfs:range xsd:string ;
                    rdfs:comment "Free text description of the location from which the physical object was collected, excavated, or discovered."@en ;
                    rdfs:label "Provenance Location"@en .


###  https://www.morphosource.org/terms/morphosource#provenanceName
:provenanceName rdf:type owl:DatatypeProperty ;
                rdfs:domain :PhysicalObject ;
                rdfs:range xsd:string ;
                rdfs:comment "Name of the collection or excavation event, if applicable and available."@en ;
                rdfs:label "Provenance Name"@en .


###  https://www.morphosource.org/terms/morphosource#recordsetID
:recordsetID rdf:type owl:DatatypeProperty ;
             rdfs:domain :Organization ;
             rdfs:range xsd:string ;
             rdfs:comment "An identifier for an entire museum, institution, or laboratory specimen collection associated with Organization. May be a global unique identifier or an identifier specific to a collection or institution."@en ;
             rdfs:label "Recordset ID"@en .


###  https://www.morphosource.org/terms/morphosource#relatedURL
:relatedURL rdf:type owl:DatatypeProperty ;
            rdfs:subPropertyOf rdfs:seeAlso ;
            rdfs:domain :Media ,
                        :Organization ,
                        :PhysicalObject ;
            rdfs:range xsd:anyURI ;
            <http://purl.org/dc/terms/isVersionOf> rdfs:seeAlso ;
            rdfs:comment "URL for additional resource that might provide additional information about the Media or Physical Object."@en ;
            rdfs:label "Related URL"@en .


###  https://www.morphosource.org/terms/morphosource#rightsHolder
:rightsHolder rdf:type owl:DatatypeProperty ;
              rdfs:subPropertyOf <http://ns.adobe.com/xap/1.0/rights/Owner> ;
              rdfs:domain :Media ,
                          :Organization ;
              rdfs:range xsd:string ;
              <http://purl.org/dc/terms/isVersionOf> <http://ns.adobe.com/xap/1.0/rights/Owner> ;
              rdfs:comment "List of holders of intellectual property rights (copyright or license-based) for the Media."@en ;
              rdfs:label "Rights Holder"@en .


###  https://www.morphosource.org/terms/morphosource#rightsHolderBlank
:rightsHolderBlank rdf:type owl:DatatypeProperty ;
                   rdfs:domain :Organization ;
                   rdfs:range xsd:string ;
                   rdfs:comment "Whether the Organization's preferred policy is for Media representing Organization Physical Objects to specify no rights holder in morphosource:rightsHolder. This is distinct from an Organization expressing no preference on rights holder statement. Values must be \"Yes\" or \"No\". If value is \"Yes\", then Organization explicitly prefers no rights holder statement."@en ;
                   rdfs:label "Rights Holder Intentionally Left Blank"@en ;
                   <http://www.w3.org/2004/02/skos/core#example> "`Yes`, `No`"@en .


###  https://www.morphosource.org/terms/morphosource#rightsStatementBlank
:rightsStatementBlank rdf:type owl:DatatypeProperty ;
                      rdfs:domain :Organization ;
                      rdfs:range xsd:string ;
                      rdfs:comment "Whether the Organization's preferred policy is for Media representing Organization Physical Objects to specify no rights statement in morphosource:rightsStatement. This is distinct from an Organization expressing no preference on rights statement. Values must be \"Yes\" or \"No\". If value is \"Yes\", then Organization explicitly prefers no rights statement."@en ;
                      rdfs:label "Rights Statement Intentionally Left Blank"@en ;
                      <http://www.w3.org/2004/02/skos/core#example> "`Yes`, `No`"@en .


###  https://www.morphosource.org/terms/morphosource#rotationNumber
:rotationNumber rdf:type owl:DatatypeProperty ;
                rdfs:subPropertyOf <http://purl.org/healthcarevocab/v1#SpiralPitchFactor> ;
                rdfs:domain :CTImageSeriesImagingEvent ;
                rdfs:range xsd:float ;
                <http://purl.org/dc/terms/isVersionOf> <http://purl.org/healthcarevocab/v1#SpiralPitchFactor> ;
                rdfs:comment "Ratio of the Table Feed per Rotation (DICOM 0018,9310) to the Total Collimation Width (DICOM 0018,9307)."@en ;
                rdfs:label "Number of Rotations"@en .


###  https://www.morphosource.org/terms/morphosource#scaleBar
:scaleBar rdf:type owl:DatatypeProperty ;
          rdfs:domain :Media ;
          rdfs:range xsd:string ;
          rdfs:comment "Details of scale bar accompany a photogrammetry image series. Value should include three elements: the scale bar target type, the scale bar distance, and the units of the scale bar distance. If values are encoded as a string, they should be separate by semicolons. This only applies to PhotogrammetryImageSeries Media."@en ;
          rdfs:label "Scale Bar"@en .


###  https://www.morphosource.org/terms/morphosource#shadingCorrection
:shadingCorrection rdf:type owl:DatatypeProperty ;
                   rdfs:domain :CTImageSeriesImagingEvent ;
                   rdfs:range xsd:string ;
                   rdfs:comment "Whether shading correction calibration is used or not. If present, value must be \"Yes\" or \"No\"."@en ;
                   rdfs:label "Shading Correction"@en ;
                   <http://www.w3.org/2004/02/skos/core#example> "`Yes`, `No`"@en .


###  https://www.morphosource.org/terms/morphosource#shortDescription
:shortDescription rdf:type owl:DatatypeProperty ;
                  rdfs:domain :Media ;
                  rdfs:range xsd:string ;
                  rdfs:comment "Brief summary description of Media. This could include a brief summary of what is represented in the Media or the context surrounding the Media."@en ;
                  rdfs:label "Short Description"@en .


###  https://www.morphosource.org/terms/morphosource#shortTitle
:shortTitle rdf:type owl:DatatypeProperty ;
            rdfs:domain :CulturalHeritageObject ;
            rdfs:range xsd:string ;
            rdfs:comment "Title or short description of an object. For MorphoSource records, value is used as part of the full title for a Cultural Heritage Object record."@en ;
            rdfs:label "Short Title"@en .


###  https://www.morphosource.org/terms/morphosource#shutterSpeed
:shutterSpeed rdf:type owl:DatatypeProperty ;
              rdfs:subPropertyOf <http://www.w3.org/2003/12/exif/ns#shutterSpeedValue> ;
              rdfs:domain :FileSet ,
                          :PhotogrammetryImagingEvent ,
                          :PhotographyImagingEvent ;
              rdfs:range xsd:string ;
              rdfs:comment "Shutter speed. The unit is the APEX (Additive System of Photographic Exposure) setting"@en ,
                           "シャッター速度（APEX値）。この値の2のベキ乗をとって逆数にすると、通常のシャッター速度表示になる。例えば'4'の場合だと1/(2^4)=1/16秒"@ja ;
              rdfs:label "Shutter Speed"@en ;
              <http://www.w3.org/2003/12/exif/ns#tagNumber> "37377"@en .


###  https://www.morphosource.org/terms/morphosource#software
:software rdf:type owl:DatatypeProperty ;
          rdfs:domain :ImagingEvent ;
          rdfs:range xsd:string ;
          rdfs:comment "Free text description of any software used in an Imaging Event."@en ;
          rdfs:label "Software"@en .


###  https://www.morphosource.org/terms/morphosource#sourceDetectorDistance
:sourceDetectorDistance rdf:type owl:DatatypeProperty ;
                        rdfs:subPropertyOf <http://purl.org/healthcarevocab/v1#DistanceSourceToDetector> ;
                        rdfs:domain :CTImageSeriesImagingEvent ;
                        rdfs:range xsd:float ;
                        <http://purl.org/dc/terms/isVersionOf> <http://purl.org/healthcarevocab/v1#DistanceSourceToDetector> ;
                        rdfs:comment "Distance in mm from X-Ray source to detector center."@en ;
                        rdfs:label "Distance From Source To Detector"@en .


###  https://www.morphosource.org/terms/morphosource#sourceObjectDistance
:sourceObjectDistance rdf:type owl:DatatypeProperty ;
                      rdfs:subPropertyOf <http://purl.org/healthcarevocab/v1#DistanceSourceToPatient> ;
                      rdfs:domain :CTImageSeriesImagingEvent ;
                      rdfs:range xsd:float ;
                      <http://purl.org/dc/terms/isVersionOf> <http://purl.org/healthcarevocab/v1#DistanceSourceToPatient> ;
                      rdfs:comment "Distance in mm from X-Ray source to isocenter (center of field of view)."@en ;
                      rdfs:label "Distance From Source To Object"@en .


###  https://www.morphosource.org/terms/morphosource#surroundingMaterial
:surroundingMaterial rdf:type owl:DatatypeProperty ;
                     rdfs:subPropertyOf <http://purl.org/healthcarevocab/v1#ContainerDescription> ;
                     rdfs:domain :CTImageSeriesImagingEvent ;
                     rdfs:range xsd:string ;
                     <http://purl.org/dc/terms/isVersionOf> <http://purl.org/healthcarevocab/v1#ContainerDescription> ;
                     rdfs:comment "Wedge, or the material surrounding and/or enveloping the focal object."@en ;
                     rdfs:label "Surrounding Material"@en .


###  https://www.morphosource.org/terms/morphosource#tag
:tag rdf:type owl:DatatypeProperty ;
     rdfs:domain :Media ;
     rdfs:range xsd:string ;
     rdfs:comment "All-purpose label attached to Media for the purpose of identification, context, or to give other information."@en ;
     rdfs:label "Tag"@en .


###  https://www.morphosource.org/terms/morphosource#targetMaterial
:targetMaterial rdf:type owl:DatatypeProperty ;
                rdfs:subPropertyOf <http://purl.org/healthcarevocab/v1#AnodeTargetMaterial> ;
                rdfs:domain :CTImageSeriesImagingEvent ;
                rdfs:range xsd:string ;
                <http://purl.org/dc/terms/isVersionOf> <http://purl.org/healthcarevocab/v1#AnodeTargetMaterial> ;
                rdfs:comment "The primary material in the anode of the X-Ray source."@en ;
                rdfs:label "Target Material"@en ;
                <http://www.w3.org/2004/02/skos/core#example> "`tungsten`, `molybdenum`, `copper`"@en .


###  https://www.morphosource.org/terms/morphosource#taxonomyID
:taxonomyID rdf:type owl:DatatypeProperty ;
            rdfs:subPropertyOf :ID ;
            rdfs:domain :BiologicalSpecimenObject ;
            rdfs:range xsd:string ;
            rdfs:comment "Morphosource-specific ID of Taxonomy record for taxonomic name attributed to the Biological Specimen."@en ;
            rdfs:label "Taxonomy ID"@en .


###  https://www.morphosource.org/terms/morphosource#teamID
:teamID rdf:type owl:DatatypeProperty ;
        rdfs:subPropertyOf :ID ;
        rdfs:domain :Organization ;
        rdfs:range xsd:string ;
        rdfs:comment "MorphoSource-specific unique ID identifier for a Team associated with the Organization and responsible for managing the Organization record."@en ;
        rdfs:label "Team ID"@en .


###  https://www.morphosource.org/terms/morphosource#vertexColor
:vertexColor rdf:type owl:DatatypeProperty ;
             rdfs:domain :FileSet ;
             rdfs:range xsd:string ;
             rdfs:comment "Whether or not a 3D object has color information encoded into vertices or points that comprise a mesh or point cloud."@en ;
             rdfs:label "Vertex Color"@en .


###  https://www.morphosource.org/terms/morphosource#voltage
:voltage rdf:type owl:DatatypeProperty ;
         rdfs:subPropertyOf <http://purl.org/healthcarevocab/v1#KVP> ;
         rdfs:domain :CTImageSeriesImagingEvent ;
         rdfs:range xsd:float ;
         <http://purl.org/dc/terms/isVersionOf> <http://purl.org/healthcarevocab/v1#KVP> ;
         rdfs:comment "Peak kilo voltage output of the X-Ray generator used."@en ;
         rdfs:label "Voltage"@en .


###  https://www.morphosource.org/terms/morphosource#vouchered
:vouchered rdf:type owl:DatatypeProperty ;
           rdfs:subPropertyOf <http://rs.tdwg.org/dwc/terms/disposition> ;
           rdfs:domain :PhysicalObject ;
           rdfs:range xsd:string ;
           <http://purl.org/dc/terms/isVersionOf> <http://rs.tdwg.org/dwc/terms/disposition> ;
           <http://rs.tdwg.org/dwc/terms/attributes/abcdEquivalence> "DataSets/DataSet/Units/Unit/SpecimenUnit/Disposition" ;
           <http://rs.tdwg.org/dwc/terms/attributes/usageScope> "simple" ;
           rdfs:comment "Whether the specimen is vouchered or not, or in other words, whether the physical specimen object exists and is preserved and maintained in an accessible collection. Value must be \"Yes\" or \"No\"."@en ;
           rdfs:label "Vouchered"@en ;
           <http://www.w3.org/2004/02/skos/core#example> "`Yes`, `No`"@en .


###  https://www.morphosource.org/terms/morphosource#width
:width rdf:type owl:DatatypeProperty ;
       rdfs:domain :FileSet ;
       rdfs:range xsd:int ;
       rdfs:comment "Width of a 2D image in pixels."@en ;
       rdfs:label "Width in Pixels"@en .


###  https://www.morphosource.org/terms/morphosource#xSpacing
:xSpacing rdf:type owl:DatatypeProperty ;
          rdfs:subPropertyOf :dicomPixelSpacingWidth ;
          rdfs:domain :Media ;
          rdfs:range xsd:float ;
          rdfs:comment "Distance between centers of adjacent pixels in the X axis, for Media with pixel data where pixel spacing corresponds to real-world length measurement. Unit of measurement is described by morphosource:unit. Applies to Image and CTImageSeries media."@en ;
          rdfs:label "X Pixel Spacing"@en .


###  https://www.morphosource.org/terms/morphosource#xrayTubeType
:xrayTubeType rdf:type owl:DatatypeProperty ;
              rdfs:subPropertyOf <http://purl.org/healthcarevocab/v1#GeneratorID> ;
              rdfs:domain :CTImageSeriesImagingEvent ;
              rdfs:range xsd:string ;
              <http://purl.org/dc/terms/isVersionOf> <http://purl.org/healthcarevocab/v1#GeneratorID> ;
              rdfs:comment "Free text describing type of X-Ray tube, possibly including brand and/or model of tube."@en ;
              rdfs:label "X-Ray Tube Type"@en .


###  https://www.morphosource.org/terms/morphosource#ySpacing
:ySpacing rdf:type owl:DatatypeProperty ;
          rdfs:subPropertyOf :dicomPixelSpacingHeight ;
          rdfs:domain :Media ;
          rdfs:range xsd:float ;
          rdfs:comment "Distance between centers of adjacent pixels in the Y axis, for Media with pixel data where pixel spacing corresponds to real-world length measurement. Unit of measurement is described by morphosource:unit. Applies to Image and CTImageSeries media."@en ;
          rdfs:label "Y Pixel Spacing"@en .


###  https://www.morphosource.org/terms/morphosource#zSpacing
:zSpacing rdf:type owl:DatatypeProperty ;
          rdfs:subPropertyOf :dicomSpacingBetweenSlices ;
          rdfs:domain :Media ;
          rdfs:range xsd:float ;
          rdfs:comment "Distance between centers of adjacent pixels in the Z axis, for Media with 3D pixel data where pixel spacing corresponds to real-world length measurement. Unit of measurement is described by morphosource:unit. Applies to CTImageSeries media."@en ;
          rdfs:label "Z Pixel Spacing"@en .


#################################################################
#    Classes
#################################################################

###  http://creativecommons.org/ns#License
<http://creativecommons.org/ns#License> rdf:type owl:Class ;
                                        rdfs:subClassOf <http://purl.org/dc/terms/LicenseDocument> ;
                                        rdfs:comment """a set of
		    requests/permissions to users of a Work, e.g. a
		    copyright license, the public domain, information
		    for distributors"""@en-us ;
                                        rdfs:label "License"@en-us .


###  http://pcdm.org/models#File
<http://pcdm.org/models#File> rdf:type owl:Class ;
                              <http://purl.org/dc/terms/isPartOf> "http://pcdm.org/models#"@en ;
                              rdfs:comment "A File is a sequence of binary data and is described by some accompanying metadata. The metadata typically includes at least basic technical metadata (size, content type, modification date, etc.), but can also include properties related to preservation, digitization process, provenance, etc. Files MUST be contained by exactly one Object."@en ;
                              rdfs:isDefinedBy "http://pcdm.org/models#"@en ;
                              rdfs:label "File"@en .


###  http://pcdm.org/models#Object
<http://pcdm.org/models#Object> rdf:type owl:Class ;
                                <http://purl.org/dc/terms/isPartOf> "http://pcdm.org/models"@en ;
                                rdfs:comment "An Object is an intellectual entity, sometimes called a \"work\", \"digital object\", etc. Objects have descriptive metadata, access metadata, may contain files and other Objects as member \"components\". Each level of a work is therefore represented by an Object instance, and is capable of standing on its own, being linked to from Collections and other Objects. Member Objects can be ordered using the ORE Proxy class."@en ;
                                rdfs:isDefinedBy "http://pcdm.org/models"@en ;
                                rdfs:label "Object"@en .


###  http://pcdm.org/works#Work
<http://pcdm.org/works#Work> rdf:type owl:Class ;
                             rdfs:subClassOf <http://pcdm.org/models#Object> ;
                             <http://purl.org/dc/terms/isPartOf> "http://pcdm.org/works"@en ;
                             rdfs:comment """
      A work or intellectual entity, such as a book, film, dissertation, etc.
      Works have member Objects representing their physical structure (e.g., pages in a book),
      FileSets to maintain representations of the entire resource (e.g. a PDF of all the pages),
      and TopRanges representing their logical structure or structures (e.g., sections
      and chapters in a book).
    """@en ;
                             rdfs:isDefinedBy <http://pcdm.org/works> ;
                             rdfs:label "Work"@en .


###  http://purl.org/dc/terms/LicenseDocument
<http://purl.org/dc/terms/LicenseDocument> rdf:type owl:Class ;
                                           rdfs:subClassOf <http://purl.org/dc/terms/RightsStatement> .


###  http://purl.org/dc/terms/RightsStatement
<http://purl.org/dc/terms/RightsStatement> rdf:type owl:Class ;
                                           <http://purl.org/dc/terms/issued> "2008-01-14"^^xsd:date ;
                                           rdfs:comment "A statement about the intellectual property rights (IPR) held in or over a resource, a legal document giving official permission to do something with a resource, or a statement about access rights."@en ;
                                           rdfs:isDefinedBy <http://purl.org/dc/terms/> ;
                                           rdfs:label "Rights Statement"@en .


###  http://vocab.getty.edu/aat/300264087
<http://vocab.getty.edu/aat/300264087> rdf:type owl:Class .


###  http://vocab.getty.edu/aat/300264088
<http://vocab.getty.edu/aat/300264088> rdf:type owl:Class .


###  http://vocab.getty.edu/aat/300264091
<http://vocab.getty.edu/aat/300264091> rdf:type owl:Class .


###  http://vocab.getty.edu/aat/300264092
<http://vocab.getty.edu/aat/300264092> rdf:type owl:Class .


###  http://vocab.getty.edu/tgn/7029392
<http://vocab.getty.edu/tgn/7029392> rdf:type owl:Class .


###  https://www.morphosource.org/terms/morphosource#AcquisitionType
:AcquisitionType rdf:type owl:Class ;
                 rdfs:comment "CT acqusition method type. Entities comprise a controlled vocabulary as defined by DICOM C.8.15.3.2.1 Acquisition Type."@en ;
                 rdfs:label "Acquisition Type"@en .


###  https://www.morphosource.org/terms/morphosource#BiologicalSpecimenObject
:BiologicalSpecimenObject rdf:type owl:Class ;
                          rdfs:subClassOf :PhysicalObject ;
                          rdfs:comment "A physical object that is a biological specimen, such as a skeleton, a whole body, or a fossil."@en ;
                          rdfs:label "Biological Specimen Object"@en .


###  https://www.morphosource.org/terms/morphosource#CTImageSeriesImagingEvent
:CTImageSeriesImagingEvent rdf:type owl:Class ;
                           rdfs:subClassOf :ImagingEvent ;
                           rdfs:label "CT Image Series Imaging Event"@en .


###  https://www.morphosource.org/terms/morphosource#CTImageSeriesType
:CTImageSeriesType rdf:type owl:Class ;
                   rdfs:comment "Broad type or kind of CT image series, distinguishing between initial X-Ray projections and other derived series forms."@en ;
                   rdfs:label "CT Image Series Type"@en .


###  https://www.morphosource.org/terms/morphosource#CommercialUsePermission
:CommercialUsePermission rdf:type owl:Class ;
                         rdfs:comment "Permission statement describing whether a digital resource may be used for commercial purposes."@en ;
                         rdfs:label "Commercial Use Permission"@en .


###  https://www.morphosource.org/terms/morphosource#CulturalHeritageObject
:CulturalHeritageObject rdf:type owl:Class ;
                        rdfs:subClassOf :PhysicalObject ;
                        rdfs:comment "A physical object that is usually non-biological and is of some human cultural significance."@en ;
                        rdfs:label "Cultural Heritage Object"@en .


###  https://www.morphosource.org/terms/morphosource#DerivativeRearchivalStatement
:DerivativeRearchivalStatement rdf:type owl:Class ;
                               rdfs:comment "Statement describing whether and how any future derivatives must or should be rearchived to a public facing digital repository."@en ;
                               rdfs:label "Derivative Rearchival Statement"@en .


###  https://www.morphosource.org/terms/morphosource#Device
:Device rdf:type owl:Class ;
        rdfs:subClassOf <http://pcdm.org/works#Work> ;
        rdfs:comment "A device used to image a physical object to create media."@en ;
        rdfs:label "Device"@en .


###  https://www.morphosource.org/terms/morphosource#FileSet
:FileSet rdf:type owl:Class ;
         rdfs:subClassOf <http://pcdm.org/works#Work> ;
         rdfs:comment "A sequence of binary data accompanied by technical metadata."@en ;
         rdfs:label "FileSet"@en .


###  https://www.morphosource.org/terms/morphosource#FocalLengthType
:FocalLengthType rdf:type owl:Class ;
                 rdfs:comment "Type of camera focal length setting. Elements comprise a controlled vocabulary."@en ;
                 rdfs:label "Focal Length Type"@en .


###  https://www.morphosource.org/terms/morphosource#ImageModalityType
:ImageModalityType rdf:type owl:Class ;
                   rdfs:comment "Modality used to create 3D, 2D, or AV images. The individual entities of this class in the MorphoSource data vocabulary comprise a controlled vocabulary of specific image modalities used to describe imaging of media in MorphoSource."@en ;
                   rdfs:label "Image Modality Type"@en .


###  https://www.morphosource.org/terms/morphosource#ImagingEvent
:ImagingEvent rdf:type owl:Class ;
              rdfs:subClassOf <http://pcdm.org/works#Work> ;
              rdfs:comment "An active event in which a physical object is imaging to produce media."@en ;
              rdfs:label "Imaging Event"@en .


###  https://www.morphosource.org/terms/morphosource#LengthMeasurementUnit
:LengthMeasurementUnit rdf:type owl:Class ;
                       rdfs:comment "Unit of measurement used in measuring length."@en ;
                       rdfs:label "Length Measurement Unit"@en .


###  https://www.morphosource.org/terms/morphosource#LightSourceType
:LightSourceType rdf:type owl:Class ;
                 rdfs:comment "Type of light source. Elements comprise a controlled vocabulary."@en ;
                 rdfs:label "Light Source Type"@en .


###  https://www.morphosource.org/terms/morphosource#Media
:Media rdf:type owl:Class ;
       rdfs:subClassOf <http://pcdm.org/works#Work> ;
       rdfs:comment "3D, 2D, or AV media representing a physical object."@en ;
       rdfs:label "Media"@en .


###  https://www.morphosource.org/terms/morphosource#MediaType
:MediaType rdf:type owl:Class ;
           rdfs:comment "Type, nature, or classification of a Media file dataset, which may include one or more specific files. This is the general or high-level type of all file data, it is not the file type of any specific file. Most Media Types encompass a variety of different specific file types."@en ;
           rdfs:label "Media Type"@en .


###  https://www.morphosource.org/terms/morphosource#MeshMapType
:MeshMapType rdf:type owl:Class ;
             rdfs:comment "A type of 3D texture map or projection that associates two-dimensional space coordinates to the surface of a 3D object, usually in order to map a texture or other attribute onto the 3D object's surface."@en ;
             rdfs:label "Mesh Map Type"@en .


###  https://www.morphosource.org/terms/morphosource#Organization
:Organization rdf:type owl:Class ;
              rdfs:subClassOf <http://pcdm.org/works#Work> ;
              rdfs:comment "A relatively autonomous bureaucratic unit responsible for controlling physical objects or devices. Often a museum collection, an entire museum institution, or a faculty lab department."@en ;
              rdfs:label "Organization"@en .


###  https://www.morphosource.org/terms/morphosource#OrganizationType
:OrganizationType rdf:type owl:Class ;
                  rdfs:comment "Type of Organization, distinguishing between collections managing Physical Objects, scanning facilities, and entities that both operate scanning equipment and manage Physical Objects."@en ;
                  rdfs:label "Organization Type"@en .


###  https://www.morphosource.org/terms/morphosource#PhotogrammetryImagingEvent
:PhotogrammetryImagingEvent rdf:type owl:Class ;
                            rdfs:subClassOf :ImagingEvent ;
                            rdfs:label "Photogrammetry Imaging Event"@en .


###  https://www.morphosource.org/terms/morphosource#PhotographyImagingEvent
:PhotographyImagingEvent rdf:type owl:Class ;
                         rdfs:subClassOf :ImagingEvent ;
                         rdfs:label "Photography Imaging Event"@en .


###  https://www.morphosource.org/terms/morphosource#PhysicalObject
:PhysicalObject rdf:type owl:Class ;
                rdfs:subClassOf <http://pcdm.org/works#Work> ;
                rdfs:comment "A physical object, usually of scholarly interest, that is imaged to create media."@en ;
                rdfs:label "Physical Object"@en .


###  https://www.morphosource.org/terms/morphosource#PixelSpacingCalibrationType
:PixelSpacingCalibrationType rdf:type owl:Class ;
                             rdfs:comment "A type of correction for the effect of geometric magnification or calibration against an object of known size, as described in the Enumerated Values of the DICOM Pixel Spacing Calibration Type attribute (0028,0A02). The individual entities of this class in the MorphoSource data vocabulary comprise a controlled vocabulary used to describe the pixel calibration type for relevant Image Events."@en ;
                             rdfs:label "Pixel Spacing Calibration Type"@en .


###  https://www.morphosource.org/terms/morphosource#ProcessingActivityType
:ProcessingActivityType rdf:type owl:Class ;
                        rdfs:comment "Type statement describing a specific discrete processing activity step. It is often the case that in reality, multiple processing activity steps are used in the generation of any derived digital resource."@en ;
                        rdfs:label "Processing Activity Type"@en .


###  https://www.morphosource.org/terms/morphosource#ProcessingEvent
:ProcessingEvent rdf:type owl:Class ;
                 rdfs:subClassOf <http://pcdm.org/works#Work> ;
                 rdfs:comment "An active event in which a media is processed to produce another media. Belongs to Imaging Event or Media as a member (as either of these can lead to a processing event), and has member Media (as the processing event leads to the production of Media)."@en ;
                 rdfs:label "Processing Event"@en .


###  https://www.morphosource.org/terms/morphosource#PublicationStatus
:PublicationStatus rdf:type owl:Class ;
                   rdfs:comment "Status type indicating whether or not Media is published and under what conditions it is published."@en ;
                   rdfs:label "Publication Status"@en .


###  https://www.morphosource.org/terms/morphosource#SequentialSectionImagingEvent
:SequentialSectionImagingEvent rdf:type owl:Class ;
                               rdfs:subClassOf :ImagingEvent ;
                               rdfs:label "Sequential Section Imaging Event"@en .


###  https://www.morphosource.org/terms/morphosource#Sex
:Sex rdf:type owl:Class ;
     rdfs:comment "A categorical description or identification pertaining an organism's sex. The individual entities of this class in the MorphoSource data vocabulary comprise a controlled vocabulary of specific sex categorizations and identification statements used to describe Biological Specimens."@en ;
     rdfs:label "Sex"@en .


###  https://www.morphosource.org/terms/morphosource#Side
:Side rdf:type owl:Class ;
      rdfs:comment "For objects with bilateral or some other kind of symmetry, a term description statement pertaining to a particular side, the object midline, lack of knowledge relating to side, or inapplicability of this concept for an object."@en ;
      rdfs:label "Side"@en .


###  https://www.morphosource.org/terms/morphosource#SlideType
:SlideType rdf:type owl:Class ;
           rdfs:label "Type of Sequential Section Slide. Entities comprise a controlled vocabulary."@en .


###  https://www.morphosource.org/terms/morphosource#UseAgreementType
:UseAgreementType rdf:type owl:Class ;
                  rdfs:comment "Type of MorphoSource-specific Media download use agreement. This explicitly does not include types of non-MorphoSource use agreements, such as use agreements provided by third-party museums."@en ;
                  rdfs:label "Use Agreement Type"@en .


###  https://www.morphosource.org/terms/morphosource#User
:User rdf:type owl:Class ;
      rdfs:label "User"@en .


###  https://www.morphosource.org/terms/morphosource#XRayDetectorConfiguration
:XRayDetectorConfiguration rdf:type owl:Class ;
                           rdfs:comment "Physical configuration of X-Ray detector used to acquire an image for CT, MRI, and other related modalities, as described in the DICOM Dectector Configuration attribute (0018,7005). The individual entities of this class in the MorphoSource data vocabulary comprise a controlled vocabulary used to describe detector configuration for relevant Image Events."@en ;
                           rdfs:label "X-Ray Detector Configuration"@en .


###  https://www.morphosource.org/terms/morphosource#XRayDetectorType
:XRayDetectorType rdf:type owl:Class ;
                  rdfs:comment "Type of X-Ray detector used to acquire an image for CT, MRI, and other related modalities, as described in the DICOM Dectector Type attribute (0018,7004). The individual entities of this class in the MorphoSource data vocabulary comprise a controlled vocabulary used to describe detector type for relevant Image Events."@en ;
                  rdfs:label "X-Ray Detector Type"@en .


###  https://www.morphosource.org/terms/morphosource#XRayTargetType
:XRayTargetType rdf:type owl:Class ;
                rdfs:comment "Type of X-Ray target used to acquire an image for CT, MRI, and other related modalities. The individual entities of this class in the MorphoSource data vocabulary comprise a controlled vocabulary used to describe target type for relevant Image Events."@en ;
                rdfs:label "X-Ray Target Type"@en .


###  https://www.morphosource.org/terms/morphosource#3DPrintingPermission
<https://www.morphosource.org/terms/morphosource#3DPrintingPermission> rdf:type owl:Class ;
                                                                       rdfs:comment "Permission statement describing whether 3D printing of a digital resource is permitted, prohibited, or permitted with conditions."@en ;
                                                                       rdfs:label "3D Printing Permission"@en .


#################################################################
#    Individuals
#################################################################

###  http://purl.org/dc/terms/TGN
<http://purl.org/dc/terms/TGN> rdf:type owl:NamedIndividual .


###  http://www.getty.edu/research/tools/vocabulary/tgn/index.html
<http://www.getty.edu/research/tools/vocabulary/tgn/index.html> rdf:type owl:NamedIndividual .


###  https://www.morphosource.org/terms/morphosource#AlignParts
:AlignParts rdf:type owl:NamedIndividual ,
                     :ProcessingActivityType ;
            rdfs:label "Align Parts"@en .


###  https://www.morphosource.org/terms/morphosource#Area
:Area rdf:type owl:NamedIndividual ,
               :XRayDetectorConfiguration ;
      rdfs:label "Area (single or tiled detector)"@en .


###  https://www.morphosource.org/terms/morphosource#BackgroundRemovalMasking
:BackgroundRemovalMasking rdf:type owl:NamedIndividual ,
                                   :ProcessingActivityType ;
                          rdfs:label "Background Removal and/or Masking"@en .


###  https://www.morphosource.org/terms/morphosource#BitDepthChange
:BitDepthChange rdf:type owl:NamedIndividual ,
                         :ProcessingActivityType ;
                rdfs:label "Bit Depth Change"@en .


###  https://www.morphosource.org/terms/morphosource#BornDigital
:BornDigital rdf:type owl:NamedIndividual ,
                      :ImageModalityType ;
             rdfs:comment "Born Digital refers to digital content that is created and stored in digital format from the outset. Born-digital content includes digital photos, videos, documents, and other types of digital media."@en ;
             rdfs:label "Born Digital"@en ;
             <http://www.w3.org/2004/02/skos/core#altLabel> "BD"@en .


###  https://www.morphosource.org/terms/morphosource#CTImageSeries
:CTImageSeries rdf:type owl:NamedIndividual ,
                        :MediaType ;
               rdfs:label "CT/MRI image series (multiple files of type *.tiff, *.png, *.dcm, *.zip, etc.)"@en .


###  https://www.morphosource.org/terms/morphosource#Cm
:Cm rdf:type owl:NamedIndividual ,
             :LengthMeasurementUnit ;
    rdfs:label "Centimeters"@en .


###  https://www.morphosource.org/terms/morphosource#CollectionAndScanningFacility
:CollectionAndScanningFacility rdf:type owl:NamedIndividual ,
                                        :OrganizationType ;
                               rdfs:label "Collection and Scanning Facility"@en .


###  https://www.morphosource.org/terms/morphosource#Color
:Color rdf:type owl:NamedIndividual ,
                :MeshMapType ;
       rdfs:label "Color Map"@en .


###  https://www.morphosource.org/terms/morphosource#CommercialUseNotPermitted
:CommercialUseNotPermitted rdf:type owl:NamedIndividual ,
                                    :CommercialUsePermission ;
                           rdfs:comment "Commercial use of digital resource is not permitted."@en ;
                           rdfs:label "Commercial Use Not Permitted"@en .


###  https://www.morphosource.org/terms/morphosource#CommercialUsePermitted
:CommercialUsePermitted rdf:type owl:NamedIndividual ,
                                 :CommercialUsePermission ;
                        rdfs:comment "Commercial use of digital resource is permitted."@en ;
                        rdfs:label "Commercial Use Permitted"@en .


###  https://www.morphosource.org/terms/morphosource#ConfocalImageStacking
:ConfocalImageStacking rdf:type owl:NamedIndividual ,
                                :ImageModalityType ;
                       rdfs:comment "Confocal Image Stacking is an imaging technique that uses a series of images taken at different depths to create a 3D image of an object. By focusing a laser beam on a specific point in the object and measuring the reflected light, confocal microscopy can create high-resolution 3D images of cells and tissues."@en ;
                       rdfs:label "Confocal Image Stacking"@en ;
                       <http://www.w3.org/2004/02/skos/core#altLabel> "Confocal"@en .


###  https://www.morphosource.org/terms/morphosource#ConstantAngle
:ConstantAngle rdf:type owl:NamedIndividual ,
                        :AcquisitionType ;
               rdfs:label "Constant Angle"@en .


###  https://www.morphosource.org/terms/morphosource#Crop
:Crop rdf:type owl:NamedIndividual ,
               :ProcessingActivityType ;
      rdfs:label "Crop"@en .


###  https://www.morphosource.org/terms/morphosource#CrossPolarized
:CrossPolarized rdf:type owl:NamedIndividual ,
                         :LightSourceType ;
                rdfs:label "Cross polarized"@en .


###  https://www.morphosource.org/terms/morphosource#Direct
:Direct rdf:type owl:NamedIndividual ,
                 :XRayDetectorType ;
        rdfs:label "Direct (X-Ray photoconductor)"@en .


###  https://www.morphosource.org/terms/morphosource#EncouragedButNotRequired
:EncouragedButNotRequired rdf:type owl:NamedIndividual ,
                                   :DerivativeRearchivalStatement ;
                          rdfs:comment "Future derivatives are encouraged to be rearchived on a public-facing digital repository, but are not required to be rearchived."@en ;
                          rdfs:label "Encouraged But Not Required"@en .


###  https://www.morphosource.org/terms/morphosource#Female
:Female rdf:type owl:NamedIndividual ,
                 :Sex ;
        rdfs:label "Female"@en .


###  https://www.morphosource.org/terms/morphosource#Fiducial
:Fiducial rdf:type owl:NamedIndividual ,
                   :PixelSpacingCalibrationType ;
          rdfs:label "Fiducial"@en .


###  https://www.morphosource.org/terms/morphosource#Film
:Film rdf:type owl:NamedIndividual ,
               :XRayDetectorType ;
      rdfs:label "Film (Scanned film/screen)"@en .


###  https://www.morphosource.org/terms/morphosource#Fixed
:Fixed rdf:type owl:NamedIndividual ,
                :FocalLengthType ;
       rdfs:label "Fixed"@en .


###  https://www.morphosource.org/terms/morphosource#Free
:Free rdf:type owl:NamedIndividual ,
               :AcquisitionType ;
      rdfs:label "Free"@en .


###  https://www.morphosource.org/terms/morphosource#Ft
:Ft rdf:type owl:NamedIndividual ,
             :LengthMeasurementUnit ;
    rdfs:label "Feet"@en .


###  https://www.morphosource.org/terms/morphosource#Geometry
:Geometry rdf:type owl:NamedIndividual ,
                   :PixelSpacingCalibrationType ;
          rdfs:label "Geometry"@en .


###  https://www.morphosource.org/terms/morphosource#Gynandromorph
:Gynandromorph rdf:type owl:NamedIndividual ,
                        :Sex ;
               rdfs:label "Gynandromorph"@en .


###  https://www.morphosource.org/terms/morphosource#Hermaphrodite
:Hermaphrodite rdf:type owl:NamedIndividual ,
                        :Sex ;
               rdfs:label "Hermaphrodite"@en .


###  https://www.morphosource.org/terms/morphosource#HistogramEditing
:HistogramEditing rdf:type owl:NamedIndividual ,
                           :ProcessingActivityType ;
                  rdfs:label "Histogram Editing"@en .


###  https://www.morphosource.org/terms/morphosource#HistologicalSlide
:HistologicalSlide rdf:type owl:NamedIndividual ,
                            :SlideType ;
                   rdfs:label "Histological Slide"@en .


###  https://www.morphosource.org/terms/morphosource#Image
:Image rdf:type owl:NamedIndividual ,
                :MediaType ;
       rdfs:label "Image (*.tiff, *.png, *.dcm, etc.)"@en .


###  https://www.morphosource.org/terms/morphosource#ImageMeshCompression
:ImageMeshCompression rdf:type owl:NamedIndividual ,
                               :ProcessingActivityType ;
                      rdfs:label "Image and/or Mesh Compression"@en .


###  https://www.morphosource.org/terms/morphosource#In
:In rdf:type owl:NamedIndividual ,
             :LengthMeasurementUnit ;
    rdfs:label "Inches"@en .


###  https://www.morphosource.org/terms/morphosource#Infrared
:Infrared rdf:type owl:NamedIndividual ,
                   :ImageModalityType ;
          rdfs:comment "Infrared imaging is an imaging technique that uses infrared radiation to create images of objects. Infrared imaging can be used to detect and analyze heat signatures, as well as to create detailed images of objects and structures that are difficult to see with visible light."@en ;
          rdfs:label "Infrared"@en ;
          <http://www.w3.org/2004/02/skos/core#altLabel> "Infrared"@en .


###  https://www.morphosource.org/terms/morphosource#Km
:Km rdf:type owl:NamedIndividual ,
             :LengthMeasurementUnit ;
    rdfs:label "Kilometers"@en .


###  https://www.morphosource.org/terms/morphosource#LaserAidedProfiling
:LaserAidedProfiling rdf:type owl:NamedIndividual ,
                              :ImageModalityType ;
                     rdfs:comment "Laser Aided Profiling (LAP) is an imaging technique that uses a laser beam to create a 3D image of an object's surface. LAP can be used to create high-resolution, accurate models of complex shapes and structures, making it useful in manufacturing and other industries."@en ;
                     rdfs:label "Laser Aided Profiling"@en ;
                     <http://www.w3.org/2004/02/skos/core#altLabel> "LAP"@en .


###  https://www.morphosource.org/terms/morphosource#LaserScan
:LaserScan rdf:type owl:NamedIndividual ,
                    :ImageModalityType ;
           rdfs:comment "Laser Scan is an imaging technique that uses laser beams to create a 3D image of an object's surface. Laser scans are commonly used in industrial design and manufacturing to create accurate models of parts and components."@en ;
           rdfs:label "Laser Scan"@en ;
           <http://www.w3.org/2004/02/skos/core#altLabel> "Laser"@en .


###  https://www.morphosource.org/terms/morphosource#Left
:Left rdf:type owl:NamedIndividual ,
               :Side ;
      rdfs:label "Left"@en .


###  https://www.morphosource.org/terms/morphosource#M
:M rdf:type owl:NamedIndividual ,
            :LengthMeasurementUnit ;
   rdfs:label "Meters"@en .


###  https://www.morphosource.org/terms/morphosource#MagneticResonanceImaging
:MagneticResonanceImaging rdf:type owl:NamedIndividual ,
                                   :ImageModalityType ;
                          rdfs:comment "Magnetic Resonance Imaging (MRI) is a non-invasive imaging technique that uses a strong magnetic field and radio waves to produce detailed images of the body's internal structures. MRI is widely used in medical diagnosis and research, especially for imaging soft tissues like the brain, spinal cord, and organs."@en ;
                          rdfs:label "Magnetic Resonance Imaging (MRI)"@en ;
                          <http://www.w3.org/2004/02/skos/core#altLabel> "MRI"@en .


###  https://www.morphosource.org/terms/morphosource#Male
:Male rdf:type owl:NamedIndividual ,
               :Sex ;
      rdfs:label "Male"@en .


###  https://www.morphosource.org/terms/morphosource#Merge
:Merge rdf:type owl:NamedIndividual ,
                :ProcessingActivityType ;
       rdfs:label "Merge"@en .


###  https://www.morphosource.org/terms/morphosource#Mesh
:Mesh rdf:type owl:NamedIndividual ,
               :MediaType ;
      rdfs:label "Mesh or point cloud (*.stl, *.ply, .etc, with optional associated texture or color file)"@en .


###  https://www.morphosource.org/terms/morphosource#MeshPointCloudTexturing
:MeshPointCloudTexturing rdf:type owl:NamedIndividual ,
                                  :ProcessingActivityType ;
                         rdfs:label "Mesh and/or Point Cloud Texturing"@en .


###  https://www.morphosource.org/terms/morphosource#MeshToPointCloud
:MeshToPointCloud rdf:type owl:NamedIndividual ,
                           :ProcessingActivityType ;
                  rdfs:label "Mesh to Point Cloud"@en .


###  https://www.morphosource.org/terms/morphosource#Mi
:Mi rdf:type owl:NamedIndividual ,
             :LengthMeasurementUnit ;
    rdfs:label "Miles"@en .


###  https://www.morphosource.org/terms/morphosource#MicroNanoXRayComputedTomography
:MicroNanoXRayComputedTomography rdf:type owl:NamedIndividual ,
                                          :ImageModalityType ;
                                 rdfs:comment "X-Ray Computed Tomography (CT/microCT) is a non-invasive imaging technique that uses X-rays to produce cross-sectional images of an object. It involves rotating an X-ray source and detector around the object, collecting data that is processed by a computer to create a 3D image. CT is widely used in medical imaging, as well as in materials science, engineering, and geology to visualize the internal structure of objects. MicroCT is a variation of CT that uses higher resolution X-rays to produce images of smaller objects."@en ;
                                 rdfs:label "X-Ray Computed Tomography (CT/microCT)"@en ;
                                 <http://www.w3.org/2004/02/skos/core#altLabel> "CT"@en .


###  https://www.morphosource.org/terms/morphosource#Midline
:Midline rdf:type owl:NamedIndividual ,
                  :Side ;
         rdfs:label "Midline"@en .


###  https://www.morphosource.org/terms/morphosource#Mm
:Mm rdf:type owl:NamedIndividual ,
             :LengthMeasurementUnit ;
    rdfs:label "Millimeters"@en .


###  https://www.morphosource.org/terms/morphosource#MuseumDepartmentOrLabCollection
:MuseumDepartmentOrLabCollection rdf:type owl:NamedIndividual ,
                                          :OrganizationType ;
                                 rdfs:label "Museum, Department, or Lab Collection"@en .


###  https://www.morphosource.org/terms/morphosource#NeutronComputedTomography
:NeutronComputedTomography rdf:type owl:NamedIndividual ,
                                    :ImageModalityType ;
                           rdfs:comment "Neutron Computed Tomography (NCT) is an imaging technique that uses neutrons instead of X-rays to create cross-sectional images of an object. NCT is particularly useful for imaging materials that are difficult to penetrate with X-rays, such as ceramics and rocks."@en ;
                           rdfs:label "Neutron Computed Tomography (NCT)"@en ;
                           <http://www.w3.org/2004/02/skos/core#altLabel> "NCT"@en .


###  https://www.morphosource.org/terms/morphosource#Normal
:Normal rdf:type owl:NamedIndividual ,
                 :MeshMapType ;
        rdfs:label "Normal Map"@en .


###  https://www.morphosource.org/terms/morphosource#NotApplicable
:NotApplicable rdf:type owl:NamedIndividual ,
                        :Side ;
               rdfs:label "Not Applicable"@en .


###  https://www.morphosource.org/terms/morphosource#OnAnyRepository
:OnAnyRepository rdf:type owl:NamedIndividual ,
                          :DerivativeRearchivalStatement ;
                 rdfs:comment "Future derivatives are required to be rearchived on any public-facing digital repository."@en ;
                 rdfs:label "On Any Repository"@en .


###  https://www.morphosource.org/terms/morphosource#OnMorphoSource
:OnMorphoSource rdf:type owl:NamedIndividual ,
                         :DerivativeRearchivalStatement ;
                rdfs:comment "Future derivatives are required to be rearchived on MorphoSource."@en ;
                rdfs:label "On MorphoSource"@en .


###  https://www.morphosource.org/terms/morphosource#Open
:Open rdf:type owl:NamedIndividual ,
               :PublicationStatus ;
      rdfs:comment "Published with Open Download. Media record may be found in public search. Media file(s) may be downloaded openly, after downloader submits a simple download usage survey."@en ;
      rdfs:label "Open Download"@en .


###  https://www.morphosource.org/terms/morphosource#Other
:Other rdf:type owl:NamedIndividual ,
                :MediaType ;
       rdfs:label "Other"@en .


###  https://www.morphosource.org/terms/morphosource#OtherSlide
:OtherSlide rdf:type owl:NamedIndividual ,
                     :SlideType ;
            rdfs:label "Other Slide"@en .


###  https://www.morphosource.org/terms/morphosource#Patch
:Patch rdf:type owl:NamedIndividual ,
                :ProcessingActivityType ;
       rdfs:label "Patch"@en .


###  https://www.morphosource.org/terms/morphosource#Patterned
:Patterned rdf:type owl:NamedIndividual ,
                    :LightSourceType ;
           rdfs:label "Patterned"@en .


###  https://www.morphosource.org/terms/morphosource#Permissive
:Permissive rdf:type owl:NamedIndividual ,
                     :UseAgreementType ;
            rdfs:comment "Permissive MorphoSource use agreement."@en ;
            rdfs:label "Permissive"@en .


###  https://www.morphosource.org/terms/morphosource#Photogrammetry
:Photogrammetry rdf:type owl:NamedIndividual ,
                         :ImageModalityType ;
                rdfs:comment "Photogrammetry is the use of photography to measure and map the physical properties of an object. Photogrammetry can be used to create 3D models of objects and structures from 2D photographs, allowing for accurate measurements and analysis."@en ;
                rdfs:label "Photogrammetry"@en ;
                <http://www.w3.org/2004/02/skos/core#altLabel> "Photogram"@en .


###  https://www.morphosource.org/terms/morphosource#PhotogrammetryImageSeries
:PhotogrammetryImageSeries rdf:type owl:NamedIndividual ,
                                    :MediaType ;
                           rdfs:label "Photogrammetry image series (multiple files of type *.tiff, *.png, etc.)"@en .


###  https://www.morphosource.org/terms/morphosource#Photography
:Photography rdf:type owl:NamedIndividual ,
                      :ImageModalityType ;
             rdfs:comment "Photography is the use of light to capture images of objects and scenes. Photography can be used for a wide range of purposes, from capturing memories to documenting scientific observations and creating works of art."@en ;
             rdfs:label "Photography"@en ;
             <http://www.w3.org/2004/02/skos/core#altLabel> "Photo"@en .


###  https://www.morphosource.org/terms/morphosource#PhotosToDensePointCloud
:PhotosToDensePointCloud rdf:type owl:NamedIndividual ,
                                  :ProcessingActivityType ;
                         rdfs:label "Photos to Dense Point Cloud"@en .


###  https://www.morphosource.org/terms/morphosource#PhotosToDigitalElevationModel
:PhotosToDigitalElevationModel rdf:type owl:NamedIndividual ,
                                        :ProcessingActivityType ;
                               rdfs:label "Photos to Digital Elevation Model"@en .


###  https://www.morphosource.org/terms/morphosource#PhotosToMesh
:PhotosToMesh rdf:type owl:NamedIndividual ,
                       :ProcessingActivityType ;
              rdfs:label "Photos to Mesh"@en .


###  https://www.morphosource.org/terms/morphosource#PhotosToSparseMeshDepthMap
:PhotosToSparseMeshDepthMap rdf:type owl:NamedIndividual ,
                                     :ProcessingActivityType ;
                            rdfs:label "Photos to Sparse Mesh and Depth Map"@en .


###  https://www.morphosource.org/terms/morphosource#PhotosToSparsePointCloudDepthMap
:PhotosToSparsePointCloudDepthMap rdf:type owl:NamedIndividual ,
                                           :ProcessingActivityType ;
                                  rdfs:label "Photos to Sparse Point Cloud and Depth Map"@en .


###  https://www.morphosource.org/terms/morphosource#PointCloudToMesh
:PointCloudToMesh rdf:type owl:NamedIndividual ,
                           :ProcessingActivityType ;
                  rdfs:label "Point Cloud to Mesh"@en .


###  https://www.morphosource.org/terms/morphosource#PositronEmissionTomography
:PositronEmissionTomography rdf:type owl:NamedIndividual ,
                                     :ImageModalityType ;
                            rdfs:comment "Positron Emission Tomography (PET) is a non-invasive imaging technique that uses small amounts of radioactive tracers to visualize metabolic processes in the body. The tracer is injected into the body and collects in areas of high metabolic activity, emitting positrons that are detected by the PET scanner. PET is widely used in medical diagnosis and research, especially for imaging cancer, heart disease, and neurological disorders."@en ;
                            rdfs:label "Positron Emission Tomography (PET)"@en ;
                            <http://www.w3.org/2004/02/skos/core#altLabel> "PET"@en .


###  https://www.morphosource.org/terms/morphosource#Private
:Private rdf:type owl:NamedIndividual ,
                  :PublicationStatus ;
         rdfs:label "Private"@en ,
                    "Unpublished. Media may not be found in public search, and media file(s) may not be downloaded by users without explicit access to Media."@en .


###  https://www.morphosource.org/terms/morphosource#Projections
:Projections rdf:type owl:NamedIndividual ,
                      :CTImageSeriesType ;
             rdfs:label "Projections"@en .


###  https://www.morphosource.org/terms/morphosource#ReconstructedImageStack
:ReconstructedImageStack rdf:type owl:NamedIndividual ,
                                  :CTImageSeriesType ;
                         rdfs:label "Reconstructed image stack"@en .


###  https://www.morphosource.org/terms/morphosource#ReconstructedTomographyToMesh
:ReconstructedTomographyToMesh rdf:type owl:NamedIndividual ,
                                        :ProcessingActivityType ;
                               rdfs:label "Reconstructed Tomography to Mesh"@en .


###  https://www.morphosource.org/terms/morphosource#Reconstruction
:Reconstruction rdf:type owl:NamedIndividual ,
                         :ProcessingActivityType ;
                rdfs:label "Reconstruction"@en .


###  https://www.morphosource.org/terms/morphosource#ReflectanceTransformationImaging
:ReflectanceTransformationImaging rdf:type owl:NamedIndividual ,
                                           :ImageModalityType ;
                                  rdfs:comment "Reflectance Transformation Imaging (RTI) is an imaging technique that uses a series of photographs taken under different lighting conditions to create a detailed 3D model of an object's surface. RTI is particularly useful for analyzing the surface texture and details of objects such as artwork and historical artifacts."@en ;
                                  rdfs:label "Reflectance Transformation Imaging"@en ;
                                  <http://www.w3.org/2004/02/skos/core#altLabel> "RTI"@en .


###  https://www.morphosource.org/terms/morphosource#Reflection
:Reflection rdf:type owl:NamedIndividual ,
                     :XRayTargetType ;
            rdfs:label "Reflection"@en .


###  https://www.morphosource.org/terms/morphosource#Restricted
:Restricted rdf:type owl:NamedIndividual ,
                     :PublicationStatus ;
            rdfs:comment "Published with Restricted Download. Media may be found in public search. Media file(s) may only be downloaded after user has sought and received download approval from the Media data manager."@en ;
            rdfs:label "Restricted Download"@en .


###  https://www.morphosource.org/terms/morphosource#Right
:Right rdf:type owl:NamedIndividual ,
                :Side ;
       rdfs:label "Right"@en .


###  https://www.morphosource.org/terms/morphosource#ScanningElectronMicroscopy
:ScanningElectronMicroscopy rdf:type owl:NamedIndividual ,
                                     :ImageModalityType ;
                            rdfs:comment "Scanning Electron Microscopy (SEM) is an imaging technique that uses a beam of electrons to create high-resolution images of the surface of an object. SEM can produce images with extremely high magnification and resolution, making it useful for analyzing the microstructure of materials and biological specimens."@en ;
                            rdfs:label "Scanning Electron Microscopy"@en ;
                            <http://www.w3.org/2004/02/skos/core#altLabel> "SEM"@en .


###  https://www.morphosource.org/terms/morphosource#ScanningFacility
:ScanningFacility rdf:type owl:NamedIndividual ,
                           :OrganizationType ;
                  rdfs:label "Scanning Facility"@en .


###  https://www.morphosource.org/terms/morphosource#Scintillator
:Scintillator rdf:type owl:NamedIndividual ,
                       :XRayDetectorType ;
              rdfs:label "Scintillator (Phosphor used)"@en .


###  https://www.morphosource.org/terms/morphosource#Sequenced
:Sequenced rdf:type owl:NamedIndividual ,
                    :AcquisitionType ;
           rdfs:label "Sequenced (Rotational)"@en .


###  https://www.morphosource.org/terms/morphosource#SequentialSectionImageSeries
:SequentialSectionImageSeries rdf:type owl:NamedIndividual ,
                                       :MediaType ;
                              rdfs:label "Sequential section image series (multiple files of type *.tiff, *.png, *.zip, etc.)"@en .


###  https://www.morphosource.org/terms/morphosource#SequentialSectionScan
:SequentialSectionScan rdf:type owl:NamedIndividual ,
                                :ImageModalityType ;
                       rdfs:comment "Sequential Section Scan is an imaging technique that involves cutting an object into thin sections, then imaging each section individually to create a 3D image. This technique is commonly used in medical imaging and histology to visualize the internal structure of tissues and organs."@en ;
                       rdfs:label "Sequential Section Scan"@en ;
                       <http://www.w3.org/2004/02/skos/core#altLabel> "Section"@en .


###  https://www.morphosource.org/terms/morphosource#Simplification
:Simplification rdf:type owl:NamedIndividual ,
                         :ProcessingActivityType ;
                rdfs:label "Simplification"@en .


###  https://www.morphosource.org/terms/morphosource#SinglePhotonEmissionComputedTomography
:SinglePhotonEmissionComputedTomography rdf:type owl:NamedIndividual ,
                                                 :ImageModalityType ;
                                        rdfs:comment "Single Photon Emission Computed Tomography (SPECT) is a non-invasive imaging technique that uses a small amount of radioactive tracer to produce 3D images of the body's internal structures. The tracer is injected into the body and emits gamma rays, which are detected by a SPECT scanner. SPECT is used in medical diagnosis and research, especially for imaging the brain, heart, and bones."@en ;
                                        rdfs:label "Single Photon Emission Computed Tomography (SPECT)"@en ;
                                        <http://www.w3.org/2004/02/skos/core#altLabel> "SPECT"@en .


###  https://www.morphosource.org/terms/morphosource#Sinograms
:Sinograms rdf:type owl:NamedIndividual ,
                    :CTImageSeriesType ;
           rdfs:label "Sinograms"@en .


###  https://www.morphosource.org/terms/morphosource#Slot
:Slot rdf:type owl:NamedIndividual ,
               :XRayDetectorConfiguration ;
      rdfs:label "Slot (scanned slot, slit, or spot)"@en .


###  https://www.morphosource.org/terms/morphosource#SmoothingNoiseReduction
:SmoothingNoiseReduction rdf:type owl:NamedIndividual ,
                                  :ProcessingActivityType ;
                         rdfs:label "Smoothing and/or Noise Reduction"@en .


###  https://www.morphosource.org/terms/morphosource#SparseMeshDepthMapToMesh
:SparseMeshDepthMapToMesh rdf:type owl:NamedIndividual ,
                                   :ProcessingActivityType ;
                          rdfs:label "Sparse Mesh and Depth Map to Mesh"@en .


###  https://www.morphosource.org/terms/morphosource#SparsePointCloudDepthMapToDensePointCloud
:SparsePointCloudDepthMapToDensePointCloud rdf:type owl:NamedIndividual ,
                                                    :ProcessingActivityType ;
                                           rdfs:label "Sparse Point Cloud and Depth Map to Dense Point Cloud"@en .


###  https://www.morphosource.org/terms/morphosource#Spiral
:Spiral rdf:type owl:NamedIndividual ,
                 :AcquisitionType ;
        rdfs:label "Spiral"@en .


###  https://www.morphosource.org/terms/morphosource#Standard
:Standard rdf:type owl:NamedIndividual ,
                   :UseAgreementType ;
          rdfs:comment "Standard MorphoSource use agreement."@en ;
          rdfs:label "Standard"@en .


###  https://www.morphosource.org/terms/morphosource#Static
:Static rdf:type owl:NamedIndividual ,
                 :LightSourceType ;
        rdfs:label "Static"@en .


###  https://www.morphosource.org/terms/morphosource#Stationary
:Stationary rdf:type owl:NamedIndividual ,
                     :AcquisitionType ;
            rdfs:label "Stationary"@en .


###  https://www.morphosource.org/terms/morphosource#Storage
:Storage rdf:type owl:NamedIndividual ,
                  :XRayDetectorType ;
         rdfs:label "Storage (Storage Phosphor)"@en .


###  https://www.morphosource.org/terms/morphosource#Strobe
:Strobe rdf:type owl:NamedIndividual ,
                 :LightSourceType ;
        rdfs:label "Strobe"@en .


###  https://www.morphosource.org/terms/morphosource#StructuredLight
:StructuredLight rdf:type owl:NamedIndividual ,
                          :ImageModalityType ;
                 rdfs:comment "Structured Light is an imaging technique that uses a pattern of light projected onto an object to create a 3D image. By analyzing how the pattern of light is distorted by the object, structured light can create high-resolution, accurate 3D models of complex shapes and structures."@en ;
                 rdfs:label "Structured Light"@en ;
                 <http://www.w3.org/2004/02/skos/core#altLabel> "StrLight"@en .


###  https://www.morphosource.org/terms/morphosource#SynchrotronImaging
:SynchrotronImaging rdf:type owl:NamedIndividual ,
                             :ImageModalityType ;
                    rdfs:comment "Synchrotron Imaging is a type of X-ray imaging that uses synchrotron radiation, which is produced when high-energy particles are accelerated to near the speed of light. Synchrotron imaging can produce high-resolution, 3D images of a wide range of materials and structures."@en ;
                    rdfs:label "Synchrotron Imaging"@en ;
                    <http://www.w3.org/2004/02/skos/core#altLabel> "Synchro"@en .


###  https://www.morphosource.org/terms/morphosource#TransformReflection
:TransformReflection rdf:type owl:NamedIndividual ,
                              :ProcessingActivityType ;
                     rdfs:label "Transform: Reflection"@en .


###  https://www.morphosource.org/terms/morphosource#TransformRotation
:TransformRotation rdf:type owl:NamedIndividual ,
                            :ProcessingActivityType ;
                   rdfs:label "Transform: Rotation"@en .


###  https://www.morphosource.org/terms/morphosource#TransformScale
:TransformScale rdf:type owl:NamedIndividual ,
                         :ProcessingActivityType ;
                rdfs:label "Transform: Scale"@en .


###  https://www.morphosource.org/terms/morphosource#TransformTranslation
:TransformTranslation rdf:type owl:NamedIndividual ,
                               :ProcessingActivityType ;
                      rdfs:label "Transform: Translation"@en .


###  https://www.morphosource.org/terms/morphosource#Transmission
:Transmission rdf:type owl:NamedIndividual ,
                       :XRayTargetType ;
              rdfs:label "Transmission"@en .


###  https://www.morphosource.org/terms/morphosource#Um
:Um rdf:type owl:NamedIndividual ,
             :LengthMeasurementUnit ;
    rdfs:label "Micrometers"@en .


###  https://www.morphosource.org/terms/morphosource#Undetermined
:Undetermined rdf:type owl:NamedIndividual ,
                       :Sex ;
              rdfs:label "Undetermined"@en .


###  https://www.morphosource.org/terms/morphosource#Unknowable
:Unknowable rdf:type owl:NamedIndividual ,
                     :Sex ;
            rdfs:label "Unknowable"@en .


###  https://www.morphosource.org/terms/morphosource#Unknown
:Unknown rdf:type owl:NamedIndividual ,
                  :Side ;
         rdfs:label "Unknown"@en .


###  https://www.morphosource.org/terms/morphosource#Variable
:Variable rdf:type owl:NamedIndividual ,
                   :FocalLengthType ;
          rdfs:label "Variable"@en .


###  https://www.morphosource.org/terms/morphosource#Video
:Video rdf:type owl:NamedIndividual ,
                :MediaType ;
       rdfs:label "Video (*.avi, *.mp4, *.mov, .etc.)"@en .


###  https://www.morphosource.org/terms/morphosource#Videography
:Videography rdf:type owl:NamedIndividual ,
                      :ImageModalityType ;
             rdfs:comment "The recording of moving images and sound (video). It is a widely used medium for recording and displaying visual information, including images of physical objects. Video can be captured using a variety of devices, from smartphones to professional cameras, and can be stored in a variety of digital formats."@en ;
             rdfs:label "Videography"@en ;
             <http://www.w3.org/2004/02/skos/core#altLabel> "Video"@en .


###  https://www.morphosource.org/terms/morphosource#XRay
:XRay rdf:type owl:NamedIndividual ,
               :ImageModalityType ;
      rdfs:comment "X-Ray imaging is an imaging technique that uses X-rays to create images of the internal structures of an object. X-ray imaging is widely used in medical diagnosis and research, as well as in materials science and other fields to visualize the internal structure of objects."@en ;
      rdfs:label "X-Ray"@en ;
      <http://www.w3.org/2004/02/skos/core#altLabel> "XRay"@en .


###  https://www.morphosource.org/terms/morphosource#3DPrintingLimited
<https://www.morphosource.org/terms/morphosource#3DPrintingLimited> rdf:type owl:NamedIndividual ,
                                                                             <https://www.morphosource.org/terms/morphosource#3DPrintingPermission> ;
                                                                    rdfs:comment "3D printing of digital resources is permitted only if the data was initially downloaded with the intent to 3D print as explicitly indicated by communication from the downloader or from an automated download usage survey form, and where sharing of 3D prints is permitted only in small-scale informal circumstances that should be explicitly outlined elsewhere."@en ;
                                                                    rdfs:label "3D Printing Limited"@en .


###  https://www.morphosource.org/terms/morphosource#3DPrintingPermitted
<https://www.morphosource.org/terms/morphosource#3DPrintingPermitted> rdf:type owl:NamedIndividual ,
                                                                               <https://www.morphosource.org/terms/morphosource#3DPrintingPermission> ;
                                                                      rdfs:comment "3D printing of digital resource is freely permitted."@en ;
                                                                      rdfs:label "3D Printing Permitted"@en .


###  https://www.morphosource.org/terms/morphosource#3DPrintingProhibited
<https://www.morphosource.org/terms/morphosource#3DPrintingProhibited> rdf:type owl:NamedIndividual ,
                                                                                <https://www.morphosource.org/terms/morphosource#3DPrintingPermission> ;
                                                                       rdfs:comment "3D printing of digital resource is prohibited."@en ;
                                                                       rdfs:label "3D Printing Prohibited"@en .


#################################################################
#    Annotations
#################################################################

<http://purl.org/dc/terms/TGN> <http://purl.org/dc/terms/issued> "2000-07-11"^^xsd:date ;
                               rdfs:comment "The set of places specified by the Getty Thesaurus of Geographic Names."@en ;
                               rdfs:isDefinedBy <http://purl.org/dc/terms/> ;
                               rdfs:label "TGN"@en ;
                               rdfs:seeAlso <http://www.getty.edu/research/tools/vocabulary/tgn/index.html> .


###  Generated by the OWL API (version 5.1.18) https://github.com/owlcs/owlapi/
