<?xml version="1.0"?>
<rdf:RDF xmlns="https://www.morphosource.org/terms/morphosource#"
     xml:base="https://www.morphosource.org/terms/morphosource"
     xmlns:dc="http://purl.org/dc/elements/1.1/"
     xmlns:ns="http://www.w3.org/2003/12/exif/ns#"
     xmlns:v1="http://www.loc.gov/mads/rdf/v1#"
     xmlns:owl="http://www.w3.org/2002/07/owl#"
     xmlns:rdf="http://www.w3.org/1999/02/22-rdf-syntax-ns#"
     xmlns:xml="http://www.w3.org/XML/1998/namespace"
     xmlns:xsd="http://www.w3.org/2001/XMLSchema#"
     xmlns:dcam="http://purl.org/dc/dcam/"
     xmlns:rdfs="http://www.w3.org/2000/01/rdf-schema#"
     xmlns:skos="http://www.w3.org/2004/02/skos/core#"
     xmlns:terms="http://purl.org/dc/terms/"
     xmlns:attributes="http://rs.tdwg.org/dwc/terms/attributes/">
    <owl:Ontology rdf:about="https://www.morphosource.org/terms/morphosource">
        <rdfs:comment xml:lang="en">Test description for MorphoSource Terms Vocabulary</rdfs:comment>
        <rdfs:label xml:lang="en">MorphoSource Terms Vocabulary</rdfs:label>
        <owl:versionInfo>0.4.0</owl:versionInfo>
    </owl:Ontology>
    


    <!-- 
    ///////////////////////////////////////////////////////////////////////////////////////
    //
    // Annotation properties
    //
    ///////////////////////////////////////////////////////////////////////////////////////
     -->


    


    <!-- http://purl.org/dc/dcam/domainIncludes -->


    <owl:AnnotationProperty rdf:about="http://purl.org/dc/dcam/domainIncludes"/>
    


    <!-- http://purl.org/dc/dcam/memberOf -->


    <owl:AnnotationProperty rdf:about="http://purl.org/dc/dcam/memberOf"/>
    


    <!-- http://purl.org/dc/dcam/rangeIncludes -->


    <owl:AnnotationProperty rdf:about="http://purl.org/dc/dcam/rangeIncludes"/>
    


    <!-- http://purl.org/dc/elements/1.1/format -->


    <owl:AnnotationProperty rdf:about="http://purl.org/dc/elements/1.1/format"/>
    


    <!-- http://purl.org/dc/terms/description -->


    <owl:AnnotationProperty rdf:about="http://purl.org/dc/terms/description"/>
    


    <!-- http://purl.org/dc/terms/hasVersion -->


    <owl:AnnotationProperty rdf:about="http://purl.org/dc/terms/hasVersion"/>
    


    <!-- http://purl.org/dc/terms/isPartOf -->


    <owl:AnnotationProperty rdf:about="http://purl.org/dc/terms/isPartOf"/>
    


    <!-- http://purl.org/dc/terms/isVersionOf -->


    <owl:AnnotationProperty rdf:about="http://purl.org/dc/terms/isVersionOf"/>
    


    <!-- http://purl.org/dc/terms/issued -->


    <owl:AnnotationProperty rdf:about="http://purl.org/dc/terms/issued"/>
    


    <!-- http://purl.org/dc/terms/references -->


    <owl:AnnotationProperty rdf:about="http://purl.org/dc/terms/references"/>
    


    <!-- http://purl.org/dc/terms/replaces -->


    <owl:AnnotationProperty rdf:about="http://purl.org/dc/terms/replaces"/>
    


    <!-- http://rs.tdwg.org/dwc/terms/attributes/abcdEquivalence -->


    <owl:AnnotationProperty rdf:about="http://rs.tdwg.org/dwc/terms/attributes/abcdEquivalence"/>
    


    <!-- http://rs.tdwg.org/dwc/terms/attributes/decision -->


    <owl:AnnotationProperty rdf:about="http://rs.tdwg.org/dwc/terms/attributes/decision"/>
    


    <!-- http://rs.tdwg.org/dwc/terms/attributes/organizedInClass -->


    <owl:AnnotationProperty rdf:about="http://rs.tdwg.org/dwc/terms/attributes/organizedInClass"/>
    


    <!-- http://rs.tdwg.org/dwc/terms/attributes/repeatable -->


    <owl:AnnotationProperty rdf:about="http://rs.tdwg.org/dwc/terms/attributes/repeatable"/>
    


    <!-- http://rs.tdwg.org/dwc/terms/attributes/required -->


    <owl:AnnotationProperty rdf:about="http://rs.tdwg.org/dwc/terms/attributes/required"/>
    


    <!-- http://rs.tdwg.org/dwc/terms/attributes/usageScope -->


    <owl:AnnotationProperty rdf:about="http://rs.tdwg.org/dwc/terms/attributes/usageScope"/>
    


    <!-- http://www.loc.gov/mads/rdf/v1#authoritativeLabel -->


    <owl:AnnotationProperty rdf:about="http://www.loc.gov/mads/rdf/v1#authoritativeLabel"/>
    


    <!-- http://www.loc.gov/mads/rdf/v1#code -->


    <owl:AnnotationProperty rdf:about="http://www.loc.gov/mads/rdf/v1#code"/>
    


    <!-- http://www.loc.gov/mads/rdf/v1#definitionNote -->


    <owl:AnnotationProperty rdf:about="http://www.loc.gov/mads/rdf/v1#definitionNote"/>
    


    <!-- http://www.loc.gov/mads/rdf/v1#hasBroaderAuthority -->


    <owl:AnnotationProperty rdf:about="http://www.loc.gov/mads/rdf/v1#hasBroaderAuthority"/>
    


    <!-- http://www.loc.gov/mads/rdf/v1#historyNote -->


    <owl:AnnotationProperty rdf:about="http://www.loc.gov/mads/rdf/v1#historyNote"/>
    


    <!-- http://www.loc.gov/mads/rdf/v1#isMemberOfMADSCollection -->


    <owl:AnnotationProperty rdf:about="http://www.loc.gov/mads/rdf/v1#isMemberOfMADSCollection"/>
    


    <!-- http://www.loc.gov/mads/rdf/v1#isMemberOfMADSScheme -->


    <owl:AnnotationProperty rdf:about="http://www.loc.gov/mads/rdf/v1#isMemberOfMADSScheme"/>
    


    <!-- http://www.w3.org/1999/02/22-rdf-syntax-ns#type -->


    <owl:AnnotationProperty rdf:about="http://www.w3.org/1999/02/22-rdf-syntax-ns#type"/>
    


    <!-- http://www.w3.org/2003/12/exif/ns#tagNumber -->


    <owl:AnnotationProperty rdf:about="http://www.w3.org/2003/12/exif/ns#tagNumber"/>
    


    <!-- http://www.w3.org/2004/02/skos/core#altLabel -->


    <owl:AnnotationProperty rdf:about="http://www.w3.org/2004/02/skos/core#altLabel"/>
    


    <!-- http://www.w3.org/2004/02/skos/core#broader -->


    <owl:AnnotationProperty rdf:about="http://www.w3.org/2004/02/skos/core#broader"/>
    


    <!-- http://www.w3.org/2004/02/skos/core#changeNote -->


    <owl:AnnotationProperty rdf:about="http://www.w3.org/2004/02/skos/core#changeNote"/>
    


    <!-- http://www.w3.org/2004/02/skos/core#definition -->


    <owl:AnnotationProperty rdf:about="http://www.w3.org/2004/02/skos/core#definition"/>
    


    <!-- http://www.w3.org/2004/02/skos/core#example -->


    <owl:AnnotationProperty rdf:about="http://www.w3.org/2004/02/skos/core#example"/>
    


    <!-- http://www.w3.org/2004/02/skos/core#historyNote -->


    <owl:AnnotationProperty rdf:about="http://www.w3.org/2004/02/skos/core#historyNote"/>
    


    <!-- http://www.w3.org/2004/02/skos/core#inScheme -->


    <owl:AnnotationProperty rdf:about="http://www.w3.org/2004/02/skos/core#inScheme"/>
    


    <!-- http://www.w3.org/2004/02/skos/core#notation -->


    <owl:AnnotationProperty rdf:about="http://www.w3.org/2004/02/skos/core#notation"/>
    


    <!-- http://www.w3.org/2004/02/skos/core#note -->


    <owl:AnnotationProperty rdf:about="http://www.w3.org/2004/02/skos/core#note"/>
    


    <!-- http://www.w3.org/2004/02/skos/core#prefLabel -->


    <owl:AnnotationProperty rdf:about="http://www.w3.org/2004/02/skos/core#prefLabel"/>
    


    <!-- http://www.w3.org/2004/02/skos/core#scopeNote -->


    <owl:AnnotationProperty rdf:about="http://www.w3.org/2004/02/skos/core#scopeNote"/>
    


    <!-- 
    ///////////////////////////////////////////////////////////////////////////////////////
    //
    // Datatypes
    //
    ///////////////////////////////////////////////////////////////////////////////////////
     -->


    


    <!-- http://www.w3.org/2001/XMLSchema#date -->


    <rdfs:Datatype rdf:about="http://www.w3.org/2001/XMLSchema#date"/>
    


    <!-- 
    ///////////////////////////////////////////////////////////////////////////////////////
    //
    // Object Properties
    //
    ///////////////////////////////////////////////////////////////////////////////////////
     -->


    


    <!-- http://id.loc.gov/vocabulary/relators/dpt -->


    <owl:ObjectProperty rdf:about="http://id.loc.gov/vocabulary/relators/dpt">
        <owl:equivalentProperty rdf:resource="https://www.morphosource.org/terms/morphosource#depositor"/>
        <v1:authoritativeLabel>Depositor</v1:authoritativeLabel>
        <v1:code>dpt</v1:code>
        <v1:definitionNote xml:lang="en">A current owner of an item who deposited the item into the custody of another person, family, or organization, while still retaining ownership</v1:definitionNote>
        <v1:hasBroaderAuthority rdf:resource="http://id.loc.gov/vocabulary/relators/own"/>
        <v1:historyNote xml:lang="en">MARC bib: 1XX/7XX/8XX $4</v1:historyNote>
        <v1:isMemberOfMADSCollection rdf:resource="http://id.loc.gov/vocabulary/relators/collection_BIBFRAME"/>
        <v1:isMemberOfMADSCollection rdf:resource="http://id.loc.gov/vocabulary/relators/collection_PastPresentRelatorsEntries"/>
        <v1:isMemberOfMADSCollection rdf:resource="http://id.loc.gov/vocabulary/relators/collection_RDA"/>
        <v1:isMemberOfMADSCollection rdf:resource="http://id.loc.gov/vocabulary/relators/collection_RDAItem"/>
        <v1:isMemberOfMADSCollection rdf:resource="http://id.loc.gov/vocabulary/relators/collection_RDAOwner"/>
        <v1:isMemberOfMADSScheme rdf:resource="http://id.loc.gov/vocabulary/relators"/>
        <skos:broader rdf:resource="http://id.loc.gov/vocabulary/relators/own"/>
        <skos:changeNote rdf:nodeID="genid1"/>
        <skos:definition xml:lang="en">A current owner of an item who deposited the item into the custody of another person, family, or organization, while still retaining ownership</skos:definition>
        <skos:historyNote xml:lang="en">MARC bib: 1XX/7XX/8XX $4</skos:historyNote>
        <skos:inScheme rdf:resource="http://id.loc.gov/vocabulary/relators"/>
        <skos:notation>dpt</skos:notation>
        <skos:prefLabel>Depositor</skos:prefLabel>
    </owl:ObjectProperty>
    <rdf:Description rdf:nodeID="genid1"/>
    


    <!-- http://pcdm.org/models#fileOf -->


    <owl:ObjectProperty rdf:about="http://pcdm.org/models#fileOf">
        <owl:inverseOf rdf:resource="http://pcdm.org/models#hasFile"/>
        <rdfs:domain rdf:resource="http://pcdm.org/models#File"/>
        <rdfs:range rdf:resource="https://www.morphosource.org/terms/morphosource#FileSet"/>
        <rdfs:comment xml:lang="en">Links from a File to its containing Object.</rdfs:comment>
        <rdfs:isDefinedBy rdf:resource="http://pcdm.org/models#"/>
        <rdfs:label xml:lang="en">is file of</rdfs:label>
    </owl:ObjectProperty>
    


    <!-- http://pcdm.org/models#hasFile -->


    <owl:ObjectProperty rdf:about="http://pcdm.org/models#hasFile">
        <rdfs:domain rdf:resource="https://www.morphosource.org/terms/morphosource#FileSet"/>
        <rdfs:range rdf:resource="http://pcdm.org/models#File"/>
        <rdfs:comment xml:lang="en">Links to a File contained by this Object.</rdfs:comment>
        <rdfs:isDefinedBy rdf:resource="http://pcdm.org/models#"/>
        <rdfs:label xml:lang="en">has file</rdfs:label>
    </owl:ObjectProperty>
    


    <!-- http://pcdm.org/models#hasMember -->


    <owl:ObjectProperty rdf:about="http://pcdm.org/models#hasMember">
        <owl:inverseOf rdf:resource="http://pcdm.org/models#memberOf"/>
        <rdfs:domain rdf:resource="https://www.morphosource.org/terms/morphosource#ImagingEvent"/>
        <rdfs:domain rdf:resource="https://www.morphosource.org/terms/morphosource#Media"/>
        <rdfs:domain rdf:resource="https://www.morphosource.org/terms/morphosource#Organization"/>
        <rdfs:domain rdf:resource="https://www.morphosource.org/terms/morphosource#ProcessingEvent"/>
        <rdfs:range rdf:resource="https://www.morphosource.org/terms/morphosource#Device"/>
        <rdfs:range rdf:resource="https://www.morphosource.org/terms/morphosource#FileSet"/>
        <rdfs:range rdf:resource="https://www.morphosource.org/terms/morphosource#Media"/>
        <rdfs:range rdf:resource="https://www.morphosource.org/terms/morphosource#ProcessingEvent"/>
        <rdfs:comment xml:lang="en">Links to a subsidiary Object or Collection. Typically used to link
          to component parts, such as a book linking to a page.  Note on transitivity: hasMember is
          not defined as transitive, but applications may treat it as transitive as local needs
          dictate.</rdfs:comment>
        <rdfs:isDefinedBy rdf:resource="http://pcdm.org/models#"/>
        <rdfs:label xml:lang="en">has member</rdfs:label>
    </owl:ObjectProperty>
    


    <!-- http://pcdm.org/models#memberOf -->


    <owl:ObjectProperty rdf:about="http://pcdm.org/models#memberOf">
        <rdfs:domain rdf:resource="https://www.morphosource.org/terms/morphosource#Device"/>
        <rdfs:domain rdf:resource="https://www.morphosource.org/terms/morphosource#FileSet"/>
        <rdfs:domain rdf:resource="https://www.morphosource.org/terms/morphosource#Media"/>
        <rdfs:domain rdf:resource="https://www.morphosource.org/terms/morphosource#ProcessingEvent"/>
        <rdfs:range rdf:resource="https://www.morphosource.org/terms/morphosource#ImagingEvent"/>
        <rdfs:range rdf:resource="https://www.morphosource.org/terms/morphosource#Media"/>
        <rdfs:range rdf:resource="https://www.morphosource.org/terms/morphosource#Organization"/>
        <rdfs:range rdf:resource="https://www.morphosource.org/terms/morphosource#ProcessingEvent"/>
        <rdfs:comment xml:lang="en">Links from an Object or Collection to a containing Object or Collection.</rdfs:comment>
        <rdfs:isDefinedBy rdf:resource="http://pcdm.org/models#"/>
        <rdfs:label xml:lang="en">is member of</rdfs:label>
    </owl:ObjectProperty>
    


    <!-- http://purl.org/dc/terms/TGN -->


    <owl:ObjectProperty rdf:about="http://purl.org/dc/terms/TGN">
        <rdfs:domain rdf:resource="https://www.morphosource.org/terms/morphosource#PhysicalObject"/>
        <rdfs:range rdf:resource="http://vocab.getty.edu/tgn/7029392"/>
    </owl:ObjectProperty>
    


    <!-- http://purl.org/dc/terms/license -->


    <owl:ObjectProperty rdf:about="http://purl.org/dc/terms/license">
        <rdfs:domain rdf:resource="https://www.morphosource.org/terms/morphosource#Media"/>
        <rdfs:domain rdf:resource="https://www.morphosource.org/terms/morphosource#Organization"/>
        <rdfs:range rdf:resource="http://creativecommons.org/ns#License"/>
        <dcam:rangeIncludes rdf:resource="http://purl.org/dc/terms/LicenseDocument"/>
        <terms:description xml:lang="en">Recommended practice is to identify the license document with a URI. If this is not possible or feasible, a literal value that identifies the license may be provided.</terms:description>
        <rdfs:comment xml:lang="en">A legal document giving official permission to do something with the resource.</rdfs:comment>
        <rdfs:isDefinedBy rdf:resource="http://purl.org/dc/terms/"/>
        <rdfs:label xml:lang="en">License</rdfs:label>
    </owl:ObjectProperty>
    


    <!-- http://purl.org/healthcarevocab/v1#AcquisitionType -->


    <owl:ObjectProperty rdf:about="http://purl.org/healthcarevocab/v1#AcquisitionType">
        <rdfs:domain rdf:resource="https://www.morphosource.org/terms/morphosource#CTImageSeriesImagingEvent"/>
        <rdfs:range rdf:resource="https://www.morphosource.org/terms/morphosource#AcquisitionType"/>
        <rdfs:comment xml:lang="en">Description of the method used during acquisition of this frame. See Section C.8.15.3.2.1 for Defined Terms.

Required if Frame Type (0008,9007) Value 1 of this frame is ORIGINAL. May be present otherwise.</rdfs:comment>
        <rdfs:label xml:lang="en">Acquisition Type</rdfs:label>
    </owl:ObjectProperty>
    


    <!-- http://purl.org/healthcarevocab/v1#DetectorDescription -->


    <owl:ObjectProperty rdf:about="http://purl.org/healthcarevocab/v1#DetectorDescription">
        <rdfs:domain rdf:resource="https://www.morphosource.org/terms/morphosource#FileSet"/>
        <rdfs:comment xml:lang="en">Free text description of detector.</rdfs:comment>
        <rdfs:label xml:lang="en">Detector Description</rdfs:label>
    </owl:ObjectProperty>
    


    <!-- http://purl.org/healthcarevocab/v1#Modality -->


    <owl:ObjectProperty rdf:about="http://purl.org/healthcarevocab/v1#Modality">
        <rdfs:domain rdf:resource="https://www.morphosource.org/terms/morphosource#FileSet"/>
        <rdfs:comment xml:lang="en">Type of equipment that originally acquired the data used to create the images in this Series. See Section C.7.3.1.1.1 for Defined Terms.</rdfs:comment>
        <rdfs:label xml:lang="en">Modality</rdfs:label>
    </owl:ObjectProperty>
    


    <!-- http://purl.org/healthcarevocab/v1#PhotometricInterpretation -->


    <owl:ObjectProperty rdf:about="http://purl.org/healthcarevocab/v1#PhotometricInterpretation">
        <rdfs:domain rdf:resource="https://www.morphosource.org/terms/morphosource#FileSet"/>
        <rdfs:comment xml:lang="en">Specifies the intended interpretation of the pixel data. See Section C.7.6.3.1.2 for further explanation.</rdfs:comment>
        <rdfs:label xml:lang="en">Photometric Interpretation</rdfs:label>
    </owl:ObjectProperty>
    


    <!-- http://purl.org/healthcarevocab/v1#PixelSpacingCalibrationType -->


    <owl:ObjectProperty rdf:about="http://purl.org/healthcarevocab/v1#PixelSpacingCalibrationType">
        <rdfs:domain rdf:resource="https://www.morphosource.org/terms/morphosource#FileSet"/>
        <rdfs:comment xml:lang="en">The type of correction for the effect of geometric magnification or calibration against an object of known size, if any. See Section 10.7.1.2.</rdfs:comment>
        <rdfs:label xml:lang="en">Pixel Spacing Calibration Type</rdfs:label>
    </owl:ObjectProperty>
    


    <!-- http://rs.tdwg.org/ac/terms/captureDevice -->


    <owl:ObjectProperty rdf:about="http://rs.tdwg.org/ac/terms/captureDevice">
        <terms:description xml:lang="en">It is best practice to record the device; this may include a combination such as camera plus lens, or camera plus microscope. Examples: &quot;Canon Supershot 2000&quot;, &quot;Makroscan Scanner 2000&quot;, &quot;Zeiss Axioscope with Camera IIIu&quot;, &quot;SEM (Scanning Electron Microscope)&quot;.</terms:description>
        <terms:hasVersion rdf:resource="http://rs.tdwg.org/ac/terms/version/captureDevice-2013-10-28"/>
        <terms:hasVersion rdf:resource="http://rs.tdwg.org/ac/terms/version/captureDevice-2020-01-27"/>
        <terms:isPartOf rdf:resource="http://rs.tdwg.org/ac/terms/"/>
        <attributes:organizedInClass rdf:resource="http://rs.tdwg.org/dwc/terms/attributes/ResourceCreation"/>
        <attributes:repeatable>No</attributes:repeatable>
        <attributes:required>No</attributes:required>
        <rdfs:comment xml:lang="en">Free form text describing the device or devices used to create the resource.</rdfs:comment>
        <rdfs:isDefinedBy rdf:resource="http://rs.tdwg.org/ac/terms/"/>
        <rdfs:label xml:lang="en">Capture Device</rdfs:label>
    </owl:ObjectProperty>
    


    <!-- http://rs.tdwg.org/ac/terms/comments -->


    <owl:ObjectProperty rdf:about="http://rs.tdwg.org/ac/terms/comments">
        <terms:description xml:lang="en">Comments may refer to the resource itself (e. g., asserting a taxon name or location of a biological subject in an image), or to the relation between resource and associated metadata (e. g., asserting that the taxon name given in the metadata is wrong, without asserting a positive identification). There is a separate item for Reviewer Comments, which is defined more as an expert-level review. Implementers or communities of practice might establish conventions about the meaning of the absence of a commenter, but this specification is silent on that matter.</terms:description>
        <terms:hasVersion rdf:resource="http://rs.tdwg.org/ac/terms/version/comments-2013-10-28"/>
        <terms:hasVersion rdf:resource="http://rs.tdwg.org/ac/terms/version/comments-2020-01-27"/>
        <terms:isPartOf rdf:resource="http://rs.tdwg.org/ac/terms/"/>
        <attributes:organizedInClass rdf:resource="http://rs.tdwg.org/dwc/terms/attributes/Management"/>
        <attributes:repeatable>Yes</attributes:repeatable>
        <attributes:required>No</attributes:required>
        <rdfs:comment xml:lang="en">Any comment provided on the media resource, as free-form text.</rdfs:comment>
        <rdfs:isDefinedBy rdf:resource="http://rs.tdwg.org/ac/terms/"/>
        <rdfs:label xml:lang="en">Comments</rdfs:label>
        <skos:scopeNote xml:lang="en">Best practice would also identify the commenter.</skos:scopeNote>
    </owl:ObjectProperty>
    


    <!-- http://rs.tdwg.org/ac/terms/subtypeLiteral -->


    <owl:ObjectProperty rdf:about="http://rs.tdwg.org/ac/terms/subtypeLiteral">
        <terms:hasVersion rdf:resource="http://rs.tdwg.org/ac/terms/version/subtypeLiteral-2013-10-28"/>
        <terms:hasVersion rdf:resource="http://rs.tdwg.org/ac/terms/version/subtypeLiteral-2020-01-27"/>
        <terms:hasVersion rdf:resource="http://rs.tdwg.org/ac/terms/version/subtypeLiteral-2020-10-13"/>
        <terms:hasVersion rdf:resource="http://rs.tdwg.org/ac/terms/version/subtypeLiteral-2021-02-01"/>
        <terms:isPartOf rdf:resource="http://rs.tdwg.org/ac/terms/"/>
        <attributes:organizedInClass rdf:resource="http://rs.tdwg.org/dwc/terms/attributes/Management"/>
        <attributes:repeatable>Yes</attributes:repeatable>
        <attributes:required>No</attributes:required>
        <rdfs:comment xml:lang="en">A class, represented by a controlled value string, that provides for more specialization of the media item type than dc:type.</rdfs:comment>
        <rdfs:isDefinedBy rdf:resource="http://rs.tdwg.org/ac/terms/"/>
        <rdfs:label xml:lang="en">Subtype (literal)</rdfs:label>
        <skos:scopeNote xml:lang="en">The subtypeLiteral term MUST NOT be applied to Collection objects. However, the Description term in the Content Coverage Vocabulary might add further description to a Collection object. Controlled string values SHOULD be selected from the Controlled Vocabulary for Audubon Core subtype. Human-readable information about the Controlled Vocabulary for subtype is at http://rs.tdwg.org/ac/doc/subtype/ . It is best practice to use ac:subtype instead of ac:subytpeLiteral whenever practical.</skos:scopeNote>
    </owl:ObjectProperty>
    


    <!-- http://rs.tdwg.org/dwc/terms/country -->


    <owl:ObjectProperty rdf:about="http://rs.tdwg.org/dwc/terms/country">
        <rdfs:domain rdf:resource="https://www.morphosource.org/terms/morphosource#Organization"/>
        <rdfs:domain rdf:resource="https://www.morphosource.org/terms/morphosource#PhysicalObject"/>
        <terms:description xml:lang="en">Recommended best practice is to use a controlled vocabulary such as the Getty Thesaurus of Geographic Names. Recommended best practice is to leave this field blank if the Location spans multiple entities at this administrative level or if the Location might be in one or another of multiple possible entities at this level. Multiplicity and uncertainty of the geographic entity can be captured either in the term higherGeography or in the term locality, or both.</terms:description>
        <terms:hasVersion rdf:resource="http://rs.tdwg.org/dwc/terms/version/country-2009-04-24"/>
        <terms:hasVersion rdf:resource="http://rs.tdwg.org/dwc/terms/version/country-2017-10-06"/>
        <terms:hasVersion rdf:resource="http://rs.tdwg.org/dwc/terms/version/country-2021-07-15"/>
        <terms:isPartOf rdf:resource="http://rs.tdwg.org/dwc/terms/"/>
        <terms:replaces rdf:resource="http://rs.tdwg.org/dwc/dwcore/Country"/>
        <attributes:abcdEquivalence>DataSets/DataSet/Units/Unit/Gathering/Country/Name</attributes:abcdEquivalence>
        <attributes:organizedInClass rdf:resource="http://purl.org/dc/terms/Location"/>
        <attributes:usageScope>simple</attributes:usageScope>
        <rdfs:comment xml:lang="en">The name of the country or major administrative unit in which the Location occurs.</rdfs:comment>
        <rdfs:isDefinedBy rdf:resource="http://rs.tdwg.org/dwc/terms/"/>
        <rdfs:label xml:lang="en">Country</rdfs:label>
        <skos:example xml:lang="en">`Denmark`, `Colombia`, `España`</skos:example>
    </owl:ObjectProperty>
    


    <!-- http://rs.tdwg.org/dwc/terms/sex -->


    <owl:ObjectProperty rdf:about="http://rs.tdwg.org/dwc/terms/sex">
        <rdfs:domain rdf:resource="https://www.morphosource.org/terms/morphosource#BiologicalSpecimenObject"/>
        <rdfs:range rdf:resource="https://www.morphosource.org/terms/morphosource#Sex"/>
        <terms:description xml:lang="en">Recommended best practice is to use a controlled vocabulary.</terms:description>
        <terms:hasVersion rdf:resource="http://rs.tdwg.org/dwc/terms/version/sex-2009-04-24"/>
        <terms:hasVersion rdf:resource="http://rs.tdwg.org/dwc/terms/version/sex-2017-10-06"/>
        <terms:isPartOf rdf:resource="http://rs.tdwg.org/dwc/terms/"/>
        <terms:replaces rdf:resource="http://rs.tdwg.org/dwc/dwcore/Sex"/>
        <attributes:abcdEquivalence>DataSets/DataSet/Units/Unit/Sex</attributes:abcdEquivalence>
        <attributes:organizedInClass rdf:resource="http://rs.tdwg.org/dwc/terms/Occurrence"/>
        <attributes:usageScope>simple</attributes:usageScope>
        <rdfs:comment xml:lang="en">The sex of the biological individual(s) represented in the Occurrence.</rdfs:comment>
        <rdfs:isDefinedBy rdf:resource="http://rs.tdwg.org/dwc/terms/"/>
        <rdfs:label xml:lang="en">Sex</rdfs:label>
        <skos:example xml:lang="en">`female`, `male`, `hermaphrodite`</skos:example>
    </owl:ObjectProperty>
    


    <!-- http://rs.tdwg.org/dwc/terms/stateProvince -->


    <owl:ObjectProperty rdf:about="http://rs.tdwg.org/dwc/terms/stateProvince">
        <rdfs:domain rdf:resource="https://www.morphosource.org/terms/morphosource#Organization"/>
        <rdfs:domain rdf:resource="https://www.morphosource.org/terms/morphosource#PhysicalObject"/>
        <terms:description xml:lang="en">Recommended best practice is to use a controlled vocabulary such as the Getty Thesaurus of Geographic Names.</terms:description>
        <terms:hasVersion rdf:resource="http://rs.tdwg.org/dwc/terms/version/stateProvince-2009-04-24"/>
        <terms:hasVersion rdf:resource="http://rs.tdwg.org/dwc/terms/version/stateProvince-2017-10-06"/>
        <terms:isPartOf rdf:resource="http://rs.tdwg.org/dwc/terms/"/>
        <terms:replaces rdf:resource="http://rs.tdwg.org/dwc/dwcore/StateProvince"/>
        <attributes:abcdEquivalence>DataSets/DataSet/Units/Unit/Gathering/NamedAreas/NamedArea/AreaName with NamedAreas/NamedArea/AreaClass= State or = Province (etc.)</attributes:abcdEquivalence>
        <attributes:organizedInClass rdf:resource="http://purl.org/dc/terms/Location"/>
        <attributes:usageScope>simple</attributes:usageScope>
        <rdfs:comment xml:lang="en">The name of the next smaller administrative region than country (state, province, canton, department, region, etc.) in which the Location occurs.</rdfs:comment>
        <rdfs:isDefinedBy rdf:resource="http://rs.tdwg.org/dwc/terms/"/>
        <rdfs:label xml:lang="en">State Province</rdfs:label>
        <skos:example xml:lang="en">`Montana`, `Minas Gerais`, `Córdoba`</skos:example>
    </owl:ObjectProperty>
    


    <!-- http://www.europeana.eu/schemas/edm/rights -->


    <owl:ObjectProperty rdf:about="http://www.europeana.eu/schemas/edm/rights">
        <rdfs:comment xml:lang="en">Information about copyright of the digital object.</rdfs:comment>
        <rdfs:label xml:lang="en">Europeana Rights</rdfs:label>
    </owl:ObjectProperty>
    


    <!-- http://www.w3.org/2003/12/exif/ns#lightSource -->


    <owl:ObjectProperty rdf:about="http://www.w3.org/2003/12/exif/ns#lightSource">
        <rdfs:domain rdf:resource="https://www.morphosource.org/terms/morphosource#PhotogrammetryImagingEvent"/>
        <rdfs:domain rdf:resource="https://www.morphosource.org/terms/morphosource#PhotographyImagingEvent"/>
        <rdfs:range rdf:resource="https://www.morphosource.org/terms/morphosource#LightSourceType"/>
        <rdfs:comment xml:lang="en">Light source such as Daylight, Tungsten, Flash etc.</rdfs:comment>
        <rdfs:comment xml:lang="ja">光源。これはマニュアルでホワイトバランスを設定した場合のモード値となる</rdfs:comment>
        <rdfs:label xml:lang="en">LightSource</rdfs:label>
        <ns:tagNumber xml:lang="en">37384</ns:tagNumber>
    </owl:ObjectProperty>
    


    <!-- https://www.morphosource.org/terms/morphosource#aatAttribute -->


    <owl:ObjectProperty rdf:about="https://www.morphosource.org/terms/morphosource#aatAttribute">
        <rdfs:domain rdf:resource="https://www.morphosource.org/terms/morphosource#CulturalHeritageObject"/>
        <rdfs:range rdf:resource="http://vocab.getty.edu/aat/300264087"/>
        <rdfs:comment xml:lang="en">Physical attributes of an object, including characteristics such as size and shape, chemical properties of materials, qualities of texture and hardness, and features such as surface ornament. Values must be from the controlled vocabulary Getty Arts and Architecture Thesaurus Physical Attributes Facet (http://vocab.getty.edu/page/aat/300264087). Use of this property is preferred over the custom morphosource:choAttribute property.</rdfs:comment>
        <rdfs:label xml:lang="en">Getty Arts and Architecture Thesaurus Attribute</rdfs:label>
        <skos:example xml:lang="en">`round`, `waterlogged`, `brittleness`</skos:example>
    </owl:ObjectProperty>
    


    <!-- https://www.morphosource.org/terms/morphosource#aatMaterial -->


    <owl:ObjectProperty rdf:about="https://www.morphosource.org/terms/morphosource#aatMaterial">
        <rdfs:domain rdf:resource="https://www.morphosource.org/terms/morphosource#CulturalHeritageObject"/>
        <rdfs:range rdf:resource="http://vocab.getty.edu/aat/300264091"/>
        <rdfs:comment xml:lang="en">Material(s) from which an object is made. Values must be from the controlled vocabulary Getty Arts and Architecture Thesaurus Materials Facet (http://vocab.getty.edu/page/aat/300264091). Use of this property is preferred over the custom morphosource:Material property.</rdfs:comment>
        <rdfs:label xml:lang="en">Getty Arts and Architecture Thesaurus Material</rdfs:label>
        <skos:example xml:lang="en">`iron`, `clay`, `millwork`</skos:example>
    </owl:ObjectProperty>
    


    <!-- https://www.morphosource.org/terms/morphosource#aatPeriod -->


    <owl:ObjectProperty rdf:about="https://www.morphosource.org/terms/morphosource#aatPeriod">
        <rdfs:domain rdf:resource="https://www.morphosource.org/terms/morphosource#CulturalHeritageObject"/>
        <rdfs:range rdf:resource="http://vocab.getty.edu/aat/300264088"/>
        <rdfs:comment xml:lang="en">Time period associated with the production or creation of an object. Values must be from the controlled vocabulary Getty Arts and Architecture Thesaurus Styles and Periods Facet (http://vocab.getty.edu/page/aat/300264088).</rdfs:comment>
        <rdfs:label xml:lang="en">Getty Arts and Architecture Thesaurus Time Period</rdfs:label>
        <skos:example xml:lang="en">`Neolithic`,`Pliocene`</skos:example>
    </owl:ObjectProperty>
    


    <!-- https://www.morphosource.org/terms/morphosource#aatType -->


    <owl:ObjectProperty rdf:about="https://www.morphosource.org/terms/morphosource#aatType">
        <rdfs:domain rdf:resource="https://www.morphosource.org/terms/morphosource#CulturalHeritageObject"/>
        <rdfs:range rdf:resource="http://vocab.getty.edu/aat/300264092"/>
        <rdfs:comment xml:lang="en">Type, genre, category, or classification of an object. Values must be from the controlled vocabulary Getty Arts and Architecture Thesaurus Objects Facet (http://vocab.getty.edu/page/aat/300264092). Use of this property is preferred over the custom morphosource:choType property.</rdfs:comment>
        <rdfs:label xml:lang="en">Getty Arts and Architecture Thesaurus Type</rdfs:label>
        <skos:example xml:lang="en">`vases`, `paintings (visual works)`, `hammers (tools)`</skos:example>
    </owl:ObjectProperty>
    


    <!-- https://www.morphosource.org/terms/morphosource#colorFormat -->


    <owl:ObjectProperty rdf:about="https://www.morphosource.org/terms/morphosource#colorFormat">
        <rdfs:domain rdf:resource="https://www.morphosource.org/terms/morphosource#FileSet"/>
        <rdfs:comment xml:lang="en">How 3D color information is formatted and codified for a 3D object, if color information is present with the object. Values may include &quot;vertex color&quot;, &quot;face color&quot;, &quot;UV texture&quot;, or others.</rdfs:comment>
        <rdfs:label xml:lang="en">Color Format</rdfs:label>
    </owl:ObjectProperty>
    


    <!-- https://www.morphosource.org/terms/morphosource#colorSpace -->


    <owl:ObjectProperty rdf:about="https://www.morphosource.org/terms/morphosource#colorSpace">
        <rdfs:domain rdf:resource="https://www.morphosource.org/terms/morphosource#FileSet"/>
        <rdfs:comment xml:lang="en">Color space of image data. Values should be from the controlled vocabulary of short string labels for color spaces defined in the TIFF Tag PhotometricInterpretation (https://www.awaresystems.be/imaging/tiff/tifftags/photometricinterpretation.html).</rdfs:comment>
        <rdfs:label xml:lang="en">Color Space</rdfs:label>
        <skos:example xml:lang="en">`BlackIsZero`, `RGB`, `YCbCr`</skos:example>
    </owl:ObjectProperty>
    


    <!-- https://www.morphosource.org/terms/morphosource#compression -->


    <owl:ObjectProperty rdf:about="https://www.morphosource.org/terms/morphosource#compression">
        <rdfs:domain rdf:resource="https://www.morphosource.org/terms/morphosource#FileSet"/>
        <rdfs:comment xml:lang="en">Compression scheme used on image data. Values should be from the controlled vocabulary of short string labels for compression schemes defined in the TIFF Tag Compression (https://www.awaresystems.be/imaging/tiff/tifftags/compression.html).</rdfs:comment>
        <rdfs:label xml:lang="en">Compression</rdfs:label>
        <skos:example xml:lang="en">`Uncompressed`, `JPEG`, `PackBits`</skos:example>
    </owl:ObjectProperty>
    


    <!-- https://www.morphosource.org/terms/morphosource#dataManager -->


    <owl:ObjectProperty rdf:about="https://www.morphosource.org/terms/morphosource#dataManager">
        <rdfs:domain rdf:resource="https://www.morphosource.org/terms/morphosource#Organization"/>
        <rdfs:range rdf:resource="https://www.morphosource.org/terms/morphosource#User"/>
        <rdfs:comment xml:lang="en">User intended to have long-term data management over Media representing Organization Physical Objects.</rdfs:comment>
        <rdfs:label xml:lang="en">Data Manager</rdfs:label>
    </owl:ObjectProperty>
    


    <!-- https://www.morphosource.org/terms/morphosource#depositor -->


    <owl:ObjectProperty rdf:about="https://www.morphosource.org/terms/morphosource#depositor">
        <rdfs:domain rdf:resource="https://www.morphosource.org/terms/morphosource#Device"/>
        <rdfs:domain rdf:resource="https://www.morphosource.org/terms/morphosource#FileSet"/>
        <rdfs:domain rdf:resource="https://www.morphosource.org/terms/morphosource#ImagingEvent"/>
        <rdfs:domain rdf:resource="https://www.morphosource.org/terms/morphosource#Media"/>
        <rdfs:domain rdf:resource="https://www.morphosource.org/terms/morphosource#Organization"/>
        <rdfs:domain rdf:resource="https://www.morphosource.org/terms/morphosource#PhysicalObject"/>
        <rdfs:domain rdf:resource="https://www.morphosource.org/terms/morphosource#ProcessingEvent"/>
        <rdfs:range rdf:resource="https://www.morphosource.org/terms/morphosource#User"/>
        <v1:authoritativeLabel>Depositor</v1:authoritativeLabel>
        <v1:code>dpt</v1:code>
        <v1:definitionNote xml:lang="en">A current owner of an item who deposited the item into the custody of another person, family, or organization, while still retaining ownership</v1:definitionNote>
        <v1:hasBroaderAuthority rdf:resource="http://id.loc.gov/vocabulary/relators/own"/>
        <v1:historyNote xml:lang="en">MARC bib: 1XX/7XX/8XX $4</v1:historyNote>
        <rdfs:comment xml:lang="en">A current owner of an item who deposited the item into the custody of another person, family, or organization, while still retaining ownership</rdfs:comment>
        <rdfs:label xml:lang="en">Depositor</rdfs:label>
        <skos:broader rdf:resource="http://id.loc.gov/vocabulary/relators/own"/>
        <skos:changeNote rdf:nodeID="genid1"/>
        <skos:historyNote xml:lang="en">MARC bib: 1XX/7XX/8XX $4</skos:historyNote>
        <skos:notation>dpt</skos:notation>
    </owl:ObjectProperty>
    


    <!-- https://www.morphosource.org/terms/morphosource#detectorConfiguration -->


    <owl:ObjectProperty rdf:about="https://www.morphosource.org/terms/morphosource#detectorConfiguration">
        <rdfs:domain rdf:resource="https://www.morphosource.org/terms/morphosource#CTImageSeriesImagingEvent"/>
        <rdfs:range rdf:resource="https://www.morphosource.org/terms/morphosource#XRayDetectorConfiguration"/>
        <rdfs:comment xml:lang="en">The physical configuration of the X-Ray detector. Value must be from the X-Ray Detector Configuration controlled vocabulary (https://www.morphosource.org/terms/morphosource#XRayDetectorConfiguration). This property should be a sub-property of dicom:DetectorConfiguration.</rdfs:comment>
        <rdfs:label xml:lang="en">Detector Configuration</rdfs:label>
        <skos:example xml:lang="en">`Area (single or tiled detector)`, `Slot (scanned slot, slit, or spot)`</skos:example>
    </owl:ObjectProperty>
    


    <!-- https://www.morphosource.org/terms/morphosource#detectorType -->


    <owl:ObjectProperty rdf:about="https://www.morphosource.org/terms/morphosource#detectorType">
        <rdfs:subPropertyOf rdf:resource="http://purl.org/healthcarevocab/v1#DetectorDescription"/>
        <rdfs:domain rdf:resource="https://www.morphosource.org/terms/morphosource#CTImageSeriesImagingEvent"/>
        <rdfs:range rdf:resource="https://www.morphosource.org/terms/morphosource#XRayDetectorType"/>
        <terms:isVersionOf rdf:resource="http://purl.org/healthcarevocab/v1#DetectorDescription"/>
        <rdfs:comment xml:lang="en">Type of detector used to acquire this image. This property is more accurately a sub-property of dicom:DetectorType and should be changed accordingly. Value must be from X-Ray Detector Type controlled vocabulary (https://www.morphosource.org/terms/morphosource#XRayDetectorType).</rdfs:comment>
        <rdfs:label xml:lang="en">Detector Type</rdfs:label>
        <skos:example xml:lang="en">`Direct (X-Ray photoconductor)`, `Scintillator (Phosphor used)`, `Storage (Storage Phosphor)`, `Film (Scanned film/screen)`</skos:example>
    </owl:ObjectProperty>
    


    <!-- https://www.morphosource.org/terms/morphosource#downloadPermission -->


    <owl:ObjectProperty rdf:about="https://www.morphosource.org/terms/morphosource#downloadPermission">
        <rdfs:domain rdf:resource="https://www.morphosource.org/terms/morphosource#Organization"/>
        <rdfs:range rdf:resource="https://www.morphosource.org/terms/morphosource#PublicationStatus"/>
        <rdfs:comment xml:lang="en">Preferred Publication Status (morphosource:visibility) for Media representing Organization Physical Objects. Value must be from Publication Status controlled vocabulary (https://www.morphosource.org/terms/morphosource#PublicationStatus).</rdfs:comment>
        <rdfs:label xml:lang="en">Download Permission</rdfs:label>
        <skos:example xml:lang="en">`Open`, `Restricted`, `Private`</skos:example>
    </owl:ObjectProperty>
    


    <!-- https://www.morphosource.org/terms/morphosource#downloadReviewer -->


    <owl:ObjectProperty rdf:about="https://www.morphosource.org/terms/morphosource#downloadReviewer">
        <rdfs:domain rdf:resource="https://www.morphosource.org/terms/morphosource#Media"/>
        <rdfs:domain rdf:resource="https://www.morphosource.org/terms/morphosource#Organization"/>
        <rdfs:range rdf:resource="https://www.morphosource.org/terms/morphosource#User"/>
        <rdfs:comment xml:lang="en">User(s) that receive and may decide approval requests to download media that is Published with Restricted Download.</rdfs:comment>
        <rdfs:label xml:lang="en">Download Reviewer</rdfs:label>
    </owl:ObjectProperty>
    


    <!-- https://www.morphosource.org/terms/morphosource#filesetAccessibility -->


    <owl:ObjectProperty rdf:about="https://www.morphosource.org/terms/morphosource#filesetAccessibility">
        <rdfs:label xml:lang="en">FileSet Accessibility</rdfs:label>
    </owl:ObjectProperty>
    


    <!-- https://www.morphosource.org/terms/morphosource#focalLengthType -->


    <owl:ObjectProperty rdf:about="https://www.morphosource.org/terms/morphosource#focalLengthType">
        <rdfs:domain rdf:resource="https://www.morphosource.org/terms/morphosource#PhotogrammetryImagingEvent"/>
        <rdfs:range rdf:resource="https://www.morphosource.org/terms/morphosource#FocalLengthType"/>
        <rdfs:comment xml:lang="en">Whether focal length is variable or fixed. Values must be from FocalLengthType controlled vocabulary (https://www.morphosource.org/terms/morphosource#FocalLengthType).</rdfs:comment>
        <rdfs:label xml:lang="en">Focal Length Type</rdfs:label>
        <skos:example xml:lang="en">`Variable`, `Fixed`</skos:example>
    </owl:ObjectProperty>
    


    <!-- https://www.morphosource.org/terms/morphosource#ieModality -->


    <owl:ObjectProperty rdf:about="https://www.morphosource.org/terms/morphosource#ieModality">
        <rdfs:subPropertyOf rdf:resource="http://rs.tdwg.org/ac/terms/captureDevice"/>
        <rdfs:domain rdf:resource="https://www.morphosource.org/terms/morphosource#ImagingEvent"/>
        <rdfs:range rdf:resource="https://www.morphosource.org/terms/morphosource#ImageModalityType"/>
        <terms:isVersionOf rdf:resource="http://rs.tdwg.org/ac/terms/captureDevice"/>
        <rdfs:comment xml:lang="en">The imaging modality used in the imaging event. Value must be from Image Modality controlled vocabulary (https://www.morphosource.org/terms/morphosource#ImageModality).</rdfs:comment>
        <rdfs:label xml:lang="en">Imaging Event Modality</rdfs:label>
        <skos:example xml:lang="en">`MicroNanoXRayComputedTomography`, `Photogrammetry`, `Video`</skos:example>
    </owl:ObjectProperty>
    


    <!-- https://www.morphosource.org/terms/morphosource#mapType -->


    <owl:ObjectProperty rdf:about="https://www.morphosource.org/terms/morphosource#mapType">
        <rdfs:domain rdf:resource="https://www.morphosource.org/terms/morphosource#Media"/>
        <rdfs:range rdf:resource="https://www.morphosource.org/terms/morphosource#MeshMapType"/>
        <rdfs:comment xml:lang="en">Type of texture map or projection that accompanies a 3D mesh model Media, such as color or normal maps. Values must be from the Mesh Map Type controlled vocabulary (https://www.morphosource.org/terms/morphosource#MeshMapType). This only applies to Mesh Media.</rdfs:comment>
        <rdfs:label xml:lang="en">Map Type</rdfs:label>
        <skos:example xml:lang="en">`Color`, `Normal`</skos:example>
    </owl:ObjectProperty>
    


    <!-- https://www.morphosource.org/terms/morphosource#mediaType -->


    <owl:ObjectProperty rdf:about="https://www.morphosource.org/terms/morphosource#mediaType">
        <rdfs:subPropertyOf rdf:resource="http://rs.tdwg.org/ac/terms/subtypeLiteral"/>
        <rdfs:domain rdf:resource="https://www.morphosource.org/terms/morphosource#Media"/>
        <rdfs:range rdf:resource="https://www.morphosource.org/terms/morphosource#MediaType"/>
        <terms:isVersionOf rdf:resource="http://rs.tdwg.org/ac/terms/subtypeLiteral"/>
        <rdfs:comment xml:lang="en">Type, nature, or classification of a Media file dataset, which may include one or more specific files. This is the general or high-level type of all file data, it is not the file type of any specific file. Most Media Types encompass a variety of different specific file types. Values must be from the Media Type controlled vocabulary (https://www.morphosource.org/terms/morphosource#MediaType).</rdfs:comment>
        <rdfs:label xml:lang="en">Media Type</rdfs:label>
        <skos:example xml:lang="en">`Mesh`,`Image`,`CTImageSeries`</skos:example>
    </owl:ObjectProperty>
    


    <!-- https://www.morphosource.org/terms/morphosource#modality3D -->


    <owl:ObjectProperty rdf:about="https://www.morphosource.org/terms/morphosource#modality3D">
        <rdfs:domain rdf:resource="https://www.morphosource.org/terms/morphosource#Device"/>
        <rdfs:range rdf:resource="https://www.morphosource.org/terms/morphosource#ImageModalityType"/>
        <rdfs:comment xml:lang="en">The list of imaging modalities that a device is capable of using when imaging objects. Despite the name, this can include non-3D imaging event modalities. Value must be from Image Modality controlled vocabulary (https://www.morphosource.org/terms/morphosource#ImageModality).</rdfs:comment>
        <rdfs:label xml:lang="en">Modality</rdfs:label>
        <skos:example xml:lang="en">`MicroNanoXRayComputedTomography`, `Photogrammetry`, `Video`</skos:example>
    </owl:ObjectProperty>
    


    <!-- https://www.morphosource.org/terms/morphosource#morphosourceUseAgreementType -->


    <owl:ObjectProperty rdf:about="https://www.morphosource.org/terms/morphosource#morphosourceUseAgreementType">
        <rdfs:domain rdf:resource="https://www.morphosource.org/terms/morphosource#Media"/>
        <rdfs:domain rdf:resource="https://www.morphosource.org/terms/morphosource#Organization"/>
        <rdfs:range rdf:resource="https://www.morphosource.org/terms/morphosource#UseAgreementType"/>
        <rdfs:comment xml:lang="en">Type of MorphoSource use agreement that users must agree to in order to download Media and that is packaged with an associated Media download. Values must be from the Use Agreement Type controlled vocabulary (https://www.morphosource.org/terms/morphosource#UseAgreementType).</rdfs:comment>
        <rdfs:label xml:lang="en">MorphoSource Use Agreement Type</rdfs:label>
        <skos:example xml:lang="en">`Standard`, `Permissive`</skos:example>
    </owl:ObjectProperty>
    


    <!-- https://www.morphosource.org/terms/morphosource#organizationType -->


    <owl:ObjectProperty rdf:about="https://www.morphosource.org/terms/morphosource#organizationType">
        <rdfs:domain rdf:resource="https://www.morphosource.org/terms/morphosource#Organization"/>
        <rdfs:range rdf:resource="https://www.morphosource.org/terms/morphosource#OrganizationType"/>
        <rdfs:comment xml:lang="en">Type of Organization to distinguish between collections managing Physical Objects, scanning facilities, and entities that both operate scanning equipment and manage Physical Objects. Values must be from Organization Type controlled vocabulary (https://www.morphosource.org/terms/morphosource#OrganizationType).</rdfs:comment>
        <rdfs:label xml:lang="en">Organization Type</rdfs:label>
        <skos:example xml:lang="en">`Museum, Department, or Lab Collection`, `Scanning Facility`, `Collection and Scanning Facility`</skos:example>
    </owl:ObjectProperty>
    


    <!-- https://www.morphosource.org/terms/morphosource#owner -->


    <owl:ObjectProperty rdf:about="https://www.morphosource.org/terms/morphosource#owner">
        <rdfs:domain rdf:resource="https://www.morphosource.org/terms/morphosource#FileSet"/>
        <rdfs:domain rdf:resource="https://www.morphosource.org/terms/morphosource#Media"/>
        <rdfs:range rdf:resource="https://www.morphosource.org/terms/morphosource#User"/>
        <rdfs:comment xml:lang="en">The user that has the highest level of management control over a Media or another Work record. For Media, this user is also known as the Data Manager.</rdfs:comment>
        <rdfs:label xml:lang="en">Owner</rdfs:label>
    </owl:ObjectProperty>
    


    <!-- https://www.morphosource.org/terms/morphosource#permits3DUse -->


    <owl:ObjectProperty rdf:about="https://www.morphosource.org/terms/morphosource#permits3DUse">
        <rdfs:domain rdf:resource="https://www.morphosource.org/terms/morphosource#Media"/>
        <rdfs:domain rdf:resource="https://www.morphosource.org/terms/morphosource#Organization"/>
        <rdfs:range rdf:resource="https://www.morphosource.org/terms/morphosource#3DPrintingPermission"/>
        <rdfs:comment xml:lang="en">Whether Media may be 3D printed freely, may be 3D printed in limited ways, or if 3D printing is prohibited. Values must be from the 3D Printing Permission controlled vocabulary (https://www.morphosource.org/terms/morphosource#3DPrintingPermission).</rdfs:comment>
        <rdfs:label xml:lang="en">Permits 3D Use</rdfs:label>
        <skos:example xml:lang="en">`3DPrintingPermitted`, `3DPrintingLimited`, `3DPrintingProhibited`</skos:example>
    </owl:ObjectProperty>
    


    <!-- https://www.morphosource.org/terms/morphosource#permitsCommercialUse -->


    <owl:ObjectProperty rdf:about="https://www.morphosource.org/terms/morphosource#permitsCommercialUse">
        <rdfs:domain rdf:resource="https://www.morphosource.org/terms/morphosource#Media"/>
        <rdfs:domain rdf:resource="https://www.morphosource.org/terms/morphosource#Organization"/>
        <rdfs:range rdf:resource="https://www.morphosource.org/terms/morphosource#CommercialUsePermission"/>
        <rdfs:comment xml:lang="en">Whether commercial use of Media is permitted. Values must be from the Commercial Use Permission controlled vocabulary (https://www.morphosource.org/terms/morphosource#CommercialUsePermission).</rdfs:comment>
        <rdfs:label xml:lang="en">Permits Commercial Use</rdfs:label>
        <skos:example xml:lang="en">`CommercialUseNotPermitted`, `CommercialUsePermitted`</skos:example>
    </owl:ObjectProperty>
    


    <!-- https://www.morphosource.org/terms/morphosource#pixelSpacingCalibration -->


    <owl:ObjectProperty rdf:about="https://www.morphosource.org/terms/morphosource#pixelSpacingCalibration">
        <rdfs:subPropertyOf rdf:resource="http://purl.org/healthcarevocab/v1#PixelSpacingCalibrationType"/>
        <rdfs:domain rdf:resource="https://www.morphosource.org/terms/morphosource#CTImageSeriesImagingEvent"/>
        <rdfs:range rdf:resource="https://www.morphosource.org/terms/morphosource#PixelSpacingCalibrationType"/>
        <terms:isVersionOf rdf:resource="http://purl.org/healthcarevocab/v1#PixelSpacingCalibrationType"/>
        <rdfs:comment xml:lang="en">The type of correction for the effect of geometric magnification or calibration against an object of known size, if any. Value must be from Pixel Spacing Calibration Type controlled vocabulary (https://www.morphosource.org/terms/morphosource#PixelSpacingCalibrationType).</rdfs:comment>
        <rdfs:label xml:lang="en">Pixel Spacing Calibration</rdfs:label>
        <skos:example xml:lang="en">`Geometry`, `Fiducial`</skos:example>
    </owl:ObjectProperty>
    


    <!-- https://www.morphosource.org/terms/morphosource#processingActivityType -->


    <owl:ObjectProperty rdf:about="https://www.morphosource.org/terms/morphosource#processingActivityType">
        <rdfs:domain rdf:resource="https://www.morphosource.org/terms/morphosource#ProcessingEvent"/>
        <rdfs:range rdf:resource="https://www.morphosource.org/terms/morphosource#ProcessingActivityType"/>
        <rdfs:comment xml:lang="en">Type of a specific discrete processing activity. Value must be from Processing Activity Type controlled vocabulary (https://www.morphosource.org/terms/morphosource#ProcessingActivityType).</rdfs:comment>
        <rdfs:label xml:lang="en">Processing Activity Type</rdfs:label>
        <skos:example xml:lang="en">`AlignParts`, `Patch`, `Reconstruction`</skos:example>
    </owl:ObjectProperty>
    


    <!-- https://www.morphosource.org/terms/morphosource#requiredArchivalOfPublishedDerivatives -->


    <owl:ObjectProperty rdf:about="https://www.morphosource.org/terms/morphosource#requiredArchivalOfPublishedDerivatives">
        <rdfs:domain rdf:resource="https://www.morphosource.org/terms/morphosource#Media"/>
        <rdfs:domain rdf:resource="https://www.morphosource.org/terms/morphosource#Organization"/>
        <rdfs:range rdf:resource="https://www.morphosource.org/terms/morphosource#DerivativeRearchivalStatement"/>
        <rdfs:comment xml:lang="en">Whether and how future derivatives created from Media must be rearchived on a public-facing digital repository such as MorphoSource. Values may include mandatory requirements or optional suggestions. Values must be from Derivative Rearchival Statement controlled vocabulary (https://www.morphosource.org/terms/morphosource#DerivativeRearchivalStatement).</rdfs:comment>
        <rdfs:label xml:lang="en">Required Archival Of Published Derivatives</rdfs:label>
        <skos:example xml:lang="en">`OnMorphoSource`, `OnAnyRepository`, `EncouragedButNotRequired`</skos:example>
    </owl:ObjectProperty>
    


    <!-- https://www.morphosource.org/terms/morphosource#rightsStatement -->


    <owl:ObjectProperty rdf:about="https://www.morphosource.org/terms/morphosource#rightsStatement">
        <rdfs:subPropertyOf rdf:resource="http://www.europeana.eu/schemas/edm/rights"/>
        <rdfs:domain rdf:resource="https://www.morphosource.org/terms/morphosource#Media"/>
        <rdfs:domain rdf:resource="https://www.morphosource.org/terms/morphosource#Organization"/>
        <rdfs:range rdf:resource="http://purl.org/dc/terms/RightsStatement"/>
        <terms:isVersionOf rdf:resource="http://www.europeana.eu/schemas/edm/rights"/>
        <rdfs:comment xml:lang="en">Standardized rights statement used to communicate the copyright and/or reuse status of digital objects. Values must be from the Rights Statement controlled vocabulary (https://rightsstatements.org).</rdfs:comment>
        <rdfs:label xml:lang="en">Rights Statement</rdfs:label>
        <skos:example xml:lang="en">`http://rightsstatements.org/vocab/NoC-NC/1.0/`, `http://rightsstatements.org/vocab/UND/1.0/`, `http://rightsstatements.org/vocab/InC/1.0/`</skos:example>
    </owl:ObjectProperty>
    


    <!-- https://www.morphosource.org/terms/morphosource#seriesType -->


    <owl:ObjectProperty rdf:about="https://www.morphosource.org/terms/morphosource#seriesType">
        <rdfs:domain rdf:resource="https://www.morphosource.org/terms/morphosource#Media"/>
        <rdfs:range rdf:resource="https://www.morphosource.org/terms/morphosource#CTImageSeriesType"/>
        <rdfs:comment xml:lang="en">Broad type or kind of CT image series, distiguishing between initial X-Ray projections and other derived series forms. Values must be from the CT Image Series Type controlled vocabulary (https://www.morphosource.org/terms/morphosource#CTImageSeriesType).</rdfs:comment>
        <rdfs:label xml:lang="en">Series Type</rdfs:label>
        <skos:example xml:lang="en">`Projections`, `Sinograms`, `Reconstructed image stack`</skos:example>
    </owl:ObjectProperty>
    


    <!-- https://www.morphosource.org/terms/morphosource#side -->


    <owl:ObjectProperty rdf:about="https://www.morphosource.org/terms/morphosource#side">
        <rdfs:subPropertyOf rdf:resource="http://rs.tdwg.org/ac/terms/comments"/>
        <rdfs:domain rdf:resource="https://www.morphosource.org/terms/morphosource#Media"/>
        <rdfs:range rdf:resource="https://www.morphosource.org/terms/morphosource#Side"/>
        <terms:isVersionOf rdf:resource="http://rs.tdwg.org/ac/terms/comments"/>
        <rdfs:comment xml:lang="en">The side of a larger object on which is located a represented component part, if media represents a component part of a larger whole object. Values must be from the Side controlled vocabulary (https://www.morphosource.org/terms/morphosource#Side). Values are somewhat oriented toward objects with bilateral symmetry, but may in some cases be applied for objects with other kinds of symmetry.</rdfs:comment>
        <rdfs:label xml:lang="en">Side</rdfs:label>
        <skos:example xml:lang="en">`Left`, `Midline`, `Not Applicable`</skos:example>
    </owl:ObjectProperty>
    


    <!-- https://www.morphosource.org/terms/morphosource#slideType -->


    <owl:ObjectProperty rdf:about="https://www.morphosource.org/terms/morphosource#slideType">
        <rdfs:domain rdf:resource="https://www.morphosource.org/terms/morphosource#SequentialSectionImagingEvent"/>
        <rdfs:range rdf:resource="https://www.morphosource.org/terms/morphosource#SlideType"/>
        <rdfs:comment xml:lang="en">Type of sequential section slide imaged. Value must be &quot;Histological&quot; or &quot;Other&quot;.</rdfs:comment>
        <rdfs:label xml:lang="en">Slide Type</rdfs:label>
        <skos:example xml:lang="en">`Histological`, `Other`</skos:example>
    </owl:ObjectProperty>
    


    <!-- https://www.morphosource.org/terms/morphosource#targetType -->


    <owl:ObjectProperty rdf:about="https://www.morphosource.org/terms/morphosource#targetType">
        <rdfs:domain rdf:resource="https://www.morphosource.org/terms/morphosource#CTImageSeriesImagingEvent"/>
        <rdfs:range rdf:resource="https://www.morphosource.org/terms/morphosource#XRayTargetType"/>
        <rdfs:comment xml:lang="en">Type of the anode of the X-Ray source. Value must be from the X-Ray Target Type controlled vocabulary (https://www.morphosource.org/terms/morphosource#XRayTargetType).</rdfs:comment>
        <rdfs:label xml:lang="en">Target Type</rdfs:label>
        <skos:example xml:lang="en">`Reflection`,`Transmission`</skos:example>
    </owl:ObjectProperty>
    


    <!-- https://www.morphosource.org/terms/morphosource#unit -->


    <owl:ObjectProperty rdf:about="https://www.morphosource.org/terms/morphosource#unit">
        <rdfs:domain rdf:resource="https://www.morphosource.org/terms/morphosource#Media"/>
        <rdfs:range rdf:resource="https://www.morphosource.org/terms/morphosource#LengthMeasurementUnit"/>
        <rdfs:comment xml:lang="en">Length measurement unit. For Mesh Media, this is the length unit associated with the 3D coordinate space of the mesh. For CTImageSeries Media, this is the length unit for X/Y/Z pixel spacing. Values must be from the Length Measurement Unit controlled vocabulary (https://www.morphosource.org/terms/morphosource#LengthMeasurementUnit).</rdfs:comment>
        <rdfs:label xml:lang="en">Unit</rdfs:label>
        <skos:example xml:lang="en">`Mm`, `Um`, `M`</skos:example>
    </owl:ObjectProperty>
    


    <!-- https://www.morphosource.org/terms/morphosource#visibility -->


    <owl:ObjectProperty rdf:about="https://www.morphosource.org/terms/morphosource#visibility">
        <rdfs:subPropertyOf rdf:resource="https://www.morphosource.org/terms/morphosource#filesetAccessibility"/>
        <rdfs:domain rdf:resource="https://www.morphosource.org/terms/morphosource#Media"/>
        <rdfs:range rdf:resource="https://www.morphosource.org/terms/morphosource#PublicationStatus"/>
        <rdfs:comment xml:lang="en">Publication status, denoting whether or not Media may be found in public search and whether or not Media files may be downloaded. Values must be from Publication Status controlled vocabulary (https://www.morphosource.org/terms/morphosource#PublicationStatus).</rdfs:comment>
        <rdfs:label xml:lang="en">Visibility</rdfs:label>
        <skos:example xml:lang="en">`Open`, `Restricted`, `Private`</skos:example>
    </owl:ObjectProperty>
    


    <!-- 
    ///////////////////////////////////////////////////////////////////////////////////////
    //
    // Data properties
    //
    ///////////////////////////////////////////////////////////////////////////////////////
     -->


    


    <!-- http://ns.adobe.com/photoshop/1.0/Credit -->


    <owl:DatatypeProperty rdf:about="http://ns.adobe.com/photoshop/1.0/Credit">
        <rdfs:comment xml:lang="en">The credit to person(s) and/or organisation(s) required by the supplier of the item to be used when published. This is a free-text field.</rdfs:comment>
        <rdfs:label xml:lang="en">Credit Line</rdfs:label>
    </owl:DatatypeProperty>
    


    <!-- http://ns.adobe.com/xap/1.0/rights/Owner -->


    <owl:DatatypeProperty rdf:about="http://ns.adobe.com/xap/1.0/rights/Owner">
        <rdfs:comment xml:lang="en">A list of legal owners of the resource.</rdfs:comment>
        <rdfs:label xml:lang="en">Owner</rdfs:label>
    </owl:DatatypeProperty>
    


    <!-- http://ns.adobe.com/xap/1.0/rights/UsageTerms -->


    <owl:DatatypeProperty rdf:about="http://ns.adobe.com/xap/1.0/rights/UsageTerms">
        <rdfs:comment xml:lang="en">A collection of text instructions on how a resource can be legally used, given in a variety of languages.</rdfs:comment>
        <rdfs:label xml:lang="en">Usage Rights</rdfs:label>
    </owl:DatatypeProperty>
    


    <!-- http://purl.org/dc/dcmitype/Software -->


    <owl:DatatypeProperty rdf:about="http://purl.org/dc/dcmitype/Software">
        <rdfs:domain rdf:resource="https://www.morphosource.org/terms/morphosource#ProcessingEvent"/>
        <dcam:memberOf rdf:resource="http://purl.org/dc/terms/DCMIType"/>
        <terms:description xml:lang="en">Examples include a C source file, MS-Windows .exe executable, or Perl script.</terms:description>
        <terms:issued rdf:datatype="http://www.w3.org/2001/XMLSchema#date">2000-07-11</terms:issued>
        <rdfs:comment xml:lang="en">A computer program in source or compiled form.</rdfs:comment>
        <rdfs:isDefinedBy rdf:resource="http://purl.org/dc/dcmitype/"/>
        <rdfs:label xml:lang="en">Software</rdfs:label>
    </owl:DatatypeProperty>
    


    <!-- http://purl.org/dc/elements/1.1/creator -->


    <owl:DatatypeProperty rdf:about="http://purl.org/dc/elements/1.1/creator">
        <rdfs:domain rdf:resource="https://www.morphosource.org/terms/morphosource#Device"/>
        <rdfs:domain rdf:resource="https://www.morphosource.org/terms/morphosource#ImagingEvent"/>
        <rdfs:domain rdf:resource="https://www.morphosource.org/terms/morphosource#Media"/>
        <rdfs:domain rdf:resource="https://www.morphosource.org/terms/morphosource#PhysicalObject"/>
        <rdfs:domain rdf:resource="https://www.morphosource.org/terms/morphosource#ProcessingEvent"/>
        <rdfs:range rdf:resource="http://www.w3.org/2001/XMLSchema#string"/>
        <terms:description xml:lang="en">Examples of a Creator include a person, an organization, or a service. Typically, the name of a Creator should be used to indicate the entity.</terms:description>
        <terms:issued rdf:datatype="http://www.w3.org/2001/XMLSchema#date">1999-07-02</terms:issued>
        <rdfs:comment xml:lang="en">An entity primarily responsible for making the resource.</rdfs:comment>
        <rdfs:isDefinedBy rdf:resource="http://purl.org/dc/elements/1.1/"/>
        <rdfs:label xml:lang="en">Creator</rdfs:label>
        <skos:note xml:lang="en">A [second property](/specifications/dublin-core/dcmi-terms/#http://purl.org/dc/terms/creator) with the same name as this property has been declared in the [dcterms: namespace](http://purl.org/dc/terms/).  See the Introduction to the document [DCMI Metadata Terms](/specifications/dublin-core/dcmi-terms/) for an explanation.</skos:note>
    </owl:DatatypeProperty>
    


    <!-- http://purl.org/dc/elements/1.1/description -->


    <owl:DatatypeProperty rdf:about="http://purl.org/dc/elements/1.1/description">
        <rdfs:domain rdf:resource="https://www.morphosource.org/terms/morphosource#Device"/>
        <rdfs:domain rdf:resource="https://www.morphosource.org/terms/morphosource#ImagingEvent"/>
        <rdfs:domain rdf:resource="https://www.morphosource.org/terms/morphosource#Media"/>
        <rdfs:domain rdf:resource="https://www.morphosource.org/terms/morphosource#Organization"/>
        <rdfs:domain rdf:resource="https://www.morphosource.org/terms/morphosource#PhysicalObject"/>
        <rdfs:domain rdf:resource="https://www.morphosource.org/terms/morphosource#ProcessingEvent"/>
        <terms:description xml:lang="en">Description may include but is not limited to: an abstract, a table of contents, a graphical representation, or a free-text account of the resource.</terms:description>
        <terms:issued rdf:datatype="http://www.w3.org/2001/XMLSchema#date">1999-07-02</terms:issued>
        <rdfs:comment xml:lang="en">An account of the resource.</rdfs:comment>
        <rdfs:isDefinedBy rdf:resource="http://purl.org/dc/elements/1.1/"/>
        <rdfs:label xml:lang="en">Description</rdfs:label>
        <skos:note xml:lang="en">A [second property](/specifications/dublin-core/dcmi-terms/#http://purl.org/dc/terms/description) with the same name as this property has been declared in the [dcterms: namespace](http://purl.org/dc/terms/).  See the Introduction to the document [DCMI Metadata Terms](/specifications/dublin-core/dcmi-terms/) for an explanation.</skos:note>
    </owl:DatatypeProperty>
    


    <!-- http://purl.org/dc/elements/1.1/publisher -->


    <owl:DatatypeProperty rdf:about="http://purl.org/dc/elements/1.1/publisher">
        <rdfs:domain rdf:resource="https://www.morphosource.org/terms/morphosource#Media"/>
        <rdfs:range rdf:resource="http://www.w3.org/2001/XMLSchema#string"/>
        <terms:description xml:lang="en">Examples of a Publisher include a person, an organization, or a service. Typically, the name of a Publisher should be used to indicate the entity.</terms:description>
        <terms:issued rdf:datatype="http://www.w3.org/2001/XMLSchema#date">1999-07-02</terms:issued>
        <rdfs:comment xml:lang="en">An entity responsible for making the resource available.</rdfs:comment>
        <rdfs:isDefinedBy rdf:resource="http://purl.org/dc/elements/1.1/"/>
        <rdfs:label xml:lang="en">Publisher</rdfs:label>
        <skos:note xml:lang="en">A [second property](/specifications/dublin-core/dcmi-terms/#http://purl.org/dc/terms/publisher) with the same name as this property has been declared in the [dcterms: namespace](http://purl.org/dc/terms/).  See the Introduction to the document [DCMI Metadata Terms](/specifications/dublin-core/dcmi-terms/) for an explanation.</skos:note>
    </owl:DatatypeProperty>
    


    <!-- http://purl.org/dc/terms/available -->


    <owl:DatatypeProperty rdf:about="http://purl.org/dc/terms/available">
        <rdfs:domain rdf:resource="https://www.morphosource.org/terms/morphosource#Media"/>
        <rdfs:range rdf:resource="http://www.w3.org/2001/XMLSchema#dateTime"/>
        <terms:description xml:lang="en">Recommended practice is to describe the date, date/time, or period of time as recommended for the property Date, of which this is a subproperty.</terms:description>
        <terms:issued rdf:datatype="http://www.w3.org/2001/XMLSchema#date">2000-07-11</terms:issued>
        <rdfs:comment xml:lang="en">Date that the resource became or will become available.</rdfs:comment>
        <rdfs:isDefinedBy rdf:resource="http://purl.org/dc/terms/"/>
        <rdfs:label xml:lang="en">Date Available</rdfs:label>
    </owl:DatatypeProperty>
    


    <!-- http://purl.org/dc/terms/created -->


    <owl:DatatypeProperty rdf:about="http://purl.org/dc/terms/created">
        <rdfs:domain rdf:resource="https://www.morphosource.org/terms/morphosource#ImagingEvent"/>
        <rdfs:domain rdf:resource="https://www.morphosource.org/terms/morphosource#Media"/>
        <rdfs:domain rdf:resource="https://www.morphosource.org/terms/morphosource#ProcessingEvent"/>
        <rdfs:range rdf:resource="http://www.w3.org/2001/XMLSchema#dateTime"/>
        <terms:description xml:lang="en">Recommended practice is to describe the date, date/time, or period of time as recommended for the property Date, of which this is a subproperty.</terms:description>
        <terms:issued rdf:datatype="http://www.w3.org/2001/XMLSchema#date">2000-07-11</terms:issued>
        <rdfs:comment xml:lang="en">Date of creation of the resource.</rdfs:comment>
        <rdfs:isDefinedBy rdf:resource="http://purl.org/dc/terms/"/>
        <rdfs:label xml:lang="en">Date Created</rdfs:label>
    </owl:DatatypeProperty>
    


    <!-- http://purl.org/dc/terms/dateSubmitted -->


    <owl:DatatypeProperty rdf:about="http://purl.org/dc/terms/dateSubmitted">
        <terms:description xml:lang="en">Recommended practice is to describe the date, date/time, or period of time as recommended for the property Date, of which this is a subproperty.  Examples of resources to which a &apos;Date Submitted&apos; may be relevant include a thesis (submitted to a university department) or an article (submitted to a journal).</terms:description>
        <rdfs:comment xml:lang="en">Date of submission of the resource.</rdfs:comment>
        <rdfs:isDefinedBy rdf:resource="http://purl.org/dc/terms/"/>
        <rdfs:label xml:lang="en">Date Submitted</rdfs:label>
    </owl:DatatypeProperty>
    


    <!-- http://purl.org/dc/terms/format -->


    <owl:DatatypeProperty rdf:about="http://purl.org/dc/terms/format">
        <dcam:rangeIncludes rdf:resource="http://purl.org/dc/terms/Extent"/>
        <dcam:rangeIncludes rdf:resource="http://purl.org/dc/terms/MediaType"/>
        <terms:description xml:lang="en">Recommended practice is to use a controlled vocabulary where available. For example, for file formats one could use the list of Internet Media Types [[MIME](https://www.iana.org/assignments/media-types/media-types.xhtml)].  Examples of dimensions include size and duration.</terms:description>
        <terms:issued rdf:datatype="http://www.w3.org/2001/XMLSchema#date">2008-01-14</terms:issued>
        <rdfs:comment xml:lang="en">The file format, physical medium, or dimensions of the resource.</rdfs:comment>
        <rdfs:isDefinedBy rdf:resource="http://purl.org/dc/terms/"/>
        <rdfs:label xml:lang="en">Format</rdfs:label>
    </owl:DatatypeProperty>
    


    <!-- http://purl.org/dc/terms/identifier -->


    <owl:DatatypeProperty rdf:about="http://purl.org/dc/terms/identifier">
        <rdfs:domain rdf:resource="https://www.morphosource.org/terms/morphosource#Media"/>
        <rdfs:domain rdf:resource="https://www.morphosource.org/terms/morphosource#PhysicalObject"/>
        <rdfs:range rdf:resource="http://www.w3.org/2001/XMLSchema#string"/>
        <terms:description xml:lang="en">Recommended practice is to identify the resource by means of a string conforming to an identification system. Examples include International Standard Book Number (ISBN), Digital Object Identifier (DOI), and Uniform Resource Name (URN).  Persistent identifiers should be provided as HTTP URIs.</terms:description>
        <terms:issued rdf:datatype="http://www.w3.org/2001/XMLSchema#date">2008-01-14</terms:issued>
        <rdfs:comment xml:lang="en">An unambiguous reference to the resource within a given context.</rdfs:comment>
        <rdfs:isDefinedBy rdf:resource="http://purl.org/dc/terms/"/>
        <rdfs:label xml:lang="en">Identifier</rdfs:label>
    </owl:DatatypeProperty>
    


    <!-- http://purl.org/dc/terms/medium -->


    <owl:DatatypeProperty rdf:about="http://purl.org/dc/terms/medium">
        <dcam:domainIncludes rdf:resource="http://purl.org/dc/terms/PhysicalResource"/>
        <dcam:rangeIncludes rdf:resource="http://purl.org/dc/terms/PhysicalMedium"/>
        <terms:issued rdf:datatype="http://www.w3.org/2001/XMLSchema#date">2000-07-11</terms:issued>
        <rdfs:comment xml:lang="en">The material or physical carrier of the resource.</rdfs:comment>
        <rdfs:isDefinedBy rdf:resource="http://purl.org/dc/terms/"/>
        <rdfs:label xml:lang="en">Medium</rdfs:label>
    </owl:DatatypeProperty>
    


    <!-- http://purl.org/dc/terms/modified -->


    <owl:DatatypeProperty rdf:about="http://purl.org/dc/terms/modified">
        <owl:equivalentProperty rdf:resource="https://www.morphosource.org/terms/morphosource#dateModified"/>
        <terms:description xml:lang="en">Recommended practice is to describe the date, date/time, or period of time as recommended for the property Date, of which this is a subproperty.</terms:description>
        <terms:issued rdf:datatype="http://www.w3.org/2001/XMLSchema#date">2000-07-11</terms:issued>
        <rdfs:comment xml:lang="en">Date on which the resource was changed.</rdfs:comment>
        <rdfs:isDefinedBy rdf:resource="http://purl.org/dc/terms/"/>
        <rdfs:label xml:lang="en">Date Modified</rdfs:label>
    </owl:DatatypeProperty>
    


    <!-- http://purl.org/dc/terms/provenance -->


    <owl:DatatypeProperty rdf:about="http://purl.org/dc/terms/provenance">
        <dcam:rangeIncludes rdf:resource="http://purl.org/dc/terms/ProvenanceStatement"/>
        <terms:description xml:lang="en">The statement may include a description of any changes successive custodians made to the resource.</terms:description>
        <terms:issued rdf:datatype="http://www.w3.org/2001/XMLSchema#date">2004-09-20</terms:issued>
        <rdfs:comment xml:lang="en">A statement of any changes in ownership and custody of the resource since its creation that are significant for its authenticity, integrity, and interpretation.</rdfs:comment>
        <rdfs:isDefinedBy rdf:resource="http://purl.org/dc/terms/"/>
        <rdfs:label xml:lang="en">Provenance</rdfs:label>
    </owl:DatatypeProperty>
    


    <!-- http://purl.org/dc/terms/title -->


    <owl:DatatypeProperty rdf:about="http://purl.org/dc/terms/title">
        <rdfs:domain rdf:resource="https://www.morphosource.org/terms/morphosource#Device"/>
        <rdfs:domain rdf:resource="https://www.morphosource.org/terms/morphosource#FileSet"/>
        <rdfs:domain rdf:resource="https://www.morphosource.org/terms/morphosource#ImagingEvent"/>
        <rdfs:domain rdf:resource="https://www.morphosource.org/terms/morphosource#Media"/>
        <rdfs:domain rdf:resource="https://www.morphosource.org/terms/morphosource#Organization"/>
        <rdfs:domain rdf:resource="https://www.morphosource.org/terms/morphosource#PhysicalObject"/>
        <rdfs:domain rdf:resource="https://www.morphosource.org/terms/morphosource#ProcessingEvent"/>
        <rdfs:range rdf:resource="http://www.w3.org/2001/XMLSchema#string"/>
        <rdfs:comment xml:lang="en">A name given to the resource.</rdfs:comment>
        <rdfs:isDefinedBy rdf:resource="http://purl.org/dc/terms/"/>
        <rdfs:label xml:lang="en">Title</rdfs:label>
    </owl:DatatypeProperty>
    


    <!-- http://purl.org/healthcarevocab/v1#AccessionNumber -->


    <owl:DatatypeProperty rdf:about="http://purl.org/healthcarevocab/v1#AccessionNumber">
        <rdfs:domain rdf:resource="https://www.morphosource.org/terms/morphosource#FileSet"/>
        <rdfs:range rdf:resource="http://www.w3.org/2001/XMLSchema#string"/>
        <rdfs:comment xml:lang="en">A RIS generated number that identifies the order for the Study.</rdfs:comment>
        <rdfs:label xml:lang="en">Accession Number</rdfs:label>
    </owl:DatatypeProperty>
    


    <!-- http://purl.org/healthcarevocab/v1#AnodeTargetMaterial -->


    <owl:DatatypeProperty rdf:about="http://purl.org/healthcarevocab/v1#AnodeTargetMaterial">
        <rdfs:domain rdf:resource="https://www.morphosource.org/terms/morphosource#FileSet"/>
        <rdfs:comment xml:lang="en">The primary material in the anode of the X-Ray source.</rdfs:comment>
        <rdfs:label xml:lang="en">Anode Target Material</rdfs:label>
        <skos:example xml:lang="en">`tungsten`, `molybdenum`, `copper`</skos:example>
    </owl:DatatypeProperty>
    


    <!-- http://purl.org/healthcarevocab/v1#BitsAllocated -->


    <owl:DatatypeProperty rdf:about="http://purl.org/healthcarevocab/v1#BitsAllocated">
        <rdfs:domain rdf:resource="https://www.morphosource.org/terms/morphosource#FileSet"/>
        <rdfs:range rdf:resource="http://www.w3.org/2001/XMLSchema#int"/>
        <rdfs:comment xml:lang="en">Number of bits allocated for each pixel sample. Each sample shall have the same number of bits allocated. Bits Allocated (0028,0100) shall be either 1, or a multiple of 8. See PS3.5 for further explanation.</rdfs:comment>
        <rdfs:label xml:lang="en">Bits Allocated</rdfs:label>
    </owl:DatatypeProperty>
    


    <!-- http://purl.org/healthcarevocab/v1#BitsStored -->


    <owl:DatatypeProperty rdf:about="http://purl.org/healthcarevocab/v1#BitsStored">
        <rdfs:domain rdf:resource="https://www.morphosource.org/terms/morphosource#FileSet"/>
        <rdfs:range rdf:resource="http://www.w3.org/2001/XMLSchema#int"/>
        <rdfs:comment xml:lang="en">Number of bits stored for each pixel sample. Each sample shall have the same number of bits stored. See PS3.5 for further explanation.</rdfs:comment>
        <rdfs:label xml:lang="en">Bits Stored</rdfs:label>
    </owl:DatatypeProperty>
    


    <!-- http://purl.org/healthcarevocab/v1#Columns -->


    <owl:DatatypeProperty rdf:about="http://purl.org/healthcarevocab/v1#Columns">
        <rdfs:domain rdf:resource="https://www.morphosource.org/terms/morphosource#FileSet"/>
        <rdfs:range rdf:resource="http://www.w3.org/2001/XMLSchema#int"/>
        <rdfs:comment xml:lang="en">Number of columns in the image.

Shall be an exact multiple of the horizontal downsampling factor if any of the samples (planes) are encoded downsampled in the horizontal direction for pixel data encoded in a Native (uncompressed) format. E.g., required to be an even value for a Photometric Interpretation (0028,0004) of YBR_FULL_422.</rdfs:comment>
        <rdfs:label xml:lang="en">Columns</rdfs:label>
    </owl:DatatypeProperty>
    


    <!-- http://purl.org/healthcarevocab/v1#ContainerDescription -->


    <owl:DatatypeProperty rdf:about="http://purl.org/healthcarevocab/v1#ContainerDescription">
        <rdfs:domain rdf:resource="https://www.morphosource.org/terms/morphosource#FileSet"/>
        <rdfs:comment xml:lang="en">Description of the container.</rdfs:comment>
        <rdfs:label xml:lang="en">Container Description</rdfs:label>
    </owl:DatatypeProperty>
    


    <!-- http://purl.org/healthcarevocab/v1#ContentDate -->


    <owl:DatatypeProperty rdf:about="http://purl.org/healthcarevocab/v1#ContentDate">
        <rdfs:domain rdf:resource="https://www.morphosource.org/terms/morphosource#FileSet"/>
        <rdfs:range rdf:resource="http://www.w3.org/2001/XMLSchema#date"/>
        <rdfs:comment xml:lang="en">The date the image pixel data creation started.

Required if image is part of a Series in which the images are temporally related. May be present otherwise.</rdfs:comment>
        <rdfs:label xml:lang="en">Content Date</rdfs:label>
    </owl:DatatypeProperty>
    


    <!-- http://purl.org/healthcarevocab/v1#ContentTime -->


    <owl:DatatypeProperty rdf:about="http://purl.org/healthcarevocab/v1#ContentTime">
        <rdfs:domain rdf:resource="https://www.morphosource.org/terms/morphosource#FileSet"/>
        <rdfs:range rdf:resource="http://www.w3.org/2001/XMLSchema#dateTime"/>
        <rdfs:comment xml:lang="en">The time the image pixel data creation started.

Required if image is part of a Series in which the images are temporally related. May be present otherwise.</rdfs:comment>
        <rdfs:label xml:lang="en">Content Time</rdfs:label>
    </owl:DatatypeProperty>
    


    <!-- http://purl.org/healthcarevocab/v1#ContrastFrameAveraging -->


    <owl:DatatypeProperty rdf:about="http://purl.org/healthcarevocab/v1#ContrastFrameAveraging">
        <rdfs:domain rdf:resource="https://www.morphosource.org/terms/morphosource#FileSet"/>
        <rdfs:range rdf:resource="http://www.w3.org/2001/XMLSchema#int"/>
        <rdfs:comment xml:lang="en">Specifies the number of contrast frames to average together before performing the mask operation. If the Attribute is missing, no averaging is performed.</rdfs:comment>
        <rdfs:label xml:lang="en">Contrast Frame Averaging</rdfs:label>
    </owl:DatatypeProperty>
    


    <!-- http://purl.org/healthcarevocab/v1#DistanceSourceToDetector -->


    <owl:DatatypeProperty rdf:about="http://purl.org/healthcarevocab/v1#DistanceSourceToDetector">
        <rdfs:domain rdf:resource="https://www.morphosource.org/terms/morphosource#FileSet"/>
        <rdfs:range rdf:resource="http://www.w3.org/2001/XMLSchema#float"/>
        <rdfs:comment xml:lang="en">Distance in mm from source to detector center.</rdfs:comment>
        <rdfs:label xml:lang="en">Distance From Source To Detector</rdfs:label>
    </owl:DatatypeProperty>
    


    <!-- http://purl.org/healthcarevocab/v1#DistanceSourceToPatient -->


    <owl:DatatypeProperty rdf:about="http://purl.org/healthcarevocab/v1#DistanceSourceToPatient">
        <rdfs:domain rdf:resource="https://www.morphosource.org/terms/morphosource#FileSet"/>
        <rdfs:range rdf:resource="http://www.w3.org/2001/XMLSchema#float"/>
        <rdfs:comment xml:lang="en">Distance in mm from source to isocenter (center of field of view).</rdfs:comment>
        <rdfs:label xml:lang="en">Distance From Source To Patient</rdfs:label>
    </owl:DatatypeProperty>
    


    <!-- http://purl.org/healthcarevocab/v1#ExposureTime -->


    <owl:DatatypeProperty rdf:about="http://purl.org/healthcarevocab/v1#ExposureTime">
        <rdfs:domain rdf:resource="https://www.morphosource.org/terms/morphosource#CTImageSeriesImagingEvent"/>
        <rdfs:domain rdf:resource="https://www.morphosource.org/terms/morphosource#FileSet"/>
        <rdfs:range rdf:resource="http://www.w3.org/2001/XMLSchema#float"/>
        <rdfs:comment xml:lang="en">Time of X-Ray exposure in msec.

If Acquisition Type (0018,9302) equals SPIRAL, the value of this Attribute shall be Revolution Time (0018,9305) divided by the Spiral Pitch Factor (0018,9311). See Section C.8.15.3.8.1 and Section C.8.15.3.2.1.

Shall not be present if this Attribute is present in Multi-energy CT Acquisition Sequence (0018,9362) and the value of this Attribute is not the same in all Items of the Multi-energy CT Acquisition Sequence (0018,9362).</rdfs:comment>
        <rdfs:label xml:lang="en">Exposure Time</rdfs:label>
    </owl:DatatypeProperty>
    


    <!-- http://purl.org/healthcarevocab/v1#GeneratorID -->


    <owl:DatatypeProperty rdf:about="http://purl.org/healthcarevocab/v1#GeneratorID">
        <rdfs:domain rdf:resource="https://www.morphosource.org/terms/morphosource#FileSet"/>
        <rdfs:range rdf:resource="http://www.w3.org/2001/XMLSchema#string"/>
        <rdfs:comment xml:lang="en">Identifier of the generator.</rdfs:comment>
        <rdfs:label xml:lang="en">Generator ID</rdfs:label>
    </owl:DatatypeProperty>
    


    <!-- http://purl.org/healthcarevocab/v1#GeneratorPower -->


    <owl:DatatypeProperty rdf:about="http://purl.org/healthcarevocab/v1#GeneratorPower">
        <rdfs:domain rdf:resource="https://www.morphosource.org/terms/morphosource#FileSet"/>
        <rdfs:range rdf:resource="http://www.w3.org/2001/XMLSchema#float"/>
        <rdfs:comment xml:lang="en">Power in kW to the X-Ray generator.

Shall not be present if this Attribute is present in Multi-energy CT Acquisition Sequence (0018,9362) and the value of this Attribute is not the same in all Items of the Multi-energy CT Acquisition Sequence (0018,9362).</rdfs:comment>
        <rdfs:label xml:lang="en">Generator Power</rdfs:label>
    </owl:DatatypeProperty>
    


    <!-- http://purl.org/healthcarevocab/v1#HighBit -->


    <owl:DatatypeProperty rdf:about="http://purl.org/healthcarevocab/v1#HighBit">
        <rdfs:domain rdf:resource="https://www.morphosource.org/terms/morphosource#FileSet"/>
        <rdfs:range rdf:resource="http://www.w3.org/2001/XMLSchema#int"/>
        <rdfs:comment xml:lang="en">Most significant bit for pixel sample data. Each sample shall have the same high bit. High Bit (0028,0102) shall be one less than Bits Stored (0028,0101). See PS3.5 for further explanation.</rdfs:comment>
        <rdfs:label xml:lang="en">High Bit</rdfs:label>
    </owl:DatatypeProperty>
    


    <!-- http://purl.org/healthcarevocab/v1#ImageOrientationPatient -->


    <owl:DatatypeProperty rdf:about="http://purl.org/healthcarevocab/v1#ImageOrientationPatient">
        <rdfs:domain rdf:resource="https://www.morphosource.org/terms/morphosource#FileSet"/>
        <rdfs:range rdf:resource="http://www.w3.org/2001/XMLSchema#string"/>
        <rdfs:comment xml:lang="en">The direction cosines of the first row and the first column with respect to the patient. See Section C.7.6.2.1.1 for further explanation.</rdfs:comment>
        <rdfs:label xml:lang="en">Image Orientation Patient</rdfs:label>
    </owl:DatatypeProperty>
    


    <!-- http://purl.org/healthcarevocab/v1#ImagePositionPatient -->


    <owl:DatatypeProperty rdf:about="http://purl.org/healthcarevocab/v1#ImagePositionPatient">
        <rdfs:domain rdf:resource="https://www.morphosource.org/terms/morphosource#FileSet"/>
        <rdfs:range rdf:resource="http://www.w3.org/2001/XMLSchema#string"/>
        <rdfs:comment xml:lang="en">Patient position descriptor relative to the equipment. See Section C.7.1.4.1.1.1.

See Section C.7.3.1.1.2 for Defined Terms and further explanation.</rdfs:comment>
        <rdfs:label xml:lang="en">Image Position Patient</rdfs:label>
    </owl:DatatypeProperty>
    


    <!-- http://purl.org/healthcarevocab/v1#ImageType -->


    <owl:DatatypeProperty rdf:about="http://purl.org/healthcarevocab/v1#ImageType">
        <rdfs:domain rdf:resource="https://www.morphosource.org/terms/morphosource#FileSet"/>
        <rdfs:range rdf:resource="http://www.w3.org/2001/XMLSchema#string"/>
        <rdfs:comment xml:lang="en">Image identification characteristics. See Section C.7.6.1.1.2 for Defined Terms and further explanation.</rdfs:comment>
        <rdfs:label xml:lang="en">Image Type</rdfs:label>
    </owl:DatatypeProperty>
    


    <!-- http://purl.org/healthcarevocab/v1#ImagesInAcquisition -->


    <owl:DatatypeProperty rdf:about="http://purl.org/healthcarevocab/v1#ImagesInAcquisition">
        <rdfs:domain rdf:resource="https://www.morphosource.org/terms/morphosource#FileSet"/>
        <rdfs:range rdf:resource="http://www.w3.org/2001/XMLSchema#int"/>
        <rdfs:comment xml:lang="en">Number of images that resulted from this acquisition of data.</rdfs:comment>
        <rdfs:label xml:lang="en">Images in Acquisition</rdfs:label>
    </owl:DatatypeProperty>
    


    <!-- http://purl.org/healthcarevocab/v1#InstanceNumber -->


    <owl:DatatypeProperty rdf:about="http://purl.org/healthcarevocab/v1#InstanceNumber">
        <rdfs:domain rdf:resource="https://www.morphosource.org/terms/morphosource#FileSet"/>
        <rdfs:range rdf:resource="http://www.w3.org/2001/XMLSchema#string"/>
        <rdfs:comment xml:lang="en">A number that identifies this image.</rdfs:comment>
        <rdfs:label xml:lang="en">Instance Number</rdfs:label>
    </owl:DatatypeProperty>
    


    <!-- http://purl.org/healthcarevocab/v1#KVP -->


    <owl:DatatypeProperty rdf:about="http://purl.org/healthcarevocab/v1#KVP">
        <rdfs:domain rdf:resource="https://www.morphosource.org/terms/morphosource#FileSet"/>
        <rdfs:range rdf:resource="http://www.w3.org/2001/XMLSchema#float"/>
        <rdfs:comment xml:lang="en">Peak kilo voltage output of the X-Ray generator used.

Shall be empty if this Attribute is present in Multi-energy CT Acquisition Sequence (0018,9362).</rdfs:comment>
        <rdfs:label xml:lang="en">KVP</rdfs:label>
    </owl:DatatypeProperty>
    


    <!-- http://purl.org/healthcarevocab/v1#PixelRepresentation -->


    <owl:DatatypeProperty rdf:about="http://purl.org/healthcarevocab/v1#PixelRepresentation">
        <rdfs:domain rdf:resource="https://www.morphosource.org/terms/morphosource#FileSet"/>
        <rdfs:range rdf:resource="http://www.w3.org/2001/XMLSchema#string"/>
        <rdfs:comment xml:lang="en">Data representation of the pixel samples. Each sample shall have the same pixel representation.</rdfs:comment>
        <rdfs:label xml:lang="en">Pixel Representation</rdfs:label>
    </owl:DatatypeProperty>
    


    <!-- http://purl.org/healthcarevocab/v1#PixelSpacing -->


    <owl:DatatypeProperty rdf:about="http://purl.org/healthcarevocab/v1#PixelSpacing">
        <rdfs:domain rdf:resource="https://www.morphosource.org/terms/morphosource#FileSet"/>
        <rdfs:range rdf:resource="http://www.w3.org/2001/XMLSchema#string"/>
        <rdfs:comment xml:lang="en">Physical distance in the patient between the center of each pixel, specified by a numeric pair - adjacent row spacing (delimiter) adjacent column spacing in mm. See Section 10.7.1.3 for further explanation.</rdfs:comment>
        <rdfs:label xml:lang="en">Pixel Spacing</rdfs:label>
    </owl:DatatypeProperty>
    


    <!-- http://purl.org/healthcarevocab/v1#RescaleIntercept -->


    <owl:DatatypeProperty rdf:about="http://purl.org/healthcarevocab/v1#RescaleIntercept">
        <rdfs:domain rdf:resource="https://www.morphosource.org/terms/morphosource#FileSet"/>
        <rdfs:range rdf:resource="http://www.w3.org/2001/XMLSchema#string"/>
        <rdfs:comment xml:lang="en">The value b in relationship between stored values (SV) and the output units.

Output units = m*SV+b

If Image Type (0008,0008) Value 1 is ORIGINAL and Value 3 is not LOCALIZER, and Multi-energy CT Acquisition (0018,9361) is either absent or NO, output units shall be Hounsfield Units (HU).</rdfs:comment>
        <rdfs:label xml:lang="en">Rescale Intercept</rdfs:label>
    </owl:DatatypeProperty>
    


    <!-- http://purl.org/healthcarevocab/v1#RescaleSlope -->


    <owl:DatatypeProperty rdf:about="http://purl.org/healthcarevocab/v1#RescaleSlope">
        <rdfs:domain rdf:resource="https://www.morphosource.org/terms/morphosource#FileSet"/>
        <rdfs:range rdf:resource="http://www.w3.org/2001/XMLSchema#float"/>
        <rdfs:comment xml:lang="en">m in the equation specified in Rescale Intercept (0028,1052).</rdfs:comment>
        <rdfs:label xml:lang="en">Rescale Slope</rdfs:label>
    </owl:DatatypeProperty>
    


    <!-- http://purl.org/healthcarevocab/v1#Rows -->


    <owl:DatatypeProperty rdf:about="http://purl.org/healthcarevocab/v1#Rows">
        <rdfs:domain rdf:resource="https://www.morphosource.org/terms/morphosource#FileSet"/>
        <rdfs:range rdf:resource="http://www.w3.org/2001/XMLSchema#int"/>
        <rdfs:comment xml:lang="en">Number of rows in the image.

Shall be an exact multiple of the vertical downsampling factor if any of the samples (planes) are encoded downsampled in the vertical direction for pixel data encoded in a Native (uncompressed) format. E.g., required to be an even value for a Photometric Interpretation (0028,0004) of YBR_FULL_422.</rdfs:comment>
        <rdfs:label xml:lang="en">Rows</rdfs:label>
    </owl:DatatypeProperty>
    


    <!-- http://purl.org/healthcarevocab/v1#SamplesPerPixel -->


    <owl:DatatypeProperty rdf:about="http://purl.org/healthcarevocab/v1#SamplesPerPixel">
        <rdfs:domain rdf:resource="https://www.morphosource.org/terms/morphosource#FileSet"/>
        <rdfs:range rdf:resource="http://www.w3.org/2001/XMLSchema#int"/>
        <rdfs:comment xml:lang="en">Number of samples (planes) in this image. See Section C.7.6.3.1.1 for further explanation.</rdfs:comment>
        <rdfs:label xml:lang="en">Samples Per Pixel</rdfs:label>
    </owl:DatatypeProperty>
    


    <!-- http://purl.org/healthcarevocab/v1#SeriesDate -->


    <owl:DatatypeProperty rdf:about="http://purl.org/healthcarevocab/v1#SeriesDate">
        <rdfs:domain rdf:resource="https://www.morphosource.org/terms/morphosource#FileSet"/>
        <rdfs:range rdf:resource="http://www.w3.org/2001/XMLSchema#date"/>
        <rdfs:comment xml:lang="en">Date the Series started.</rdfs:comment>
        <rdfs:label xml:lang="en">Series Date</rdfs:label>
    </owl:DatatypeProperty>
    


    <!-- http://purl.org/healthcarevocab/v1#SeriesTime -->


    <owl:DatatypeProperty rdf:about="http://purl.org/healthcarevocab/v1#SeriesTime">
        <rdfs:domain rdf:resource="https://www.morphosource.org/terms/morphosource#FileSet"/>
        <rdfs:range rdf:resource="http://www.w3.org/2001/XMLSchema#dateTime"/>
        <rdfs:comment xml:lang="en">Time the Series started.</rdfs:comment>
        <rdfs:label xml:lang="en">Series Time</rdfs:label>
    </owl:DatatypeProperty>
    


    <!-- http://purl.org/healthcarevocab/v1#SliceThickness -->


    <owl:DatatypeProperty rdf:about="http://purl.org/healthcarevocab/v1#SliceThickness">
        <rdfs:domain rdf:resource="https://www.morphosource.org/terms/morphosource#FileSet"/>
        <rdfs:domain rdf:resource="https://www.morphosource.org/terms/morphosource#Media"/>
        <rdfs:range rdf:resource="http://www.w3.org/2001/XMLSchema#float"/>
        <rdfs:comment xml:lang="en">Nominal slice thickness, in mm.</rdfs:comment>
        <rdfs:label xml:lang="en">Slice Thickness</rdfs:label>
    </owl:DatatypeProperty>
    


    <!-- http://purl.org/healthcarevocab/v1#SpacingBetweenSlices -->


    <owl:DatatypeProperty rdf:about="http://purl.org/healthcarevocab/v1#SpacingBetweenSlices">
        <rdfs:domain rdf:resource="https://www.morphosource.org/terms/morphosource#FileSet"/>
        <rdfs:range rdf:resource="http://www.w3.org/2001/XMLSchema#float"/>
        <rdfs:comment xml:lang="en">Spacing between slices, in mm. The spacing is measured from the center-to-center of each slice.</rdfs:comment>
        <rdfs:label xml:lang="en">Spacing Between Slices</rdfs:label>
    </owl:DatatypeProperty>
    


    <!-- http://purl.org/healthcarevocab/v1#SpiralPitchFactor -->


    <owl:DatatypeProperty rdf:about="http://purl.org/healthcarevocab/v1#SpiralPitchFactor">
        <rdfs:domain rdf:resource="https://www.morphosource.org/terms/morphosource#FileSet"/>
        <rdfs:range rdf:resource="http://www.w3.org/2001/XMLSchema#float"/>
        <rdfs:comment xml:lang="en">Ratio of the Table Feed per Rotation (0018,9310) to the Total Collimation Width (0018,9307).</rdfs:comment>
        <rdfs:label xml:lang="en">Spiral Pitch Factor</rdfs:label>
    </owl:DatatypeProperty>
    


    <!-- http://purl.org/healthcarevocab/v1#StudyDate -->


    <owl:DatatypeProperty rdf:about="http://purl.org/healthcarevocab/v1#StudyDate">
        <rdfs:domain rdf:resource="https://www.morphosource.org/terms/morphosource#FileSet"/>
        <rdfs:range rdf:resource="http://www.w3.org/2001/XMLSchema#date"/>
        <rdfs:comment xml:lang="en">Date the Study started.</rdfs:comment>
        <rdfs:label xml:lang="en">Study Date</rdfs:label>
    </owl:DatatypeProperty>
    


    <!-- http://purl.org/healthcarevocab/v1#StudyTime -->


    <owl:DatatypeProperty rdf:about="http://purl.org/healthcarevocab/v1#StudyTime">
        <rdfs:domain rdf:resource="https://www.morphosource.org/terms/morphosource#FileSet"/>
        <rdfs:range rdf:resource="http://www.w3.org/2001/XMLSchema#dateTime"/>
        <rdfs:comment xml:lang="en">Time the Study started.</rdfs:comment>
        <rdfs:label xml:lang="en">Study Time</rdfs:label>
    </owl:DatatypeProperty>
    


    <!-- http://purl.org/healthcarevocab/v1#WindowCenter -->


    <owl:DatatypeProperty rdf:about="http://purl.org/healthcarevocab/v1#WindowCenter">
        <rdfs:domain rdf:resource="https://www.morphosource.org/terms/morphosource#FileSet"/>
        <rdfs:range rdf:resource="http://www.w3.org/2001/XMLSchema#string"/>
        <rdfs:comment xml:lang="en">Window Center for display.

See Section C.11.2.1.2 for further explanation.

Required if VOI LUT Sequence (0028,3010) is not present. May be present otherwise.</rdfs:comment>
        <rdfs:label xml:lang="en">Window Center</rdfs:label>
    </owl:DatatypeProperty>
    


    <!-- http://purl.org/healthcarevocab/v1#WindowWidth -->


    <owl:DatatypeProperty rdf:about="http://purl.org/healthcarevocab/v1#WindowWidth">
        <rdfs:domain rdf:resource="https://www.morphosource.org/terms/morphosource#FileSet"/>
        <rdfs:range rdf:resource="http://www.w3.org/2001/XMLSchema#string"/>
        <rdfs:comment xml:lang="en">Window Width for display. See Section C.11.2.1.2 for further explanation.

Required if Window Center (0028,1050) is present.</rdfs:comment>
        <rdfs:label xml:lang="en">Window Width</rdfs:label>
    </owl:DatatypeProperty>
    


    <!-- http://purl.org/healthcarevocab/v1#XRayTubeCurrent -->


    <owl:DatatypeProperty rdf:about="http://purl.org/healthcarevocab/v1#XRayTubeCurrent">
        <rdfs:domain rdf:resource="https://www.morphosource.org/terms/morphosource#FileSet"/>
        <rdfs:range rdf:resource="http://www.w3.org/2001/XMLSchema#float"/>
        <rdfs:comment xml:lang="en">X-Ray Tube Current in mA. Required if Exposure (0018,1152) is not present. May be present otherwise.</rdfs:comment>
        <rdfs:label xml:lang="en">X-Ray Tube Current</rdfs:label>
    </owl:DatatypeProperty>
    


    <!-- http://rs.tdwg.org/ac/terms/IDofContainingCollection -->


    <owl:DatatypeProperty rdf:about="http://rs.tdwg.org/ac/terms/IDofContainingCollection">
        <terms:description xml:lang="en">Repeatable: A media resource may be member of multiple collections. The form of the identifier is left to implementers of specific implementations.</terms:description>
        <terms:hasVersion rdf:resource="http://rs.tdwg.org/ac/terms/version/IDofContainingCollection-2013-10-28"/>
        <terms:hasVersion rdf:resource="http://rs.tdwg.org/ac/terms/version/IDofContainingCollection-2020-01-27"/>
        <terms:isPartOf rdf:resource="http://rs.tdwg.org/ac/terms/"/>
        <attributes:organizedInClass rdf:resource="http://rs.tdwg.org/dwc/terms/attributes/RelatedResources"/>
        <attributes:repeatable>Yes</attributes:repeatable>
        <attributes:required>No</attributes:required>
        <rdfs:comment xml:lang="en">If the resource is contained in a Collection, this field identifies that Collection uniquely.</rdfs:comment>
        <rdfs:isDefinedBy rdf:resource="http://rs.tdwg.org/ac/terms/"/>
        <rdfs:label xml:lang="en">ID of Containing Collection</rdfs:label>
    </owl:DatatypeProperty>
    


    <!-- http://rs.tdwg.org/ac/terms/fundingAttribution -->


    <owl:DatatypeProperty rdf:about="http://rs.tdwg.org/ac/terms/fundingAttribution">
        <dc:format>application/rdf+xml</dc:format>
        <terms:hasVersion rdf:resource="http://rs.tdwg.org/ac/terms/version/fundingAttribution-2013-10-28"/>
        <terms:hasVersion rdf:resource="http://rs.tdwg.org/ac/terms/version/fundingAttribution-2020-01-27"/>
        <terms:isPartOf rdf:resource="http://rs.tdwg.org/ac/terms/"/>
        <terms:references rdf:resource="http://rs.tdwg.org/ac/terms/fundingAttribution"/>
        <attributes:organizedInClass rdf:resource="http://rs.tdwg.org/dwc/terms/attributes/Attribution"/>
        <attributes:repeatable>Yes</attributes:repeatable>
        <attributes:required>No</attributes:required>
        <rdfs:comment xml:lang="en">Text description of organizations or individuals who funded the creation of the resource.</rdfs:comment>
        <rdfs:isDefinedBy rdf:resource="http://rs.tdwg.org/ac/terms/"/>
        <rdfs:label xml:lang="en">Funding</rdfs:label>
    </owl:DatatypeProperty>
    


    <!-- http://rs.tdwg.org/ac/terms/providerManagedID -->


    <owl:DatatypeProperty rdf:about="http://rs.tdwg.org/ac/terms/providerManagedID">
        <terms:description xml:lang="en">Ideally, this would be a globally unique identifier (GUID), but the provider is encouraged to supply any form of identifier that simplifies communications on resources within their project and helps to locate individual data items in the provider&apos;s data repositories. It is the provider&apos;s decision whether to expose this value or not.</terms:description>
        <terms:hasVersion rdf:resource="http://rs.tdwg.org/ac/terms/version/providerManagedID-2013-10-28"/>
        <terms:hasVersion rdf:resource="http://rs.tdwg.org/ac/terms/version/providerManagedID-2020-01-27"/>
        <terms:isPartOf rdf:resource="http://rs.tdwg.org/ac/terms/"/>
        <attributes:organizedInClass rdf:resource="http://rs.tdwg.org/dwc/terms/attributes/Management"/>
        <attributes:repeatable>No</attributes:repeatable>
        <attributes:required>No</attributes:required>
        <rdfs:comment xml:lang="en">A free-form identifier (a simple number, an alphanumeric code, a URL, etc.) for the resource that is unique and meaningful primarily for the data provider.</rdfs:comment>
        <rdfs:isDefinedBy rdf:resource="http://rs.tdwg.org/ac/terms/"/>
        <rdfs:label xml:lang="en">Provider-managed ID</rdfs:label>
    </owl:DatatypeProperty>
    


    <!-- http://rs.tdwg.org/ac/terms/subjectOrientation -->


    <owl:DatatypeProperty rdf:about="http://rs.tdwg.org/ac/terms/subjectOrientation">
        <terms:hasVersion rdf:resource="http://rs.tdwg.org/ac/terms/version/subjectOrientation-2013-10-28"/>
        <terms:hasVersion rdf:resource="http://rs.tdwg.org/ac/terms/version/subjectOrientation-2020-01-27"/>
        <terms:hasVersion rdf:resource="http://rs.tdwg.org/ac/terms/version/subjectOrientation-2022-02-23"/>
        <terms:isPartOf rdf:resource="http://rs.tdwg.org/ac/terms/"/>
        <attributes:organizedInClass rdf:resource="http://rs.tdwg.org/dwc/terms/attributes/TaxonomicCoverage"/>
        <attributes:repeatable>No</attributes:repeatable>
        <attributes:required>No</attributes:required>
        <rdfs:comment xml:lang="en">Specific orientation (= direction, view angle) of the subject represented in the media resource with respect to the acquisition device, denoted by an IRI.</rdfs:comment>
        <rdfs:isDefinedBy rdf:resource="http://rs.tdwg.org/ac/terms/"/>
        <rdfs:label xml:lang="en">Subject Orientation</rdfs:label>
        <skos:scopeNote xml:lang="en">Values SHOULD be selected from the Controlled Vocabulary for Audubon Core subjectOrientation. In text-based systems such as tables, IRI values MUST be in unabbreviated form.</skos:scopeNote>
    </owl:DatatypeProperty>
    


    <!-- http://rs.tdwg.org/ac/terms/subjectPart -->


    <owl:DatatypeProperty rdf:about="http://rs.tdwg.org/ac/terms/subjectPart">
        <terms:hasVersion rdf:resource="http://rs.tdwg.org/ac/terms/version/subjectPart-2013-10-28"/>
        <terms:hasVersion rdf:resource="http://rs.tdwg.org/ac/terms/version/subjectPart-2020-01-27"/>
        <terms:hasVersion rdf:resource="http://rs.tdwg.org/ac/terms/version/subjectPart-2022-02-23"/>
        <terms:isPartOf rdf:resource="http://rs.tdwg.org/ac/terms/"/>
        <attributes:organizedInClass rdf:resource="http://rs.tdwg.org/dwc/terms/attributes/TaxonomicCoverage"/>
        <attributes:repeatable>No</attributes:repeatable>
        <attributes:required>No</attributes:required>
        <rdfs:comment xml:lang="en">The portion or product of organism morphology, behaviour, environment, etc. that is either predominantly shown or particularly well exemplified by the media resource, denoted by an IRI.</rdfs:comment>
        <rdfs:isDefinedBy rdf:resource="http://rs.tdwg.org/ac/terms/"/>
        <rdfs:label xml:lang="en">Subject Part</rdfs:label>
        <skos:scopeNote xml:lang="en">Values SHOULD be selected from the Controlled Vocabulary for Audubon Core subjectPart. In text-based systems such as tables, IRI values MUST be in unabbreviated form.</skos:scopeNote>
    </owl:DatatypeProperty>
    


    <!-- http://rs.tdwg.org/dwc/terms/catalogNumber -->


    <owl:DatatypeProperty rdf:about="http://rs.tdwg.org/dwc/terms/catalogNumber">
        <rdfs:domain rdf:resource="https://www.morphosource.org/terms/morphosource#PhysicalObject"/>
        <rdfs:range rdf:resource="http://www.w3.org/2001/XMLSchema#string"/>
        <terms:hasVersion rdf:resource="http://rs.tdwg.org/dwc/terms/version/catalogNumber-2009-04-24"/>
        <terms:hasVersion rdf:resource="http://rs.tdwg.org/dwc/terms/version/catalogNumber-2017-10-06"/>
        <terms:isPartOf rdf:resource="http://rs.tdwg.org/dwc/terms/"/>
        <terms:replaces rdf:resource="http://rs.tdwg.org/dwc/dwcore/CatalogNumber"/>
        <attributes:abcdEquivalence>DataSets/DataSet/Units/Unit/UnitID</attributes:abcdEquivalence>
        <attributes:organizedInClass rdf:resource="http://rs.tdwg.org/dwc/terms/Occurrence"/>
        <attributes:usageScope>simple</attributes:usageScope>
        <rdfs:comment xml:lang="en">An identifier (preferably unique) for the record within the data set or collection.</rdfs:comment>
        <rdfs:isDefinedBy rdf:resource="http://rs.tdwg.org/dwc/terms/"/>
        <rdfs:label xml:lang="en">Catalog Number</rdfs:label>
        <skos:example xml:lang="en">`145732`, `145732a`, `2008.1334`, `R-4313`</skos:example>
    </owl:DatatypeProperty>
    


    <!-- http://rs.tdwg.org/dwc/terms/collectionCode -->


    <owl:DatatypeProperty rdf:about="http://rs.tdwg.org/dwc/terms/collectionCode">
        <rdfs:domain rdf:resource="https://www.morphosource.org/terms/morphosource#Organization"/>
        <rdfs:domain rdf:resource="https://www.morphosource.org/terms/morphosource#PhysicalObject"/>
        <rdfs:range rdf:resource="http://www.w3.org/2001/XMLSchema#string"/>
        <terms:hasVersion rdf:resource="http://rs.tdwg.org/dwc/terms/version/collectionCode-2009-04-24"/>
        <terms:hasVersion rdf:resource="http://rs.tdwg.org/dwc/terms/version/collectionCode-2009-08-24"/>
        <terms:hasVersion rdf:resource="http://rs.tdwg.org/dwc/terms/version/collectionCode-2009-09-11"/>
        <terms:hasVersion rdf:resource="http://rs.tdwg.org/dwc/terms/version/collectionCode-2017-10-06"/>
        <terms:isPartOf rdf:resource="http://rs.tdwg.org/dwc/terms/"/>
        <terms:replaces rdf:resource="http://rs.tdwg.org/dwc/dwcore/CollectionCode"/>
        <attributes:abcdEquivalence>DataSets/DataSet/Units/Unit/SourceID</attributes:abcdEquivalence>
        <attributes:organizedInClass rdf:resource="http://rs.tdwg.org/dwc/terms/"/>
        <attributes:usageScope>simple</attributes:usageScope>
        <rdfs:comment xml:lang="en">The name, acronym, coden, or initialism identifying the collection or data set from which the record was derived.</rdfs:comment>
        <rdfs:isDefinedBy rdf:resource="http://rs.tdwg.org/dwc/terms/"/>
        <rdfs:label xml:lang="en">Collection Code</rdfs:label>
        <skos:example xml:lang="en">`Mammals`, `Hildebrandt`, `EBIRD`, `VP`</skos:example>
    </owl:DatatypeProperty>
    


    <!-- http://rs.tdwg.org/dwc/terms/datasetID -->


    <owl:DatatypeProperty rdf:about="http://rs.tdwg.org/dwc/terms/datasetID">
        <terms:hasVersion rdf:resource="http://rs.tdwg.org/dwc/terms/version/datasetID-2009-04-24"/>
        <terms:hasVersion rdf:resource="http://rs.tdwg.org/dwc/terms/version/datasetID-2009-09-11"/>
        <terms:hasVersion rdf:resource="http://rs.tdwg.org/dwc/terms/version/datasetID-2017-10-06"/>
        <terms:isPartOf rdf:resource="http://rs.tdwg.org/dwc/terms/"/>
        <attributes:abcdEquivalence>DataSets/DataSet/DataSetGUID</attributes:abcdEquivalence>
        <attributes:organizedInClass rdf:resource="http://rs.tdwg.org/dwc/terms/"/>
        <attributes:usageScope>simple</attributes:usageScope>
        <rdfs:comment xml:lang="en">An identifier for the set of data. May be a global unique identifier or an identifier specific to a collection or institution.</rdfs:comment>
        <rdfs:isDefinedBy rdf:resource="http://rs.tdwg.org/dwc/terms/"/>
        <rdfs:label xml:lang="en">Dataset ID</rdfs:label>
        <skos:example xml:lang="en">`b15d4952-7d20-46f1-8a3e-556a512b04c5`</skos:example>
    </owl:DatatypeProperty>
    


    <!-- http://rs.tdwg.org/dwc/terms/disposition -->


    <owl:DatatypeProperty rdf:about="http://rs.tdwg.org/dwc/terms/disposition">
        <terms:description xml:lang="en">Recommended best practice is to use a controlled vocabulary.</terms:description>
        <terms:hasVersion rdf:resource="http://rs.tdwg.org/dwc/terms/version/disposition-2009-04-24"/>
        <terms:hasVersion rdf:resource="http://rs.tdwg.org/dwc/terms/version/disposition-2017-10-06"/>
        <terms:isPartOf rdf:resource="http://rs.tdwg.org/dwc/terms/"/>
        <terms:replaces rdf:resource="http://rs.tdwg.org/dwc/curatorial/Disposition"/>
        <attributes:abcdEquivalence>DataSets/DataSet/Units/Unit/SpecimenUnit/Disposition</attributes:abcdEquivalence>
        <attributes:organizedInClass rdf:resource="http://rs.tdwg.org/dwc/terms/Occurrence"/>
        <attributes:usageScope>simple</attributes:usageScope>
        <rdfs:comment xml:lang="en">The current state of a specimen with respect to the collection identified in collectionCode or collectionID.</rdfs:comment>
        <rdfs:isDefinedBy rdf:resource="http://rs.tdwg.org/dwc/terms/"/>
        <rdfs:label xml:lang="en">Disposition</rdfs:label>
        <skos:example xml:lang="en">`in collection`, `missing`, `voucher elsewhere`, `duplicates elsewhere`</skos:example>
    </owl:DatatypeProperty>
    


    <!-- http://rs.tdwg.org/dwc/terms/earliestEonOrLowestEonothem -->


    <owl:DatatypeProperty rdf:about="http://rs.tdwg.org/dwc/terms/earliestEonOrLowestEonothem">
        <terms:hasVersion rdf:resource="http://rs.tdwg.org/dwc/terms/version/earliestEonOrLowestEonothem-2009-04-24"/>
        <terms:hasVersion rdf:resource="http://rs.tdwg.org/dwc/terms/version/earliestEonOrLowestEonothem-2017-10-06"/>
        <terms:isPartOf rdf:resource="http://rs.tdwg.org/dwc/terms/"/>
        <terms:replaces rdf:resource="http://digir.net/schema/conceptual/darwin/extension/paleontology/1.0/EarliestEonOrLowestEonothem"/>
        <attributes:abcdEquivalence>not in ABCD</attributes:abcdEquivalence>
        <attributes:organizedInClass rdf:resource="http://rs.tdwg.org/dwc/terms/GeologicalContext"/>
        <attributes:usageScope>simple</attributes:usageScope>
        <rdfs:comment xml:lang="en">The full name of the earliest possible geochronologic eon or lowest chrono-stratigraphic eonothem or the informal name (&quot;Precambrian&quot;) attributable to the stratigraphic horizon from which the cataloged item was collected.</rdfs:comment>
        <rdfs:isDefinedBy rdf:resource="http://rs.tdwg.org/dwc/terms/"/>
        <rdfs:label xml:lang="en">Earliest Eon Or Lowest Eonothem</rdfs:label>
        <skos:example xml:lang="en">`Phanerozoic`, `Proterozoic`</skos:example>
    </owl:DatatypeProperty>
    


    <!-- http://rs.tdwg.org/dwc/terms/formation -->


    <owl:DatatypeProperty rdf:about="http://rs.tdwg.org/dwc/terms/formation">
        <rdfs:domain rdf:resource="https://www.morphosource.org/terms/morphosource#PhysicalObject"/>
        <rdfs:range rdf:resource="http://www.w3.org/2001/XMLSchema#string"/>
        <terms:hasVersion rdf:resource="http://rs.tdwg.org/dwc/terms/version/formation-2009-04-24"/>
        <terms:hasVersion rdf:resource="http://rs.tdwg.org/dwc/terms/version/formation-2017-10-06"/>
        <terms:isPartOf rdf:resource="http://rs.tdwg.org/dwc/terms/"/>
        <terms:replaces rdf:resource="http://digir.net/schema/conceptual/darwin/extension/paleontology/1.0/Formation"/>
        <attributes:abcdEquivalence>not in ABCD</attributes:abcdEquivalence>
        <attributes:organizedInClass rdf:resource="http://rs.tdwg.org/dwc/terms/GeologicalContext"/>
        <attributes:usageScope>simple</attributes:usageScope>
        <rdfs:comment xml:lang="en">The full name of the lithostratigraphic formation from which the cataloged item was collected.</rdfs:comment>
        <rdfs:isDefinedBy rdf:resource="http://rs.tdwg.org/dwc/terms/"/>
        <rdfs:label xml:lang="en">Formation</rdfs:label>
        <skos:example xml:lang="en">`Notch Peak Formation`, `House Limestone`, `Fillmore Formation`</skos:example>
    </owl:DatatypeProperty>
    


    <!-- http://rs.tdwg.org/dwc/terms/geologicalContextID -->


    <owl:DatatypeProperty rdf:about="http://rs.tdwg.org/dwc/terms/geologicalContextID">
        <terms:hasVersion rdf:resource="http://rs.tdwg.org/dwc/terms/version/geologicalContextID-2009-07-06"/>
        <terms:hasVersion rdf:resource="http://rs.tdwg.org/dwc/terms/version/geologicalContextID-2017-10-06"/>
        <terms:isPartOf rdf:resource="http://rs.tdwg.org/dwc/terms/"/>
        <attributes:abcdEquivalence>not in ABCD</attributes:abcdEquivalence>
        <attributes:organizedInClass rdf:resource="http://rs.tdwg.org/dwc/terms/GeologicalContext"/>
        <attributes:usageScope>simple</attributes:usageScope>
        <rdfs:comment xml:lang="en">An identifier for the set of information associated with a GeologicalContext (the location within a geological context, such as stratigraphy). May be a global unique identifier or an identifier specific to the data set.</rdfs:comment>
        <rdfs:isDefinedBy rdf:resource="http://rs.tdwg.org/dwc/terms/"/>
        <rdfs:label xml:lang="en">Geological Context ID</rdfs:label>
        <skos:example xml:lang="en">`https://opencontext.org/subjects/e54377f7-4452-4315-b676-40679b10c4d9`</skos:example>
    </owl:DatatypeProperty>
    


    <!-- http://rs.tdwg.org/dwc/terms/institutionCode -->


    <owl:DatatypeProperty rdf:about="http://rs.tdwg.org/dwc/terms/institutionCode">
        <rdfs:domain rdf:resource="https://www.morphosource.org/terms/morphosource#Organization"/>
        <rdfs:domain rdf:resource="https://www.morphosource.org/terms/morphosource#PhysicalObject"/>
        <rdfs:range rdf:resource="http://www.w3.org/2001/XMLSchema#string"/>
        <terms:hasVersion rdf:resource="http://rs.tdwg.org/dwc/terms/version/institutionCode-2009-04-24"/>
        <terms:hasVersion rdf:resource="http://rs.tdwg.org/dwc/terms/version/institutionCode-2009-08-24"/>
        <terms:hasVersion rdf:resource="http://rs.tdwg.org/dwc/terms/version/institutionCode-2009-09-11"/>
        <terms:hasVersion rdf:resource="http://rs.tdwg.org/dwc/terms/version/institutionCode-2017-10-06"/>
        <terms:isPartOf rdf:resource="http://rs.tdwg.org/dwc/terms/"/>
        <terms:replaces rdf:resource="http://rs.tdwg.org/dwc/dwcore/InstitutionCode"/>
        <attributes:abcdEquivalence>DataSets/DataSet/Units/Unit/SourceInstitutionID</attributes:abcdEquivalence>
        <attributes:organizedInClass rdf:resource="http://rs.tdwg.org/dwc/terms/"/>
        <attributes:usageScope>simple</attributes:usageScope>
        <rdfs:comment xml:lang="en">The name (or acronym) in use by the institution having custody of the object(s) or information referred to in the record.</rdfs:comment>
        <rdfs:isDefinedBy rdf:resource="http://rs.tdwg.org/dwc/terms/"/>
        <rdfs:label xml:lang="en">Institution Code</rdfs:label>
        <skos:example xml:lang="en">`MVZ`, `FMNH`, `CLO`, `UCMP`</skos:example>
    </owl:DatatypeProperty>
    


    <!-- http://rs.tdwg.org/dwc/terms/locality -->


    <owl:DatatypeProperty rdf:about="http://rs.tdwg.org/dwc/terms/locality">
        <terms:description xml:lang="en">Less specific geographic information can be provided in other geographic terms (higherGeography, continent, country, stateProvince, county, municipality, waterBody, island, islandGroup). This term may contain information modified from the original to correct perceived errors or standardize the description.</terms:description>
        <terms:hasVersion rdf:resource="http://rs.tdwg.org/dwc/terms/version/locality-2009-04-24"/>
        <terms:hasVersion rdf:resource="http://rs.tdwg.org/dwc/terms/version/locality-2017-10-06"/>
        <terms:hasVersion rdf:resource="http://rs.tdwg.org/dwc/terms/version/locality-2021-07-15"/>
        <terms:isPartOf rdf:resource="http://rs.tdwg.org/dwc/terms/"/>
        <terms:replaces rdf:resource="http://rs.tdwg.org/dwc/dwcore/Locality"/>
        <attributes:abcdEquivalence>DataSets/DataSet/Units/Unit/Gathering/NamedAreas/NamedArea/AreaName</attributes:abcdEquivalence>
        <attributes:organizedInClass rdf:resource="http://purl.org/dc/terms/Location"/>
        <attributes:usageScope>simple</attributes:usageScope>
        <rdfs:comment xml:lang="en">The specific description of the place.</rdfs:comment>
        <rdfs:isDefinedBy rdf:resource="http://rs.tdwg.org/dwc/terms/"/>
        <rdfs:label xml:lang="en">Locality</rdfs:label>
        <skos:example xml:lang="en">`Bariloche, 25 km NNE via Ruta Nacional 40 (=Ruta 237)`, `Queets Rainforest, Olympic National Park`</skos:example>
    </owl:DatatypeProperty>
    


    <!-- http://rs.tdwg.org/dwc/terms/municipality -->


    <owl:DatatypeProperty rdf:about="http://rs.tdwg.org/dwc/terms/municipality">
        <terms:description xml:lang="en">Recommended best practice is to use a controlled vocabulary such as the Getty Thesaurus of Geographic Names.</terms:description>
        <terms:hasVersion rdf:resource="http://rs.tdwg.org/dwc/terms/version/municipality-2009-08-24"/>
        <terms:hasVersion rdf:resource="http://rs.tdwg.org/dwc/terms/version/municipality-2017-10-06"/>
        <terms:isPartOf rdf:resource="http://rs.tdwg.org/dwc/terms/"/>
        <attributes:abcdEquivalence>DataSets/DataSet/Units/Unit/Gathering/NamedAreas/NamedArea/AreaName</attributes:abcdEquivalence>
        <attributes:organizedInClass rdf:resource="http://purl.org/dc/terms/Location"/>
        <attributes:usageScope>simple</attributes:usageScope>
        <rdfs:comment xml:lang="en">The full, unabbreviated name of the next smaller administrative region than county (city, municipality, etc.) in which the Location occurs. Do not use this term for a nearby named place that does not contain the actual location.</rdfs:comment>
        <rdfs:isDefinedBy rdf:resource="http://rs.tdwg.org/dwc/terms/"/>
        <rdfs:label xml:lang="en">Municipality</rdfs:label>
        <skos:example xml:lang="en">`Holzminden`, `Araçatuba`, `Ga-Segonyana`</skos:example>
    </owl:DatatypeProperty>
    


    <!-- http://rs.tdwg.org/dwc/terms/occurrenceID -->


    <owl:DatatypeProperty rdf:about="http://rs.tdwg.org/dwc/terms/occurrenceID">
        <rdfs:domain rdf:resource="https://www.morphosource.org/terms/morphosource#BiologicalSpecimenObject"/>
        <rdfs:range rdf:resource="http://www.w3.org/2001/XMLSchema#string"/>
        <terms:description xml:lang="en">Recommended best practice is to use a persistent, globally unique identifier.</terms:description>
        <terms:hasVersion rdf:resource="http://rs.tdwg.org/dwc/terms/version/occurrenceID-2009-04-24"/>
        <terms:hasVersion rdf:resource="http://rs.tdwg.org/dwc/terms/version/occurrenceID-2017-10-06"/>
        <terms:isPartOf rdf:resource="http://rs.tdwg.org/dwc/terms/"/>
        <terms:replaces rdf:resource="http://rs.tdwg.org/dwc/dwcore/GlobalUniqueIdentifier"/>
        <attributes:abcdEquivalence>DataSets/DataSet/Units/Unit/UnitGUID</attributes:abcdEquivalence>
        <attributes:organizedInClass rdf:resource="http://rs.tdwg.org/dwc/terms/Occurrence"/>
        <attributes:usageScope>simple</attributes:usageScope>
        <rdfs:comment xml:lang="en">An identifier for the Occurrence (as opposed to a particular digital record of the occurrence). In the absence of a persistent global unique identifier, construct one from a combination of identifiers in the record that will most closely make the occurrenceID globally unique.</rdfs:comment>
        <rdfs:isDefinedBy rdf:resource="http://rs.tdwg.org/dwc/terms/"/>
        <rdfs:label xml:lang="en">Occurrence ID</rdfs:label>
        <skos:example xml:lang="en">`http://arctos.database.museum/guid/MSB:Mamm:233627`, `000866d2-c177-4648-a200-ead4007051b9`, `urn:catalog:UWBM:Bird:89776`</skos:example>
    </owl:DatatypeProperty>
    


    <!-- http://rs.tdwg.org/dwc/terms/typeStatus -->


    <owl:DatatypeProperty rdf:about="http://rs.tdwg.org/dwc/terms/typeStatus">
        <terms:description xml:lang="en">Recommended best practice is to separate the values in a list with space vertical bar space (` | `).</terms:description>
        <terms:hasVersion rdf:resource="http://rs.tdwg.org/dwc/terms/version/typeStatus-2009-04-24"/>
        <terms:hasVersion rdf:resource="http://rs.tdwg.org/dwc/terms/version/typeStatus-2014-10-23"/>
        <terms:hasVersion rdf:resource="http://rs.tdwg.org/dwc/terms/version/typeStatus-2017-10-06"/>
        <terms:isPartOf rdf:resource="http://rs.tdwg.org/dwc/terms/"/>
        <terms:replaces rdf:resource="http://rs.tdwg.org/dwc/curatorial/TypeStatus"/>
        <attributes:abcdEquivalence>DataSets/DataSet/Units/Unit/SpecimenUnit/NomenclaturalTypeDesignations/NomenclaturalTypeText</attributes:abcdEquivalence>
        <attributes:decision rdf:resource="http://rs.tdwg.org/dwc/terms/history/decisions/#Decision-2014-10-30_16"/>
        <attributes:organizedInClass rdf:resource="http://rs.tdwg.org/dwc/terms/Identification"/>
        <attributes:usageScope>simple</attributes:usageScope>
        <rdfs:comment xml:lang="en">A list (concatenated and separated) of nomenclatural types (type status, typified scientific name, publication) applied to the subject.</rdfs:comment>
        <rdfs:isDefinedBy rdf:resource="http://rs.tdwg.org/dwc/terms/"/>
        <rdfs:label xml:lang="en">Type Status</rdfs:label>
        <skos:definition xml:lang="en">A list (concatenated and separated) of nomenclatural types (type status, typified scientific name, publication) applied to the subject.</skos:definition>
        <skos:example xml:lang="en">`holotype of Ctenomys sociabilis. Pearson O. P., and M. I. Christie. 1985. Historia Natural, 5(37):388`, `holotype of Pinus abies | holotype of Picea abies`</skos:example>
        <skos:prefLabel xml:lang="en">Type Status</skos:prefLabel>
    </owl:DatatypeProperty>
    


    <!-- http://www.europeana.eu/schemas/edm/currentLocation -->


    <owl:DatatypeProperty rdf:about="http://www.europeana.eu/schemas/edm/currentLocation">
        <rdfs:domain rdf:resource="https://www.morphosource.org/terms/morphosource#PhysicalObject"/>
        <rdfs:range rdf:resource="http://www.w3.org/2001/XMLSchema#string"/>
        <rdfs:comment xml:lang="en">The geographic location and/or name of the repository, building, site, or other entity whose boundaries presently include the resource.</rdfs:comment>
        <rdfs:label xml:lang="en">Current Location</rdfs:label>
    </owl:DatatypeProperty>
    


    <!-- http://www.w3.org/2000/01/rdf-schema#seeAlso -->


    <owl:DatatypeProperty rdf:about="http://www.w3.org/2000/01/rdf-schema#seeAlso"/>
    


    <!-- http://www.w3.org/2003/12/exif/ns#apertureValue -->


    <owl:DatatypeProperty rdf:about="http://www.w3.org/2003/12/exif/ns#apertureValue">
        <rdfs:domain rdf:resource="https://www.morphosource.org/terms/morphosource#FileSet"/>
        <rdfs:domain rdf:resource="https://www.morphosource.org/terms/morphosource#PhotogrammetryImagingEvent"/>
        <rdfs:domain rdf:resource="https://www.morphosource.org/terms/morphosource#PhotographyImagingEvent"/>
        <rdfs:range rdf:resource="http://www.w3.org/2001/XMLSchema#float"/>
        <rdfs:comment xml:lang="en">The lens aperture. The unit is the APEX value.</rdfs:comment>
        <rdfs:comment xml:lang="ja">レンズ絞り値（APEX値）。この値のルート2のベキ乗を取ると、通常の絞り値となる。例えば&apos;5&apos;の場合だと√2^5=F5.6</rdfs:comment>
        <rdfs:label xml:lang="en">ApertureValue</rdfs:label>
        <ns:tagNumber xml:lang="en">37378</ns:tagNumber>
    </owl:DatatypeProperty>
    


    <!-- http://www.w3.org/2003/12/exif/ns#bitsPerSample -->


    <owl:DatatypeProperty rdf:about="http://www.w3.org/2003/12/exif/ns#bitsPerSample">
        <rdfs:domain rdf:resource="https://www.morphosource.org/terms/morphosource#FileSet"/>
        <rdfs:range rdf:resource="http://www.w3.org/2001/XMLSchema#int"/>
        <rdfs:comment xml:lang="en">The number of bits per image component. In this standard each component of the image is 8 bits, so the value for this tag is 8. See also SamplesPerPixel. In JPEG compressed data a JPEG marker is used instead of this tag.</rdfs:comment>
        <rdfs:label xml:lang="en">BitsPerSample</rdfs:label>
        <ns:tagNumber xml:lang="en">258</ns:tagNumber>
    </owl:DatatypeProperty>
    


    <!-- http://www.w3.org/2003/12/exif/ns#focalLength -->


    <owl:DatatypeProperty rdf:about="http://www.w3.org/2003/12/exif/ns#focalLength">
        <rdfs:domain rdf:resource="https://www.morphosource.org/terms/morphosource#FileSet"/>
        <rdfs:range rdf:resource="http://www.w3.org/2001/XMLSchema#float"/>
        <rdfs:comment xml:lang="en">The actual focal length of the lens, in mm. Conversion is not made to the focal length of a 35 mm film camera.</rdfs:comment>
        <rdfs:comment xml:lang="ja">レンズの焦点距離。単位はmm</rdfs:comment>
        <rdfs:label xml:lang="en">FocalLength</rdfs:label>
        <ns:tagNumber xml:lang="en">37386</ns:tagNumber>
    </owl:DatatypeProperty>
    


    <!-- http://www.w3.org/2003/12/exif/ns#gpsLatitude -->


    <owl:DatatypeProperty rdf:about="http://www.w3.org/2003/12/exif/ns#gpsLatitude">
        <rdfs:comment xml:lang="en">The latitude, expressed as three values giving the degrees, minutes, and seconds, respectively.</rdfs:comment>
        <rdfs:comment xml:lang="ja">緯度</rdfs:comment>
        <rdfs:label xml:lang="en">GPSLatitude</rdfs:label>
        <ns:tagNumber xml:lang="en">2</ns:tagNumber>
    </owl:DatatypeProperty>
    


    <!-- http://www.w3.org/2003/12/exif/ns#gpsLongitude -->


    <owl:DatatypeProperty rdf:about="http://www.w3.org/2003/12/exif/ns#gpsLongitude">
        <rdfs:comment xml:lang="en">The longitude, expressed as three values giving the degrees, minutes, and seconds, respectively.</rdfs:comment>
        <rdfs:comment xml:lang="ja">経度</rdfs:comment>
        <rdfs:label xml:lang="en">GPSLongitude</rdfs:label>
        <ns:tagNumber xml:lang="en">4</ns:tagNumber>
    </owl:DatatypeProperty>
    


    <!-- http://www.w3.org/2003/12/exif/ns#isoSpeedRatings -->


    <owl:DatatypeProperty rdf:about="http://www.w3.org/2003/12/exif/ns#isoSpeedRatings">
        <rdfs:domain rdf:resource="https://www.morphosource.org/terms/morphosource#FileSet"/>
        <rdfs:domain rdf:resource="https://www.morphosource.org/terms/morphosource#PhotogrammetryImagingEvent"/>
        <rdfs:domain rdf:resource="https://www.morphosource.org/terms/morphosource#PhotographyImagingEvent"/>
        <rdfs:range rdf:resource="http://www.w3.org/2001/XMLSchema#string"/>
        <rdfs:comment xml:lang="ja">CCD感度の銀塩フィルム換算値</rdfs:comment>
        <rdfs:comment xml:lang="en">Indicates the ISO Speed and ISO Latitude of the camera or input device as specified in ISO 12232.</rdfs:comment>
        <rdfs:label xml:lang="en">ISOSpeedRatings</rdfs:label>
        <ns:tagNumber xml:lang="en">34855</ns:tagNumber>
    </owl:DatatypeProperty>
    


    <!-- http://www.w3.org/2003/12/exif/ns#shutterSpeedValue -->


    <owl:DatatypeProperty rdf:about="http://www.w3.org/2003/12/exif/ns#shutterSpeedValue">
        <rdfs:comment xml:lang="en">Shutter speed. The unit is the APEX (Additive System of Photographic Exposure) setting</rdfs:comment>
        <rdfs:comment xml:lang="ja">シャッター速度（APEX値）。この値の2のベキ乗をとって逆数にすると、通常のシャッター速度表示になる。例えば&apos;4&apos;の場合だと1/(2^4)=1/16秒</rdfs:comment>
        <rdfs:label xml:lang="en">ShutterSpeedValue</rdfs:label>
        <ns:tagNumber xml:lang="en">37377</ns:tagNumber>
    </owl:DatatypeProperty>
    


    <!-- https://www.morphosource.org/terms/morphosource#ID -->


    <owl:DatatypeProperty rdf:about="https://www.morphosource.org/terms/morphosource#ID">
        <rdfs:domain rdf:resource="https://www.morphosource.org/terms/morphosource#Device"/>
        <rdfs:domain rdf:resource="https://www.morphosource.org/terms/morphosource#FileSet"/>
        <rdfs:domain rdf:resource="https://www.morphosource.org/terms/morphosource#ImagingEvent"/>
        <rdfs:domain rdf:resource="https://www.morphosource.org/terms/morphosource#Media"/>
        <rdfs:domain rdf:resource="https://www.morphosource.org/terms/morphosource#Organization"/>
        <rdfs:domain rdf:resource="https://www.morphosource.org/terms/morphosource#PhysicalObject"/>
        <rdfs:domain rdf:resource="https://www.morphosource.org/terms/morphosource#ProcessingEvent"/>
        <rdfs:range rdf:resource="http://www.w3.org/2001/XMLSchema#string"/>
        <rdfs:comment xml:lang="en">Morphosource-specific unique ID identifier for a Work (Media, Organization, Device, etc.).</rdfs:comment>
        <rdfs:label xml:lang="en">ID</rdfs:label>
    </owl:DatatypeProperty>
    


    <!-- https://www.morphosource.org/terms/morphosource#address -->


    <owl:DatatypeProperty rdf:about="https://www.morphosource.org/terms/morphosource#address">
        <rdfs:subPropertyOf rdf:resource="http://rs.tdwg.org/dwc/terms/locality"/>
        <rdfs:domain rdf:resource="https://www.morphosource.org/terms/morphosource#Organization"/>
        <rdfs:domain rdf:resource="https://www.morphosource.org/terms/morphosource#PhysicalObject"/>
        <rdfs:range rdf:resource="http://www.w3.org/2001/XMLSchema#string"/>
        <terms:isVersionOf>http://rs.tdwg.org/dwc/terms/locality</terms:isVersionOf>
        <attributes:abcdEquivalence>DataSets/DataSet/Units/Unit/Gathering/NamedAreas/NamedArea/AreaName</attributes:abcdEquivalence>
        <attributes:organizedInClass rdf:resource="http://purl.org/dc/terms/Location"/>
        <attributes:usageScope>simple</attributes:usageScope>
        <rdfs:comment xml:lang="en">The street address or other specific description of the place or location.</rdfs:comment>
        <rdfs:label xml:lang="en">Address</rdfs:label>
        <skos:example xml:lang="en">`130 Science Dr`</skos:example>
    </owl:DatatypeProperty>
    


    <!-- https://www.morphosource.org/terms/morphosource#agreementURI -->


    <owl:DatatypeProperty rdf:about="https://www.morphosource.org/terms/morphosource#agreementURI">
        <rdfs:subPropertyOf rdf:resource="http://ns.adobe.com/xap/1.0/rights/UsageTerms"/>
        <rdfs:domain rdf:resource="https://www.morphosource.org/terms/morphosource#Media"/>
        <rdfs:domain rdf:resource="https://www.morphosource.org/terms/morphosource#Organization"/>
        <rdfs:range rdf:resource="http://www.w3.org/2001/XMLSchema#anyURI"/>
        <terms:isVersionOf rdf:resource="http://ns.adobe.com/xap/1.0/rights/UsageTerms"/>
        <rdfs:comment xml:lang="en">A Web URI for a statement of the ownership and usage rights for Media. This more accurately maps to xmpRights:WebStatement than xmpRights:UsageTerms, and should be changed accordingly.</rdfs:comment>
        <rdfs:label xml:lang="en">Agreement URI</rdfs:label>
    </owl:DatatypeProperty>
    


    <!-- https://www.morphosource.org/terms/morphosource#amperage -->


    <owl:DatatypeProperty rdf:about="https://www.morphosource.org/terms/morphosource#amperage">
        <rdfs:subPropertyOf rdf:resource="http://purl.org/healthcarevocab/v1#XRayTubeCurrent"/>
        <rdfs:domain rdf:resource="https://www.morphosource.org/terms/morphosource#CTImageSeriesImagingEvent"/>
        <rdfs:range rdf:resource="http://www.w3.org/2001/XMLSchema#float"/>
        <terms:isVersionOf rdf:resource="http://purl.org/healthcarevocab/v1#XRayTubeCurrent"/>
        <rdfs:comment xml:lang="en">X-Ray Tube Current in mA.</rdfs:comment>
        <rdfs:label xml:lang="en">Amperage</rdfs:label>
    </owl:DatatypeProperty>
    


    <!-- https://www.morphosource.org/terms/morphosource#ark -->


    <owl:DatatypeProperty rdf:about="https://www.morphosource.org/terms/morphosource#ark">
        <rdfs:subPropertyOf rdf:resource="https://www.morphosource.org/terms/morphosource#mediaARK"/>
        <rdfs:domain rdf:resource="https://www.morphosource.org/terms/morphosource#Media"/>
        <rdfs:range rdf:resource="http://www.w3.org/2001/XMLSchema#string"/>
        <rdfs:comment xml:lang="en">Persistent identifier for MorphoSource Media automatically created on Media submission. ARKs can apply to both unpublished and published media.</rdfs:comment>
        <rdfs:label xml:lang="en">ARK (Archival Resource Key)</rdfs:label>
    </owl:DatatypeProperty>
    


    <!-- https://www.morphosource.org/terms/morphosource#attachmentFile -->


    <owl:DatatypeProperty rdf:about="https://www.morphosource.org/terms/morphosource#attachmentFile">
        <rdfs:domain rdf:resource="https://www.morphosource.org/terms/morphosource#ImagingEvent"/>
        <rdfs:domain rdf:resource="https://www.morphosource.org/terms/morphosource#Media"/>
        <rdfs:domain rdf:resource="https://www.morphosource.org/terms/morphosource#Organization"/>
        <rdfs:domain rdf:resource="https://www.morphosource.org/terms/morphosource#ProcessingEvent"/>
        <rdfs:comment xml:lang="en">A binary attachment file associated with a Work record. Often used to provide additional description beyond that allowed by object properties.</rdfs:comment>
        <rdfs:label xml:lang="en">Attachment File</rdfs:label>
    </owl:DatatypeProperty>
    


    <!-- https://www.morphosource.org/terms/morphosource#boundingBoxX -->


    <owl:DatatypeProperty rdf:about="https://www.morphosource.org/terms/morphosource#boundingBoxX">
        <rdfs:domain rdf:resource="https://www.morphosource.org/terms/morphosource#FileSet"/>
        <rdfs:range rdf:resource="http://www.w3.org/2001/XMLSchema#float"/>
        <rdfs:comment xml:lang="en">Length across the X axis of the rectangular bounding box surrounding a 3D digital object.</rdfs:comment>
        <rdfs:label xml:lang="en">Bounding Box X</rdfs:label>
    </owl:DatatypeProperty>
    


    <!-- https://www.morphosource.org/terms/morphosource#boundingBoxY -->


    <owl:DatatypeProperty rdf:about="https://www.morphosource.org/terms/morphosource#boundingBoxY">
        <rdfs:domain rdf:resource="https://www.morphosource.org/terms/morphosource#FileSet"/>
        <rdfs:range rdf:resource="http://www.w3.org/2001/XMLSchema#float"/>
        <rdfs:comment xml:lang="en">Length across the Y axis of the rectangular bounding box surrounding a 3D digital object.</rdfs:comment>
        <rdfs:label xml:lang="en">Bounding Box Y</rdfs:label>
    </owl:DatatypeProperty>
    


    <!-- https://www.morphosource.org/terms/morphosource#boundingBoxZ -->


    <owl:DatatypeProperty rdf:about="https://www.morphosource.org/terms/morphosource#boundingBoxZ">
        <rdfs:domain rdf:resource="https://www.morphosource.org/terms/morphosource#FileSet"/>
        <rdfs:range rdf:resource="http://www.w3.org/2001/XMLSchema#float"/>
        <rdfs:comment xml:lang="en">Length across the Z axis of the rectangular bounding box surrounding a 3D digital object.</rdfs:comment>
        <rdfs:label xml:lang="en">Bounding Box Z</rdfs:label>
    </owl:DatatypeProperty>
    


    <!-- https://www.morphosource.org/terms/morphosource#canonicalTaxonomy -->


    <owl:DatatypeProperty rdf:about="https://www.morphosource.org/terms/morphosource#canonicalTaxonomy">
        <rdfs:subPropertyOf rdf:resource="https://www.morphosource.org/terms/morphosource#ID"/>
        <rdfs:domain rdf:resource="https://www.morphosource.org/terms/morphosource#BiologicalSpecimenObject"/>
        <rdfs:range rdf:resource="http://www.w3.org/2001/XMLSchema#string"/>
        <rdfs:comment xml:lang="en">MorphoSource-specific ID of Taxonomy record for taxonomic name attributed to the specimen physical object by the provider organization (museum, institution, or laboratory) responsible for managing the specimen. May not be present if no provider-supplied taxonomy is present. This may differ from taxonomic names attributed to the specimen by researchers or other individuals. Values for this property should be a subset of values for property morphosource:taxonomyID values, but morphosource:taxonomyID may include additional values as well.</rdfs:comment>
        <rdfs:label xml:lang="en">Canonical Taxonomy</rdfs:label>
    </owl:DatatypeProperty>
    


    <!-- https://www.morphosource.org/terms/morphosource#centroidX -->


    <owl:DatatypeProperty rdf:about="https://www.morphosource.org/terms/morphosource#centroidX">
        <rdfs:domain rdf:resource="https://www.morphosource.org/terms/morphosource#FileSet"/>
        <rdfs:range rdf:resource="http://www.w3.org/2001/XMLSchema#float"/>
        <rdfs:comment xml:lang="en">X axis coordinate of the centroid of a 3D object, where the centroid is the geometric center point of the object.</rdfs:comment>
        <rdfs:label xml:lang="en">Centroid X</rdfs:label>
    </owl:DatatypeProperty>
    


    <!-- https://www.morphosource.org/terms/morphosource#centroidY -->


    <owl:DatatypeProperty rdf:about="https://www.morphosource.org/terms/morphosource#centroidY">
        <rdfs:domain rdf:resource="https://www.morphosource.org/terms/morphosource#FileSet"/>
        <rdfs:range rdf:resource="http://www.w3.org/2001/XMLSchema#float"/>
        <rdfs:comment xml:lang="en">Y axis coordinate of the centroid of a 3D object, where the centroid is the geometric center point of the object.</rdfs:comment>
        <rdfs:label xml:lang="en">Centroid Y</rdfs:label>
    </owl:DatatypeProperty>
    


    <!-- https://www.morphosource.org/terms/morphosource#centroidZ -->


    <owl:DatatypeProperty rdf:about="https://www.morphosource.org/terms/morphosource#centroidZ">
        <rdfs:domain rdf:resource="https://www.morphosource.org/terms/morphosource#FileSet"/>
        <rdfs:range rdf:resource="http://www.w3.org/2001/XMLSchema#float"/>
        <rdfs:comment xml:lang="en">Z axis coordinate of the centroid of a 3D object, where the centroid is the geometric center point of the object.</rdfs:comment>
        <rdfs:label xml:lang="en">Centroid Z</rdfs:label>
    </owl:DatatypeProperty>
    


    <!-- https://www.morphosource.org/terms/morphosource#choAttribute -->


    <owl:DatatypeProperty rdf:about="https://www.morphosource.org/terms/morphosource#choAttribute">
        <rdfs:domain rdf:resource="https://www.morphosource.org/terms/morphosource#CulturalHeritageObject"/>
        <rdfs:range rdf:resource="http://www.w3.org/2001/XMLSchema#string"/>
        <rdfs:comment xml:lang="en">Physical attributes of an object, including characteristics such as size and shape, chemical properties of materials, qualities of texture and hardness, and features such as surface ornament. It is preferred to use morphosource:aatAttribute when it is possible to express attributes using the Getty Arts and Architecture Thesaurus controlled vocabulary. This property is for custom attribute values not listed in the Getty AAT controlled vocabulary.</rdfs:comment>
        <rdfs:label xml:lang="en">Cultural Heritage Object Attribute</rdfs:label>
    </owl:DatatypeProperty>
    


    <!-- https://www.morphosource.org/terms/morphosource#choType -->


    <owl:DatatypeProperty rdf:about="https://www.morphosource.org/terms/morphosource#choType">
        <rdfs:domain rdf:resource="https://www.morphosource.org/terms/morphosource#CulturalHeritageObject"/>
        <rdfs:range rdf:resource="http://www.w3.org/2001/XMLSchema#string"/>
        <rdfs:comment xml:lang="en">Type, genre, category, or classification of an object. It is preferred to use morphosource:aatType when it is possible to express type using the Getty Arts and Architecture Thesaurus controlled vocabulary. This property is for custom type values not listed in the Getty AAT controlled vocabulary.</rdfs:comment>
        <rdfs:label xml:lang="en">Cultural Heritage Object Type</rdfs:label>
    </owl:DatatypeProperty>
    


    <!-- https://www.morphosource.org/terms/morphosource#citeAs -->


    <owl:DatatypeProperty rdf:about="https://www.morphosource.org/terms/morphosource#citeAs">
        <rdfs:subPropertyOf rdf:resource="http://ns.adobe.com/photoshop/1.0/Credit"/>
        <rdfs:domain rdf:resource="https://www.morphosource.org/terms/morphosource#Media"/>
        <rdfs:range rdf:resource="http://www.w3.org/2001/XMLSchema#string"/>
        <terms:isVersionOf rdf:resource="http://ns.adobe.com/photoshop/1.0/Credit"/>
        <rdfs:comment xml:lang="en">Instructions and guidelines for the citation of a Media. This should include additional instructions beyond those included in other metadata fields or in any download usage agreement.</rdfs:comment>
        <rdfs:label xml:lang="en">Cite As</rdfs:label>
    </owl:DatatypeProperty>
    


    <!-- https://www.morphosource.org/terms/morphosource#city -->


    <owl:DatatypeProperty rdf:about="https://www.morphosource.org/terms/morphosource#city">
        <rdfs:subPropertyOf rdf:resource="http://rs.tdwg.org/dwc/terms/municipality"/>
        <rdfs:domain rdf:resource="https://www.morphosource.org/terms/morphosource#Organization"/>
        <rdfs:domain rdf:resource="https://www.morphosource.org/terms/morphosource#PhysicalObject"/>
        <rdfs:range rdf:resource="http://www.w3.org/2001/XMLSchema#string"/>
        <terms:description xml:lang="en">Recommended best practice is to use a controlled vocabulary such as the Getty Thesaurus of Geographic Names.</terms:description>
        <terms:isVersionOf rdf:resource="http://rs.tdwg.org/dwc/terms/municipality"/>
        <attributes:abcdEquivalence>DataSets/DataSet/Units/Unit/Gathering/NamedAreas/NamedArea/AreaName</attributes:abcdEquivalence>
        <attributes:organizedInClass rdf:resource="http://purl.org/dc/terms/Location"/>
        <attributes:usageScope>simple</attributes:usageScope>
        <rdfs:comment xml:lang="en">The full, unabbreviated name of the next smaller administrative region than county (city, municipality, etc.) in which the Location occurs. Do not use this term for a nearby named place that does not contain the actual location.</rdfs:comment>
        <rdfs:label xml:lang="en">City</rdfs:label>
        <skos:example xml:lang="en">`Holzminden`, `Araçatuba`, `Ga-Segonyana`</skos:example>
    </owl:DatatypeProperty>
    


    <!-- https://www.morphosource.org/terms/morphosource#contactUser -->


    <owl:DatatypeProperty rdf:about="https://www.morphosource.org/terms/morphosource#contactUser">
        <rdfs:domain rdf:resource="https://www.morphosource.org/terms/morphosource#Organization"/>
        <rdfs:range rdf:resource="http://www.w3.org/2001/XMLSchema#string"/>
        <rdfs:comment xml:lang="en">Contact individual associated with the Organization. Does not need to be a MorphoSource User.</rdfs:comment>
        <rdfs:label xml:lang="en">Contact User</rdfs:label>
    </owl:DatatypeProperty>
    


    <!-- https://www.morphosource.org/terms/morphosource#contentsAcceptedFileCount -->


    <owl:DatatypeProperty rdf:about="https://www.morphosource.org/terms/morphosource#contentsAcceptedFileCount">
        <rdfs:domain rdf:resource="https://www.morphosource.org/terms/morphosource#FileSet"/>
        <rdfs:range rdf:resource="http://www.w3.org/2001/XMLSchema#int"/>
        <rdfs:comment xml:lang="en">For a ZIP archive file, the largest number of system-recognized files with the same system-permissible file type located in a single directory. In MorphoSource, this is used to document the number of files in the primary image collection in a CT image stack or photogrammetry image collection.</rdfs:comment>
        <rdfs:label xml:lang="en">Contents Accepted File Count</rdfs:label>
    </owl:DatatypeProperty>
    


    <!-- https://www.morphosource.org/terms/morphosource#contentsFileName -->


    <owl:DatatypeProperty rdf:about="https://www.morphosource.org/terms/morphosource#contentsFileName">
        <rdfs:domain rdf:resource="https://www.morphosource.org/terms/morphosource#FileSet"/>
        <rdfs:range rdf:resource="http://www.w3.org/2001/XMLSchema#string"/>
        <rdfs:comment xml:lang="en">For a ZIP archive file, the file name of a single representative example of the largest number of system-recognized files with the same system-permissible file type located in a single directory. In MorphoSource, this is used to document a single file that is representative of the primary image collection in a CT image stack or photogrammetry image collection or the central mesh in a multi-file mesh archive.</rdfs:comment>
        <rdfs:label xml:lang="en">Contents File Name</rdfs:label>
    </owl:DatatypeProperty>
    


    <!-- https://www.morphosource.org/terms/morphosource#contentsFileSize -->


    <owl:DatatypeProperty rdf:about="https://www.morphosource.org/terms/morphosource#contentsFileSize">
        <rdfs:domain rdf:resource="https://www.morphosource.org/terms/morphosource#FileSet"/>
        <rdfs:range rdf:resource="http://www.w3.org/2001/XMLSchema#int"/>
        <rdfs:comment xml:lang="en">For a ZIP archive file, the file size of a single representative example of the largest number of system-recognized files with the same system-permissible file type located in a single directory. In MorphoSource, this is used to document file size for a single file that is representative of the primary image collection in a CT image stack or photogrammetry image collection or the central mesh in a multi-file mesh archive.</rdfs:comment>
        <rdfs:label xml:lang="en">Contents File Size</rdfs:label>
    </owl:DatatypeProperty>
    


    <!-- https://www.morphosource.org/terms/morphosource#contentsMimeType -->


    <owl:DatatypeProperty rdf:about="https://www.morphosource.org/terms/morphosource#contentsMimeType">
        <rdfs:domain rdf:resource="https://www.morphosource.org/terms/morphosource#FileSet"/>
        <rdfs:range rdf:resource="http://www.w3.org/2001/XMLSchema#string"/>
        <rdfs:comment xml:lang="en">For a ZIP archive file, the mime type of a single representative example of the largest number of system-recognized files with the same system-permissible file type located in a single directory. In MorphoSource, this is used to document a single file that is representative of the primary image collection in a CT image stack or photogrammetry image collection or the central mesh in a multi-file mesh archive.</rdfs:comment>
        <rdfs:label xml:lang="en">Contents Mime Type</rdfs:label>
        <skos:example xml:lang="en">`image/jpeg`, `image/tiff`, `application/stl`</skos:example>
    </owl:DatatypeProperty>
    


    <!-- https://www.morphosource.org/terms/morphosource#context -->


    <owl:DatatypeProperty rdf:about="https://www.morphosource.org/terms/morphosource#context">
        <rdfs:subPropertyOf rdf:resource="http://rs.tdwg.org/dwc/terms/geologicalContextID"/>
        <rdfs:domain rdf:resource="https://www.morphosource.org/terms/morphosource#PhysicalObject"/>
        <rdfs:range rdf:resource="http://www.w3.org/2001/XMLSchema#string"/>
        <terms:isVersionOf rdf:resource="http://rs.tdwg.org/dwc/terms/geologicalContextID"/>
        <attributes:abcdEquivalence>not in ABCD</attributes:abcdEquivalence>
        <attributes:organizedInClass rdf:resource="http://rs.tdwg.org/dwc/terms/GeologicalContext"/>
        <attributes:usageScope>simple</attributes:usageScope>
        <rdfs:comment xml:lang="en">An identifier for the set of information associated with a GeologicalContext (the location within a geological context, such as stratigraphy). May be a global unique identifier or an identifier specific to the data set.</rdfs:comment>
        <rdfs:label xml:lang="en">Geological Context</rdfs:label>
        <skos:example xml:lang="en">`https://opencontext.org/subjects/e54377f7-4452-4315-b676-40679b10c4d9`</skos:example>
    </owl:DatatypeProperty>
    


    <!-- https://www.morphosource.org/terms/morphosource#crc32 -->


    <owl:DatatypeProperty rdf:about="https://www.morphosource.org/terms/morphosource#crc32">
        <rdfs:domain rdf:resource="https://www.morphosource.org/terms/morphosource#FileSet"/>
        <rdfs:range rdf:resource="http://www.w3.org/2001/XMLSchema#string"/>
        <rdfs:comment xml:lang="en">Checksum hash used to verify the identity of a file and to detect accidental corruption.</rdfs:comment>
        <rdfs:label xml:lang="en">CRC32</rdfs:label>
    </owl:DatatypeProperty>
    


    <!-- https://www.morphosource.org/terms/morphosource#dateModified -->


    <owl:DatatypeProperty rdf:about="https://www.morphosource.org/terms/morphosource#dateModified">
        <rdfs:domain rdf:resource="https://www.morphosource.org/terms/morphosource#Device"/>
        <rdfs:domain rdf:resource="https://www.morphosource.org/terms/morphosource#FileSet"/>
        <rdfs:domain rdf:resource="https://www.morphosource.org/terms/morphosource#ImagingEvent"/>
        <rdfs:domain rdf:resource="https://www.morphosource.org/terms/morphosource#Media"/>
        <rdfs:domain rdf:resource="https://www.morphosource.org/terms/morphosource#Organization"/>
        <rdfs:domain rdf:resource="https://www.morphosource.org/terms/morphosource#PhysicalObject"/>
        <rdfs:domain rdf:resource="https://www.morphosource.org/terms/morphosource#ProcessingEvent"/>
        <rdfs:range rdf:resource="http://www.w3.org/2001/XMLSchema#dateTime"/>
        <terms:description xml:lang="en">Recommended practice is to describe the date, date/time, or period of time as recommended for the property Date, of which this is a subproperty.</terms:description>
        <rdfs:comment xml:lang="en">Date on which the resource was changed.</rdfs:comment>
        <rdfs:label xml:lang="en">Date Modified</rdfs:label>
    </owl:DatatypeProperty>
    


    <!-- https://www.morphosource.org/terms/morphosource#dateUploaded -->


    <owl:DatatypeProperty rdf:about="https://www.morphosource.org/terms/morphosource#dateUploaded">
        <rdfs:subPropertyOf rdf:resource="http://purl.org/dc/terms/dateSubmitted"/>
        <rdfs:domain rdf:resource="https://www.morphosource.org/terms/morphosource#Device"/>
        <rdfs:domain rdf:resource="https://www.morphosource.org/terms/morphosource#FileSet"/>
        <rdfs:domain rdf:resource="https://www.morphosource.org/terms/morphosource#ImagingEvent"/>
        <rdfs:domain rdf:resource="https://www.morphosource.org/terms/morphosource#Media"/>
        <rdfs:domain rdf:resource="https://www.morphosource.org/terms/morphosource#Organization"/>
        <rdfs:domain rdf:resource="https://www.morphosource.org/terms/morphosource#PhysicalObject"/>
        <rdfs:domain rdf:resource="https://www.morphosource.org/terms/morphosource#ProcessingEvent"/>
        <rdfs:range rdf:resource="http://www.w3.org/2001/XMLSchema#dateTime"/>
        <terms:description xml:lang="en">Recommended practice is to describe the date, date/time, or period of time as recommended for the property Date, of which this is a subproperty.</terms:description>
        <rdfs:comment xml:lang="en">Date of upload of the resource.</rdfs:comment>
        <rdfs:label xml:lang="en">Date Uploaded</rdfs:label>
    </owl:DatatypeProperty>
    


    <!-- https://www.morphosource.org/terms/morphosource#datingMethod -->


    <owl:DatatypeProperty rdf:about="https://www.morphosource.org/terms/morphosource#datingMethod">
        <rdfs:domain rdf:resource="https://www.morphosource.org/terms/morphosource#PhysicalObject"/>
        <rdfs:range rdf:resource="http://www.w3.org/2001/XMLSchema#string"/>
        <rdfs:comment xml:lang="en">Method used to determine the date an object was created, produced, fossilized, or otherwise came into being.</rdfs:comment>
        <rdfs:label xml:lang="en">Dating Method</rdfs:label>
    </owl:DatatypeProperty>
    


    <!-- https://www.morphosource.org/terms/morphosource#detectorPixelSizeX -->


    <owl:DatatypeProperty rdf:about="https://www.morphosource.org/terms/morphosource#detectorPixelSizeX">
        <rdfs:domain rdf:resource="https://www.morphosource.org/terms/morphosource#CTImageSeriesImagingEvent"/>
        <rdfs:range rdf:resource="http://www.w3.org/2001/XMLSchema#float"/>
        <rdfs:comment xml:lang="en">Length in mm of each pixel in the X direction.</rdfs:comment>
        <rdfs:label xml:lang="en">Detector Pixel Size X</rdfs:label>
    </owl:DatatypeProperty>
    


    <!-- https://www.morphosource.org/terms/morphosource#detectorPixelSizeY -->


    <owl:DatatypeProperty rdf:about="https://www.morphosource.org/terms/morphosource#detectorPixelSizeY">
        <rdfs:domain rdf:resource="https://www.morphosource.org/terms/morphosource#CTImageSeriesImagingEvent"/>
        <rdfs:range rdf:resource="http://www.w3.org/2001/XMLSchema#float"/>
        <rdfs:comment xml:lang="en">Length in mm of each pixel in the Y direction.</rdfs:comment>
        <rdfs:label xml:lang="en">Detector Pixel Size Y</rdfs:label>
    </owl:DatatypeProperty>
    


    <!-- https://www.morphosource.org/terms/morphosource#detectorPixelsX -->


    <owl:DatatypeProperty rdf:about="https://www.morphosource.org/terms/morphosource#detectorPixelsX">
        <rdfs:domain rdf:resource="https://www.morphosource.org/terms/morphosource#CTImageSeriesImagingEvent"/>
        <rdfs:range rdf:resource="http://www.w3.org/2001/XMLSchema#int"/>
        <rdfs:comment xml:lang="en">The number of pixels in the X direction of the detector (number of columns).</rdfs:comment>
        <rdfs:label xml:lang="en">Detector Pixels X</rdfs:label>
    </owl:DatatypeProperty>
    


    <!-- https://www.morphosource.org/terms/morphosource#detectorPixelsY -->


    <owl:DatatypeProperty rdf:about="https://www.morphosource.org/terms/morphosource#detectorPixelsY">
        <rdfs:domain rdf:resource="https://www.morphosource.org/terms/morphosource#CTImageSeriesImagingEvent"/>
        <rdfs:range rdf:resource="http://www.w3.org/2001/XMLSchema#int"/>
        <rdfs:comment xml:lang="en">The number of pixels in the X direction of the detector (number of rows).</rdfs:comment>
        <rdfs:label xml:lang="en">Detector Pixels Y</rdfs:label>
    </owl:DatatypeProperty>
    


    <!-- https://www.morphosource.org/terms/morphosource#deviceID -->


    <owl:DatatypeProperty rdf:about="https://www.morphosource.org/terms/morphosource#deviceID">
        <rdfs:subPropertyOf rdf:resource="https://www.morphosource.org/terms/morphosource#ID"/>
        <rdfs:domain rdf:resource="https://www.morphosource.org/terms/morphosource#ImagingEvent"/>
        <rdfs:range rdf:resource="http://www.w3.org/2001/XMLSchema#string"/>
        <rdfs:comment xml:lang="en">MorphoSource-specific unique ID identifier for a Device used in an Imaging Event to image a Physical Object.</rdfs:comment>
        <rdfs:label xml:lang="en">Imaging Device ID</rdfs:label>
    </owl:DatatypeProperty>
    


    <!-- https://www.morphosource.org/terms/morphosource#dicomFileTypeExtension -->


    <owl:DatatypeProperty rdf:about="https://www.morphosource.org/terms/morphosource#dicomFileTypeExtension">
        <rdfs:domain rdf:resource="https://www.morphosource.org/terms/morphosource#FileSet"/>
        <rdfs:range rdf:resource="http://www.w3.org/2001/XMLSchema#string"/>
        <rdfs:comment xml:lang="en">Extension code indicating the file format of a file.</rdfs:comment>
        <rdfs:label xml:lang="en">File Type Extension</rdfs:label>
        <skos:example xml:lang="en">`dcm`, `ply`, `mp4`</skos:example>
    </owl:DatatypeProperty>
    


    <!-- https://www.morphosource.org/terms/morphosource#dicomNumberOfSeriesRelatedInstances -->


    <owl:DatatypeProperty rdf:about="https://www.morphosource.org/terms/morphosource#dicomNumberOfSeriesRelatedInstances">
        <rdfs:label xml:lang="en">Number of Series Related Instances</rdfs:label>
    </owl:DatatypeProperty>
    


    <!-- https://www.morphosource.org/terms/morphosource#dicomPixelSpacingHeight -->


    <owl:DatatypeProperty rdf:about="https://www.morphosource.org/terms/morphosource#dicomPixelSpacingHeight">
        <rdfs:label xml:lang="en">Pixel Spacing Height</rdfs:label>
    </owl:DatatypeProperty>
    


    <!-- https://www.morphosource.org/terms/morphosource#dicomPixelSpacingWidth -->


    <owl:DatatypeProperty rdf:about="https://www.morphosource.org/terms/morphosource#dicomPixelSpacingWidth">
        <rdfs:label xml:lang="en">Pixel Spacing Width</rdfs:label>
    </owl:DatatypeProperty>
    


    <!-- https://www.morphosource.org/terms/morphosource#dicomSecondaryCaptureDeviceManufacturer -->


    <owl:DatatypeProperty rdf:about="https://www.morphosource.org/terms/morphosource#dicomSecondaryCaptureDeviceManufacturer">
        <rdfs:domain rdf:resource="https://www.morphosource.org/terms/morphosource#FileSet"/>
        <rdfs:range rdf:resource="http://www.w3.org/2001/XMLSchema#string"/>
        <rdfs:comment xml:lang="en">Manufacturer of the Secondary Capture Device. This field should map to some DICOM field.</rdfs:comment>
        <rdfs:label xml:lang="en">Secondary Capture Device Manufacturer</rdfs:label>
    </owl:DatatypeProperty>
    


    <!-- https://www.morphosource.org/terms/morphosource#dicomSecondaryCaptureDeviceSoftwareVers -->


    <owl:DatatypeProperty rdf:about="https://www.morphosource.org/terms/morphosource#dicomSecondaryCaptureDeviceSoftwareVers">
        <rdfs:domain rdf:resource="https://www.morphosource.org/terms/morphosource#FileSet"/>
        <rdfs:range rdf:resource="http://www.w3.org/2001/XMLSchema#string"/>
        <rdfs:comment xml:lang="en">Manufacturer&apos;s designation of software version of the Secondary Capture Device. This field should map to some DICOM field.</rdfs:comment>
        <rdfs:label xml:lang="en">Secondary Capture Device Software Vers</rdfs:label>
    </owl:DatatypeProperty>
    


    <!-- https://www.morphosource.org/terms/morphosource#dicomSpacingBetweenSlices -->


    <owl:DatatypeProperty rdf:about="https://www.morphosource.org/terms/morphosource#dicomSpacingBetweenSlices">
        <rdfs:label xml:lang="en">Spacing Between Slices</rdfs:label>
    </owl:DatatypeProperty>
    


    <!-- https://www.morphosource.org/terms/morphosource#dicomWindowCenterAndWidthExplanation -->


    <owl:DatatypeProperty rdf:about="https://www.morphosource.org/terms/morphosource#dicomWindowCenterAndWidthExplanation">
        <rdfs:domain rdf:resource="https://www.morphosource.org/terms/morphosource#FileSet"/>
        <rdfs:range rdf:resource="http://www.w3.org/2001/XMLSchema#string"/>
        <rdfs:comment xml:lang="en">Free form explanation of the meaning of the Window Center and Width. Multiple values correspond to multiple Window Center and Width values. This field should map to dicom:WindowCenterAndWidthExplanation and should be changed accordingly.</rdfs:comment>
        <rdfs:label xml:lang="en">Window Center and Width Explanation</rdfs:label>
    </owl:DatatypeProperty>
    


    <!-- https://www.morphosource.org/terms/morphosource#dimensions -->


    <owl:DatatypeProperty rdf:about="https://www.morphosource.org/terms/morphosource#dimensions">
        <rdfs:subPropertyOf rdf:resource="http://purl.org/dc/terms/format"/>
        <rdfs:domain rdf:resource="https://www.morphosource.org/terms/morphosource#PhysicalObject"/>
        <rdfs:range rdf:resource="http://www.w3.org/2001/XMLSchema#string"/>
        <terms:isVersionOf rdf:resource="http://purl.org/dc/terms/format"/>
        <terms:issued rdf:datatype="http://www.w3.org/2001/XMLSchema#date">2008-01-14</terms:issued>
        <rdfs:comment xml:lang="en">The physical dimensions or measurements of the object.</rdfs:comment>
        <rdfs:label xml:lang="en">Dimensions</rdfs:label>
    </owl:DatatypeProperty>
    


    <!-- https://www.morphosource.org/terms/morphosource#doi -->


    <owl:DatatypeProperty rdf:about="https://www.morphosource.org/terms/morphosource#doi">
        <rdfs:subPropertyOf rdf:resource="https://www.morphosource.org/terms/morphosource#mediaDOI"/>
        <rdfs:domain rdf:resource="https://www.morphosource.org/terms/morphosource#Media"/>
        <rdfs:range rdf:resource="http://www.w3.org/2001/XMLSchema#string"/>
        <rdfs:comment xml:lang="en">Persistent identifier for MorphoSource Media created only on user request. DOIs can apply only to published media.</rdfs:comment>
        <rdfs:label xml:lang="en">DOI (Digital Object Identifier)</rdfs:label>
    </owl:DatatypeProperty>
    


    <!-- https://www.morphosource.org/terms/morphosource#edgesPerFace -->


    <owl:DatatypeProperty rdf:about="https://www.morphosource.org/terms/morphosource#edgesPerFace">
        <rdfs:domain rdf:resource="https://www.morphosource.org/terms/morphosource#FileSet"/>
        <rdfs:range rdf:resource="http://www.w3.org/2001/XMLSchema#int"/>
        <rdfs:comment xml:lang="en">Number of polygonal edges that connect vertices or points and comprise each face of a polygonal 3D mesh. Values are commonly &quot;3&quot; for a triangular mesh or &quot;4&quot; for a quadrangular mesh.</rdfs:comment>
        <rdfs:label xml:lang="en">Edges Per Face</rdfs:label>
    </owl:DatatypeProperty>
    


    <!-- https://www.morphosource.org/terms/morphosource#exifLensMake -->


    <owl:DatatypeProperty rdf:about="https://www.morphosource.org/terms/morphosource#exifLensMake">
        <rdfs:label xml:lang="en">Lens Make</rdfs:label>
    </owl:DatatypeProperty>
    


    <!-- https://www.morphosource.org/terms/morphosource#exifLensModel -->


    <owl:DatatypeProperty rdf:about="https://www.morphosource.org/terms/morphosource#exifLensModel">
        <rdfs:label xml:lang="en">Lens Model</rdfs:label>
    </owl:DatatypeProperty>
    


    <!-- https://www.morphosource.org/terms/morphosource#faceCount -->


    <owl:DatatypeProperty rdf:about="https://www.morphosource.org/terms/morphosource#faceCount">
        <rdfs:domain rdf:resource="https://www.morphosource.org/terms/morphosource#FileSet"/>
        <rdfs:range rdf:resource="http://www.w3.org/2001/XMLSchema#int"/>
        <rdfs:comment xml:lang="en">Number of polygonal faces comprising a 3D mesh.</rdfs:comment>
        <rdfs:label xml:lang="en">Face Count</rdfs:label>
    </owl:DatatypeProperty>
    


    <!-- https://www.morphosource.org/terms/morphosource#fileName -->


    <owl:DatatypeProperty rdf:about="https://www.morphosource.org/terms/morphosource#fileName">
        <rdfs:domain rdf:resource="https://www.morphosource.org/terms/morphosource#FileSet"/>
        <rdfs:range rdf:resource="http://www.w3.org/2001/XMLSchema#string"/>
        <rdfs:comment xml:lang="en">Identifying name label given to a file.</rdfs:comment>
        <rdfs:label xml:lang="en">File Name</rdfs:label>
    </owl:DatatypeProperty>
    


    <!-- https://www.morphosource.org/terms/morphosource#fileSize -->


    <owl:DatatypeProperty rdf:about="https://www.morphosource.org/terms/morphosource#fileSize">
        <rdfs:domain rdf:resource="https://www.morphosource.org/terms/morphosource#FileSet"/>
        <rdfs:range rdf:resource="http://www.w3.org/2001/XMLSchema#int"/>
        <rdfs:comment xml:lang="en">Size of a file in bytes.</rdfs:comment>
        <rdfs:label xml:lang="en">File Size</rdfs:label>
    </owl:DatatypeProperty>
    


    <!-- https://www.morphosource.org/terms/morphosource#filter -->


    <owl:DatatypeProperty rdf:about="https://www.morphosource.org/terms/morphosource#filter">
        <rdfs:label xml:lang="en">Filter</rdfs:label>
    </owl:DatatypeProperty>
    


    <!-- https://www.morphosource.org/terms/morphosource#fluxNormalization -->


    <owl:DatatypeProperty rdf:about="https://www.morphosource.org/terms/morphosource#fluxNormalization">
        <rdfs:domain rdf:resource="https://www.morphosource.org/terms/morphosource#CTImageSeriesImagingEvent"/>
        <rdfs:range rdf:resource="http://www.w3.org/2001/XMLSchema#string"/>
        <rdfs:comment xml:lang="en">Whether flux normalization calibration is used or not. If present, value must be &quot;Yes&quot; or &quot;No&quot;.</rdfs:comment>
        <rdfs:label xml:lang="en">Flux Normalization</rdfs:label>
        <skos:example xml:lang="en">`Yes`, `No`</skos:example>
    </owl:DatatypeProperty>
    


    <!-- https://www.morphosource.org/terms/morphosource#focalLength -->


    <owl:DatatypeProperty rdf:about="https://www.morphosource.org/terms/morphosource#focalLength">
        <rdfs:domain rdf:resource="https://www.morphosource.org/terms/morphosource#PhotogrammetryImagingEvent"/>
        <rdfs:domain rdf:resource="https://www.morphosource.org/terms/morphosource#PhotographyImagingEvent"/>
        <rdfs:range rdf:resource="http://www.w3.org/2001/XMLSchema#float"/>
        <rdfs:comment xml:lang="en">The actual focal length of the lens, in mm. This should probably map to exif:focalLength and should be updated accordingly.</rdfs:comment>
        <rdfs:label xml:lang="en">Focal Length</rdfs:label>
    </owl:DatatypeProperty>
    


    <!-- https://www.morphosource.org/terms/morphosource#frameAveraging -->


    <owl:DatatypeProperty rdf:about="https://www.morphosource.org/terms/morphosource#frameAveraging">
        <rdfs:subPropertyOf rdf:resource="http://purl.org/healthcarevocab/v1#ContrastFrameAveraging"/>
        <rdfs:domain rdf:resource="https://www.morphosource.org/terms/morphosource#CTImageSeriesImagingEvent"/>
        <rdfs:range rdf:resource="http://www.w3.org/2001/XMLSchema#int"/>
        <terms:isVersionOf rdf:resource="http://purl.org/healthcarevocab/v1#ContrastFrameAveraging"/>
        <rdfs:comment xml:lang="en">Number of images acquired at each projection angle and their average.</rdfs:comment>
        <rdfs:label xml:lang="en">Frame Averaging</rdfs:label>
    </owl:DatatypeProperty>
    


    <!-- https://www.morphosource.org/terms/morphosource#funding -->


    <owl:DatatypeProperty rdf:about="https://www.morphosource.org/terms/morphosource#funding">
        <rdfs:subPropertyOf rdf:resource="http://rs.tdwg.org/ac/terms/fundingAttribution"/>
        <rdfs:domain rdf:resource="https://www.morphosource.org/terms/morphosource#Media"/>
        <rdfs:range rdf:resource="http://www.w3.org/2001/XMLSchema#string"/>
        <terms:isVersionOf rdf:resource="http://rs.tdwg.org/ac/terms/fundingAttribution"/>
        <attributes:repeatable>Yes</attributes:repeatable>
        <attributes:required>No</attributes:required>
        <rdfs:comment xml:lang="en">Text description of organizations or individuals who funded the creation of the resource.</rdfs:comment>
        <rdfs:label xml:lang="en">Funding</rdfs:label>
    </owl:DatatypeProperty>
    


    <!-- https://www.morphosource.org/terms/morphosource#hasUVSpace -->


    <owl:DatatypeProperty rdf:about="https://www.morphosource.org/terms/morphosource#hasUVSpace">
        <rdfs:domain rdf:resource="https://www.morphosource.org/terms/morphosource#FileSet"/>
        <rdfs:range rdf:resource="http://www.w3.org/2001/XMLSchema#string"/>
        <rdfs:comment xml:lang="en">Whether or not a mapping exists to project a 3D object&apos;s surface to a 2D image for texture mapping and is present with the 3D object. Values should be &quot;Yes&quot; or &quot;No&quot;.</rdfs:comment>
        <rdfs:label xml:lang="en">Has UV Space</rdfs:label>
        <skos:example xml:lang="en">`Yes`, `No`</skos:example>
    </owl:DatatypeProperty>
    


    <!-- https://www.morphosource.org/terms/morphosource#height -->


    <owl:DatatypeProperty rdf:about="https://www.morphosource.org/terms/morphosource#height">
        <rdfs:domain rdf:resource="https://www.morphosource.org/terms/morphosource#FileSet"/>
        <rdfs:range rdf:resource="http://www.w3.org/2001/XMLSchema#int"/>
        <rdfs:comment xml:lang="en">Height of a 2D image in pixels.</rdfs:comment>
        <rdfs:label xml:lang="en">Height in Pixels</rdfs:label>
    </owl:DatatypeProperty>
    


    <!-- https://www.morphosource.org/terms/morphosource#idigbioRecordsetID -->


    <owl:DatatypeProperty rdf:about="https://www.morphosource.org/terms/morphosource#idigbioRecordsetID">
        <rdfs:subPropertyOf rdf:resource="http://rs.tdwg.org/dwc/terms/datasetID"/>
        <rdfs:domain rdf:resource="https://www.morphosource.org/terms/morphosource#BiologicalSpecimenObject"/>
        <rdfs:range rdf:resource="http://www.w3.org/2001/XMLSchema#string"/>
        <terms:isVersionOf rdf:resource="http://rs.tdwg.org/dwc/terms/datasetID"/>
        <attributes:abcdEquivalence>DataSets/DataSet/DataSetGUID</attributes:abcdEquivalence>
        <attributes:usageScope>simple</attributes:usageScope>
        <rdfs:comment xml:lang="en">An identifier for an entire museum, institution, or laboratory specimen collection which includes the Biological Specimen. May be a global unique identifier or an identifier specific to a collection or institution.</rdfs:comment>
        <rdfs:label xml:lang="en">iDigBio Recordset ID</rdfs:label>
        <skos:example xml:lang="en">`b15d4952-7d20-46f1-8a3e-556a512b04c5`</skos:example>
    </owl:DatatypeProperty>
    


    <!-- https://www.morphosource.org/terms/morphosource#idigbioUUID -->


    <owl:DatatypeProperty rdf:about="https://www.morphosource.org/terms/morphosource#idigbioUUID">
        <rdfs:domain rdf:resource="https://www.morphosource.org/terms/morphosource#BiologicalSpecimenObject"/>
        <rdfs:range rdf:resource="http://www.w3.org/2001/XMLSchema#string"/>
        <rdfs:comment xml:lang="en">Global unique identifier for the Biological Specimen provided by iDigBio and used as the primary identifier of the Biological Specimen&apos;s record in the iDigBio aggregator if present. This is sometimes used in addition to more general identifiers or Darwin Core triplets (institution code : collection code : catalog number) to uniquely identify Biological Specimen.</rdfs:comment>
        <rdfs:label xml:lang="en">iDigBio UUID</rdfs:label>
    </owl:DatatypeProperty>
    


    <!-- https://www.morphosource.org/terms/morphosource#ieFilter -->


    <owl:DatatypeProperty rdf:about="https://www.morphosource.org/terms/morphosource#ieFilter">
        <rdfs:subPropertyOf rdf:resource="https://www.morphosource.org/terms/morphosource#filter"/>
        <rdfs:domain rdf:resource="https://www.morphosource.org/terms/morphosource#CTImageSeriesImagingEvent"/>
        <rdfs:range rdf:resource="http://www.w3.org/2001/XMLSchema#string"/>
        <rdfs:comment xml:lang="en">Type of filter(s) inserted into the X-Ray beam.</rdfs:comment>
        <rdfs:label xml:lang="en">Imaging Event Filter</rdfs:label>
    </owl:DatatypeProperty>
    


    <!-- https://www.morphosource.org/terms/morphosource#imagingEventID -->


    <owl:DatatypeProperty rdf:about="https://www.morphosource.org/terms/morphosource#imagingEventID">
        <rdfs:subPropertyOf rdf:resource="https://www.morphosource.org/terms/morphosource#ID"/>
        <rdfs:domain rdf:resource="https://www.morphosource.org/terms/morphosource#Media"/>
        <rdfs:range rdf:resource="http://www.w3.org/2001/XMLSchema#string"/>
        <rdfs:label xml:lang="en">Imaging Event ID</rdfs:label>
    </owl:DatatypeProperty>
    


    <!-- https://www.morphosource.org/terms/morphosource#institutionName -->


    <owl:DatatypeProperty rdf:about="https://www.morphosource.org/terms/morphosource#institutionName">
        <rdfs:domain rdf:resource="https://www.morphosource.org/terms/morphosource#Organization"/>
        <rdfs:range rdf:resource="http://www.w3.org/2001/XMLSchema#string"/>
        <rdfs:comment xml:lang="en">Name of institution affiliated with Organization. This may be a university in the case of departments or a museum in the case of specific museum collections.</rdfs:comment>
        <rdfs:label xml:lang="en">Institution Name</rdfs:label>
    </owl:DatatypeProperty>
    


    <!-- https://www.morphosource.org/terms/morphosource#isTypeSpecimen -->


    <owl:DatatypeProperty rdf:about="https://www.morphosource.org/terms/morphosource#isTypeSpecimen">
        <rdfs:subPropertyOf rdf:resource="http://rs.tdwg.org/dwc/terms/typeStatus"/>
        <rdfs:domain rdf:resource="https://www.morphosource.org/terms/morphosource#BiologicalSpecimenObject"/>
        <rdfs:range rdf:resource="http://www.w3.org/2001/XMLSchema#string"/>
        <terms:isVersionOf rdf:resource="http://rs.tdwg.org/dwc/terms/typeStatus"/>
        <attributes:abcdEquivalence>DataSets/DataSet/Units/Unit/SpecimenUnit/NomenclaturalTypeDesignations/NomenclaturalTypeText</attributes:abcdEquivalence>
        <attributes:organizedInClass rdf:resource="http://rs.tdwg.org/dwc/terms/Identification"/>
        <attributes:usageScope>simple</attributes:usageScope>
        <rdfs:comment xml:lang="en">Whether the Biological Specimen is a holotype or not. If present, value must be &quot;Yes&quot; or &quot;No&quot;.</rdfs:comment>
        <rdfs:label xml:lang="en">Is Type Specimen</rdfs:label>
        <skos:example xml:lang="en">`Yes`, `No`</skos:example>
    </owl:DatatypeProperty>
    


    <!-- https://www.morphosource.org/terms/morphosource#latitude -->


    <owl:DatatypeProperty rdf:about="https://www.morphosource.org/terms/morphosource#latitude">
        <rdfs:subPropertyOf rdf:resource="http://www.w3.org/2003/12/exif/ns#gpsLatitude"/>
        <rdfs:domain rdf:resource="https://www.morphosource.org/terms/morphosource#PhysicalObject"/>
        <rdfs:range rdf:resource="http://www.w3.org/2001/XMLSchema#string"/>
        <terms:isVersionOf rdf:resource="http://www.w3.org/2003/12/exif/ns#gpsLatitude"/>
        <rdfs:comment xml:lang="en">The latitude, expressed as three values giving the degrees, minutes, and seconds, respectively.</rdfs:comment>
        <rdfs:comment xml:lang="ja">緯度</rdfs:comment>
        <rdfs:label xml:lang="en">Latitude</rdfs:label>
        <ns:tagNumber xml:lang="en">2</ns:tagNumber>
        <skos:example xml:lang="en">`41d 05&apos; 54.03&quot; S`</skos:example>
    </owl:DatatypeProperty>
    


    <!-- https://www.morphosource.org/terms/morphosource#legacyMediaFileID -->


    <owl:DatatypeProperty rdf:about="https://www.morphosource.org/terms/morphosource#legacyMediaFileID">
        <rdfs:subPropertyOf rdf:resource="http://rs.tdwg.org/ac/terms/providerManagedID"/>
        <rdf:type rdf:resource="http://www.w3.org/2002/07/owl#FunctionalProperty"/>
        <rdfs:domain rdf:resource="https://www.morphosource.org/terms/morphosource#Media"/>
        <rdfs:range rdf:resource="http://www.w3.org/2001/XMLSchema#string"/>
        <terms:isVersionOf rdf:resource="http://rs.tdwg.org/ac/terms/providerManagedID"/>
        <attributes:repeatable>No</attributes:repeatable>
        <attributes:required>No</attributes:required>
        <rdfs:comment xml:lang="en">MorphoSource-specific unique ID identifier that was used to represent a Media in the now-defunct 1.0 version of the MorphoSource repository. Only present if Media was originally contributed to MorphoSource 1.0. Different from morphosource:ID identifier.</rdfs:comment>
        <rdfs:label xml:lang="en">Legacy Media File ID</rdfs:label>
    </owl:DatatypeProperty>
    


    <!-- https://www.morphosource.org/terms/morphosource#legacyMediaGroupID -->


    <owl:DatatypeProperty rdf:about="https://www.morphosource.org/terms/morphosource#legacyMediaGroupID">
        <rdfs:subPropertyOf rdf:resource="http://rs.tdwg.org/ac/terms/IDofContainingCollection"/>
        <rdf:type rdf:resource="http://www.w3.org/2002/07/owl#FunctionalProperty"/>
        <rdfs:domain rdf:resource="https://www.morphosource.org/terms/morphosource#Media"/>
        <rdfs:range rdf:resource="http://www.w3.org/2001/XMLSchema#string"/>
        <terms:isVersionOf rdf:resource="http://rs.tdwg.org/ac/terms/IDofContainingCollection"/>
        <attributes:repeatable xml:lang="en">No</attributes:repeatable>
        <attributes:required>No</attributes:required>
        <rdfs:comment xml:lang="en">MorphoSource-specific unique ID identifier that was used to group Media together in the now-defunct 1.0 version of the MorphoSource repository. In MorphoSource 1.0, Media groups were used to collect all media derived from the same Imaging Event. Media groups are no longer used, with media-to-media imaging and processing event relationships now being used instead to track hierarchical relationships between Media. Only present if Media was originally contributed to MorphoSource 1.0. Different from morphosource:ID identifier.</rdfs:comment>
        <rdfs:label xml:lang="en">Legacy Media Group ID</rdfs:label>
    </owl:DatatypeProperty>
    


    <!-- https://www.morphosource.org/terms/morphosource#lensMake -->


    <owl:DatatypeProperty rdf:about="https://www.morphosource.org/terms/morphosource#lensMake">
        <rdfs:subPropertyOf rdf:resource="https://www.morphosource.org/terms/morphosource#exifLensMake"/>
        <rdfs:domain rdf:resource="https://www.morphosource.org/terms/morphosource#PhotogrammetryImagingEvent"/>
        <rdfs:domain rdf:resource="https://www.morphosource.org/terms/morphosource#PhotographyImagingEvent"/>
        <rdfs:range rdf:resource="http://www.w3.org/2001/XMLSchema#string"/>
        <rdfs:comment xml:lang="en">The manufacturer of the camera lens. This should probably map directly to an EXIF term and should be updated accordingly.</rdfs:comment>
        <rdfs:label xml:lang="en">Lens Make</rdfs:label>
    </owl:DatatypeProperty>
    


    <!-- https://www.morphosource.org/terms/morphosource#lensModel -->


    <owl:DatatypeProperty rdf:about="https://www.morphosource.org/terms/morphosource#lensModel">
        <rdfs:subPropertyOf rdf:resource="https://www.morphosource.org/terms/morphosource#exifLensModel"/>
        <rdfs:domain rdf:resource="https://www.morphosource.org/terms/morphosource#PhotogrammetryImagingEvent"/>
        <rdfs:domain rdf:resource="https://www.morphosource.org/terms/morphosource#PhotographyImagingEvent"/>
        <rdfs:range rdf:resource="http://www.w3.org/2001/XMLSchema#string"/>
        <rdfs:comment xml:lang="en">The model of the camera lens. This should probably map directly to an EXIF term and should be updated accordingly.</rdfs:comment>
        <rdfs:label xml:lang="en">Lens Model</rdfs:label>
    </owl:DatatypeProperty>
    


    <!-- https://www.morphosource.org/terms/morphosource#licenseBlank -->


    <owl:DatatypeProperty rdf:about="https://www.morphosource.org/terms/morphosource#licenseBlank">
        <rdfs:domain rdf:resource="https://www.morphosource.org/terms/morphosource#Organization"/>
        <rdfs:range rdf:resource="http://www.w3.org/2001/XMLSchema#string"/>
        <rdfs:comment xml:lang="en">Whether the Organization&apos;s preferred policy is for Media representing Organization Physical Objects to specify no license in dc:license. This is distinct from an Organization expressing no preference on license choice. Values must be &quot;Yes&quot; or &quot;No&quot;. If value is &quot;Yes&quot;, then Organization explicitly prefers no license to be chosen.</rdfs:comment>
        <rdfs:label xml:lang="en">License Intentionally Left Blank</rdfs:label>
        <skos:example xml:lang="en">`Yes`, `No`</skos:example>
    </owl:DatatypeProperty>
    


    <!-- https://www.morphosource.org/terms/morphosource#longitude -->


    <owl:DatatypeProperty rdf:about="https://www.morphosource.org/terms/morphosource#longitude">
        <rdfs:subPropertyOf rdf:resource="http://www.w3.org/2003/12/exif/ns#gpsLongitude"/>
        <rdfs:domain rdf:resource="https://www.morphosource.org/terms/morphosource#PhysicalObject"/>
        <rdfs:range rdf:resource="http://www.w3.org/2001/XMLSchema#string"/>
        <terms:isVersionOf rdf:resource="http://www.w3.org/2003/12/exif/ns#gpsLongitude"/>
        <rdfs:comment xml:lang="en">The longitude, expressed as three values giving the degrees, minutes, and seconds, respectively.</rdfs:comment>
        <rdfs:comment xml:lang="ja">経度</rdfs:comment>
        <rdfs:label xml:lang="en">Longitude</rdfs:label>
        <ns:tagNumber xml:lang="en">4</ns:tagNumber>
        <skos:example xml:lang="en">`121d 10&apos; 34&quot; W`</skos:example>
    </owl:DatatypeProperty>
    


    <!-- https://www.morphosource.org/terms/morphosource#material -->


    <owl:DatatypeProperty rdf:about="https://www.morphosource.org/terms/morphosource#material">
        <rdfs:subPropertyOf rdf:resource="http://purl.org/dc/terms/medium"/>
        <rdfs:domain rdf:resource="https://www.morphosource.org/terms/morphosource#CulturalHeritageObject"/>
        <rdfs:range rdf:resource="http://www.w3.org/2001/XMLSchema#string"/>
        <terms:isVersionOf rdf:resource="http://purl.org/dc/terms/medium"/>
        <rdfs:comment xml:lang="en">Material(s) from which an object is made. It is preferred to use morphosource:aatMaterial when it is possible to express materials using the Getty Arts and Architecture Thesaurus controlled vocabulary. This property is for custom material values not listed in the Getty AAT controlled vocabulary.</rdfs:comment>
        <rdfs:label xml:lang="en">Material</rdfs:label>
    </owl:DatatypeProperty>
    


    <!-- https://www.morphosource.org/terms/morphosource#mediaARK -->


    <owl:DatatypeProperty rdf:about="https://www.morphosource.org/terms/morphosource#mediaARK">
        <rdfs:label xml:lang="en">Media ARK</rdfs:label>
    </owl:DatatypeProperty>
    


    <!-- https://www.morphosource.org/terms/morphosource#mediaDOI -->


    <owl:DatatypeProperty rdf:about="https://www.morphosource.org/terms/morphosource#mediaDOI">
        <rdfs:label xml:lang="en">Media DOI</rdfs:label>
    </owl:DatatypeProperty>
    


    <!-- https://www.morphosource.org/terms/morphosource#mediaParentID -->


    <owl:DatatypeProperty rdf:about="https://www.morphosource.org/terms/morphosource#mediaParentID">
        <rdfs:subPropertyOf rdf:resource="https://www.morphosource.org/terms/morphosource#ID"/>
        <rdfs:domain rdf:resource="https://www.morphosource.org/terms/morphosource#Media"/>
        <rdfs:range rdf:resource="http://www.w3.org/2001/XMLSchema#string"/>
        <rdfs:comment xml:lang="en">MorphoSource-specific unique ID identifier for the parent Media of a Media. This is the ID of the Media from which the current Media is immediately derived.</rdfs:comment>
        <rdfs:label xml:lang="en">Media Parent ID</rdfs:label>
    </owl:DatatypeProperty>
    


    <!-- https://www.morphosource.org/terms/morphosource#mimeType -->


    <owl:DatatypeProperty rdf:about="https://www.morphosource.org/terms/morphosource#mimeType">
        <rdfs:subPropertyOf rdf:resource="http://purl.org/dc/terms/format"/>
        <rdfs:domain rdf:resource="https://www.morphosource.org/terms/morphosource#FileSet"/>
        <rdfs:range rdf:resource="http://www.w3.org/2001/XMLSchema#string"/>
        <terms:isVersionOf rdf:resource="http://purl.org/dc/terms/format"/>
        <rdfs:comment xml:lang="en">Media type describing the nature and format of a file.</rdfs:comment>
        <rdfs:label xml:lang="en">Mime Type</rdfs:label>
        <skos:example xml:lang="en">`image/jpeg`, `image/tiff`, `application/stl`</skos:example>
    </owl:DatatypeProperty>
    


    <!-- https://www.morphosource.org/terms/morphosource#normalsFormat -->


    <owl:DatatypeProperty rdf:about="https://www.morphosource.org/terms/morphosource#normalsFormat">
        <rdfs:domain rdf:resource="https://www.morphosource.org/terms/morphosource#FileSet"/>
        <rdfs:range rdf:resource="http://www.w3.org/2001/XMLSchema#string"/>
        <rdfs:comment xml:lang="en">How vertex or face normal information is formatted and codified for a 3D object, if normal information is present with the object.</rdfs:comment>
        <rdfs:label xml:lang="en">Normals Format</rdfs:label>
    </owl:DatatypeProperty>
    


    <!-- https://www.morphosource.org/terms/morphosource#numberOfImagesInSet -->


    <owl:DatatypeProperty rdf:about="https://www.morphosource.org/terms/morphosource#numberOfImagesInSet">
        <rdfs:subPropertyOf rdf:resource="https://www.morphosource.org/terms/morphosource#dicomNumberOfSeriesRelatedInstances"/>
        <rdfs:domain rdf:resource="https://www.morphosource.org/terms/morphosource#Media"/>
        <rdfs:range rdf:resource="http://www.w3.org/2001/XMLSchema#int"/>
        <rdfs:comment xml:lang="en">For Media with a ZIP archive with many component files, this is the number of files in the primary image collection in a CT image stack or photogrammetry image collection. This only applies to CTImageSeries or PhotogrammetryImageSeries Media.</rdfs:comment>
        <rdfs:label xml:lang="en">Number of Images In Set</rdfs:label>
    </owl:DatatypeProperty>
    


    <!-- https://www.morphosource.org/terms/morphosource#numericTime -->


    <owl:DatatypeProperty rdf:about="https://www.morphosource.org/terms/morphosource#numericTime">
        <rdfs:subPropertyOf rdf:resource="http://rs.tdwg.org/dwc/terms/earliestEonOrLowestEonothem"/>
        <rdfs:domain rdf:resource="https://www.morphosource.org/terms/morphosource#PhysicalObject"/>
        <rdfs:range rdf:resource="http://www.w3.org/2001/XMLSchema#string"/>
        <terms:isVersionOf rdf:resource="http://rs.tdwg.org/dwc/terms/earliestEonOrLowestEonothem"/>
        <attributes:abcdEquivalence>not in ABCD</attributes:abcdEquivalence>
        <attributes:usageScope>simple</attributes:usageScope>
        <rdfs:comment xml:lang="en">Free text numeric description of the absolute or specific chronological age of the physical object.</rdfs:comment>
        <rdfs:label xml:lang="en">Numeric Time</rdfs:label>
        <skos:example xml:lang="en">`20 MYA`,`4th Century`,`1142 C.E.`</skos:example>
    </owl:DatatypeProperty>
    


    <!-- https://www.morphosource.org/terms/morphosource#objectID -->


    <owl:DatatypeProperty rdf:about="https://www.morphosource.org/terms/morphosource#objectID">
        <rdfs:subPropertyOf rdf:resource="https://www.morphosource.org/terms/morphosource#ID"/>
        <rdfs:range rdf:resource="http://www.w3.org/2001/XMLSchema#string"/>
        <rdfs:comment xml:lang="en">MorphoSource-specific unique ID identifier for a Physical Object.</rdfs:comment>
        <rdfs:label xml:lang="en">Physical Object ID</rdfs:label>
    </owl:DatatypeProperty>
    


    <!-- https://www.morphosource.org/terms/morphosource#opticalMagnification -->


    <owl:DatatypeProperty rdf:about="https://www.morphosource.org/terms/morphosource#opticalMagnification">
        <rdfs:domain rdf:resource="https://www.morphosource.org/terms/morphosource#CTImageSeriesImagingEvent"/>
        <rdfs:range rdf:resource="http://www.w3.org/2001/XMLSchema#string"/>
        <rdfs:comment xml:lang="en">Whether optical magnification is used or not. This property is only for indicating optical magnification specifically, and is different from geometric magnification. If present, value must be &quot;Yes&quot; or &quot;No&quot;.</rdfs:comment>
        <rdfs:label xml:lang="en">Optical Magnification</rdfs:label>
        <skos:example xml:lang="en">`Yes`, `No`</skos:example>
    </owl:DatatypeProperty>
    


    <!-- https://www.morphosource.org/terms/morphosource#organizationID -->


    <owl:DatatypeProperty rdf:about="https://www.morphosource.org/terms/morphosource#organizationID">
        <rdfs:subPropertyOf rdf:resource="https://www.morphosource.org/terms/morphosource#ID"/>
        <rdfs:domain rdf:resource="https://www.morphosource.org/terms/morphosource#PhysicalObject"/>
        <rdfs:range rdf:resource="http://www.w3.org/2001/XMLSchema#string"/>
        <rdfs:comment xml:lang="en">MorphoSource-specific unique ID identifier for the provider Organization (museum, institution, or laboratory) responsible for managing the physical object.</rdfs:comment>
        <rdfs:label xml:lang="en">Organization ID</rdfs:label>
    </owl:DatatypeProperty>
    


    <!-- https://www.morphosource.org/terms/morphosource#orientation -->


    <owl:DatatypeProperty rdf:about="https://www.morphosource.org/terms/morphosource#orientation">
        <rdfs:subPropertyOf rdf:resource="http://rs.tdwg.org/ac/terms/subjectOrientation"/>
        <rdfs:domain rdf:resource="https://www.morphosource.org/terms/morphosource#Media"/>
        <rdfs:range rdf:resource="http://www.w3.org/2001/XMLSchema#string"/>
        <terms:isVersionOf rdf:resource="http://rs.tdwg.org/ac/terms/subjectOrientation"/>
        <attributes:repeatable>No</attributes:repeatable>
        <attributes:required>No</attributes:required>
        <rdfs:comment xml:lang="en">Specific orientation (= direction, view angle) of the subject represented in the media resource with respect to the acquisition device, denoted by an IRI.</rdfs:comment>
        <rdfs:label xml:lang="en">Orientation</rdfs:label>
    </owl:DatatypeProperty>
    


    <!-- https://www.morphosource.org/terms/morphosource#originalLocation -->


    <owl:DatatypeProperty rdf:about="https://www.morphosource.org/terms/morphosource#originalLocation">
        <rdfs:domain rdf:resource="https://www.morphosource.org/terms/morphosource#PhysicalObject"/>
        <rdfs:range rdf:resource="http://www.w3.org/2001/XMLSchema#string"/>
        <rdfs:comment xml:lang="en">Free text description of the original location where the physical object was created, produced, fossilized, or otherwise came into being.</rdfs:comment>
        <rdfs:label xml:lang="en">Original Location</rdfs:label>
    </owl:DatatypeProperty>
    


    <!-- https://www.morphosource.org/terms/morphosource#part -->


    <owl:DatatypeProperty rdf:about="https://www.morphosource.org/terms/morphosource#part">
        <rdfs:subPropertyOf rdf:resource="http://rs.tdwg.org/ac/terms/subjectPart"/>
        <rdfs:domain rdf:resource="https://www.morphosource.org/terms/morphosource#Media"/>
        <rdfs:range rdf:resource="http://www.w3.org/2001/XMLSchema#string"/>
        <terms:isVersionOf rdf:resource="http://rs.tdwg.org/ac/terms/subjectPart"/>
        <attributes:repeatable xml:lang="en">Yes</attributes:repeatable>
        <attributes:required>No</attributes:required>
        <rdfs:comment xml:lang="en">The portion or product of organism morphology, behaviour, environment, etc. that is either predominantly shown or particularly well exemplified by the media resource, denoted by an IRI.</rdfs:comment>
        <rdfs:label xml:lang="en">Part</rdfs:label>
    </owl:DatatypeProperty>
    


    <!-- https://www.morphosource.org/terms/morphosource#periodicTime -->


    <owl:DatatypeProperty rdf:about="https://www.morphosource.org/terms/morphosource#periodicTime">
        <rdfs:domain rdf:resource="https://www.morphosource.org/terms/morphosource#PhysicalObject"/>
        <rdfs:range rdf:resource="http://www.w3.org/2001/XMLSchema#string"/>
        <rdfs:comment xml:lang="en">Free text description of the time period associated with the production or creation of the physical object.</rdfs:comment>
        <rdfs:label xml:lang="en">Periodic Time</rdfs:label>
    </owl:DatatypeProperty>
    


    <!-- https://www.morphosource.org/terms/morphosource#phaseContrast -->


    <owl:DatatypeProperty rdf:about="https://www.morphosource.org/terms/morphosource#phaseContrast">
        <rdfs:domain rdf:resource="https://www.morphosource.org/terms/morphosource#CTImageSeriesImagingEvent"/>
        <rdfs:range rdf:resource="http://www.w3.org/2001/XMLSchema#string"/>
        <rdfs:comment xml:lang="en">Whether phase contrast of X-Ray beam - in other words, modulating the beam between higher and lower energies to increase contrast between materials - is used or not. If present, value must be &quot;Yes&quot; or &quot;No&quot;.</rdfs:comment>
        <rdfs:label xml:lang="en">Phase Contrast</rdfs:label>
        <skos:example xml:lang="en">`Yes`, `No`</skos:example>
    </owl:DatatypeProperty>
    


    <!-- https://www.morphosource.org/terms/morphosource#photogrammetryBackgroundRemoval -->


    <owl:DatatypeProperty rdf:about="https://www.morphosource.org/terms/morphosource#photogrammetryBackgroundRemoval">
        <rdfs:domain rdf:resource="https://www.morphosource.org/terms/morphosource#PhotogrammetryImagingEvent"/>
        <rdfs:range rdf:resource="http://www.w3.org/2001/XMLSchema#string"/>
        <rdfs:comment xml:lang="en">Free text description of background removal method.</rdfs:comment>
        <rdfs:label xml:lang="en">Photogrammetry Background Removal</rdfs:label>
    </owl:DatatypeProperty>
    


    <!-- https://www.morphosource.org/terms/morphosource#photographicReference -->


    <owl:DatatypeProperty rdf:about="https://www.morphosource.org/terms/morphosource#photographicReference">
        <rdfs:subPropertyOf rdf:resource="https://www.morphosource.org/terms/morphosource#attachmentFile"/>
        <rdfs:domain rdf:resource="https://www.morphosource.org/terms/morphosource#ImagingEvent"/>
        <rdfs:range rdf:resource="http://www.w3.org/2001/XMLSchema#anyURI"/>
        <rdfs:comment xml:lang="en">A reference photograph image, often used to represent and record the object at the initial time of scanning.</rdfs:comment>
        <rdfs:label xml:lang="en">Photographic Reference</rdfs:label>
    </owl:DatatypeProperty>
    


    <!-- https://www.morphosource.org/terms/morphosource#physicalObjectID -->


    <owl:DatatypeProperty rdf:about="https://www.morphosource.org/terms/morphosource#physicalObjectID">
        <rdfs:subPropertyOf rdf:resource="https://www.morphosource.org/terms/morphosource#objectID"/>
        <rdfs:domain rdf:resource="https://www.morphosource.org/terms/morphosource#ImagingEvent"/>
        <rdfs:domain rdf:resource="https://www.morphosource.org/terms/morphosource#Media"/>
        <terms:isVersionOf rdf:resource="https://www.morphosource.org/terms/morphosource#objectID"/>
        <rdfs:comment xml:lang="en">MorphoSource-specific unique ID identifier for a Physical Object represented by a Media.</rdfs:comment>
        <rdfs:label xml:lang="en">Physical Object ID</rdfs:label>
    </owl:DatatypeProperty>
    


    <!-- https://www.morphosource.org/terms/morphosource#pointCount -->


    <owl:DatatypeProperty rdf:about="https://www.morphosource.org/terms/morphosource#pointCount">
        <rdfs:domain rdf:resource="https://www.morphosource.org/terms/morphosource#FileSet"/>
        <rdfs:range rdf:resource="http://www.w3.org/2001/XMLSchema#int"/>
        <rdfs:comment xml:lang="en">Number of 3D coordinate points comprising a 3D mesh or point cloud.</rdfs:comment>
        <rdfs:label xml:lang="en">Point Count</rdfs:label>
    </owl:DatatypeProperty>
    


    <!-- https://www.morphosource.org/terms/morphosource#postalCode -->


    <owl:DatatypeProperty rdf:about="https://www.morphosource.org/terms/morphosource#postalCode">
        <rdfs:domain rdf:resource="https://www.morphosource.org/terms/morphosource#Organization"/>
        <rdfs:range rdf:resource="http://www.w3.org/2001/XMLSchema#string"/>
        <rdfs:comment xml:lang="en">Group of numbers or letters added to a postal address to assist in sorting of mail, such as a ZIP code in the United States.</rdfs:comment>
        <rdfs:label xml:lang="en">Postal Code</rdfs:label>
        <skos:example xml:lang="en">`27708`</skos:example>
    </owl:DatatypeProperty>
    


    <!-- https://www.morphosource.org/terms/morphosource#power -->


    <owl:DatatypeProperty rdf:about="https://www.morphosource.org/terms/morphosource#power">
        <rdfs:subPropertyOf rdf:resource="http://purl.org/healthcarevocab/v1#GeneratorPower"/>
        <rdfs:domain rdf:resource="https://www.morphosource.org/terms/morphosource#CTImageSeriesImagingEvent"/>
        <rdfs:range rdf:resource="http://www.w3.org/2001/XMLSchema#float"/>
        <terms:isVersionOf rdf:resource="http://purl.org/healthcarevocab/v1#GeneratorPower"/>
        <rdfs:comment xml:lang="en">Power in kW to the X-Ray generator.</rdfs:comment>
        <rdfs:label xml:lang="en">Power</rdfs:label>
    </owl:DatatypeProperty>
    


    <!-- https://www.morphosource.org/terms/morphosource#processingActivityDescription -->


    <owl:DatatypeProperty rdf:about="https://www.morphosource.org/terms/morphosource#processingActivityDescription">
        <rdfs:subPropertyOf rdf:resource="http://purl.org/dc/elements/1.1/description"/>
        <rdfs:domain rdf:resource="https://www.morphosource.org/terms/morphosource#ProcessingEvent"/>
        <rdfs:range rdf:resource="http://www.w3.org/2001/XMLSchema#string"/>
        <rdfs:comment xml:lang="en">Description of a specific discrete processing activity step.</rdfs:comment>
        <rdfs:label xml:lang="en">Processing Activity Description</rdfs:label>
    </owl:DatatypeProperty>
    


    <!-- https://www.morphosource.org/terms/morphosource#processingActivitySoftware -->


    <owl:DatatypeProperty rdf:about="https://www.morphosource.org/terms/morphosource#processingActivitySoftware">
        <rdfs:subPropertyOf rdf:resource="http://purl.org/dc/dcmitype/Software"/>
        <rdfs:domain rdf:resource="https://www.morphosource.org/terms/morphosource#ProcessingEvent"/>
        <rdfs:range rdf:resource="http://www.w3.org/2001/XMLSchema#string"/>
        <rdfs:comment xml:lang="en">Description of software used in a specific discrete processing activity step.</rdfs:comment>
        <rdfs:label xml:lang="en">Processing Activity Software</rdfs:label>
    </owl:DatatypeProperty>
    


    <!-- https://www.morphosource.org/terms/morphosource#projections -->


    <owl:DatatypeProperty rdf:about="https://www.morphosource.org/terms/morphosource#projections">
        <rdfs:subPropertyOf rdf:resource="http://purl.org/healthcarevocab/v1#ImagesInAcquisition"/>
        <rdfs:domain rdf:resource="https://www.morphosource.org/terms/morphosource#CTImageSeriesImagingEvent"/>
        <rdfs:range rdf:resource="http://www.w3.org/2001/XMLSchema#int"/>
        <terms:isVersionOf rdf:resource="http://purl.org/healthcarevocab/v1#ImagesInAcquisition"/>
        <rdfs:comment xml:lang="en">Number of images at distinct angles used to create a 3D image.</rdfs:comment>
        <rdfs:label xml:lang="en">Number of Projections</rdfs:label>
    </owl:DatatypeProperty>
    


    <!-- https://www.morphosource.org/terms/morphosource#provenanceDate -->


    <owl:DatatypeProperty rdf:about="https://www.morphosource.org/terms/morphosource#provenanceDate">
        <rdfs:domain rdf:resource="https://www.morphosource.org/terms/morphosource#PhysicalObject"/>
        <rdfs:range rdf:resource="http://www.w3.org/2001/XMLSchema#date"/>
        <rdfs:comment xml:lang="en">Date the physical object was collected, excavated, or discovered. Values must be in MM/DD/YYYY date format.</rdfs:comment>
        <rdfs:label xml:lang="en">Provenance Date</rdfs:label>
        <skos:example xml:lang="en">`01/01/1985`, `12/30/2021`</skos:example>
    </owl:DatatypeProperty>
    


    <!-- https://www.morphosource.org/terms/morphosource#provenanceDetails -->


    <owl:DatatypeProperty rdf:about="https://www.morphosource.org/terms/morphosource#provenanceDetails">
        <rdfs:subPropertyOf rdf:resource="http://purl.org/dc/terms/provenance"/>
        <rdfs:domain rdf:resource="https://www.morphosource.org/terms/morphosource#PhysicalObject"/>
        <rdfs:range rdf:resource="http://www.w3.org/2001/XMLSchema#string"/>
        <terms:description xml:lang="en">The statement may include a description of any changes successive custodians made to the resource.</terms:description>
        <terms:isVersionOf rdf:resource="http://purl.org/dc/terms/provenance"/>
        <rdfs:comment xml:lang="en">A statement detailing production, discovery, and/or ownership, describing the initial production/discovery context and listing any changes in ownership and custody of the resource since its creation that are significant for its authenticity, integrity, and interpretation.</rdfs:comment>
        <rdfs:label xml:lang="en">Provenance Details</rdfs:label>
    </owl:DatatypeProperty>
    


    <!-- https://www.morphosource.org/terms/morphosource#provenanceLocation -->


    <owl:DatatypeProperty rdf:about="https://www.morphosource.org/terms/morphosource#provenanceLocation">
        <rdfs:domain rdf:resource="https://www.morphosource.org/terms/morphosource#PhysicalObject"/>
        <rdfs:range rdf:resource="http://www.w3.org/2001/XMLSchema#string"/>
        <rdfs:comment xml:lang="en">Free text description of the location from which the physical object was collected, excavated, or discovered.</rdfs:comment>
        <rdfs:label xml:lang="en">Provenance Location</rdfs:label>
    </owl:DatatypeProperty>
    


    <!-- https://www.morphosource.org/terms/morphosource#provenanceName -->


    <owl:DatatypeProperty rdf:about="https://www.morphosource.org/terms/morphosource#provenanceName">
        <rdfs:domain rdf:resource="https://www.morphosource.org/terms/morphosource#PhysicalObject"/>
        <rdfs:range rdf:resource="http://www.w3.org/2001/XMLSchema#string"/>
        <rdfs:comment xml:lang="en">Name of the collection or excavation event, if applicable and available.</rdfs:comment>
        <rdfs:label xml:lang="en">Provenance Name</rdfs:label>
    </owl:DatatypeProperty>
    


    <!-- https://www.morphosource.org/terms/morphosource#recordsetID -->


    <owl:DatatypeProperty rdf:about="https://www.morphosource.org/terms/morphosource#recordsetID">
        <rdfs:domain rdf:resource="https://www.morphosource.org/terms/morphosource#Organization"/>
        <rdfs:range rdf:resource="http://www.w3.org/2001/XMLSchema#string"/>
        <rdfs:comment xml:lang="en">An identifier for an entire museum, institution, or laboratory specimen collection associated with Organization. May be a global unique identifier or an identifier specific to a collection or institution.</rdfs:comment>
        <rdfs:label xml:lang="en">Recordset ID</rdfs:label>
    </owl:DatatypeProperty>
    


    <!-- https://www.morphosource.org/terms/morphosource#relatedURL -->


    <owl:DatatypeProperty rdf:about="https://www.morphosource.org/terms/morphosource#relatedURL">
        <rdfs:subPropertyOf rdf:resource="http://www.w3.org/2000/01/rdf-schema#seeAlso"/>
        <rdfs:domain rdf:resource="https://www.morphosource.org/terms/morphosource#Media"/>
        <rdfs:domain rdf:resource="https://www.morphosource.org/terms/morphosource#Organization"/>
        <rdfs:domain rdf:resource="https://www.morphosource.org/terms/morphosource#PhysicalObject"/>
        <rdfs:range rdf:resource="http://www.w3.org/2001/XMLSchema#anyURI"/>
        <terms:isVersionOf rdf:resource="http://www.w3.org/2000/01/rdf-schema#seeAlso"/>
        <rdfs:comment xml:lang="en">URL for additional resource that might provide additional information about the Media or Physical Object.</rdfs:comment>
        <rdfs:label xml:lang="en">Related URL</rdfs:label>
    </owl:DatatypeProperty>
    


    <!-- https://www.morphosource.org/terms/morphosource#rightsHolder -->


    <owl:DatatypeProperty rdf:about="https://www.morphosource.org/terms/morphosource#rightsHolder">
        <rdfs:subPropertyOf rdf:resource="http://ns.adobe.com/xap/1.0/rights/Owner"/>
        <rdfs:domain rdf:resource="https://www.morphosource.org/terms/morphosource#Media"/>
        <rdfs:domain rdf:resource="https://www.morphosource.org/terms/morphosource#Organization"/>
        <rdfs:range rdf:resource="http://www.w3.org/2001/XMLSchema#string"/>
        <terms:isVersionOf rdf:resource="http://ns.adobe.com/xap/1.0/rights/Owner"/>
        <rdfs:comment xml:lang="en">List of holders of intellectual property rights (copyright or license-based) for the Media.</rdfs:comment>
        <rdfs:label xml:lang="en">Rights Holder</rdfs:label>
    </owl:DatatypeProperty>
    


    <!-- https://www.morphosource.org/terms/morphosource#rightsHolderBlank -->


    <owl:DatatypeProperty rdf:about="https://www.morphosource.org/terms/morphosource#rightsHolderBlank">
        <rdfs:domain rdf:resource="https://www.morphosource.org/terms/morphosource#Organization"/>
        <rdfs:range rdf:resource="http://www.w3.org/2001/XMLSchema#string"/>
        <rdfs:comment xml:lang="en">Whether the Organization&apos;s preferred policy is for Media representing Organization Physical Objects to specify no rights holder in morphosource:rightsHolder. This is distinct from an Organization expressing no preference on rights holder statement. Values must be &quot;Yes&quot; or &quot;No&quot;. If value is &quot;Yes&quot;, then Organization explicitly prefers no rights holder statement.</rdfs:comment>
        <rdfs:label xml:lang="en">Rights Holder Intentionally Left Blank</rdfs:label>
        <skos:example xml:lang="en">`Yes`, `No`</skos:example>
    </owl:DatatypeProperty>
    


    <!-- https://www.morphosource.org/terms/morphosource#rightsStatementBlank -->


    <owl:DatatypeProperty rdf:about="https://www.morphosource.org/terms/morphosource#rightsStatementBlank">
        <rdfs:domain rdf:resource="https://www.morphosource.org/terms/morphosource#Organization"/>
        <rdfs:range rdf:resource="http://www.w3.org/2001/XMLSchema#string"/>
        <rdfs:comment xml:lang="en">Whether the Organization&apos;s preferred policy is for Media representing Organization Physical Objects to specify no rights statement in morphosource:rightsStatement. This is distinct from an Organization expressing no preference on rights statement. Values must be &quot;Yes&quot; or &quot;No&quot;. If value is &quot;Yes&quot;, then Organization explicitly prefers no rights statement.</rdfs:comment>
        <rdfs:label xml:lang="en">Rights Statement Intentionally Left Blank</rdfs:label>
        <skos:example xml:lang="en">`Yes`, `No`</skos:example>
    </owl:DatatypeProperty>
    


    <!-- https://www.morphosource.org/terms/morphosource#rotationNumber -->


    <owl:DatatypeProperty rdf:about="https://www.morphosource.org/terms/morphosource#rotationNumber">
        <rdfs:subPropertyOf rdf:resource="http://purl.org/healthcarevocab/v1#SpiralPitchFactor"/>
        <rdfs:domain rdf:resource="https://www.morphosource.org/terms/morphosource#CTImageSeriesImagingEvent"/>
        <rdfs:range rdf:resource="http://www.w3.org/2001/XMLSchema#float"/>
        <terms:isVersionOf rdf:resource="http://purl.org/healthcarevocab/v1#SpiralPitchFactor"/>
        <rdfs:comment xml:lang="en">Ratio of the Table Feed per Rotation (DICOM 0018,9310) to the Total Collimation Width (DICOM 0018,9307).</rdfs:comment>
        <rdfs:label xml:lang="en">Number of Rotations</rdfs:label>
    </owl:DatatypeProperty>
    


    <!-- https://www.morphosource.org/terms/morphosource#scaleBar -->


    <owl:DatatypeProperty rdf:about="https://www.morphosource.org/terms/morphosource#scaleBar">
        <rdfs:domain rdf:resource="https://www.morphosource.org/terms/morphosource#Media"/>
        <rdfs:range rdf:resource="http://www.w3.org/2001/XMLSchema#string"/>
        <rdfs:comment xml:lang="en">Details of scale bar accompany a photogrammetry image series. Value should include three elements: the scale bar target type, the scale bar distance, and the units of the scale bar distance. If values are encoded as a string, they should be separate by semicolons. This only applies to PhotogrammetryImageSeries Media.</rdfs:comment>
        <rdfs:label xml:lang="en">Scale Bar</rdfs:label>
    </owl:DatatypeProperty>
    


    <!-- https://www.morphosource.org/terms/morphosource#shadingCorrection -->


    <owl:DatatypeProperty rdf:about="https://www.morphosource.org/terms/morphosource#shadingCorrection">
        <rdfs:domain rdf:resource="https://www.morphosource.org/terms/morphosource#CTImageSeriesImagingEvent"/>
        <rdfs:range rdf:resource="http://www.w3.org/2001/XMLSchema#string"/>
        <rdfs:comment xml:lang="en">Whether shading correction calibration is used or not. If present, value must be &quot;Yes&quot; or &quot;No&quot;.</rdfs:comment>
        <rdfs:label xml:lang="en">Shading Correction</rdfs:label>
        <skos:example xml:lang="en">`Yes`, `No`</skos:example>
    </owl:DatatypeProperty>
    


    <!-- https://www.morphosource.org/terms/morphosource#shortDescription -->


    <owl:DatatypeProperty rdf:about="https://www.morphosource.org/terms/morphosource#shortDescription">
        <rdfs:domain rdf:resource="https://www.morphosource.org/terms/morphosource#Media"/>
        <rdfs:range rdf:resource="http://www.w3.org/2001/XMLSchema#string"/>
        <rdfs:comment xml:lang="en">Brief summary description of Media. This could include a brief summary of what is represented in the Media or the context surrounding the Media.</rdfs:comment>
        <rdfs:label xml:lang="en">Short Description</rdfs:label>
    </owl:DatatypeProperty>
    


    <!-- https://www.morphosource.org/terms/morphosource#shortTitle -->


    <owl:DatatypeProperty rdf:about="https://www.morphosource.org/terms/morphosource#shortTitle">
        <rdfs:domain rdf:resource="https://www.morphosource.org/terms/morphosource#CulturalHeritageObject"/>
        <rdfs:range rdf:resource="http://www.w3.org/2001/XMLSchema#string"/>
        <rdfs:comment xml:lang="en">Title or short description of an object. For MorphoSource records, value is used as part of the full title for a Cultural Heritage Object record.</rdfs:comment>
        <rdfs:label xml:lang="en">Short Title</rdfs:label>
    </owl:DatatypeProperty>
    


    <!-- https://www.morphosource.org/terms/morphosource#shutterSpeed -->


    <owl:DatatypeProperty rdf:about="https://www.morphosource.org/terms/morphosource#shutterSpeed">
        <rdfs:subPropertyOf rdf:resource="http://www.w3.org/2003/12/exif/ns#shutterSpeedValue"/>
        <rdfs:domain rdf:resource="https://www.morphosource.org/terms/morphosource#FileSet"/>
        <rdfs:domain rdf:resource="https://www.morphosource.org/terms/morphosource#PhotogrammetryImagingEvent"/>
        <rdfs:domain rdf:resource="https://www.morphosource.org/terms/morphosource#PhotographyImagingEvent"/>
        <rdfs:range rdf:resource="http://www.w3.org/2001/XMLSchema#string"/>
        <rdfs:comment xml:lang="en">Shutter speed. The unit is the APEX (Additive System of Photographic Exposure) setting</rdfs:comment>
        <rdfs:comment xml:lang="ja">シャッター速度（APEX値）。この値の2のベキ乗をとって逆数にすると、通常のシャッター速度表示になる。例えば&apos;4&apos;の場合だと1/(2^4)=1/16秒</rdfs:comment>
        <rdfs:label xml:lang="en">Shutter Speed</rdfs:label>
        <ns:tagNumber xml:lang="en">37377</ns:tagNumber>
    </owl:DatatypeProperty>
    


    <!-- https://www.morphosource.org/terms/morphosource#software -->


    <owl:DatatypeProperty rdf:about="https://www.morphosource.org/terms/morphosource#software">
        <rdfs:domain rdf:resource="https://www.morphosource.org/terms/morphosource#ImagingEvent"/>
        <rdfs:range rdf:resource="http://www.w3.org/2001/XMLSchema#string"/>
        <rdfs:comment xml:lang="en">Free text description of any software used in an Imaging Event.</rdfs:comment>
        <rdfs:label xml:lang="en">Software</rdfs:label>
    </owl:DatatypeProperty>
    


    <!-- https://www.morphosource.org/terms/morphosource#sourceDetectorDistance -->


    <owl:DatatypeProperty rdf:about="https://www.morphosource.org/terms/morphosource#sourceDetectorDistance">
        <rdfs:subPropertyOf rdf:resource="http://purl.org/healthcarevocab/v1#DistanceSourceToDetector"/>
        <rdfs:domain rdf:resource="https://www.morphosource.org/terms/morphosource#CTImageSeriesImagingEvent"/>
        <rdfs:range rdf:resource="http://www.w3.org/2001/XMLSchema#float"/>
        <terms:isVersionOf rdf:resource="http://purl.org/healthcarevocab/v1#DistanceSourceToDetector"/>
        <rdfs:comment xml:lang="en">Distance in mm from X-Ray source to detector center.</rdfs:comment>
        <rdfs:label xml:lang="en">Distance From Source To Detector</rdfs:label>
    </owl:DatatypeProperty>
    


    <!-- https://www.morphosource.org/terms/morphosource#sourceObjectDistance -->


    <owl:DatatypeProperty rdf:about="https://www.morphosource.org/terms/morphosource#sourceObjectDistance">
        <rdfs:subPropertyOf rdf:resource="http://purl.org/healthcarevocab/v1#DistanceSourceToPatient"/>
        <rdfs:domain rdf:resource="https://www.morphosource.org/terms/morphosource#CTImageSeriesImagingEvent"/>
        <rdfs:range rdf:resource="http://www.w3.org/2001/XMLSchema#float"/>
        <terms:isVersionOf rdf:resource="http://purl.org/healthcarevocab/v1#DistanceSourceToPatient"/>
        <rdfs:comment xml:lang="en">Distance in mm from X-Ray source to isocenter (center of field of view).</rdfs:comment>
        <rdfs:label xml:lang="en">Distance From Source To Object</rdfs:label>
    </owl:DatatypeProperty>
    


    <!-- https://www.morphosource.org/terms/morphosource#surroundingMaterial -->


    <owl:DatatypeProperty rdf:about="https://www.morphosource.org/terms/morphosource#surroundingMaterial">
        <rdfs:subPropertyOf rdf:resource="http://purl.org/healthcarevocab/v1#ContainerDescription"/>
        <rdfs:domain rdf:resource="https://www.morphosource.org/terms/morphosource#CTImageSeriesImagingEvent"/>
        <rdfs:range rdf:resource="http://www.w3.org/2001/XMLSchema#string"/>
        <terms:isVersionOf rdf:resource="http://purl.org/healthcarevocab/v1#ContainerDescription"/>
        <rdfs:comment xml:lang="en">Wedge, or the material surrounding and/or enveloping the focal object.</rdfs:comment>
        <rdfs:label xml:lang="en">Surrounding Material</rdfs:label>
    </owl:DatatypeProperty>
    


    <!-- https://www.morphosource.org/terms/morphosource#tag -->


    <owl:DatatypeProperty rdf:about="https://www.morphosource.org/terms/morphosource#tag">
        <rdfs:domain rdf:resource="https://www.morphosource.org/terms/morphosource#Media"/>
        <rdfs:range rdf:resource="http://www.w3.org/2001/XMLSchema#string"/>
        <rdfs:comment xml:lang="en">All-purpose label attached to Media for the purpose of identification, context, or to give other information.</rdfs:comment>
        <rdfs:label xml:lang="en">Tag</rdfs:label>
    </owl:DatatypeProperty>
    


    <!-- https://www.morphosource.org/terms/morphosource#targetMaterial -->


    <owl:DatatypeProperty rdf:about="https://www.morphosource.org/terms/morphosource#targetMaterial">
        <rdfs:subPropertyOf rdf:resource="http://purl.org/healthcarevocab/v1#AnodeTargetMaterial"/>
        <rdfs:domain rdf:resource="https://www.morphosource.org/terms/morphosource#CTImageSeriesImagingEvent"/>
        <rdfs:range rdf:resource="http://www.w3.org/2001/XMLSchema#string"/>
        <terms:isVersionOf rdf:resource="http://purl.org/healthcarevocab/v1#AnodeTargetMaterial"/>
        <rdfs:comment xml:lang="en">The primary material in the anode of the X-Ray source.</rdfs:comment>
        <rdfs:label xml:lang="en">Target Material</rdfs:label>
        <skos:example xml:lang="en">`tungsten`, `molybdenum`, `copper`</skos:example>
    </owl:DatatypeProperty>
    


    <!-- https://www.morphosource.org/terms/morphosource#taxonomyID -->


    <owl:DatatypeProperty rdf:about="https://www.morphosource.org/terms/morphosource#taxonomyID">
        <rdfs:subPropertyOf rdf:resource="https://www.morphosource.org/terms/morphosource#ID"/>
        <rdfs:domain rdf:resource="https://www.morphosource.org/terms/morphosource#BiologicalSpecimenObject"/>
        <rdfs:range rdf:resource="http://www.w3.org/2001/XMLSchema#string"/>
        <rdfs:comment xml:lang="en">Morphosource-specific ID of Taxonomy record for taxonomic name attributed to the Biological Specimen.</rdfs:comment>
        <rdfs:label xml:lang="en">Taxonomy ID</rdfs:label>
    </owl:DatatypeProperty>
    


    <!-- https://www.morphosource.org/terms/morphosource#teamID -->


    <owl:DatatypeProperty rdf:about="https://www.morphosource.org/terms/morphosource#teamID">
        <rdfs:subPropertyOf rdf:resource="https://www.morphosource.org/terms/morphosource#ID"/>
        <rdfs:domain rdf:resource="https://www.morphosource.org/terms/morphosource#Organization"/>
        <rdfs:range rdf:resource="http://www.w3.org/2001/XMLSchema#string"/>
        <rdfs:comment xml:lang="en">MorphoSource-specific unique ID identifier for a Team associated with the Organization and responsible for managing the Organization record.</rdfs:comment>
        <rdfs:label xml:lang="en">Team ID</rdfs:label>
    </owl:DatatypeProperty>
    


    <!-- https://www.morphosource.org/terms/morphosource#vertexColor -->


    <owl:DatatypeProperty rdf:about="https://www.morphosource.org/terms/morphosource#vertexColor">
        <rdfs:domain rdf:resource="https://www.morphosource.org/terms/morphosource#FileSet"/>
        <rdfs:range rdf:resource="http://www.w3.org/2001/XMLSchema#string"/>
        <rdfs:comment xml:lang="en">Whether or not a 3D object has color information encoded into vertices or points that comprise a mesh or point cloud.</rdfs:comment>
        <rdfs:label xml:lang="en">Vertex Color</rdfs:label>
    </owl:DatatypeProperty>
    


    <!-- https://www.morphosource.org/terms/morphosource#voltage -->


    <owl:DatatypeProperty rdf:about="https://www.morphosource.org/terms/morphosource#voltage">
        <rdfs:subPropertyOf rdf:resource="http://purl.org/healthcarevocab/v1#KVP"/>
        <rdfs:domain rdf:resource="https://www.morphosource.org/terms/morphosource#CTImageSeriesImagingEvent"/>
        <rdfs:range rdf:resource="http://www.w3.org/2001/XMLSchema#float"/>
        <terms:isVersionOf rdf:resource="http://purl.org/healthcarevocab/v1#KVP"/>
        <rdfs:comment xml:lang="en">Peak kilo voltage output of the X-Ray generator used.</rdfs:comment>
        <rdfs:label xml:lang="en">Voltage</rdfs:label>
    </owl:DatatypeProperty>
    


    <!-- https://www.morphosource.org/terms/morphosource#vouchered -->


    <owl:DatatypeProperty rdf:about="https://www.morphosource.org/terms/morphosource#vouchered">
        <rdfs:subPropertyOf rdf:resource="http://rs.tdwg.org/dwc/terms/disposition"/>
        <rdfs:domain rdf:resource="https://www.morphosource.org/terms/morphosource#PhysicalObject"/>
        <rdfs:range rdf:resource="http://www.w3.org/2001/XMLSchema#string"/>
        <terms:isVersionOf rdf:resource="http://rs.tdwg.org/dwc/terms/disposition"/>
        <attributes:abcdEquivalence>DataSets/DataSet/Units/Unit/SpecimenUnit/Disposition</attributes:abcdEquivalence>
        <attributes:usageScope>simple</attributes:usageScope>
        <rdfs:comment xml:lang="en">Whether the specimen is vouchered or not, or in other words, whether the physical specimen object exists and is preserved and maintained in an accessible collection. Value must be &quot;Yes&quot; or &quot;No&quot;.</rdfs:comment>
        <rdfs:label xml:lang="en">Vouchered</rdfs:label>
        <skos:example xml:lang="en">`Yes`, `No`</skos:example>
    </owl:DatatypeProperty>
    


    <!-- https://www.morphosource.org/terms/morphosource#width -->


    <owl:DatatypeProperty rdf:about="https://www.morphosource.org/terms/morphosource#width">
        <rdfs:domain rdf:resource="https://www.morphosource.org/terms/morphosource#FileSet"/>
        <rdfs:range rdf:resource="http://www.w3.org/2001/XMLSchema#int"/>
        <rdfs:comment xml:lang="en">Width of a 2D image in pixels.</rdfs:comment>
        <rdfs:label xml:lang="en">Width in Pixels</rdfs:label>
    </owl:DatatypeProperty>
    


    <!-- https://www.morphosource.org/terms/morphosource#xSpacing -->


    <owl:DatatypeProperty rdf:about="https://www.morphosource.org/terms/morphosource#xSpacing">
        <rdfs:subPropertyOf rdf:resource="https://www.morphosource.org/terms/morphosource#dicomPixelSpacingWidth"/>
        <rdfs:domain rdf:resource="https://www.morphosource.org/terms/morphosource#Media"/>
        <rdfs:range rdf:resource="http://www.w3.org/2001/XMLSchema#float"/>
        <rdfs:comment xml:lang="en">Distance between centers of adjacent pixels in the X axis, for Media with pixel data where pixel spacing corresponds to real-world length measurement. Unit of measurement is described by morphosource:unit. Applies to Image and CTImageSeries media.</rdfs:comment>
        <rdfs:label xml:lang="en">X Pixel Spacing</rdfs:label>
    </owl:DatatypeProperty>
    


    <!-- https://www.morphosource.org/terms/morphosource#xrayTubeType -->


    <owl:DatatypeProperty rdf:about="https://www.morphosource.org/terms/morphosource#xrayTubeType">
        <rdfs:subPropertyOf rdf:resource="http://purl.org/healthcarevocab/v1#GeneratorID"/>
        <rdfs:domain rdf:resource="https://www.morphosource.org/terms/morphosource#CTImageSeriesImagingEvent"/>
        <rdfs:range rdf:resource="http://www.w3.org/2001/XMLSchema#string"/>
        <terms:isVersionOf rdf:resource="http://purl.org/healthcarevocab/v1#GeneratorID"/>
        <rdfs:comment xml:lang="en">Free text describing type of X-Ray tube, possibly including brand and/or model of tube.</rdfs:comment>
        <rdfs:label xml:lang="en">X-Ray Tube Type</rdfs:label>
    </owl:DatatypeProperty>
    


    <!-- https://www.morphosource.org/terms/morphosource#ySpacing -->


    <owl:DatatypeProperty rdf:about="https://www.morphosource.org/terms/morphosource#ySpacing">
        <rdfs:subPropertyOf rdf:resource="https://www.morphosource.org/terms/morphosource#dicomPixelSpacingHeight"/>
        <rdfs:domain rdf:resource="https://www.morphosource.org/terms/morphosource#Media"/>
        <rdfs:range rdf:resource="http://www.w3.org/2001/XMLSchema#float"/>
        <rdfs:comment xml:lang="en">Distance between centers of adjacent pixels in the Y axis, for Media with pixel data where pixel spacing corresponds to real-world length measurement. Unit of measurement is described by morphosource:unit. Applies to Image and CTImageSeries media.</rdfs:comment>
        <rdfs:label xml:lang="en">Y Pixel Spacing</rdfs:label>
    </owl:DatatypeProperty>
    


    <!-- https://www.morphosource.org/terms/morphosource#zSpacing -->


    <owl:DatatypeProperty rdf:about="https://www.morphosource.org/terms/morphosource#zSpacing">
        <rdfs:subPropertyOf rdf:resource="https://www.morphosource.org/terms/morphosource#dicomSpacingBetweenSlices"/>
        <rdfs:domain rdf:resource="https://www.morphosource.org/terms/morphosource#Media"/>
        <rdfs:range rdf:resource="http://www.w3.org/2001/XMLSchema#float"/>
        <rdfs:comment xml:lang="en">Distance between centers of adjacent pixels in the Z axis, for Media with 3D pixel data where pixel spacing corresponds to real-world length measurement. Unit of measurement is described by morphosource:unit. Applies to CTImageSeries media.</rdfs:comment>
        <rdfs:label xml:lang="en">Z Pixel Spacing</rdfs:label>
    </owl:DatatypeProperty>
    


    <!-- 
    ///////////////////////////////////////////////////////////////////////////////////////
    //
    // Classes
    //
    ///////////////////////////////////////////////////////////////////////////////////////
     -->


    


    <!-- http://creativecommons.org/ns#License -->


    <owl:Class rdf:about="http://creativecommons.org/ns#License">
        <rdfs:subClassOf rdf:resource="http://purl.org/dc/terms/LicenseDocument"/>
        <rdfs:comment xml:lang="en-us">a set of
		    requests/permissions to users of a Work, e.g. a
		    copyright license, the public domain, information
		    for distributors</rdfs:comment>
        <rdfs:label xml:lang="en-us">License</rdfs:label>
    </owl:Class>
    


    <!-- http://pcdm.org/models#File -->


    <owl:Class rdf:about="http://pcdm.org/models#File">
        <terms:isPartOf xml:lang="en">http://pcdm.org/models#</terms:isPartOf>
        <rdfs:comment xml:lang="en">A File is a sequence of binary data and is described by some accompanying metadata. The metadata typically includes at least basic technical metadata (size, content type, modification date, etc.), but can also include properties related to preservation, digitization process, provenance, etc. Files MUST be contained by exactly one Object.</rdfs:comment>
        <rdfs:isDefinedBy xml:lang="en">http://pcdm.org/models#</rdfs:isDefinedBy>
        <rdfs:label xml:lang="en">File</rdfs:label>
    </owl:Class>
    


    <!-- http://pcdm.org/models#Object -->


    <owl:Class rdf:about="http://pcdm.org/models#Object">
        <terms:isPartOf xml:lang="en">http://pcdm.org/models</terms:isPartOf>
        <rdfs:comment xml:lang="en">An Object is an intellectual entity, sometimes called a &quot;work&quot;, &quot;digital object&quot;, etc. Objects have descriptive metadata, access metadata, may contain files and other Objects as member &quot;components&quot;. Each level of a work is therefore represented by an Object instance, and is capable of standing on its own, being linked to from Collections and other Objects. Member Objects can be ordered using the ORE Proxy class.</rdfs:comment>
        <rdfs:isDefinedBy xml:lang="en">http://pcdm.org/models</rdfs:isDefinedBy>
        <rdfs:label xml:lang="en">Object</rdfs:label>
    </owl:Class>
    


    <!-- http://pcdm.org/works#Work -->


    <owl:Class rdf:about="http://pcdm.org/works#Work">
        <rdfs:subClassOf rdf:resource="http://pcdm.org/models#Object"/>
        <terms:isPartOf xml:lang="en">http://pcdm.org/works</terms:isPartOf>
        <rdfs:comment xml:lang="en">
      A work or intellectual entity, such as a book, film, dissertation, etc.
      Works have member Objects representing their physical structure (e.g., pages in a book),
      FileSets to maintain representations of the entire resource (e.g. a PDF of all the pages),
      and TopRanges representing their logical structure or structures (e.g., sections
      and chapters in a book).
    </rdfs:comment>
        <rdfs:isDefinedBy rdf:resource="http://pcdm.org/works"/>
        <rdfs:label xml:lang="en">Work</rdfs:label>
    </owl:Class>
    


    <!-- http://purl.org/dc/terms/LicenseDocument -->


    <owl:Class rdf:about="http://purl.org/dc/terms/LicenseDocument">
        <rdfs:subClassOf rdf:resource="http://purl.org/dc/terms/RightsStatement"/>
    </owl:Class>
    


    <!-- http://purl.org/dc/terms/RightsStatement -->


    <owl:Class rdf:about="http://purl.org/dc/terms/RightsStatement">
        <terms:issued rdf:datatype="http://www.w3.org/2001/XMLSchema#date">2008-01-14</terms:issued>
        <rdfs:comment xml:lang="en">A statement about the intellectual property rights (IPR) held in or over a resource, a legal document giving official permission to do something with a resource, or a statement about access rights.</rdfs:comment>
        <rdfs:isDefinedBy rdf:resource="http://purl.org/dc/terms/"/>
        <rdfs:label xml:lang="en">Rights Statement</rdfs:label>
    </owl:Class>
    


    <!-- http://vocab.getty.edu/aat/300264087 -->


    <owl:Class rdf:about="http://vocab.getty.edu/aat/300264087"/>
    


    <!-- http://vocab.getty.edu/aat/300264088 -->


    <owl:Class rdf:about="http://vocab.getty.edu/aat/300264088"/>
    


    <!-- http://vocab.getty.edu/aat/300264091 -->


    <owl:Class rdf:about="http://vocab.getty.edu/aat/300264091"/>
    


    <!-- http://vocab.getty.edu/aat/300264092 -->


    <owl:Class rdf:about="http://vocab.getty.edu/aat/300264092"/>
    


    <!-- http://vocab.getty.edu/tgn/7029392 -->


    <owl:Class rdf:about="http://vocab.getty.edu/tgn/7029392"/>
    


    <!-- https://www.morphosource.org/terms/morphosource#AcquisitionType -->


    <owl:Class rdf:about="https://www.morphosource.org/terms/morphosource#AcquisitionType">
        <rdfs:comment xml:lang="en">CT acqusition method type. Entities comprise a controlled vocabulary as defined by DICOM C.8.15.3.2.1 Acquisition Type.</rdfs:comment>
        <rdfs:label xml:lang="en">Acquisition Type</rdfs:label>
    </owl:Class>
    


    <!-- https://www.morphosource.org/terms/morphosource#BiologicalSpecimenObject -->


    <owl:Class rdf:about="https://www.morphosource.org/terms/morphosource#BiologicalSpecimenObject">
        <rdfs:subClassOf rdf:resource="https://www.morphosource.org/terms/morphosource#PhysicalObject"/>
        <rdfs:comment xml:lang="en">A physical object that is a biological specimen, such as a skeleton, a whole body, or a fossil.</rdfs:comment>
        <rdfs:label xml:lang="en">Biological Specimen Object</rdfs:label>
    </owl:Class>
    


    <!-- https://www.morphosource.org/terms/morphosource#CTImageSeriesImagingEvent -->


    <owl:Class rdf:about="https://www.morphosource.org/terms/morphosource#CTImageSeriesImagingEvent">
        <rdfs:subClassOf rdf:resource="https://www.morphosource.org/terms/morphosource#ImagingEvent"/>
        <rdfs:label xml:lang="en">CT Image Series Imaging Event</rdfs:label>
    </owl:Class>
    


    <!-- https://www.morphosource.org/terms/morphosource#CTImageSeriesType -->


    <owl:Class rdf:about="https://www.morphosource.org/terms/morphosource#CTImageSeriesType">
        <rdfs:comment xml:lang="en">Broad type or kind of CT image series, distinguishing between initial X-Ray projections and other derived series forms.</rdfs:comment>
        <rdfs:label xml:lang="en">CT Image Series Type</rdfs:label>
    </owl:Class>
    


    <!-- https://www.morphosource.org/terms/morphosource#CommercialUsePermission -->


    <owl:Class rdf:about="https://www.morphosource.org/terms/morphosource#CommercialUsePermission">
        <rdfs:comment xml:lang="en">Permission statement describing whether a digital resource may be used for commercial purposes.</rdfs:comment>
        <rdfs:label xml:lang="en">Commercial Use Permission</rdfs:label>
    </owl:Class>
    


    <!-- https://www.morphosource.org/terms/morphosource#CulturalHeritageObject -->


    <owl:Class rdf:about="https://www.morphosource.org/terms/morphosource#CulturalHeritageObject">
        <rdfs:subClassOf rdf:resource="https://www.morphosource.org/terms/morphosource#PhysicalObject"/>
        <rdfs:comment xml:lang="en">A physical object that is usually non-biological and is of some human cultural significance.</rdfs:comment>
        <rdfs:label xml:lang="en">Cultural Heritage Object</rdfs:label>
    </owl:Class>
    


    <!-- https://www.morphosource.org/terms/morphosource#DerivativeRearchivalStatement -->


    <owl:Class rdf:about="https://www.morphosource.org/terms/morphosource#DerivativeRearchivalStatement">
        <rdfs:comment xml:lang="en">Statement describing whether and how any future derivatives must or should be rearchived to a public facing digital repository.</rdfs:comment>
        <rdfs:label xml:lang="en">Derivative Rearchival Statement</rdfs:label>
    </owl:Class>
    


    <!-- https://www.morphosource.org/terms/morphosource#Device -->


    <owl:Class rdf:about="https://www.morphosource.org/terms/morphosource#Device">
        <rdfs:subClassOf rdf:resource="http://pcdm.org/works#Work"/>
        <rdfs:comment xml:lang="en">A device used to image a physical object to create media.</rdfs:comment>
        <rdfs:label xml:lang="en">Device</rdfs:label>
    </owl:Class>
    


    <!-- https://www.morphosource.org/terms/morphosource#FileSet -->


    <owl:Class rdf:about="https://www.morphosource.org/terms/morphosource#FileSet">
        <rdfs:subClassOf rdf:resource="http://pcdm.org/works#Work"/>
        <rdfs:comment xml:lang="en">A sequence of binary data accompanied by technical metadata.</rdfs:comment>
        <rdfs:label xml:lang="en">FileSet</rdfs:label>
    </owl:Class>
    


    <!-- https://www.morphosource.org/terms/morphosource#FocalLengthType -->


    <owl:Class rdf:about="https://www.morphosource.org/terms/morphosource#FocalLengthType">
        <rdfs:comment xml:lang="en">Type of camera focal length setting. Elements comprise a controlled vocabulary.</rdfs:comment>
        <rdfs:label xml:lang="en">Focal Length Type</rdfs:label>
    </owl:Class>
    


    <!-- https://www.morphosource.org/terms/morphosource#ImageModalityType -->


    <owl:Class rdf:about="https://www.morphosource.org/terms/morphosource#ImageModalityType">
        <rdfs:comment xml:lang="en">Modality used to create 3D, 2D, or AV images. The individual entities of this class in the MorphoSource data vocabulary comprise a controlled vocabulary of specific image modalities used to describe imaging of media in MorphoSource.</rdfs:comment>
        <rdfs:label xml:lang="en">Image Modality Type</rdfs:label>
    </owl:Class>
    


    <!-- https://www.morphosource.org/terms/morphosource#ImagingEvent -->


    <owl:Class rdf:about="https://www.morphosource.org/terms/morphosource#ImagingEvent">
        <rdfs:subClassOf rdf:resource="http://pcdm.org/works#Work"/>
        <rdfs:comment xml:lang="en">An active event in which a physical object is imaging to produce media.</rdfs:comment>
        <rdfs:label xml:lang="en">Imaging Event</rdfs:label>
    </owl:Class>
    


    <!-- https://www.morphosource.org/terms/morphosource#LengthMeasurementUnit -->


    <owl:Class rdf:about="https://www.morphosource.org/terms/morphosource#LengthMeasurementUnit">
        <rdfs:comment xml:lang="en">Unit of measurement used in measuring length.</rdfs:comment>
        <rdfs:label xml:lang="en">Length Measurement Unit</rdfs:label>
    </owl:Class>
    


    <!-- https://www.morphosource.org/terms/morphosource#LightSourceType -->


    <owl:Class rdf:about="https://www.morphosource.org/terms/morphosource#LightSourceType">
        <rdfs:comment xml:lang="en">Type of light source. Elements comprise a controlled vocabulary.</rdfs:comment>
        <rdfs:label xml:lang="en">Light Source Type</rdfs:label>
    </owl:Class>
    


    <!-- https://www.morphosource.org/terms/morphosource#Media -->


    <owl:Class rdf:about="https://www.morphosource.org/terms/morphosource#Media">
        <rdfs:subClassOf rdf:resource="http://pcdm.org/works#Work"/>
        <rdfs:comment xml:lang="en">3D, 2D, or AV media representing a physical object.</rdfs:comment>
        <rdfs:label xml:lang="en">Media</rdfs:label>
    </owl:Class>
    


    <!-- https://www.morphosource.org/terms/morphosource#MediaType -->


    <owl:Class rdf:about="https://www.morphosource.org/terms/morphosource#MediaType">
        <rdfs:comment xml:lang="en">Type, nature, or classification of a Media file dataset, which may include one or more specific files. This is the general or high-level type of all file data, it is not the file type of any specific file. Most Media Types encompass a variety of different specific file types.</rdfs:comment>
        <rdfs:label xml:lang="en">Media Type</rdfs:label>
    </owl:Class>
    


    <!-- https://www.morphosource.org/terms/morphosource#MeshMapType -->


    <owl:Class rdf:about="https://www.morphosource.org/terms/morphosource#MeshMapType">
        <rdfs:comment xml:lang="en">A type of 3D texture map or projection that associates two-dimensional space coordinates to the surface of a 3D object, usually in order to map a texture or other attribute onto the 3D object&apos;s surface.</rdfs:comment>
        <rdfs:label xml:lang="en">Mesh Map Type</rdfs:label>
    </owl:Class>
    


    <!-- https://www.morphosource.org/terms/morphosource#Organization -->


    <owl:Class rdf:about="https://www.morphosource.org/terms/morphosource#Organization">
        <rdfs:subClassOf rdf:resource="http://pcdm.org/works#Work"/>
        <rdfs:comment xml:lang="en">A relatively autonomous bureaucratic unit responsible for controlling physical objects or devices. Often a museum collection, an entire museum institution, or a faculty lab department.</rdfs:comment>
        <rdfs:label xml:lang="en">Organization</rdfs:label>
    </owl:Class>
    


    <!-- https://www.morphosource.org/terms/morphosource#OrganizationType -->


    <owl:Class rdf:about="https://www.morphosource.org/terms/morphosource#OrganizationType">
        <rdfs:comment xml:lang="en">Type of Organization, distinguishing between collections managing Physical Objects, scanning facilities, and entities that both operate scanning equipment and manage Physical Objects.</rdfs:comment>
        <rdfs:label xml:lang="en">Organization Type</rdfs:label>
    </owl:Class>
    


    <!-- https://www.morphosource.org/terms/morphosource#PhotogrammetryImagingEvent -->


    <owl:Class rdf:about="https://www.morphosource.org/terms/morphosource#PhotogrammetryImagingEvent">
        <rdfs:subClassOf rdf:resource="https://www.morphosource.org/terms/morphosource#ImagingEvent"/>
        <rdfs:label xml:lang="en">Photogrammetry Imaging Event</rdfs:label>
    </owl:Class>
    


    <!-- https://www.morphosource.org/terms/morphosource#PhotographyImagingEvent -->


    <owl:Class rdf:about="https://www.morphosource.org/terms/morphosource#PhotographyImagingEvent">
        <rdfs:subClassOf rdf:resource="https://www.morphosource.org/terms/morphosource#ImagingEvent"/>
        <rdfs:label xml:lang="en">Photography Imaging Event</rdfs:label>
    </owl:Class>
    


    <!-- https://www.morphosource.org/terms/morphosource#PhysicalObject -->


    <owl:Class rdf:about="https://www.morphosource.org/terms/morphosource#PhysicalObject">
        <rdfs:subClassOf rdf:resource="http://pcdm.org/works#Work"/>
        <rdfs:comment xml:lang="en">A physical object, usually of scholarly interest, that is imaged to create media.</rdfs:comment>
        <rdfs:label xml:lang="en">Physical Object</rdfs:label>
    </owl:Class>
    


    <!-- https://www.morphosource.org/terms/morphosource#PixelSpacingCalibrationType -->


    <owl:Class rdf:about="https://www.morphosource.org/terms/morphosource#PixelSpacingCalibrationType">
        <rdfs:comment xml:lang="en">A type of correction for the effect of geometric magnification or calibration against an object of known size, as described in the Enumerated Values of the DICOM Pixel Spacing Calibration Type attribute (0028,0A02). The individual entities of this class in the MorphoSource data vocabulary comprise a controlled vocabulary used to describe the pixel calibration type for relevant Image Events.</rdfs:comment>
        <rdfs:label xml:lang="en">Pixel Spacing Calibration Type</rdfs:label>
    </owl:Class>
    


    <!-- https://www.morphosource.org/terms/morphosource#ProcessingActivityType -->


    <owl:Class rdf:about="https://www.morphosource.org/terms/morphosource#ProcessingActivityType">
        <rdfs:comment xml:lang="en">Type statement describing a specific discrete processing activity step. It is often the case that in reality, multiple processing activity steps are used in the generation of any derived digital resource.</rdfs:comment>
        <rdfs:label xml:lang="en">Processing Activity Type</rdfs:label>
    </owl:Class>
    


    <!-- https://www.morphosource.org/terms/morphosource#ProcessingEvent -->


    <owl:Class rdf:about="https://www.morphosource.org/terms/morphosource#ProcessingEvent">
        <rdfs:subClassOf rdf:resource="http://pcdm.org/works#Work"/>
        <rdfs:comment xml:lang="en">An active event in which a media is processed to produce another media. Belongs to Imaging Event or Media as a member (as either of these can lead to a processing event), and has member Media (as the processing event leads to the production of Media).</rdfs:comment>
        <rdfs:label xml:lang="en">Processing Event</rdfs:label>
    </owl:Class>
    


    <!-- https://www.morphosource.org/terms/morphosource#PublicationStatus -->


    <owl:Class rdf:about="https://www.morphosource.org/terms/morphosource#PublicationStatus">
        <rdfs:comment xml:lang="en">Status type indicating whether or not Media is published and under what conditions it is published.</rdfs:comment>
        <rdfs:label xml:lang="en">Publication Status</rdfs:label>
    </owl:Class>
    


    <!-- https://www.morphosource.org/terms/morphosource#SequentialSectionImagingEvent -->


    <owl:Class rdf:about="https://www.morphosource.org/terms/morphosource#SequentialSectionImagingEvent">
        <rdfs:subClassOf rdf:resource="https://www.morphosource.org/terms/morphosource#ImagingEvent"/>
        <rdfs:label xml:lang="en">Sequential Section Imaging Event</rdfs:label>
    </owl:Class>
    


    <!-- https://www.morphosource.org/terms/morphosource#Sex -->


    <owl:Class rdf:about="https://www.morphosource.org/terms/morphosource#Sex">
        <rdfs:comment xml:lang="en">A categorical description or identification pertaining an organism&apos;s sex. The individual entities of this class in the MorphoSource data vocabulary comprise a controlled vocabulary of specific sex categorizations and identification statements used to describe Biological Specimens.</rdfs:comment>
        <rdfs:label xml:lang="en">Sex</rdfs:label>
    </owl:Class>
    


    <!-- https://www.morphosource.org/terms/morphosource#Side -->


    <owl:Class rdf:about="https://www.morphosource.org/terms/morphosource#Side">
        <rdfs:comment xml:lang="en">For objects with bilateral or some other kind of symmetry, a term description statement pertaining to a particular side, the object midline, lack of knowledge relating to side, or inapplicability of this concept for an object.</rdfs:comment>
        <rdfs:label xml:lang="en">Side</rdfs:label>
    </owl:Class>
    


    <!-- https://www.morphosource.org/terms/morphosource#SlideType -->


    <owl:Class rdf:about="https://www.morphosource.org/terms/morphosource#SlideType">
        <rdfs:label xml:lang="en">Type of Sequential Section Slide. Entities comprise a controlled vocabulary.</rdfs:label>
    </owl:Class>
    


    <!-- https://www.morphosource.org/terms/morphosource#UseAgreementType -->


    <owl:Class rdf:about="https://www.morphosource.org/terms/morphosource#UseAgreementType">
        <rdfs:comment xml:lang="en">Type of MorphoSource-specific Media download use agreement. This explicitly does not include types of non-MorphoSource use agreements, such as use agreements provided by third-party museums.</rdfs:comment>
        <rdfs:label xml:lang="en">Use Agreement Type</rdfs:label>
    </owl:Class>
    


    <!-- https://www.morphosource.org/terms/morphosource#User -->


    <owl:Class rdf:about="https://www.morphosource.org/terms/morphosource#User">
        <rdfs:label xml:lang="en">User</rdfs:label>
    </owl:Class>
    


    <!-- https://www.morphosource.org/terms/morphosource#XRayDetectorConfiguration -->


    <owl:Class rdf:about="https://www.morphosource.org/terms/morphosource#XRayDetectorConfiguration">
        <rdfs:comment xml:lang="en">Physical configuration of X-Ray detector used to acquire an image for CT, MRI, and other related modalities, as described in the DICOM Dectector Configuration attribute (0018,7005). The individual entities of this class in the MorphoSource data vocabulary comprise a controlled vocabulary used to describe detector configuration for relevant Image Events.</rdfs:comment>
        <rdfs:label xml:lang="en">X-Ray Detector Configuration</rdfs:label>
    </owl:Class>
    


    <!-- https://www.morphosource.org/terms/morphosource#XRayDetectorType -->


    <owl:Class rdf:about="https://www.morphosource.org/terms/morphosource#XRayDetectorType">
        <rdfs:comment xml:lang="en">Type of X-Ray detector used to acquire an image for CT, MRI, and other related modalities, as described in the DICOM Dectector Type attribute (0018,7004). The individual entities of this class in the MorphoSource data vocabulary comprise a controlled vocabulary used to describe detector type for relevant Image Events.</rdfs:comment>
        <rdfs:label xml:lang="en">X-Ray Detector Type</rdfs:label>
    </owl:Class>
    


    <!-- https://www.morphosource.org/terms/morphosource#XRayTargetType -->


    <owl:Class rdf:about="https://www.morphosource.org/terms/morphosource#XRayTargetType">
        <rdfs:comment xml:lang="en">Type of X-Ray target used to acquire an image for CT, MRI, and other related modalities. The individual entities of this class in the MorphoSource data vocabulary comprise a controlled vocabulary used to describe target type for relevant Image Events.</rdfs:comment>
        <rdfs:label xml:lang="en">X-Ray Target Type</rdfs:label>
    </owl:Class>
    


    <!-- https://www.morphosource.org/terms/morphosource#3DPrintingPermission -->


    <owl:Class rdf:about="https://www.morphosource.org/terms/morphosource#3DPrintingPermission">
        <rdfs:comment xml:lang="en">Permission statement describing whether 3D printing of a digital resource is permitted, prohibited, or permitted with conditions.</rdfs:comment>
        <rdfs:label xml:lang="en">3D Printing Permission</rdfs:label>
    </owl:Class>
    


    <!-- 
    ///////////////////////////////////////////////////////////////////////////////////////
    //
    // Individuals
    //
    ///////////////////////////////////////////////////////////////////////////////////////
     -->


    


    <!-- http://purl.org/dc/terms/TGN -->


    <owl:NamedIndividual rdf:about="http://purl.org/dc/terms/TGN"/>
    


    <!-- http://www.getty.edu/research/tools/vocabulary/tgn/index.html -->


    <owl:NamedIndividual rdf:about="http://www.getty.edu/research/tools/vocabulary/tgn/index.html"/>
    


    <!-- https://www.morphosource.org/terms/morphosource#AlignParts -->


    <owl:NamedIndividual rdf:about="https://www.morphosource.org/terms/morphosource#AlignParts">
        <rdf:type rdf:resource="https://www.morphosource.org/terms/morphosource#ProcessingActivityType"/>
        <rdfs:label xml:lang="en">Align Parts</rdfs:label>
    </owl:NamedIndividual>
    


    <!-- https://www.morphosource.org/terms/morphosource#Area -->


    <owl:NamedIndividual rdf:about="https://www.morphosource.org/terms/morphosource#Area">
        <rdf:type rdf:resource="https://www.morphosource.org/terms/morphosource#XRayDetectorConfiguration"/>
        <rdfs:label xml:lang="en">Area (single or tiled detector)</rdfs:label>
    </owl:NamedIndividual>
    


    <!-- https://www.morphosource.org/terms/morphosource#BackgroundRemovalMasking -->


    <owl:NamedIndividual rdf:about="https://www.morphosource.org/terms/morphosource#BackgroundRemovalMasking">
        <rdf:type rdf:resource="https://www.morphosource.org/terms/morphosource#ProcessingActivityType"/>
        <rdfs:label xml:lang="en">Background Removal and/or Masking</rdfs:label>
    </owl:NamedIndividual>
    


    <!-- https://www.morphosource.org/terms/morphosource#BitDepthChange -->


    <owl:NamedIndividual rdf:about="https://www.morphosource.org/terms/morphosource#BitDepthChange">
        <rdf:type rdf:resource="https://www.morphosource.org/terms/morphosource#ProcessingActivityType"/>
        <rdfs:label xml:lang="en">Bit Depth Change</rdfs:label>
    </owl:NamedIndividual>
    


    <!-- https://www.morphosource.org/terms/morphosource#BornDigital -->


    <owl:NamedIndividual rdf:about="https://www.morphosource.org/terms/morphosource#BornDigital">
        <rdf:type rdf:resource="https://www.morphosource.org/terms/morphosource#ImageModalityType"/>
        <rdfs:comment xml:lang="en">Born Digital refers to digital content that is created and stored in digital format from the outset. Born-digital content includes digital photos, videos, documents, and other types of digital media.</rdfs:comment>
        <rdfs:label xml:lang="en">Born Digital</rdfs:label>
        <skos:altLabel xml:lang="en">BD</skos:altLabel>
    </owl:NamedIndividual>
    


    <!-- https://www.morphosource.org/terms/morphosource#CTImageSeries -->


    <owl:NamedIndividual rdf:about="https://www.morphosource.org/terms/morphosource#CTImageSeries">
        <rdf:type rdf:resource="https://www.morphosource.org/terms/morphosource#MediaType"/>
        <rdfs:label xml:lang="en">CT/MRI image series (multiple files of type *.tiff, *.png, *.dcm, *.zip, etc.)</rdfs:label>
    </owl:NamedIndividual>
    


    <!-- https://www.morphosource.org/terms/morphosource#Cm -->


    <owl:NamedIndividual rdf:about="https://www.morphosource.org/terms/morphosource#Cm">
        <rdf:type rdf:resource="https://www.morphosource.org/terms/morphosource#LengthMeasurementUnit"/>
        <rdfs:label xml:lang="en">Centimeters</rdfs:label>
    </owl:NamedIndividual>
    


    <!-- https://www.morphosource.org/terms/morphosource#CollectionAndScanningFacility -->


    <owl:NamedIndividual rdf:about="https://www.morphosource.org/terms/morphosource#CollectionAndScanningFacility">
        <rdf:type rdf:resource="https://www.morphosource.org/terms/morphosource#OrganizationType"/>
        <rdfs:label xml:lang="en">Collection and Scanning Facility</rdfs:label>
    </owl:NamedIndividual>
    


    <!-- https://www.morphosource.org/terms/morphosource#Color -->


    <owl:NamedIndividual rdf:about="https://www.morphosource.org/terms/morphosource#Color">
        <rdf:type rdf:resource="https://www.morphosource.org/terms/morphosource#MeshMapType"/>
        <rdfs:label xml:lang="en">Color Map</rdfs:label>
    </owl:NamedIndividual>
    


    <!-- https://www.morphosource.org/terms/morphosource#CommercialUseNotPermitted -->


    <owl:NamedIndividual rdf:about="https://www.morphosource.org/terms/morphosource#CommercialUseNotPermitted">
        <rdf:type rdf:resource="https://www.morphosource.org/terms/morphosource#CommercialUsePermission"/>
        <rdfs:comment xml:lang="en">Commercial use of digital resource is not permitted.</rdfs:comment>
        <rdfs:label xml:lang="en">Commercial Use Not Permitted</rdfs:label>
    </owl:NamedIndividual>
    


    <!-- https://www.morphosource.org/terms/morphosource#CommercialUsePermitted -->


    <owl:NamedIndividual rdf:about="https://www.morphosource.org/terms/morphosource#CommercialUsePermitted">
        <rdf:type rdf:resource="https://www.morphosource.org/terms/morphosource#CommercialUsePermission"/>
        <rdfs:comment xml:lang="en">Commercial use of digital resource is permitted.</rdfs:comment>
        <rdfs:label xml:lang="en">Commercial Use Permitted</rdfs:label>
    </owl:NamedIndividual>
    


    <!-- https://www.morphosource.org/terms/morphosource#ConfocalImageStacking -->


    <owl:NamedIndividual rdf:about="https://www.morphosource.org/terms/morphosource#ConfocalImageStacking">
        <rdf:type rdf:resource="https://www.morphosource.org/terms/morphosource#ImageModalityType"/>
        <rdfs:comment xml:lang="en">Confocal Image Stacking is an imaging technique that uses a series of images taken at different depths to create a 3D image of an object. By focusing a laser beam on a specific point in the object and measuring the reflected light, confocal microscopy can create high-resolution 3D images of cells and tissues.</rdfs:comment>
        <rdfs:label xml:lang="en">Confocal Image Stacking</rdfs:label>
        <skos:altLabel xml:lang="en">Confocal</skos:altLabel>
    </owl:NamedIndividual>
    


    <!-- https://www.morphosource.org/terms/morphosource#ConstantAngle -->


    <owl:NamedIndividual rdf:about="https://www.morphosource.org/terms/morphosource#ConstantAngle">
        <rdf:type rdf:resource="https://www.morphosource.org/terms/morphosource#AcquisitionType"/>
        <rdfs:label xml:lang="en">Constant Angle</rdfs:label>
    </owl:NamedIndividual>
    


    <!-- https://www.morphosource.org/terms/morphosource#Crop -->


    <owl:NamedIndividual rdf:about="https://www.morphosource.org/terms/morphosource#Crop">
        <rdf:type rdf:resource="https://www.morphosource.org/terms/morphosource#ProcessingActivityType"/>
        <rdfs:label xml:lang="en">Crop</rdfs:label>
    </owl:NamedIndividual>
    


    <!-- https://www.morphosource.org/terms/morphosource#CrossPolarized -->


    <owl:NamedIndividual rdf:about="https://www.morphosource.org/terms/morphosource#CrossPolarized">
        <rdf:type rdf:resource="https://www.morphosource.org/terms/morphosource#LightSourceType"/>
        <rdfs:label xml:lang="en">Cross polarized</rdfs:label>
    </owl:NamedIndividual>
    


    <!-- https://www.morphosource.org/terms/morphosource#Direct -->


    <owl:NamedIndividual rdf:about="https://www.morphosource.org/terms/morphosource#Direct">
        <rdf:type rdf:resource="https://www.morphosource.org/terms/morphosource#XRayDetectorType"/>
        <rdfs:label xml:lang="en">Direct (X-Ray photoconductor)</rdfs:label>
    </owl:NamedIndividual>
    


    <!-- https://www.morphosource.org/terms/morphosource#EncouragedButNotRequired -->


    <owl:NamedIndividual rdf:about="https://www.morphosource.org/terms/morphosource#EncouragedButNotRequired">
        <rdf:type rdf:resource="https://www.morphosource.org/terms/morphosource#DerivativeRearchivalStatement"/>
        <rdfs:comment xml:lang="en">Future derivatives are encouraged to be rearchived on a public-facing digital repository, but are not required to be rearchived.</rdfs:comment>
        <rdfs:label xml:lang="en">Encouraged But Not Required</rdfs:label>
    </owl:NamedIndividual>
    


    <!-- https://www.morphosource.org/terms/morphosource#Female -->


    <owl:NamedIndividual rdf:about="https://www.morphosource.org/terms/morphosource#Female">
        <rdf:type rdf:resource="https://www.morphosource.org/terms/morphosource#Sex"/>
        <rdfs:label xml:lang="en">Female</rdfs:label>
    </owl:NamedIndividual>
    


    <!-- https://www.morphosource.org/terms/morphosource#Fiducial -->


    <owl:NamedIndividual rdf:about="https://www.morphosource.org/terms/morphosource#Fiducial">
        <rdf:type rdf:resource="https://www.morphosource.org/terms/morphosource#PixelSpacingCalibrationType"/>
        <rdfs:label xml:lang="en">Fiducial</rdfs:label>
    </owl:NamedIndividual>
    


    <!-- https://www.morphosource.org/terms/morphosource#Film -->


    <owl:NamedIndividual rdf:about="https://www.morphosource.org/terms/morphosource#Film">
        <rdf:type rdf:resource="https://www.morphosource.org/terms/morphosource#XRayDetectorType"/>
        <rdfs:label xml:lang="en">Film (Scanned film/screen)</rdfs:label>
    </owl:NamedIndividual>
    


    <!-- https://www.morphosource.org/terms/morphosource#Fixed -->


    <owl:NamedIndividual rdf:about="https://www.morphosource.org/terms/morphosource#Fixed">
        <rdf:type rdf:resource="https://www.morphosource.org/terms/morphosource#FocalLengthType"/>
        <rdfs:label xml:lang="en">Fixed</rdfs:label>
    </owl:NamedIndividual>
    


    <!-- https://www.morphosource.org/terms/morphosource#Free -->


    <owl:NamedIndividual rdf:about="https://www.morphosource.org/terms/morphosource#Free">
        <rdf:type rdf:resource="https://www.morphosource.org/terms/morphosource#AcquisitionType"/>
        <rdfs:label xml:lang="en">Free</rdfs:label>
    </owl:NamedIndividual>
    


    <!-- https://www.morphosource.org/terms/morphosource#Ft -->


    <owl:NamedIndividual rdf:about="https://www.morphosource.org/terms/morphosource#Ft">
        <rdf:type rdf:resource="https://www.morphosource.org/terms/morphosource#LengthMeasurementUnit"/>
        <rdfs:label xml:lang="en">Feet</rdfs:label>
    </owl:NamedIndividual>
    


    <!-- https://www.morphosource.org/terms/morphosource#Geometry -->


    <owl:NamedIndividual rdf:about="https://www.morphosource.org/terms/morphosource#Geometry">
        <rdf:type rdf:resource="https://www.morphosource.org/terms/morphosource#PixelSpacingCalibrationType"/>
        <rdfs:label xml:lang="en">Geometry</rdfs:label>
    </owl:NamedIndividual>
    


    <!-- https://www.morphosource.org/terms/morphosource#Gynandromorph -->


    <owl:NamedIndividual rdf:about="https://www.morphosource.org/terms/morphosource#Gynandromorph">
        <rdf:type rdf:resource="https://www.morphosource.org/terms/morphosource#Sex"/>
        <rdfs:label xml:lang="en">Gynandromorph</rdfs:label>
    </owl:NamedIndividual>
    


    <!-- https://www.morphosource.org/terms/morphosource#Hermaphrodite -->


    <owl:NamedIndividual rdf:about="https://www.morphosource.org/terms/morphosource#Hermaphrodite">
        <rdf:type rdf:resource="https://www.morphosource.org/terms/morphosource#Sex"/>
        <rdfs:label xml:lang="en">Hermaphrodite</rdfs:label>
    </owl:NamedIndividual>
    


    <!-- https://www.morphosource.org/terms/morphosource#HistogramEditing -->


    <owl:NamedIndividual rdf:about="https://www.morphosource.org/terms/morphosource#HistogramEditing">
        <rdf:type rdf:resource="https://www.morphosource.org/terms/morphosource#ProcessingActivityType"/>
        <rdfs:label xml:lang="en">Histogram Editing</rdfs:label>
    </owl:NamedIndividual>
    


    <!-- https://www.morphosource.org/terms/morphosource#HistologicalSlide -->


    <owl:NamedIndividual rdf:about="https://www.morphosource.org/terms/morphosource#HistologicalSlide">
        <rdf:type rdf:resource="https://www.morphosource.org/terms/morphosource#SlideType"/>
        <rdfs:label xml:lang="en">Histological Slide</rdfs:label>
    </owl:NamedIndividual>
    


    <!-- https://www.morphosource.org/terms/morphosource#Image -->


    <owl:NamedIndividual rdf:about="https://www.morphosource.org/terms/morphosource#Image">
        <rdf:type rdf:resource="https://www.morphosource.org/terms/morphosource#MediaType"/>
        <rdfs:label xml:lang="en">Image (*.tiff, *.png, *.dcm, etc.)</rdfs:label>
    </owl:NamedIndividual>
    


    <!-- https://www.morphosource.org/terms/morphosource#ImageMeshCompression -->


    <owl:NamedIndividual rdf:about="https://www.morphosource.org/terms/morphosource#ImageMeshCompression">
        <rdf:type rdf:resource="https://www.morphosource.org/terms/morphosource#ProcessingActivityType"/>
        <rdfs:label xml:lang="en">Image and/or Mesh Compression</rdfs:label>
    </owl:NamedIndividual>
    


    <!-- https://www.morphosource.org/terms/morphosource#In -->


    <owl:NamedIndividual rdf:about="https://www.morphosource.org/terms/morphosource#In">
        <rdf:type rdf:resource="https://www.morphosource.org/terms/morphosource#LengthMeasurementUnit"/>
        <rdfs:label xml:lang="en">Inches</rdfs:label>
    </owl:NamedIndividual>
    


    <!-- https://www.morphosource.org/terms/morphosource#Infrared -->


    <owl:NamedIndividual rdf:about="https://www.morphosource.org/terms/morphosource#Infrared">
        <rdf:type rdf:resource="https://www.morphosource.org/terms/morphosource#ImageModalityType"/>
        <rdfs:comment xml:lang="en">Infrared imaging is an imaging technique that uses infrared radiation to create images of objects. Infrared imaging can be used to detect and analyze heat signatures, as well as to create detailed images of objects and structures that are difficult to see with visible light.</rdfs:comment>
        <rdfs:label xml:lang="en">Infrared</rdfs:label>
        <skos:altLabel xml:lang="en">Infrared</skos:altLabel>
    </owl:NamedIndividual>
    


    <!-- https://www.morphosource.org/terms/morphosource#Km -->


    <owl:NamedIndividual rdf:about="https://www.morphosource.org/terms/morphosource#Km">
        <rdf:type rdf:resource="https://www.morphosource.org/terms/morphosource#LengthMeasurementUnit"/>
        <rdfs:label xml:lang="en">Kilometers</rdfs:label>
    </owl:NamedIndividual>
    


    <!-- https://www.morphosource.org/terms/morphosource#LaserAidedProfiling -->


    <owl:NamedIndividual rdf:about="https://www.morphosource.org/terms/morphosource#LaserAidedProfiling">
        <rdf:type rdf:resource="https://www.morphosource.org/terms/morphosource#ImageModalityType"/>
        <rdfs:comment xml:lang="en">Laser Aided Profiling (LAP) is an imaging technique that uses a laser beam to create a 3D image of an object&apos;s surface. LAP can be used to create high-resolution, accurate models of complex shapes and structures, making it useful in manufacturing and other industries.</rdfs:comment>
        <rdfs:label xml:lang="en">Laser Aided Profiling</rdfs:label>
        <skos:altLabel xml:lang="en">LAP</skos:altLabel>
    </owl:NamedIndividual>
    


    <!-- https://www.morphosource.org/terms/morphosource#LaserScan -->


    <owl:NamedIndividual rdf:about="https://www.morphosource.org/terms/morphosource#LaserScan">
        <rdf:type rdf:resource="https://www.morphosource.org/terms/morphosource#ImageModalityType"/>
        <rdfs:comment xml:lang="en">Laser Scan is an imaging technique that uses laser beams to create a 3D image of an object&apos;s surface. Laser scans are commonly used in industrial design and manufacturing to create accurate models of parts and components.</rdfs:comment>
        <rdfs:label xml:lang="en">Laser Scan</rdfs:label>
        <skos:altLabel xml:lang="en">Laser</skos:altLabel>
    </owl:NamedIndividual>
    


    <!-- https://www.morphosource.org/terms/morphosource#Left -->


    <owl:NamedIndividual rdf:about="https://www.morphosource.org/terms/morphosource#Left">
        <rdf:type rdf:resource="https://www.morphosource.org/terms/morphosource#Side"/>
        <rdfs:label xml:lang="en">Left</rdfs:label>
    </owl:NamedIndividual>
    


    <!-- https://www.morphosource.org/terms/morphosource#M -->


    <owl:NamedIndividual rdf:about="https://www.morphosource.org/terms/morphosource#M">
        <rdf:type rdf:resource="https://www.morphosource.org/terms/morphosource#LengthMeasurementUnit"/>
        <rdfs:label xml:lang="en">Meters</rdfs:label>
    </owl:NamedIndividual>
    


    <!-- https://www.morphosource.org/terms/morphosource#MagneticResonanceImaging -->


    <owl:NamedIndividual rdf:about="https://www.morphosource.org/terms/morphosource#MagneticResonanceImaging">
        <rdf:type rdf:resource="https://www.morphosource.org/terms/morphosource#ImageModalityType"/>
        <rdfs:comment xml:lang="en">Magnetic Resonance Imaging (MRI) is a non-invasive imaging technique that uses a strong magnetic field and radio waves to produce detailed images of the body&apos;s internal structures. MRI is widely used in medical diagnosis and research, especially for imaging soft tissues like the brain, spinal cord, and organs.</rdfs:comment>
        <rdfs:label xml:lang="en">Magnetic Resonance Imaging (MRI)</rdfs:label>
        <skos:altLabel xml:lang="en">MRI</skos:altLabel>
    </owl:NamedIndividual>
    


    <!-- https://www.morphosource.org/terms/morphosource#Male -->


    <owl:NamedIndividual rdf:about="https://www.morphosource.org/terms/morphosource#Male">
        <rdf:type rdf:resource="https://www.morphosource.org/terms/morphosource#Sex"/>
        <rdfs:label xml:lang="en">Male</rdfs:label>
    </owl:NamedIndividual>
    


    <!-- https://www.morphosource.org/terms/morphosource#Merge -->


    <owl:NamedIndividual rdf:about="https://www.morphosource.org/terms/morphosource#Merge">
        <rdf:type rdf:resource="https://www.morphosource.org/terms/morphosource#ProcessingActivityType"/>
        <rdfs:label xml:lang="en">Merge</rdfs:label>
    </owl:NamedIndividual>
    


    <!-- https://www.morphosource.org/terms/morphosource#Mesh -->


    <owl:NamedIndividual rdf:about="https://www.morphosource.org/terms/morphosource#Mesh">
        <rdf:type rdf:resource="https://www.morphosource.org/terms/morphosource#MediaType"/>
        <rdfs:label xml:lang="en">Mesh or point cloud (*.stl, *.ply, .etc, with optional associated texture or color file)</rdfs:label>
    </owl:NamedIndividual>
    


    <!-- https://www.morphosource.org/terms/morphosource#MeshPointCloudTexturing -->


    <owl:NamedIndividual rdf:about="https://www.morphosource.org/terms/morphosource#MeshPointCloudTexturing">
        <rdf:type rdf:resource="https://www.morphosource.org/terms/morphosource#ProcessingActivityType"/>
        <rdfs:label xml:lang="en">Mesh and/or Point Cloud Texturing</rdfs:label>
    </owl:NamedIndividual>
    


    <!-- https://www.morphosource.org/terms/morphosource#MeshToPointCloud -->


    <owl:NamedIndividual rdf:about="https://www.morphosource.org/terms/morphosource#MeshToPointCloud">
        <rdf:type rdf:resource="https://www.morphosource.org/terms/morphosource#ProcessingActivityType"/>
        <rdfs:label xml:lang="en">Mesh to Point Cloud</rdfs:label>
    </owl:NamedIndividual>
    


    <!-- https://www.morphosource.org/terms/morphosource#Mi -->


    <owl:NamedIndividual rdf:about="https://www.morphosource.org/terms/morphosource#Mi">
        <rdf:type rdf:resource="https://www.morphosource.org/terms/morphosource#LengthMeasurementUnit"/>
        <rdfs:label xml:lang="en">Miles</rdfs:label>
    </owl:NamedIndividual>
    


    <!-- https://www.morphosource.org/terms/morphosource#MicroNanoXRayComputedTomography -->


    <owl:NamedIndividual rdf:about="https://www.morphosource.org/terms/morphosource#MicroNanoXRayComputedTomography">
        <rdf:type rdf:resource="https://www.morphosource.org/terms/morphosource#ImageModalityType"/>
        <rdfs:comment xml:lang="en">X-Ray Computed Tomography (CT/microCT) is a non-invasive imaging technique that uses X-rays to produce cross-sectional images of an object. It involves rotating an X-ray source and detector around the object, collecting data that is processed by a computer to create a 3D image. CT is widely used in medical imaging, as well as in materials science, engineering, and geology to visualize the internal structure of objects. MicroCT is a variation of CT that uses higher resolution X-rays to produce images of smaller objects.</rdfs:comment>
        <rdfs:label xml:lang="en">X-Ray Computed Tomography (CT/microCT)</rdfs:label>
        <skos:altLabel xml:lang="en">CT</skos:altLabel>
    </owl:NamedIndividual>
    


    <!-- https://www.morphosource.org/terms/morphosource#Midline -->


    <owl:NamedIndividual rdf:about="https://www.morphosource.org/terms/morphosource#Midline">
        <rdf:type rdf:resource="https://www.morphosource.org/terms/morphosource#Side"/>
        <rdfs:label xml:lang="en">Midline</rdfs:label>
    </owl:NamedIndividual>
    


    <!-- https://www.morphosource.org/terms/morphosource#Mm -->


    <owl:NamedIndividual rdf:about="https://www.morphosource.org/terms/morphosource#Mm">
        <rdf:type rdf:resource="https://www.morphosource.org/terms/morphosource#LengthMeasurementUnit"/>
        <rdfs:label xml:lang="en">Millimeters</rdfs:label>
    </owl:NamedIndividual>
    


    <!-- https://www.morphosource.org/terms/morphosource#MuseumDepartmentOrLabCollection -->


    <owl:NamedIndividual rdf:about="https://www.morphosource.org/terms/morphosource#MuseumDepartmentOrLabCollection">
        <rdf:type rdf:resource="https://www.morphosource.org/terms/morphosource#OrganizationType"/>
        <rdfs:label xml:lang="en">Museum, Department, or Lab Collection</rdfs:label>
    </owl:NamedIndividual>
    


    <!-- https://www.morphosource.org/terms/morphosource#NeutronComputedTomography -->


    <owl:NamedIndividual rdf:about="https://www.morphosource.org/terms/morphosource#NeutronComputedTomography">
        <rdf:type rdf:resource="https://www.morphosource.org/terms/morphosource#ImageModalityType"/>
        <rdfs:comment xml:lang="en">Neutron Computed Tomography (NCT) is an imaging technique that uses neutrons instead of X-rays to create cross-sectional images of an object. NCT is particularly useful for imaging materials that are difficult to penetrate with X-rays, such as ceramics and rocks.</rdfs:comment>
        <rdfs:label xml:lang="en">Neutron Computed Tomography (NCT)</rdfs:label>
        <skos:altLabel xml:lang="en">NCT</skos:altLabel>
    </owl:NamedIndividual>
    


    <!-- https://www.morphosource.org/terms/morphosource#Normal -->


    <owl:NamedIndividual rdf:about="https://www.morphosource.org/terms/morphosource#Normal">
        <rdf:type rdf:resource="https://www.morphosource.org/terms/morphosource#MeshMapType"/>
        <rdfs:label xml:lang="en">Normal Map</rdfs:label>
    </owl:NamedIndividual>
    


    <!-- https://www.morphosource.org/terms/morphosource#NotApplicable -->


    <owl:NamedIndividual rdf:about="https://www.morphosource.org/terms/morphosource#NotApplicable">
        <rdf:type rdf:resource="https://www.morphosource.org/terms/morphosource#Side"/>
        <rdfs:label xml:lang="en">Not Applicable</rdfs:label>
    </owl:NamedIndividual>
    


    <!-- https://www.morphosource.org/terms/morphosource#OnAnyRepository -->


    <owl:NamedIndividual rdf:about="https://www.morphosource.org/terms/morphosource#OnAnyRepository">
        <rdf:type rdf:resource="https://www.morphosource.org/terms/morphosource#DerivativeRearchivalStatement"/>
        <rdfs:comment xml:lang="en">Future derivatives are required to be rearchived on any public-facing digital repository.</rdfs:comment>
        <rdfs:label xml:lang="en">On Any Repository</rdfs:label>
    </owl:NamedIndividual>
    


    <!-- https://www.morphosource.org/terms/morphosource#OnMorphoSource -->


    <owl:NamedIndividual rdf:about="https://www.morphosource.org/terms/morphosource#OnMorphoSource">
        <rdf:type rdf:resource="https://www.morphosource.org/terms/morphosource#DerivativeRearchivalStatement"/>
        <rdfs:comment xml:lang="en">Future derivatives are required to be rearchived on MorphoSource.</rdfs:comment>
        <rdfs:label xml:lang="en">On MorphoSource</rdfs:label>
    </owl:NamedIndividual>
    


    <!-- https://www.morphosource.org/terms/morphosource#Open -->


    <owl:NamedIndividual rdf:about="https://www.morphosource.org/terms/morphosource#Open">
        <rdf:type rdf:resource="https://www.morphosource.org/terms/morphosource#PublicationStatus"/>
        <rdfs:comment xml:lang="en">Published with Open Download. Media record may be found in public search. Media file(s) may be downloaded openly, after downloader submits a simple download usage survey.</rdfs:comment>
        <rdfs:label xml:lang="en">Open Download</rdfs:label>
    </owl:NamedIndividual>
    


    <!-- https://www.morphosource.org/terms/morphosource#Other -->


    <owl:NamedIndividual rdf:about="https://www.morphosource.org/terms/morphosource#Other">
        <rdf:type rdf:resource="https://www.morphosource.org/terms/morphosource#MediaType"/>
        <rdfs:label xml:lang="en">Other</rdfs:label>
    </owl:NamedIndividual>
    


    <!-- https://www.morphosource.org/terms/morphosource#OtherSlide -->


    <owl:NamedIndividual rdf:about="https://www.morphosource.org/terms/morphosource#OtherSlide">
        <rdf:type rdf:resource="https://www.morphosource.org/terms/morphosource#SlideType"/>
        <rdfs:label xml:lang="en">Other Slide</rdfs:label>
    </owl:NamedIndividual>
    


    <!-- https://www.morphosource.org/terms/morphosource#Patch -->


    <owl:NamedIndividual rdf:about="https://www.morphosource.org/terms/morphosource#Patch">
        <rdf:type rdf:resource="https://www.morphosource.org/terms/morphosource#ProcessingActivityType"/>
        <rdfs:label xml:lang="en">Patch</rdfs:label>
    </owl:NamedIndividual>
    


    <!-- https://www.morphosource.org/terms/morphosource#Patterned -->


    <owl:NamedIndividual rdf:about="https://www.morphosource.org/terms/morphosource#Patterned">
        <rdf:type rdf:resource="https://www.morphosource.org/terms/morphosource#LightSourceType"/>
        <rdfs:label xml:lang="en">Patterned</rdfs:label>
    </owl:NamedIndividual>
    


    <!-- https://www.morphosource.org/terms/morphosource#Permissive -->


    <owl:NamedIndividual rdf:about="https://www.morphosource.org/terms/morphosource#Permissive">
        <rdf:type rdf:resource="https://www.morphosource.org/terms/morphosource#UseAgreementType"/>
        <rdfs:comment xml:lang="en">Permissive MorphoSource use agreement.</rdfs:comment>
        <rdfs:label xml:lang="en">Permissive</rdfs:label>
    </owl:NamedIndividual>
    


    <!-- https://www.morphosource.org/terms/morphosource#Photogrammetry -->


    <owl:NamedIndividual rdf:about="https://www.morphosource.org/terms/morphosource#Photogrammetry">
        <rdf:type rdf:resource="https://www.morphosource.org/terms/morphosource#ImageModalityType"/>
        <rdfs:comment xml:lang="en">Photogrammetry is the use of photography to measure and map the physical properties of an object. Photogrammetry can be used to create 3D models of objects and structures from 2D photographs, allowing for accurate measurements and analysis.</rdfs:comment>
        <rdfs:label xml:lang="en">Photogrammetry</rdfs:label>
        <skos:altLabel xml:lang="en">Photogram</skos:altLabel>
    </owl:NamedIndividual>
    


    <!-- https://www.morphosource.org/terms/morphosource#PhotogrammetryImageSeries -->


    <owl:NamedIndividual rdf:about="https://www.morphosource.org/terms/morphosource#PhotogrammetryImageSeries">
        <rdf:type rdf:resource="https://www.morphosource.org/terms/morphosource#MediaType"/>
        <rdfs:label xml:lang="en">Photogrammetry image series (multiple files of type *.tiff, *.png, etc.)</rdfs:label>
    </owl:NamedIndividual>
    


    <!-- https://www.morphosource.org/terms/morphosource#Photography -->


    <owl:NamedIndividual rdf:about="https://www.morphosource.org/terms/morphosource#Photography">
        <rdf:type rdf:resource="https://www.morphosource.org/terms/morphosource#ImageModalityType"/>
        <rdfs:comment xml:lang="en">Photography is the use of light to capture images of objects and scenes. Photography can be used for a wide range of purposes, from capturing memories to documenting scientific observations and creating works of art.</rdfs:comment>
        <rdfs:label xml:lang="en">Photography</rdfs:label>
        <skos:altLabel xml:lang="en">Photo</skos:altLabel>
    </owl:NamedIndividual>
    


    <!-- https://www.morphosource.org/terms/morphosource#PhotosToDensePointCloud -->


    <owl:NamedIndividual rdf:about="https://www.morphosource.org/terms/morphosource#PhotosToDensePointCloud">
        <rdf:type rdf:resource="https://www.morphosource.org/terms/morphosource#ProcessingActivityType"/>
        <rdfs:label xml:lang="en">Photos to Dense Point Cloud</rdfs:label>
    </owl:NamedIndividual>
    


    <!-- https://www.morphosource.org/terms/morphosource#PhotosToDigitalElevationModel -->


    <owl:NamedIndividual rdf:about="https://www.morphosource.org/terms/morphosource#PhotosToDigitalElevationModel">
        <rdf:type rdf:resource="https://www.morphosource.org/terms/morphosource#ProcessingActivityType"/>
        <rdfs:label xml:lang="en">Photos to Digital Elevation Model</rdfs:label>
    </owl:NamedIndividual>
    


    <!-- https://www.morphosource.org/terms/morphosource#PhotosToMesh -->


    <owl:NamedIndividual rdf:about="https://www.morphosource.org/terms/morphosource#PhotosToMesh">
        <rdf:type rdf:resource="https://www.morphosource.org/terms/morphosource#ProcessingActivityType"/>
        <rdfs:label xml:lang="en">Photos to Mesh</rdfs:label>
    </owl:NamedIndividual>
    


    <!-- https://www.morphosource.org/terms/morphosource#PhotosToSparseMeshDepthMap -->


    <owl:NamedIndividual rdf:about="https://www.morphosource.org/terms/morphosource#PhotosToSparseMeshDepthMap">
        <rdf:type rdf:resource="https://www.morphosource.org/terms/morphosource#ProcessingActivityType"/>
        <rdfs:label xml:lang="en">Photos to Sparse Mesh and Depth Map</rdfs:label>
    </owl:NamedIndividual>
    


    <!-- https://www.morphosource.org/terms/morphosource#PhotosToSparsePointCloudDepthMap -->


    <owl:NamedIndividual rdf:about="https://www.morphosource.org/terms/morphosource#PhotosToSparsePointCloudDepthMap">
        <rdf:type rdf:resource="https://www.morphosource.org/terms/morphosource#ProcessingActivityType"/>
        <rdfs:label xml:lang="en">Photos to Sparse Point Cloud and Depth Map</rdfs:label>
    </owl:NamedIndividual>
    


    <!-- https://www.morphosource.org/terms/morphosource#PointCloudToMesh -->


    <owl:NamedIndividual rdf:about="https://www.morphosource.org/terms/morphosource#PointCloudToMesh">
        <rdf:type rdf:resource="https://www.morphosource.org/terms/morphosource#ProcessingActivityType"/>
        <rdfs:label xml:lang="en">Point Cloud to Mesh</rdfs:label>
    </owl:NamedIndividual>
    


    <!-- https://www.morphosource.org/terms/morphosource#PositronEmissionTomography -->


    <owl:NamedIndividual rdf:about="https://www.morphosource.org/terms/morphosource#PositronEmissionTomography">
        <rdf:type rdf:resource="https://www.morphosource.org/terms/morphosource#ImageModalityType"/>
        <rdfs:comment xml:lang="en">Positron Emission Tomography (PET) is a non-invasive imaging technique that uses small amounts of radioactive tracers to visualize metabolic processes in the body. The tracer is injected into the body and collects in areas of high metabolic activity, emitting positrons that are detected by the PET scanner. PET is widely used in medical diagnosis and research, especially for imaging cancer, heart disease, and neurological disorders.</rdfs:comment>
        <rdfs:label xml:lang="en">Positron Emission Tomography (PET)</rdfs:label>
        <skos:altLabel xml:lang="en">PET</skos:altLabel>
    </owl:NamedIndividual>
    


    <!-- https://www.morphosource.org/terms/morphosource#Private -->


    <owl:NamedIndividual rdf:about="https://www.morphosource.org/terms/morphosource#Private">
        <rdf:type rdf:resource="https://www.morphosource.org/terms/morphosource#PublicationStatus"/>
        <rdfs:label xml:lang="en">Private</rdfs:label>
        <rdfs:label xml:lang="en">Unpublished. Media may not be found in public search, and media file(s) may not be downloaded by users without explicit access to Media.</rdfs:label>
    </owl:NamedIndividual>
    


    <!-- https://www.morphosource.org/terms/morphosource#Projections -->


    <owl:NamedIndividual rdf:about="https://www.morphosource.org/terms/morphosource#Projections">
        <rdf:type rdf:resource="https://www.morphosource.org/terms/morphosource#CTImageSeriesType"/>
        <rdfs:label xml:lang="en">Projections</rdfs:label>
    </owl:NamedIndividual>
    


    <!-- https://www.morphosource.org/terms/morphosource#ReconstructedImageStack -->


    <owl:NamedIndividual rdf:about="https://www.morphosource.org/terms/morphosource#ReconstructedImageStack">
        <rdf:type rdf:resource="https://www.morphosource.org/terms/morphosource#CTImageSeriesType"/>
        <rdfs:label xml:lang="en">Reconstructed image stack</rdfs:label>
    </owl:NamedIndividual>
    


    <!-- https://www.morphosource.org/terms/morphosource#ReconstructedTomographyToMesh -->


    <owl:NamedIndividual rdf:about="https://www.morphosource.org/terms/morphosource#ReconstructedTomographyToMesh">
        <rdf:type rdf:resource="https://www.morphosource.org/terms/morphosource#ProcessingActivityType"/>
        <rdfs:label xml:lang="en">Reconstructed Tomography to Mesh</rdfs:label>
    </owl:NamedIndividual>
    


    <!-- https://www.morphosource.org/terms/morphosource#Reconstruction -->


    <owl:NamedIndividual rdf:about="https://www.morphosource.org/terms/morphosource#Reconstruction">
        <rdf:type rdf:resource="https://www.morphosource.org/terms/morphosource#ProcessingActivityType"/>
        <rdfs:label xml:lang="en">Reconstruction</rdfs:label>
    </owl:NamedIndividual>
    


    <!-- https://www.morphosource.org/terms/morphosource#ReflectanceTransformationImaging -->


    <owl:NamedIndividual rdf:about="https://www.morphosource.org/terms/morphosource#ReflectanceTransformationImaging">
        <rdf:type rdf:resource="https://www.morphosource.org/terms/morphosource#ImageModalityType"/>
        <rdfs:comment xml:lang="en">Reflectance Transformation Imaging (RTI) is an imaging technique that uses a series of photographs taken under different lighting conditions to create a detailed 3D model of an object&apos;s surface. RTI is particularly useful for analyzing the surface texture and details of objects such as artwork and historical artifacts.</rdfs:comment>
        <rdfs:label xml:lang="en">Reflectance Transformation Imaging</rdfs:label>
        <skos:altLabel xml:lang="en">RTI</skos:altLabel>
    </owl:NamedIndividual>
    


    <!-- https://www.morphosource.org/terms/morphosource#Reflection -->


    <owl:NamedIndividual rdf:about="https://www.morphosource.org/terms/morphosource#Reflection">
        <rdf:type rdf:resource="https://www.morphosource.org/terms/morphosource#XRayTargetType"/>
        <rdfs:label xml:lang="en">Reflection</rdfs:label>
    </owl:NamedIndividual>
    


    <!-- https://www.morphosource.org/terms/morphosource#Restricted -->


    <owl:NamedIndividual rdf:about="https://www.morphosource.org/terms/morphosource#Restricted">
        <rdf:type rdf:resource="https://www.morphosource.org/terms/morphosource#PublicationStatus"/>
        <rdfs:comment xml:lang="en">Published with Restricted Download. Media may be found in public search. Media file(s) may only be downloaded after user has sought and received download approval from the Media data manager.</rdfs:comment>
        <rdfs:label xml:lang="en">Restricted Download</rdfs:label>
    </owl:NamedIndividual>
    


    <!-- https://www.morphosource.org/terms/morphosource#Right -->


    <owl:NamedIndividual rdf:about="https://www.morphosource.org/terms/morphosource#Right">
        <rdf:type rdf:resource="https://www.morphosource.org/terms/morphosource#Side"/>
        <rdfs:label xml:lang="en">Right</rdfs:label>
    </owl:NamedIndividual>
    


    <!-- https://www.morphosource.org/terms/morphosource#ScanningElectronMicroscopy -->


    <owl:NamedIndividual rdf:about="https://www.morphosource.org/terms/morphosource#ScanningElectronMicroscopy">
        <rdf:type rdf:resource="https://www.morphosource.org/terms/morphosource#ImageModalityType"/>
        <rdfs:comment xml:lang="en">Scanning Electron Microscopy (SEM) is an imaging technique that uses a beam of electrons to create high-resolution images of the surface of an object. SEM can produce images with extremely high magnification and resolution, making it useful for analyzing the microstructure of materials and biological specimens.</rdfs:comment>
        <rdfs:label xml:lang="en">Scanning Electron Microscopy</rdfs:label>
        <skos:altLabel xml:lang="en">SEM</skos:altLabel>
    </owl:NamedIndividual>
    


    <!-- https://www.morphosource.org/terms/morphosource#ScanningFacility -->


    <owl:NamedIndividual rdf:about="https://www.morphosource.org/terms/morphosource#ScanningFacility">
        <rdf:type rdf:resource="https://www.morphosource.org/terms/morphosource#OrganizationType"/>
        <rdfs:label xml:lang="en">Scanning Facility</rdfs:label>
    </owl:NamedIndividual>
    


    <!-- https://www.morphosource.org/terms/morphosource#Scintillator -->


    <owl:NamedIndividual rdf:about="https://www.morphosource.org/terms/morphosource#Scintillator">
        <rdf:type rdf:resource="https://www.morphosource.org/terms/morphosource#XRayDetectorType"/>
        <rdfs:label xml:lang="en">Scintillator (Phosphor used)</rdfs:label>
    </owl:NamedIndividual>
    


    <!-- https://www.morphosource.org/terms/morphosource#Sequenced -->


    <owl:NamedIndividual rdf:about="https://www.morphosource.org/terms/morphosource#Sequenced">
        <rdf:type rdf:resource="https://www.morphosource.org/terms/morphosource#AcquisitionType"/>
        <rdfs:label xml:lang="en">Sequenced (Rotational)</rdfs:label>
    </owl:NamedIndividual>
    


    <!-- https://www.morphosource.org/terms/morphosource#SequentialSectionImageSeries -->


    <owl:NamedIndividual rdf:about="https://www.morphosource.org/terms/morphosource#SequentialSectionImageSeries">
        <rdf:type rdf:resource="https://www.morphosource.org/terms/morphosource#MediaType"/>
        <rdfs:label xml:lang="en">Sequential section image series (multiple files of type *.tiff, *.png, *.zip, etc.)</rdfs:label>
    </owl:NamedIndividual>
    


    <!-- https://www.morphosource.org/terms/morphosource#SequentialSectionScan -->


    <owl:NamedIndividual rdf:about="https://www.morphosource.org/terms/morphosource#SequentialSectionScan">
        <rdf:type rdf:resource="https://www.morphosource.org/terms/morphosource#ImageModalityType"/>
        <rdfs:comment xml:lang="en">Sequential Section Scan is an imaging technique that involves cutting an object into thin sections, then imaging each section individually to create a 3D image. This technique is commonly used in medical imaging and histology to visualize the internal structure of tissues and organs.</rdfs:comment>
        <rdfs:label xml:lang="en">Sequential Section Scan</rdfs:label>
        <skos:altLabel xml:lang="en">Section</skos:altLabel>
    </owl:NamedIndividual>
    


    <!-- https://www.morphosource.org/terms/morphosource#Simplification -->


    <owl:NamedIndividual rdf:about="https://www.morphosource.org/terms/morphosource#Simplification">
        <rdf:type rdf:resource="https://www.morphosource.org/terms/morphosource#ProcessingActivityType"/>
        <rdfs:label xml:lang="en">Simplification</rdfs:label>
    </owl:NamedIndividual>
    


    <!-- https://www.morphosource.org/terms/morphosource#SinglePhotonEmissionComputedTomography -->


    <owl:NamedIndividual rdf:about="https://www.morphosource.org/terms/morphosource#SinglePhotonEmissionComputedTomography">
        <rdf:type rdf:resource="https://www.morphosource.org/terms/morphosource#ImageModalityType"/>
        <rdfs:comment xml:lang="en">Single Photon Emission Computed Tomography (SPECT) is a non-invasive imaging technique that uses a small amount of radioactive tracer to produce 3D images of the body&apos;s internal structures. The tracer is injected into the body and emits gamma rays, which are detected by a SPECT scanner. SPECT is used in medical diagnosis and research, especially for imaging the brain, heart, and bones.</rdfs:comment>
        <rdfs:label xml:lang="en">Single Photon Emission Computed Tomography (SPECT)</rdfs:label>
        <skos:altLabel xml:lang="en">SPECT</skos:altLabel>
    </owl:NamedIndividual>
    


    <!-- https://www.morphosource.org/terms/morphosource#Sinograms -->


    <owl:NamedIndividual rdf:about="https://www.morphosource.org/terms/morphosource#Sinograms">
        <rdf:type rdf:resource="https://www.morphosource.org/terms/morphosource#CTImageSeriesType"/>
        <rdfs:label xml:lang="en">Sinograms</rdfs:label>
    </owl:NamedIndividual>
    


    <!-- https://www.morphosource.org/terms/morphosource#Slot -->


    <owl:NamedIndividual rdf:about="https://www.morphosource.org/terms/morphosource#Slot">
        <rdf:type rdf:resource="https://www.morphosource.org/terms/morphosource#XRayDetectorConfiguration"/>
        <rdfs:label xml:lang="en">Slot (scanned slot, slit, or spot)</rdfs:label>
    </owl:NamedIndividual>
    


    <!-- https://www.morphosource.org/terms/morphosource#SmoothingNoiseReduction -->


    <owl:NamedIndividual rdf:about="https://www.morphosource.org/terms/morphosource#SmoothingNoiseReduction">
        <rdf:type rdf:resource="https://www.morphosource.org/terms/morphosource#ProcessingActivityType"/>
        <rdfs:label xml:lang="en">Smoothing and/or Noise Reduction</rdfs:label>
    </owl:NamedIndividual>
    


    <!-- https://www.morphosource.org/terms/morphosource#SparseMeshDepthMapToMesh -->


    <owl:NamedIndividual rdf:about="https://www.morphosource.org/terms/morphosource#SparseMeshDepthMapToMesh">
        <rdf:type rdf:resource="https://www.morphosource.org/terms/morphosource#ProcessingActivityType"/>
        <rdfs:label xml:lang="en">Sparse Mesh and Depth Map to Mesh</rdfs:label>
    </owl:NamedIndividual>
    


    <!-- https://www.morphosource.org/terms/morphosource#SparsePointCloudDepthMapToDensePointCloud -->


    <owl:NamedIndividual rdf:about="https://www.morphosource.org/terms/morphosource#SparsePointCloudDepthMapToDensePointCloud">
        <rdf:type rdf:resource="https://www.morphosource.org/terms/morphosource#ProcessingActivityType"/>
        <rdfs:label xml:lang="en">Sparse Point Cloud and Depth Map to Dense Point Cloud</rdfs:label>
    </owl:NamedIndividual>
    


    <!-- https://www.morphosource.org/terms/morphosource#Spiral -->


    <owl:NamedIndividual rdf:about="https://www.morphosource.org/terms/morphosource#Spiral">
        <rdf:type rdf:resource="https://www.morphosource.org/terms/morphosource#AcquisitionType"/>
        <rdfs:label xml:lang="en">Spiral</rdfs:label>
    </owl:NamedIndividual>
    


    <!-- https://www.morphosource.org/terms/morphosource#Standard -->


    <owl:NamedIndividual rdf:about="https://www.morphosource.org/terms/morphosource#Standard">
        <rdf:type rdf:resource="https://www.morphosource.org/terms/morphosource#UseAgreementType"/>
        <rdfs:comment xml:lang="en">Standard MorphoSource use agreement.</rdfs:comment>
        <rdfs:label xml:lang="en">Standard</rdfs:label>
    </owl:NamedIndividual>
    


    <!-- https://www.morphosource.org/terms/morphosource#Static -->


    <owl:NamedIndividual rdf:about="https://www.morphosource.org/terms/morphosource#Static">
        <rdf:type rdf:resource="https://www.morphosource.org/terms/morphosource#LightSourceType"/>
        <rdfs:label xml:lang="en">Static</rdfs:label>
    </owl:NamedIndividual>
    


    <!-- https://www.morphosource.org/terms/morphosource#Stationary -->


    <owl:NamedIndividual rdf:about="https://www.morphosource.org/terms/morphosource#Stationary">
        <rdf:type rdf:resource="https://www.morphosource.org/terms/morphosource#AcquisitionType"/>
        <rdfs:label xml:lang="en">Stationary</rdfs:label>
    </owl:NamedIndividual>
    


    <!-- https://www.morphosource.org/terms/morphosource#Storage -->


    <owl:NamedIndividual rdf:about="https://www.morphosource.org/terms/morphosource#Storage">
        <rdf:type rdf:resource="https://www.morphosource.org/terms/morphosource#XRayDetectorType"/>
        <rdfs:label xml:lang="en">Storage (Storage Phosphor)</rdfs:label>
    </owl:NamedIndividual>
    


    <!-- https://www.morphosource.org/terms/morphosource#Strobe -->


    <owl:NamedIndividual rdf:about="https://www.morphosource.org/terms/morphosource#Strobe">
        <rdf:type rdf:resource="https://www.morphosource.org/terms/morphosource#LightSourceType"/>
        <rdfs:label xml:lang="en">Strobe</rdfs:label>
    </owl:NamedIndividual>
    


    <!-- https://www.morphosource.org/terms/morphosource#StructuredLight -->


    <owl:NamedIndividual rdf:about="https://www.morphosource.org/terms/morphosource#StructuredLight">
        <rdf:type rdf:resource="https://www.morphosource.org/terms/morphosource#ImageModalityType"/>
        <rdfs:comment xml:lang="en">Structured Light is an imaging technique that uses a pattern of light projected onto an object to create a 3D image. By analyzing how the pattern of light is distorted by the object, structured light can create high-resolution, accurate 3D models of complex shapes and structures.</rdfs:comment>
        <rdfs:label xml:lang="en">Structured Light</rdfs:label>
        <skos:altLabel xml:lang="en">StrLight</skos:altLabel>
    </owl:NamedIndividual>
    


    <!-- https://www.morphosource.org/terms/morphosource#SynchrotronImaging -->


    <owl:NamedIndividual rdf:about="https://www.morphosource.org/terms/morphosource#SynchrotronImaging">
        <rdf:type rdf:resource="https://www.morphosource.org/terms/morphosource#ImageModalityType"/>
        <rdfs:comment xml:lang="en">Synchrotron Imaging is a type of X-ray imaging that uses synchrotron radiation, which is produced when high-energy particles are accelerated to near the speed of light. Synchrotron imaging can produce high-resolution, 3D images of a wide range of materials and structures.</rdfs:comment>
        <rdfs:label xml:lang="en">Synchrotron Imaging</rdfs:label>
        <skos:altLabel xml:lang="en">Synchro</skos:altLabel>
    </owl:NamedIndividual>
    


    <!-- https://www.morphosource.org/terms/morphosource#TransformReflection -->


    <owl:NamedIndividual rdf:about="https://www.morphosource.org/terms/morphosource#TransformReflection">
        <rdf:type rdf:resource="https://www.morphosource.org/terms/morphosource#ProcessingActivityType"/>
        <rdfs:label xml:lang="en">Transform: Reflection</rdfs:label>
    </owl:NamedIndividual>
    


    <!-- https://www.morphosource.org/terms/morphosource#TransformRotation -->


    <owl:NamedIndividual rdf:about="https://www.morphosource.org/terms/morphosource#TransformRotation">
        <rdf:type rdf:resource="https://www.morphosource.org/terms/morphosource#ProcessingActivityType"/>
        <rdfs:label xml:lang="en">Transform: Rotation</rdfs:label>
    </owl:NamedIndividual>
    


    <!-- https://www.morphosource.org/terms/morphosource#TransformScale -->


    <owl:NamedIndividual rdf:about="https://www.morphosource.org/terms/morphosource#TransformScale">
        <rdf:type rdf:resource="https://www.morphosource.org/terms/morphosource#ProcessingActivityType"/>
        <rdfs:label xml:lang="en">Transform: Scale</rdfs:label>
    </owl:NamedIndividual>
    


    <!-- https://www.morphosource.org/terms/morphosource#TransformTranslation -->


    <owl:NamedIndividual rdf:about="https://www.morphosource.org/terms/morphosource#TransformTranslation">
        <rdf:type rdf:resource="https://www.morphosource.org/terms/morphosource#ProcessingActivityType"/>
        <rdfs:label xml:lang="en">Transform: Translation</rdfs:label>
    </owl:NamedIndividual>
    


    <!-- https://www.morphosource.org/terms/morphosource#Transmission -->


    <owl:NamedIndividual rdf:about="https://www.morphosource.org/terms/morphosource#Transmission">
        <rdf:type rdf:resource="https://www.morphosource.org/terms/morphosource#XRayTargetType"/>
        <rdfs:label xml:lang="en">Transmission</rdfs:label>
    </owl:NamedIndividual>
    


    <!-- https://www.morphosource.org/terms/morphosource#Um -->


    <owl:NamedIndividual rdf:about="https://www.morphosource.org/terms/morphosource#Um">
        <rdf:type rdf:resource="https://www.morphosource.org/terms/morphosource#LengthMeasurementUnit"/>
        <rdfs:label xml:lang="en">Micrometers</rdfs:label>
    </owl:NamedIndividual>
    


    <!-- https://www.morphosource.org/terms/morphosource#Undetermined -->


    <owl:NamedIndividual rdf:about="https://www.morphosource.org/terms/morphosource#Undetermined">
        <rdf:type rdf:resource="https://www.morphosource.org/terms/morphosource#Sex"/>
        <rdfs:label xml:lang="en">Undetermined</rdfs:label>
    </owl:NamedIndividual>
    


    <!-- https://www.morphosource.org/terms/morphosource#Unknowable -->


    <owl:NamedIndividual rdf:about="https://www.morphosource.org/terms/morphosource#Unknowable">
        <rdf:type rdf:resource="https://www.morphosource.org/terms/morphosource#Sex"/>
        <rdfs:label xml:lang="en">Unknowable</rdfs:label>
    </owl:NamedIndividual>
    


    <!-- https://www.morphosource.org/terms/morphosource#Unknown -->


    <owl:NamedIndividual rdf:about="https://www.morphosource.org/terms/morphosource#Unknown">
        <rdf:type rdf:resource="https://www.morphosource.org/terms/morphosource#Side"/>
        <rdfs:label xml:lang="en">Unknown</rdfs:label>
    </owl:NamedIndividual>
    


    <!-- https://www.morphosource.org/terms/morphosource#Variable -->


    <owl:NamedIndividual rdf:about="https://www.morphosource.org/terms/morphosource#Variable">
        <rdf:type rdf:resource="https://www.morphosource.org/terms/morphosource#FocalLengthType"/>
        <rdfs:label xml:lang="en">Variable</rdfs:label>
    </owl:NamedIndividual>
    


    <!-- https://www.morphosource.org/terms/morphosource#Video -->


    <owl:NamedIndividual rdf:about="https://www.morphosource.org/terms/morphosource#Video">
        <rdf:type rdf:resource="https://www.morphosource.org/terms/morphosource#MediaType"/>
        <rdfs:label xml:lang="en">Video (*.avi, *.mp4, *.mov, .etc.)</rdfs:label>
    </owl:NamedIndividual>
    


    <!-- https://www.morphosource.org/terms/morphosource#Videography -->


    <owl:NamedIndividual rdf:about="https://www.morphosource.org/terms/morphosource#Videography">
        <rdf:type rdf:resource="https://www.morphosource.org/terms/morphosource#ImageModalityType"/>
        <rdfs:comment xml:lang="en">The recording of moving images and sound (video). It is a widely used medium for recording and displaying visual information, including images of physical objects. Video can be captured using a variety of devices, from smartphones to professional cameras, and can be stored in a variety of digital formats.</rdfs:comment>
        <rdfs:label xml:lang="en">Videography</rdfs:label>
        <skos:altLabel xml:lang="en">Video</skos:altLabel>
    </owl:NamedIndividual>
    


    <!-- https://www.morphosource.org/terms/morphosource#XRay -->


    <owl:NamedIndividual rdf:about="https://www.morphosource.org/terms/morphosource#XRay">
        <rdf:type rdf:resource="https://www.morphosource.org/terms/morphosource#ImageModalityType"/>
        <rdfs:comment xml:lang="en">X-Ray imaging is an imaging technique that uses X-rays to create images of the internal structures of an object. X-ray imaging is widely used in medical diagnosis and research, as well as in materials science and other fields to visualize the internal structure of objects.</rdfs:comment>
        <rdfs:label xml:lang="en">X-Ray</rdfs:label>
        <skos:altLabel xml:lang="en">XRay</skos:altLabel>
    </owl:NamedIndividual>
    


    <!-- https://www.morphosource.org/terms/morphosource#3DPrintingLimited -->


    <owl:NamedIndividual rdf:about="https://www.morphosource.org/terms/morphosource#3DPrintingLimited">
        <rdf:type rdf:resource="https://www.morphosource.org/terms/morphosource#3DPrintingPermission"/>
        <rdfs:comment xml:lang="en">3D printing of digital resources is permitted only if the data was initially downloaded with the intent to 3D print as explicitly indicated by communication from the downloader or from an automated download usage survey form, and where sharing of 3D prints is permitted only in small-scale informal circumstances that should be explicitly outlined elsewhere.</rdfs:comment>
        <rdfs:label xml:lang="en">3D Printing Limited</rdfs:label>
    </owl:NamedIndividual>
    


    <!-- https://www.morphosource.org/terms/morphosource#3DPrintingPermitted -->


    <owl:NamedIndividual rdf:about="https://www.morphosource.org/terms/morphosource#3DPrintingPermitted">
        <rdf:type rdf:resource="https://www.morphosource.org/terms/morphosource#3DPrintingPermission"/>
        <rdfs:comment xml:lang="en">3D printing of digital resource is freely permitted.</rdfs:comment>
        <rdfs:label xml:lang="en">3D Printing Permitted</rdfs:label>
    </owl:NamedIndividual>
    


    <!-- https://www.morphosource.org/terms/morphosource#3DPrintingProhibited -->


    <owl:NamedIndividual rdf:about="https://www.morphosource.org/terms/morphosource#3DPrintingProhibited">
        <rdf:type rdf:resource="https://www.morphosource.org/terms/morphosource#3DPrintingPermission"/>
        <rdfs:comment xml:lang="en">3D printing of digital resource is prohibited.</rdfs:comment>
        <rdfs:label xml:lang="en">3D Printing Prohibited</rdfs:label>
    </owl:NamedIndividual>
    


    <!-- 
    ///////////////////////////////////////////////////////////////////////////////////////
    //
    // Annotations
    //
    ///////////////////////////////////////////////////////////////////////////////////////
     -->


    <rdf:Description rdf:about="http://purl.org/dc/terms/TGN">
        <terms:issued rdf:datatype="http://www.w3.org/2001/XMLSchema#date">2000-07-11</terms:issued>
        <rdfs:comment xml:lang="en">The set of places specified by the Getty Thesaurus of Geographic Names.</rdfs:comment>
        <rdfs:isDefinedBy rdf:resource="http://purl.org/dc/terms/"/>
        <rdfs:label xml:lang="en">TGN</rdfs:label>
        <rdfs:seeAlso rdf:resource="http://www.getty.edu/research/tools/vocabulary/tgn/index.html"/>
    </rdf:Description>
</rdf:RDF>



<!-- Generated by the OWL API (version 5.1.18) https://github.com/owlcs/owlapi/ -->


